<?xml version="1.0"?>


<!DOCTYPE rdf:RDF [
    <!ENTITY owl "http://www.w3.org/2002/07/owl#" >
    <!ENTITY sdle "http://pellet.owldl.com/ns/sdle#" >
    <!ENTITY xsd "http://www.w3.org/2001/XMLSchema#" >
    <!ENTITY rdfs "http://www.w3.org/2000/01/rdf-schema#" >
    <!ENTITY rdf "http://www.w3.org/1999/02/22-rdf-syntax-ns#" >
    <!ENTITY m "http://onto.fel.cvut.cz/ontologies/aviation-safety/" >
    <!ENTITY all2 "http://onto.fel.cvut.cz/ontologies/aviation/eccairs/1.3.0.12/all#" >
    <!ENTITY all "http://onto.fel.cvut.cz/ontologies/2014/ECCAIRS_Aviation_1.3.0.12/all#" >
]>


<rdf:RDF xmlns="&m;airline#"
     xml:base="&m;airline"
     xmlns:rdfs="http://www.w3.org/2000/01/rdf-schema#"
     xmlns:owl="http://www.w3.org/2002/07/owl#"
     xmlns:xsd="http://www.w3.org/2001/XMLSchema#"
     xmlns:rdf="http://www.w3.org/1999/02/22-rdf-syntax-ns#"
     xmlns:sdle="http://pellet.owldl.com/ns/sdle#"
     xmlns:m="http://onto.fel.cvut.cz/ontologies/aviation-safety/"
     xmlns:all2="http://onto.fel.cvut.cz/ontologies/aviation/eccairs/1.3.0.12/all#"
     xmlns:all="http://onto.fel.cvut.cz/ontologies/2014/ECCAIRS_Aviation_1.3.0.12/all#">
    <owl:Ontology rdf:about="http://onto.fel.cvut.cz/ontologies/aviation/airline">
        <owl:imports rdf:resource="http://onto.fel.cvut.cz/ontologies/aviation/core"/>
    </owl:Ontology>
    


    <!-- 
    ///////////////////////////////////////////////////////////////////////////////////////
    //
    // Annotation properties
    //
    ///////////////////////////////////////////////////////////////////////////////////////
     -->

    


    <!-- http://onto.fel.cvut.cz/ontologies/aviation-safety/generated_time -->

    <owl:AnnotationProperty rdf:about="&m;generated_time"/>
    


    <!-- http://onto.fel.cvut.cz/ontologies/aviation-safety/has_related_eccairs_term -->

    <owl:AnnotationProperty rdf:about="&m;has_related_eccairs_term"/>
    


    <!-- http://onto.fel.cvut.cz/ontologies/aviation/eccairs/1.3.0.12/all#has_ATA_code -->

    <owl:AnnotationProperty rdf:about="&all2;has_ATA_code"/>
    


    <!-- 
    ///////////////////////////////////////////////////////////////////////////////////////
    //
    // Classes
    //
    ///////////////////////////////////////////////////////////////////////////////////////
     -->

    


    <!-- http://onto.fel.cvut.cz/ontologies/aviation-safety/APU_System_Wiring -->

    <owl:Class rdf:about="&m;APU_System_Wiring">
        <rdfs:subClassOf rdf:resource="&m;Airborne_auxiliary_power_unit_system_part"/>
    </owl:Class>
    


    <!-- http://onto.fel.cvut.cz/ontologies/aviation-safety/Accessory_Gearbox_System_Wiring -->

    <owl:Class rdf:about="&m;Accessory_Gearbox_System_Wiring">
        <rdfs:subClassOf rdf:resource="&m;Accessory_gearboxes_part"/>
    </owl:Class>
    


    <!-- http://onto.fel.cvut.cz/ontologies/aviation-safety/Accessory_Gearboxes_Gearbox_Section -->

    <owl:Class rdf:about="&m;Accessory_Gearboxes_Gearbox_Section">
        <rdfs:label>Accessory Gearboxes Gearbox Section</rdfs:label>
        <rdfs:subClassOf rdf:resource="&m;Accessory_gearboxes_part"/>
        <m:generated_time rdf:datatype="&xsd;dateTime">2015-04-09T18:56:27.771+02:00</m:generated_time>
        <rdfs:comment xml:lang="en">(ATA Code:8320) The case which contains the gear trains and shafts.  Includes items such as gears, shafts, seals, oil pumps, coolers, etc</rdfs:comment>
        <m:has_related_eccairs_term rdf:resource="http://onto.fel.cvut.cz/ontologies/2014/ECCAIRS_Aviation_1.3.0.12/eccairs-descriptive-factors#category_11832000"/>
    </owl:Class>
    


    <!-- http://onto.fel.cvut.cz/ontologies/aviation-safety/Accessory_compartment_doors -->

    <owl:Class rdf:about="&m;Accessory_compartment_doors">
        <rdfs:subClassOf rdf:resource="&m;Service_doors_part"/>
    </owl:Class>
    


    <!-- http://onto.fel.cvut.cz/ontologies/aviation-safety/Accessory_compartments -->

    <owl:Class rdf:about="&m;Accessory_compartments">
        <rdfs:subClassOf rdf:resource="&m;Cabin_equipment-furnishings"/>
        <rdfs:subClassOf rdf:resource="&m;Cargo_and_accessory_compartments_part"/>
    </owl:Class>
    


    <!-- http://onto.fel.cvut.cz/ontologies/aviation-safety/Accessory_compartments_part -->

    <owl:Class rdf:about="&m;Accessory_compartments_part">
        <rdfs:label>Accessory compartments part</rdfs:label>
        <rdfs:subClassOf rdf:resource="&m;Cabin_equipment-furnishings"/>
        <rdfs:subClassOf>
            <owl:Restriction>
                <owl:onProperty rdf:resource="http://onto.fel.cvut.cz/ontologies/ufo/is_part_of"/>
                <owl:someValuesFrom rdf:resource="&m;Accessory_compartments"/>
            </owl:Restriction>
        </rdfs:subClassOf>
        <m:generated_time rdf:datatype="&xsd;dateTime">2015-04-12T02:45:54.351+02:00</m:generated_time>
        <m:has_related_eccairs_term rdf:resource="http://onto.fel.cvut.cz/ontologies/2014/ECCAIRS_Aviation_1.3.0.12/eccairs-descriptive-factors#category_11257000"/>
    </owl:Class>
    


    <!-- http://onto.fel.cvut.cz/ontologies/aviation-safety/Accessory_gearboxes -->

    <owl:Class rdf:about="&m;Accessory_gearboxes">
        <rdfs:label>Accessory gearboxes</rdfs:label>
        <rdfs:subClassOf rdf:resource="&m;Aircraft_part"/>
        <m:generated_time rdf:datatype="&xsd;dateTime">2015-04-09T18:56:27.771+02:00</m:generated_time>
        <rdfs:comment xml:lang="en">(ATA Code:8300) Accessory gearboxes: The units and components which are remote but connected to the engine by a drive shaft and which does not include those accessory drives which are bolted to and are immediately adjacent to the engine [Code 11720000]. Does not include accessory drives bolted to and adjacent to engine [Code 11726000].</rdfs:comment>
        <m:has_related_eccairs_term rdf:resource="http://onto.fel.cvut.cz/ontologies/2014/ECCAIRS_Aviation_1.3.0.12/eccairs-descriptive-factors#category_11830000"/>
    </owl:Class>
    


    <!-- http://onto.fel.cvut.cz/ontologies/aviation-safety/Accessory_gearboxes_part -->

    <owl:Class rdf:about="&m;Accessory_gearboxes_part">
        <rdfs:label>Accessory gearboxes part</rdfs:label>
        <rdfs:subClassOf rdf:resource="&m;Aircraft_part"/>
        <rdfs:subClassOf>
            <owl:Restriction>
                <owl:onProperty rdf:resource="http://onto.fel.cvut.cz/ontologies/ufo/is_part_of"/>
                <owl:someValuesFrom rdf:resource="&m;Accessory_gearboxes"/>
            </owl:Restriction>
        </rdfs:subClassOf>
        <m:generated_time rdf:datatype="&xsd;dateTime">2015-04-12T02:45:54.351+02:00</m:generated_time>
        <m:has_related_eccairs_term rdf:resource="http://onto.fel.cvut.cz/ontologies/2014/ECCAIRS_Aviation_1.3.0.12/eccairs-descriptive-factors#category_11830000"/>
    </owl:Class>
    


    <!-- http://onto.fel.cvut.cz/ontologies/aviation-safety/Aerial_tow_equipment -->

    <owl:Class rdf:about="&m;Aerial_tow_equipment">
        <rdfs:label>Aerial tow equipment</rdfs:label>
        <rdfs:subClassOf rdf:resource="&m;Fuselage_structure_(general)_part"/>
        <m:generated_time rdf:datatype="&xsd;dateTime">2015-04-09T18:56:27.771+02:00</m:generated_time>
        <rdfs:comment xml:lang="en">(ATA Code:5301) The aerial towing equipment including the attachments on fuselage and release mechanism.</rdfs:comment>
        <m:has_related_eccairs_term rdf:resource="http://onto.fel.cvut.cz/ontologies/2014/ECCAIRS_Aviation_1.3.0.12/eccairs-descriptive-factors#category_11530100"/>
    </owl:Class>
    


    <!-- http://onto.fel.cvut.cz/ontologies/aviation-safety/Aerodynamic_Load_Alleviating -->

    <owl:Class rdf:about="&m;Aerodynamic_Load_Alleviating">
        <rdfs:subClassOf rdf:resource="&m;autoflight_system"/>
        <all2:has_ATA_code rdf:datatype="&xsd;integer">2250</all2:has_ATA_code>
    </owl:Class>
    


    <!-- http://onto.fel.cvut.cz/ontologies/aviation-safety/Aerodynamic_load_alleviation -->

    <owl:Class rdf:about="&m;Aerodynamic_load_alleviation">
        <rdfs:label>Aerodynamic load alleviation</rdfs:label>
        <rdfs:subClassOf rdf:resource="&m;autoflight_system"/>
        <m:generated_time rdf:datatype="&xsd;dateTime">2015-04-09T18:56:27.771+02:00</m:generated_time>
        <rdfs:comment xml:lang="en">(ATA Code:2250) Aerodynamic load alleviation: The system that corrects and provides for gust loading/upset, aerodynamic augmentation, alleviation, suppression and ride control automatically. This includes sensing, computing, actuating, indicating, internal monitoring and warning devices.</rdfs:comment>
        <m:has_related_eccairs_term rdf:resource="http://onto.fel.cvut.cz/ontologies/2014/ECCAIRS_Aviation_1.3.0.12/eccairs-descriptive-factors#category_11225000"/>
    </owl:Class>
    


    <!-- http://onto.fel.cvut.cz/ontologies/aviation-safety/Aerofoil_anti-de-ice_system -->

    <owl:Class rdf:about="&m;Aerofoil_anti-de-ice_system">
        <rdfs:label>Aerofoil anti/de-ice system</rdfs:label>
        <rdfs:subClassOf rdf:resource="&m;Ice-rain_protection_systems"/>
        <m:generated_time rdf:datatype="&xsd;dateTime">2015-04-09T18:56:27.771+02:00</m:generated_time>
        <rdfs:comment xml:lang="en">(ATA Code:3010) Aerofoil anti/de-ice system: The system components and parts including the boots which provide for wing and empennage leading edge ice prevention or removal. Does not include ducts upstream of the aerofoil control/selector valves. Typical parts are timer, valve, switch, hose, flow valve, duct, duct coupling and thermostat.</rdfs:comment>
        <m:has_related_eccairs_term rdf:resource="http://onto.fel.cvut.cz/ontologies/2014/ECCAIRS_Aviation_1.3.0.12/eccairs-descriptive-factors#category_11301000"/>
    </owl:Class>
    


    <!-- http://onto.fel.cvut.cz/ontologies/aviation-safety/Agricultural_equipment -->

    <owl:Class rdf:about="&m;Agricultural_equipment">
        <rdfs:label>Agricultural equipment</rdfs:label>
        <rdfs:subClassOf rdf:resource="&m;Cabin_equipment-furnishings"/>
        <m:generated_time rdf:datatype="&xsd;dateTime">2015-04-09T18:56:27.771+02:00</m:generated_time>
        <rdfs:comment xml:lang="en">(ATA Code:2591) Agricultural equipment: The additional special equipment attached to an aircraft to equip it for specific agricultural work.</rdfs:comment>
        <m:has_related_eccairs_term rdf:resource="http://onto.fel.cvut.cz/ontologies/2014/ECCAIRS_Aviation_1.3.0.12/eccairs-descriptive-factors#category_11259100"/>
    </owl:Class>
    


    <!-- http://onto.fel.cvut.cz/ontologies/aviation-safety/Agricultural_spray_system -->

    <owl:Class rdf:about="&m;Agricultural_spray_system">
        <rdfs:label>Agricultural spray system</rdfs:label>
        <rdfs:subClassOf rdf:resource="&m;Cargo_compartments_part"/>
        <m:generated_time rdf:datatype="&xsd;dateTime">2015-04-09T18:56:27.771+02:00</m:generated_time>
        <rdfs:comment xml:lang="en">(ATA Code:5011) Agricultural spray system includes equipment such as hopper, tank, spray nozzle, boom, pump, bracket, valve.</rdfs:comment>
        <rdfs:comment xml:lang="en">(ATA Code:5011) Agricultural spray system: The aerial application equipment such as hopper, tank, spray nozzle, boom, pump, bracket and valves.</rdfs:comment>
        <m:has_related_eccairs_term rdf:resource="http://onto.fel.cvut.cz/ontologies/2014/ECCAIRS_Aviation_1.3.0.12/eccairs-descriptive-factors#category_11251200"/>
        <m:has_related_eccairs_term rdf:resource="http://onto.fel.cvut.cz/ontologies/2014/ECCAIRS_Aviation_1.3.0.12/eccairs-descriptive-factors#category_11501100"/>
    </owl:Class>
    


    <!-- http://onto.fel.cvut.cz/ontologies/aviation-safety/Aileron_&amp;_Tab_control_system -->

    <owl:Class rdf:about="&m;Aileron_&amp;_Tab_control_system">
        <rdfs:label>Aileron &amp; Tab control system</rdfs:label>
        <rdfs:subClassOf rdf:resource="&m;Flight_control_system_part"/>
        <m:generated_time rdf:datatype="&xsd;dateTime">2015-04-09T18:56:27.771+02:00</m:generated_time>
        <rdfs:comment xml:lang="en">(ATA Code:2710) Aileron control system: The portion of the systems which controls the position and movement of the aileron. Includes items such as the control column, tab control wheel, cables, boosters, linkages, control surfaces and position indicators.Aileron: A control surface on fixed-wing aircraft, usually mounted on the aft edge of wings, that controls roll, and is controlled by the wheel</rdfs:comment>
        <m:has_related_eccairs_term rdf:resource="http://onto.fel.cvut.cz/ontologies/2014/ECCAIRS_Aviation_1.3.0.12/eccairs-descriptive-factors#category_11271000"/>
    </owl:Class>
    


    <!-- http://onto.fel.cvut.cz/ontologies/aviation-safety/Aileron_&amp;_Tab_control_system_part -->

    <owl:Class rdf:about="&m;Aileron_&amp;_Tab_control_system_part">
        <rdfs:label>Aileron &amp; Tab control system part</rdfs:label>
        <rdfs:subClassOf rdf:resource="&m;Flight_control_system_part"/>
        <rdfs:subClassOf>
            <owl:Restriction>
                <owl:onProperty rdf:resource="http://onto.fel.cvut.cz/ontologies/ufo/is_part_of"/>
                <owl:someValuesFrom rdf:resource="&m;Aileron_&amp;_Tab_control_system"/>
            </owl:Restriction>
        </rdfs:subClassOf>
        <m:generated_time rdf:datatype="&xsd;dateTime">2015-04-12T02:45:54.351+02:00</m:generated_time>
        <m:has_related_eccairs_term rdf:resource="http://onto.fel.cvut.cz/ontologies/2014/ECCAIRS_Aviation_1.3.0.12/eccairs-descriptive-factors#category_11271000"/>
    </owl:Class>
    


    <!-- http://onto.fel.cvut.cz/ontologies/aviation-safety/Aileron_structure -->

    <owl:Class rdf:about="&m;Aileron_structure">
        <rdfs:label>Aileron structure</rdfs:label>
        <rdfs:subClassOf rdf:resource="&m;Ailerons_and_Elevons_part"/>
        <m:generated_time rdf:datatype="&xsd;dateTime">2015-04-09T18:56:27.771+02:00</m:generated_time>
        <rdfs:comment xml:lang="en">(ATA Code:5761) Aileron structure: The structural aspects of the aileron mounted on the trailing edge of wing. Includes hinges and balance weights. Does not include operating mechanism.</rdfs:comment>
        <m:has_related_eccairs_term rdf:resource="http://onto.fel.cvut.cz/ontologies/2014/ECCAIRS_Aviation_1.3.0.12/eccairs-descriptive-factors#category_11576100"/>
    </owl:Class>
    


    <!-- http://onto.fel.cvut.cz/ontologies/aviation-safety/Aileron_tab_control_system -->

    <owl:Class rdf:about="&m;Aileron_tab_control_system">
        <rdfs:label>Aileron tab control system</rdfs:label>
        <rdfs:subClassOf rdf:resource="&m;Aileron_&amp;_Tab_control_system_part"/>
        <m:generated_time rdf:datatype="&xsd;dateTime">2015-04-09T18:56:27.771+02:00</m:generated_time>
        <rdfs:comment xml:lang="en">(ATA Code:2711) Aileron tab control system: The system components and parts controlling movement and position of the trim tab on the aileron. Includes the cockpit control. Typical parts are jackscrew, cable, pulley, turnbuckle and stops.</rdfs:comment>
        <m:has_related_eccairs_term rdf:resource="http://onto.fel.cvut.cz/ontologies/2014/ECCAIRS_Aviation_1.3.0.12/eccairs-descriptive-factors#category_11271100"/>
    </owl:Class>
    


    <!-- http://onto.fel.cvut.cz/ontologies/aviation-safety/Aileron_tab_structure -->

    <owl:Class rdf:about="&m;Aileron_tab_structure">
        <rdfs:label>Aileron tab structure</rdfs:label>
        <rdfs:subClassOf rdf:resource="&m;Ailerons_and_Elevons_part"/>
        <m:generated_time rdf:datatype="&xsd;dateTime">2015-04-09T18:56:27.771+02:00</m:generated_time>
        <rdfs:comment xml:lang="en">(ATA Code:5752) Aileron tab structure: The surface mounted at the trailing edge of the aileron for lateral trim. Typical parts are spar, skin, hinge, bracket, bolt and bearings,</rdfs:comment>
        <m:has_related_eccairs_term rdf:resource="http://onto.fel.cvut.cz/ontologies/2014/ECCAIRS_Aviation_1.3.0.12/eccairs-descriptive-factors#category_11576200"/>
    </owl:Class>
    


    <!-- http://onto.fel.cvut.cz/ontologies/aviation-safety/Aileron_trim_system -->

    <owl:Class rdf:about="&m;Aileron_trim_system">
        <rdfs:label>Aileron trim system</rdfs:label>
        <rdfs:subClassOf rdf:resource="&m;Aileron_&amp;_Tab_control_system_part"/>
        <m:generated_time rdf:datatype="&xsd;dateTime">2015-04-09T18:56:27.771+02:00</m:generated_time>
        <rdfs:comment xml:lang="en">(ATA Code:2712) Aileron trim system: The system components and parts controlling movement and position of the trim tab on the aileron. Includes the cockpit control. Typical parts are jackscrew, cable, pulley, turnbuckle and stops.</rdfs:comment>
        <m:has_related_eccairs_term rdf:resource="http://onto.fel.cvut.cz/ontologies/2014/ECCAIRS_Aviation_1.3.0.12/eccairs-descriptive-factors#category_11271200"/>
    </owl:Class>
    


    <!-- http://onto.fel.cvut.cz/ontologies/aviation-safety/Ailerons_and_Elevons -->

    <owl:Class rdf:about="&m;Ailerons_and_Elevons">
        <rdfs:label>Ailerons and Elevons</rdfs:label>
        <rdfs:subClassOf rdf:resource="&m;Wing_structure_part"/>
        <m:generated_time rdf:datatype="&xsd;dateTime">2015-04-09T18:56:27.771+02:00</m:generated_time>
        <rdfs:comment xml:lang="en">(ATA Code:5760) Ailerons and Elevons The skins and structure of ailerons and elevons and tabs including balancing devices and attachment fittings.</rdfs:comment>
        <m:has_related_eccairs_term rdf:resource="http://onto.fel.cvut.cz/ontologies/2014/ECCAIRS_Aviation_1.3.0.12/eccairs-descriptive-factors#category_11576000"/>
    </owl:Class>
    


    <!-- http://onto.fel.cvut.cz/ontologies/aviation-safety/Ailerons_and_Elevons_part -->

    <owl:Class rdf:about="&m;Ailerons_and_Elevons_part">
        <rdfs:label>Ailerons and Elevons part</rdfs:label>
        <rdfs:subClassOf rdf:resource="&m;Wing_structure_part"/>
        <rdfs:subClassOf>
            <owl:Restriction>
                <owl:onProperty rdf:resource="http://onto.fel.cvut.cz/ontologies/ufo/is_part_of"/>
                <owl:someValuesFrom rdf:resource="&m;Ailerons_and_Elevons"/>
            </owl:Restriction>
        </rdfs:subClassOf>
        <m:generated_time rdf:datatype="&xsd;dateTime">2015-04-12T02:45:54.351+02:00</m:generated_time>
        <m:has_related_eccairs_term rdf:resource="http://onto.fel.cvut.cz/ontologies/2014/ECCAIRS_Aviation_1.3.0.12/eccairs-descriptive-factors#category_11576000"/>
    </owl:Class>
    


    <!-- http://onto.fel.cvut.cz/ontologies/aviation-safety/Air_Conditioning_System_Wiring -->

    <owl:Class rdf:about="&m;Air_Conditioning_System_Wiring">
        <rdfs:subClassOf rdf:resource="&m;Air_conditioning_system_part"/>
    </owl:Class>
    


    <!-- http://onto.fel.cvut.cz/ontologies/aviation-safety/Air_conditioning_compartment_doors -->

    <owl:Class rdf:about="&m;Air_conditioning_compartment_doors">
        <rdfs:label>Air conditioning compartment doors</rdfs:label>
        <rdfs:subClassOf rdf:resource="&m;Service_doors_part"/>
        <m:generated_time rdf:datatype="&xsd;dateTime">2015-04-09T18:56:27.771+02:00</m:generated_time>
        <rdfs:comment xml:lang="en">(ATA Code:5245) Air conditioning compartment doors: The exterior doors used primarily to gain access for servicing the air conditioning compartment system and components. Typical parts are hinges, structure and the latch mechanism.</rdfs:comment>
        <m:has_related_eccairs_term rdf:resource="http://onto.fel.cvut.cz/ontologies/2014/ECCAIRS_Aviation_1.3.0.12/eccairs-descriptive-factors#category_11524500"/>
    </owl:Class>
    


    <!-- http://onto.fel.cvut.cz/ontologies/aviation-safety/Air_conditioning_system -->

    <owl:Class rdf:about="&m;Air_conditioning_system">
        <rdfs:label xml:lang="en">Air conditioning system</rdfs:label>
        <rdfs:subClassOf rdf:resource="&m;Aircraft_part"/>
    </owl:Class>
    


    <!-- http://onto.fel.cvut.cz/ontologies/aviation-safety/Air_conditioning_system_part -->

    <owl:Class rdf:about="&m;Air_conditioning_system_part">
        <rdfs:label>Air conditioning system part</rdfs:label>
        <rdfs:subClassOf rdf:resource="&m;Aircraft_part"/>
        <rdfs:subClassOf>
            <owl:Restriction>
                <owl:onProperty rdf:resource="http://onto.fel.cvut.cz/ontologies/ufo/is_part_of"/>
                <owl:someValuesFrom rdf:resource="&m;Air_conditioning_system"/>
            </owl:Restriction>
        </rdfs:subClassOf>
        <m:generated_time rdf:datatype="&xsd;dateTime">2015-04-12T02:45:54.351+02:00</m:generated_time>
        <m:has_related_eccairs_term rdf:resource="http://onto.fel.cvut.cz/ontologies/2014/ECCAIRS_Aviation_1.3.0.12/eccairs-descriptive-factors#category_11210000"/>
    </owl:Class>
    


    <!-- http://onto.fel.cvut.cz/ontologies/aviation-safety/Air_conditioning_system_wiring -->

    <owl:Class rdf:about="&m;Air_conditioning_system_wiring">
        <rdfs:subClassOf rdf:resource="&m;Air_conditioning_system_part"/>
    </owl:Class>
    


    <!-- http://onto.fel.cvut.cz/ontologies/aviation-safety/Air_data_computer -->

    <owl:Class rdf:about="&m;Air_data_computer">
        <rdfs:label>Air data computer</rdfs:label>
        <rdfs:subClassOf rdf:resource="&m;Flight_environment_data_system"/>
        <m:generated_time rdf:datatype="&xsd;dateTime">2015-04-09T18:56:27.771+02:00</m:generated_time>
        <rdfs:comment xml:lang="en">(ATA Code:3417) Air data computer: The computer and its integral parts which receives data from various environmental sensing systems, computes this data and makes it available to the various navigation systems. Does not include external hardware such as cables, mounting racks and remote switches. [Code 11341000].Air data computer: A primary navigation data source. A navigation sensor based on atmospheric data sensors; usually measures static pressure, dynamic pressure, and outside air temperature; sometimes computes other atmospheric data, such as indicated airspeed, Mach number, calibrated airspeed</rdfs:comment>
        <m:has_related_eccairs_term rdf:resource="http://onto.fel.cvut.cz/ontologies/2014/ECCAIRS_Aviation_1.3.0.12/eccairs-descriptive-factors#category_11341700"/>
    </owl:Class>
    


    <!-- http://onto.fel.cvut.cz/ontologies/aviation-safety/Air_distribution_fan -->

    <owl:Class rdf:about="&m;Air_distribution_fan">
        <rdfs:label>Air distribution fan</rdfs:label>
        <rdfs:subClassOf rdf:resource="&m;Air_conditioning_system_part"/>
        <rdfs:subClassOf rdf:resource="&m;Air_distribution_system_part"/>
        <m:generated_time rdf:datatype="&xsd;dateTime">2015-04-09T18:56:27.771+02:00</m:generated_time>
        <all2:has_ATA_code rdf:datatype="&xsd;integer">2121</all2:has_ATA_code>
        <rdfs:comment xml:lang="en">(ATA Code:2121) Air distribution fan: Includes associated motor which distributes air within the confines for comfort or equipment cooling. Typical parts are bearings, bushings and motors.</rdfs:comment>
        <m:has_related_eccairs_term rdf:resource="http://onto.fel.cvut.cz/ontologies/2014/ECCAIRS_Aviation_1.3.0.12/eccairs-descriptive-factors#category_11212100"/>
    </owl:Class>
    


    <!-- http://onto.fel.cvut.cz/ontologies/aviation-safety/Air_distribution_system -->

    <owl:Class rdf:about="&m;Air_distribution_system">
        <rdfs:label>Air distribution system</rdfs:label>
        <rdfs:subClassOf rdf:resource="&m;Air_conditioning_system_part"/>
        <m:generated_time rdf:datatype="&xsd;dateTime">2015-04-09T18:56:27.771+02:00</m:generated_time>
        <all2:has_ATA_code rdf:datatype="&xsd;integer">2120</all2:has_ATA_code>
        <rdfs:comment xml:lang="en">(ATA Code:2120) That portion of the system used to induct and distribute air. Includes equipment rack cooling systems and items such as blowers, scoops, ducting, inlets, check valves, wiring, etc. Does not include valves which are part of pressurization and temperature control.</rdfs:comment>
        <m:has_related_eccairs_term rdf:resource="http://onto.fel.cvut.cz/ontologies/2014/ECCAIRS_Aviation_1.3.0.12/eccairs-descriptive-factors#category_11212000"/>
    </owl:Class>
    


    <!-- http://onto.fel.cvut.cz/ontologies/aviation-safety/Air_distribution_system_part -->

    <owl:Class rdf:about="&m;Air_distribution_system_part">
        <rdfs:label>Air distribution system part</rdfs:label>
        <rdfs:subClassOf rdf:resource="&m;Air_conditioning_system_part"/>
        <rdfs:subClassOf>
            <owl:Restriction>
                <owl:onProperty rdf:resource="http://onto.fel.cvut.cz/ontologies/ufo/is_part_of"/>
                <owl:someValuesFrom rdf:resource="&m;Air_distribution_system"/>
            </owl:Restriction>
        </rdfs:subClassOf>
        <m:generated_time rdf:datatype="&xsd;dateTime">2015-04-12T02:45:54.351+02:00</m:generated_time>
        <m:has_related_eccairs_term rdf:resource="http://onto.fel.cvut.cz/ontologies/2014/ECCAIRS_Aviation_1.3.0.12/eccairs-descriptive-factors#category_11212000"/>
    </owl:Class>
    


    <!-- http://onto.fel.cvut.cz/ontologies/aviation-safety/Air_intake_anti-de-ice_system -->

    <owl:Class rdf:about="&m;Air_intake_anti-de-ice_system">
        <rdfs:label>Air intake anti/de-ice system</rdfs:label>
        <rdfs:subClassOf rdf:resource="&m;Ice-rain_protection_systems"/>
        <m:generated_time rdf:datatype="&xsd;dateTime">2015-04-09T18:56:27.771+02:00</m:generated_time>
        <rdfs:comment xml:lang="en">(ATA Code:3020) Air intake anti/de-ice system: The system and components which eliminate or prevent the formation of ice in or around air intakes such as turbine engine cowling. Does not include engine anti-icing reports [Code 11751000]. Includes the electrically heated boot at the air intake lips.</rdfs:comment>
        <m:has_related_eccairs_term rdf:resource="http://onto.fel.cvut.cz/ontologies/2014/ECCAIRS_Aviation_1.3.0.12/eccairs-descriptive-factors#category_11302000"/>
    </owl:Class>
    


    <!-- http://onto.fel.cvut.cz/ontologies/aviation-safety/Air_supply_(water_pressure_system) -->

    <owl:Class rdf:about="&m;Air_supply_(water_pressure_system)">
        <rdfs:label>Air supply (water pressure system)</rdfs:label>
        <rdfs:subClassOf rdf:resource="&m;Water_and_waste_system_part"/>
        <m:generated_time rdf:datatype="&xsd;dateTime">2015-04-09T18:56:27.771+02:00</m:generated_time>
        <rdfs:comment xml:lang="en">(ATA Code:3840) Air supply (water pressure system): The system which provides the pressure to distribute potable water to the lavatories. Typical parts are pump, motor and lines.</rdfs:comment>
        <m:has_related_eccairs_term rdf:resource="http://onto.fel.cvut.cz/ontologies/2014/ECCAIRS_Aviation_1.3.0.12/eccairs-descriptive-factors#category_11384000"/>
    </owl:Class>
    


    <!-- http://onto.fel.cvut.cz/ontologies/aviation-safety/Airborne_auxiliary_power_unit_system -->

    <owl:Class rdf:about="&m;Airborne_auxiliary_power_unit_system">
        <rdfs:label>Airborne auxiliary power unit system</rdfs:label>
        <rdfs:subClassOf rdf:resource="&m;Aircraft_part"/>
        <m:generated_time rdf:datatype="&xsd;dateTime">2015-04-09T18:56:27.771+02:00</m:generated_time>
        <rdfs:comment xml:lang="en">(ATA Code:4900) The airborne auxiliary power units installed on aircraft for the purpose of generating and supplying a single type or combination of auxiliary electric, hydraulic, pneumatic or other power. Does not include generators, alternators or hydraulic pumps, or their connecting systems which supply and deliver power to their respective aircraft systems. Auxiliary power-unit (APU). A self-contained power-unit on an aircraft providing electrical/pneumatic power to aircraft systems during ground operations.(ICAO Annex 16)</rdfs:comment>
        <m:has_related_eccairs_term rdf:resource="http://onto.fel.cvut.cz/ontologies/2014/ECCAIRS_Aviation_1.3.0.12/eccairs-descriptive-factors#category_11490000"/>
    </owl:Class>
    


    <!-- http://onto.fel.cvut.cz/ontologies/aviation-safety/Airborne_auxiliary_power_unit_system_part -->

    <owl:Class rdf:about="&m;Airborne_auxiliary_power_unit_system_part">
        <rdfs:label>Airborne auxiliary power unit system part</rdfs:label>
        <rdfs:subClassOf rdf:resource="&m;Aircraft_part"/>
        <rdfs:subClassOf>
            <owl:Restriction>
                <owl:onProperty rdf:resource="http://onto.fel.cvut.cz/ontologies/ufo/is_part_of"/>
                <owl:someValuesFrom rdf:resource="&m;Airborne_auxiliary_power_unit_system"/>
            </owl:Restriction>
        </rdfs:subClassOf>
        <m:generated_time rdf:datatype="&xsd;dateTime">2015-04-12T02:45:54.351+02:00</m:generated_time>
        <m:has_related_eccairs_term rdf:resource="http://onto.fel.cvut.cz/ontologies/2014/ECCAIRS_Aviation_1.3.0.12/eccairs-descriptive-factors#category_11490000"/>
    </owl:Class>
    


    <!-- http://onto.fel.cvut.cz/ontologies/aviation-safety/Airborne_element_of_ATM -->

    <owl:Class rdf:about="&m;Airborne_element_of_ATM"/>
    


    <!-- http://onto.fel.cvut.cz/ontologies/aviation-safety/Aircraft_communication_related_system -->

    <owl:Class rdf:about="&m;Aircraft_communication_related_system">
        <rdfs:label xml:lang="en">Aircraft communication related system</rdfs:label>
        <rdfs:subClassOf rdf:resource="&m;Aircraft_part"/>
        <rdfs:subClassOf rdf:resource="&m;Communication_related_system"/>
        <m:generated_time rdf:datatype="&xsd;dateTime">2015-04-12T02:45:54.351+02:00</m:generated_time>
        <m:has_related_eccairs_term rdf:resource="http://onto.fel.cvut.cz/ontologies/2014/ECCAIRS_Aviation_1.3.0.12/eccairs-descriptive-factors#category_11230000"/>
    </owl:Class>
    


    <!-- http://onto.fel.cvut.cz/ontologies/aviation-safety/Aircraft_fuel_system -->

    <owl:Class rdf:about="&m;Aircraft_fuel_system">
        <rdfs:label>Aircraft fuel system</rdfs:label>
        <rdfs:subClassOf rdf:resource="&m;Aircraft_part"/>
        <m:generated_time rdf:datatype="&xsd;dateTime">2015-04-09T18:56:27.771+02:00</m:generated_time>
        <rdfs:comment xml:lang="en">(ATA Code:2800) Aircraft fuel system: The units and components storing and delivering fuel to the engine. Includes the integral tank leak detection and sealing. Does not include the structure of integral, tip fuel tanks, fuel cell backing boards, or the fuel flow rate sensing, transmitting, or indicating systems.</rdfs:comment>
        <m:has_related_eccairs_term rdf:resource="http://onto.fel.cvut.cz/ontologies/2014/ECCAIRS_Aviation_1.3.0.12/eccairs-descriptive-factors#category_11280000"/>
    </owl:Class>
    


    <!-- http://onto.fel.cvut.cz/ontologies/aviation-safety/Aircraft_fuel_system_part -->

    <owl:Class rdf:about="&m;Aircraft_fuel_system_part">
        <rdfs:label>Aircraft fuel system part</rdfs:label>
        <rdfs:subClassOf rdf:resource="&m;Aircraft_part"/>
        <rdfs:subClassOf>
            <owl:Restriction>
                <owl:onProperty rdf:resource="http://onto.fel.cvut.cz/ontologies/ufo/is_part_of"/>
                <owl:someValuesFrom rdf:resource="&m;Aircraft_fuel_system"/>
            </owl:Restriction>
        </rdfs:subClassOf>
        <m:generated_time rdf:datatype="&xsd;dateTime">2015-04-12T02:45:54.351+02:00</m:generated_time>
        <m:has_related_eccairs_term rdf:resource="http://onto.fel.cvut.cz/ontologies/2014/ECCAIRS_Aviation_1.3.0.12/eccairs-descriptive-factors#category_11280000"/>
    </owl:Class>
    


    <!-- http://onto.fel.cvut.cz/ontologies/aviation-safety/Aircraft_fuels_and_any_additives_in_the_fuel -->

    <owl:Class rdf:about="&m;Aircraft_fuels_and_any_additives_in_the_fuel">
        <rdfs:label>Aircraft fuels and any additives in the fuel</rdfs:label>
        <rdfs:subClassOf rdf:resource="&m;Aircraft_fuel_system_part"/>
        <m:generated_time rdf:datatype="&xsd;dateTime">2015-04-09T18:56:27.771+02:00</m:generated_time>
        <rdfs:comment xml:lang="en">(ATA Code:2805) The aircraft fuels and any additives contained in the fuel.</rdfs:comment>
        <m:has_related_eccairs_term rdf:resource="http://onto.fel.cvut.cz/ontologies/2014/ECCAIRS_Aviation_1.3.0.12/eccairs-descriptive-factors#category_11280500"/>
    </owl:Class>
    


    <!-- http://onto.fel.cvut.cz/ontologies/aviation-safety/Aircraft_general_information_system -->

    <owl:Class rdf:about="&m;Aircraft_general_information_system">
        <rdfs:label>Aircraft general information system</rdfs:label>
        <rdfs:subClassOf rdf:resource="&m;Information_system_part"/>
        <m:generated_time rdf:datatype="&xsd;dateTime">2015-04-09T18:56:27.771+02:00</m:generated_time>
        <rdfs:comment xml:lang="en">(ATA Code:4610) Aircraft general information system: The units and components which furnish a means of storing, updating and retrieving digital information on the aircraft, that are traditionally provided on paper, microfilm, or microfiche. Includes units that are dedicated to the information storage and retrieval function such as the electronic library mass storage and controller.</rdfs:comment>
        <m:has_related_eccairs_term rdf:resource="http://onto.fel.cvut.cz/ontologies/2014/ECCAIRS_Aviation_1.3.0.12/eccairs-descriptive-factors#category_11461000"/>
    </owl:Class>
    


    <!-- http://onto.fel.cvut.cz/ontologies/aviation-safety/Aircraft_part -->

    <owl:Class rdf:about="&m;Aircraft_part"/>
    


    <!-- http://onto.fel.cvut.cz/ontologies/aviation-safety/Aircraft_structures -->

    <owl:Class rdf:about="&m;Aircraft_structures">
        <rdfs:label>Aircraft structures</rdfs:label>
        <rdfs:subClassOf rdf:resource="&m;STANDARD_PRACTICES_AND_STRUCTURES_-_GENERAL_part"/>
        <m:generated_time rdf:datatype="&xsd;dateTime">2015-04-09T18:56:27.771+02:00</m:generated_time>
        <rdfs:comment xml:lang="en">(ATA Code:5101) Aircraft structures: Repairs to aircraft structures of a general nature.</rdfs:comment>
        <m:has_related_eccairs_term rdf:resource="http://onto.fel.cvut.cz/ontologies/2014/ECCAIRS_Aviation_1.3.0.12/eccairs-descriptive-factors#category_11510100"/>
    </owl:Class>
    


    <!-- http://onto.fel.cvut.cz/ontologies/aviation-safety/Airspeed-Mach_indication -->

    <owl:Class rdf:about="&m;Airspeed-Mach_indication">
        <rdfs:label>Airspeed/Mach indication</rdfs:label>
        <rdfs:subClassOf rdf:resource="&m;Flight_environment_data_system"/>
        <m:generated_time rdf:datatype="&xsd;dateTime">2015-04-09T18:56:27.771+02:00</m:generated_time>
        <rdfs:comment xml:lang="en">(ATA Code:3414) Airspeed/Mach indication: The instrument which measures and indicates speed of the aircraft. Does not include the doppler indicator [Code 11344300].</rdfs:comment>
        <m:has_related_eccairs_term rdf:resource="http://onto.fel.cvut.cz/ontologies/2014/ECCAIRS_Aviation_1.3.0.12/eccairs-descriptive-factors#category_11341400"/>
    </owl:Class>
    


    <!-- http://onto.fel.cvut.cz/ontologies/aviation-safety/Alternating_current_generation_system -->

    <owl:Class rdf:about="&m;Alternating_current_generation_system">
        <rdfs:label>Alternating current generation system</rdfs:label>
        <rdfs:subClassOf rdf:resource="&m;Electrical_power_system_part"/>
        <m:generated_time rdf:datatype="&xsd;dateTime">2015-04-09T18:56:27.771+02:00</m:generated_time>
        <rdfs:comment xml:lang="en">(ATA Code:2420) Alternating current generation system: The systems used to generate, regulate, control and indicate alternating current electrical power. Includes items such as inverters, alternating current generators/alternators, control and regulating components, indicating systems and all wiring to but not including main busses.</rdfs:comment>
        <m:has_related_eccairs_term rdf:resource="http://onto.fel.cvut.cz/ontologies/2014/ECCAIRS_Aviation_1.3.0.12/eccairs-descriptive-factors#category_11242000"/>
    </owl:Class>
    


    <!-- http://onto.fel.cvut.cz/ontologies/aviation-safety/Alternating_current_generation_system_part -->

    <owl:Class rdf:about="&m;Alternating_current_generation_system_part">
        <rdfs:label>Alternating current generation system part</rdfs:label>
        <rdfs:subClassOf rdf:resource="&m;Electrical_power_system_part"/>
        <rdfs:subClassOf>
            <owl:Restriction>
                <owl:onProperty rdf:resource="http://onto.fel.cvut.cz/ontologies/ufo/is_part_of"/>
                <owl:someValuesFrom rdf:resource="&m;Alternating_current_generation_system"/>
            </owl:Restriction>
        </rdfs:subClassOf>
        <m:generated_time rdf:datatype="&xsd;dateTime">2015-04-12T02:45:54.351+02:00</m:generated_time>
        <m:has_related_eccairs_term rdf:resource="http://onto.fel.cvut.cz/ontologies/2014/ECCAIRS_Aviation_1.3.0.12/eccairs-descriptive-factors#category_11242000"/>
    </owl:Class>
    


    <!-- http://onto.fel.cvut.cz/ontologies/aviation-safety/Alternating_current_generator_-_alternator -->

    <owl:Class rdf:about="&m;Alternating_current_generator_-_alternator">
        <rdfs:label>Alternating current generator - alternator</rdfs:label>
        <rdfs:subClassOf rdf:resource="&m;Alternating_current_generation_system_part"/>
        <m:generated_time rdf:datatype="&xsd;dateTime">2015-04-09T18:56:27.771+02:00</m:generated_time>
        <rdfs:comment xml:lang="en">(ATA Code:2421) Alternating current generator - alternator: The engine driven component that generates alternating current for aircraft with alternating current electrical systems. Does not include alternating current alternators on light piston-engine power aircraft with direct current electrical systems.</rdfs:comment>
        <m:has_related_eccairs_term rdf:resource="http://onto.fel.cvut.cz/ontologies/2014/ECCAIRS_Aviation_1.3.0.12/eccairs-descriptive-factors#category_11242100"/>
    </owl:Class>
    


    <!-- http://onto.fel.cvut.cz/ontologies/aviation-safety/Alternating_current_indicating_system -->

    <owl:Class rdf:about="&m;Alternating_current_indicating_system">
        <rdfs:label>Alternating current indicating system</rdfs:label>
        <rdfs:subClassOf rdf:resource="&m;Alternating_current_generation_system_part"/>
        <m:generated_time rdf:datatype="&xsd;dateTime">2015-04-09T18:56:27.771+02:00</m:generated_time>
        <rdfs:comment xml:lang="en">(ATA Code:2425) Alternating current indicating system: The equipment indicating, voltage, current flow and system faults in the alternating current power systems.</rdfs:comment>
        <m:has_related_eccairs_term rdf:resource="http://onto.fel.cvut.cz/ontologies/2014/ECCAIRS_Aviation_1.3.0.12/eccairs-descriptive-factors#category_11242500"/>
    </owl:Class>
    


    <!-- http://onto.fel.cvut.cz/ontologies/aviation-safety/Alternating_current_inverter -->

    <owl:Class rdf:about="&m;Alternating_current_inverter">
        <rdfs:label>Alternating current inverter</rdfs:label>
        <rdfs:subClassOf rdf:resource="&m;Alternating_current_generation_system_part"/>
        <m:generated_time rdf:datatype="&xsd;dateTime">2015-04-09T18:56:27.771+02:00</m:generated_time>
        <rdfs:comment xml:lang="en">(ATA Code:2422) Alternating current inverter: The component which converts direct current to alternating current.</rdfs:comment>
        <m:has_related_eccairs_term rdf:resource="http://onto.fel.cvut.cz/ontologies/2014/ECCAIRS_Aviation_1.3.0.12/eccairs-descriptive-factors#category_11242200"/>
    </owl:Class>
    


    <!-- http://onto.fel.cvut.cz/ontologies/aviation-safety/Alternating_current_power_distribution_system -->

    <owl:Class rdf:about="&m;Alternating_current_power_distribution_system">
        <rdfs:label>Alternating current power distribution system</rdfs:label>
        <rdfs:subClassOf rdf:resource="&m;Electrical_power_system_part"/>
        <m:generated_time rdf:datatype="&xsd;dateTime">2015-04-09T18:56:27.771+02:00</m:generated_time>
        <rdfs:comment xml:lang="en">(ATA Code:2450) Alternating current power distribution system: The electrical system which provides for connection of alternating current to using systems. Does not include the using system. Typical parts are main and secondary system bus, circuit breaker, limiter, jumper and load meter switch.</rdfs:comment>
        <m:has_related_eccairs_term rdf:resource="http://onto.fel.cvut.cz/ontologies/2014/ECCAIRS_Aviation_1.3.0.12/eccairs-descriptive-factors#category_11245000"/>
    </owl:Class>
    


    <!-- http://onto.fel.cvut.cz/ontologies/aviation-safety/Alternating_current_voltage_regulator -->

    <owl:Class rdf:about="&m;Alternating_current_voltage_regulator">
        <rdfs:label>Alternating current voltage regulator</rdfs:label>
        <rdfs:subClassOf rdf:resource="&m;Alternating_current_generation_system_part"/>
        <m:generated_time rdf:datatype="&xsd;dateTime">2015-04-09T18:56:27.771+02:00</m:generated_time>
        <rdfs:comment xml:lang="en">(ATA Code:2424) Alternating current voltage regulator: The component that regulates the alternating current voltage from the alternator-generator to maintain a set voltage output for the using systems i.e. generator control unit.</rdfs:comment>
        <m:has_related_eccairs_term rdf:resource="http://onto.fel.cvut.cz/ontologies/2014/ECCAIRS_Aviation_1.3.0.12/eccairs-descriptive-factors#category_11242400"/>
    </owl:Class>
    


    <!-- http://onto.fel.cvut.cz/ontologies/aviation-safety/Alternator-generator_drive -->

    <owl:Class rdf:about="&m;Alternator-generator_drive">
        <rdfs:label>Alternator-generator drive</rdfs:label>
        <rdfs:subClassOf rdf:resource="&m;Electrical_power_system_part"/>
        <m:generated_time rdf:datatype="&xsd;dateTime">2015-04-09T18:56:27.771+02:00</m:generated_time>
        <rdfs:comment xml:lang="en">(ATA Code:2410) Alternator-generator drive: The alternator and generator drives mounted on reciprocating engines. Does not include alternator cases. Typical parts are bracket, pulley, belt, link, idler pulley, bolt, drive shaft and gears that stay with the alternator. Includes constant speed drive unit mounted on turbine engines to drive alternating current producing alternators at a predetermined and constant RPM. Typical parts are shaft seal and shafts.</rdfs:comment>
        <m:has_related_eccairs_term rdf:resource="http://onto.fel.cvut.cz/ontologies/2014/ECCAIRS_Aviation_1.3.0.12/eccairs-descriptive-factors#category_11241000"/>
    </owl:Class>
    


    <!-- http://onto.fel.cvut.cz/ontologies/aviation-safety/Altitude_controller -->

    <owl:Class rdf:about="&m;Altitude_controller">
        <rdfs:label>Altitude controller</rdfs:label>
        <rdfs:subClassOf rdf:resource="&m;Autopilot_system_part"/>
        <m:generated_time rdf:datatype="&xsd;dateTime">2015-04-09T18:56:27.771+02:00</m:generated_time>
        <all2:has_ATA_code rdf:datatype="&xsd;integer">2212</all2:has_ATA_code>
        <rdfs:comment xml:lang="en">(ATA Code:2212) Altitude controller: The units transmitting output information signals to maintain a predetermined altitude, rate of climb or descent automatically. Does not include the connecting system parts such as the sensor switch.</rdfs:comment>
        <m:has_related_eccairs_term rdf:resource="http://onto.fel.cvut.cz/ontologies/2014/ECCAIRS_Aviation_1.3.0.12/eccairs-descriptive-factors#category_11221200"/>
    </owl:Class>
    


    <!-- http://onto.fel.cvut.cz/ontologies/aviation-safety/Antenna-radome_anti-ice-de-ice_system -->

    <owl:Class rdf:about="&m;Antenna-radome_anti-ice-de-ice_system">
        <rdfs:label>Antenna/radome anti-ice/de-ice system</rdfs:label>
        <rdfs:subClassOf rdf:resource="&m;Ice-rain_protection_systems"/>
        <m:generated_time rdf:datatype="&xsd;dateTime">2015-04-09T18:56:27.771+02:00</m:generated_time>
        <rdfs:comment xml:lang="en">(ATA Code:3050) Antenna/radome anti-ice/de-ice system: The system which is used to remove ice from, or prevent the formation of ice on, antennas and radomes.</rdfs:comment>
        <m:has_related_eccairs_term rdf:resource="http://onto.fel.cvut.cz/ontologies/2014/ECCAIRS_Aviation_1.3.0.12/eccairs-descriptive-factors#category_11305000"/>
    </owl:Class>
    


    <!-- http://onto.fel.cvut.cz/ontologies/aviation-safety/Anti-torque_Rotor_control_(Yaw_control) -->

    <owl:Class rdf:about="&m;Anti-torque_Rotor_control_(Yaw_control)">
        <rdfs:label>Anti-torque Rotor control (Yaw control)</rdfs:label>
        <rdfs:subClassOf rdf:resource="&m;Rotorcraft_flight_control_part"/>
        <m:generated_time rdf:datatype="&xsd;dateTime">2015-04-09T18:56:27.771+02:00</m:generated_time>
        <rdfs:comment xml:lang="en">(ATA Code 6720) That portion of the controls which control the direction of the helicopter (yaw control). Includes items such as tail rotor control pedals, relevant linkage and cable controls, bellcranks constituting the yaw control channel and the control position indicating system.</rdfs:comment>
        <m:has_related_eccairs_term rdf:resource="http://onto.fel.cvut.cz/ontologies/2014/ECCAIRS_Aviation_1.3.0.12/eccairs-descriptive-factors#category_11672000"/>
    </owl:Class>
    


    <!-- http://onto.fel.cvut.cz/ontologies/aviation-safety/Attachment_fitting_(empennage_flight_control_surfaces) -->

    <owl:Class rdf:about="&m;Attachment_fitting_(empennage_flight_control_surfaces)">
        <rdfs:label>Attachment fitting [empennage flight control surfaces]</rdfs:label>
        <rdfs:subClassOf rdf:resource="&m;Empennage_structure_part"/>
        <m:generated_time rdf:datatype="&xsd;dateTime">2015-04-09T18:56:27.771+02:00</m:generated_time>
        <rdfs:comment xml:lang="en">(ATA Code:5550) Attachment fitting [empennage flight control surfaces]: The fittings on the empennage structure which are used for the support of the flight control aerofoils.</rdfs:comment>
        <m:has_related_eccairs_term rdf:resource="http://onto.fel.cvut.cz/ontologies/2014/ECCAIRS_Aviation_1.3.0.12/eccairs-descriptive-factors#category_11555000"/>
    </owl:Class>
    


    <!-- http://onto.fel.cvut.cz/ontologies/aviation-safety/Attachment_fitting_(empennage_flight_control_surfaces)_part -->

    <owl:Class rdf:about="&m;Attachment_fitting_(empennage_flight_control_surfaces)_part">
        <rdfs:label>Attachment fitting [empennage flight control surfaces] part</rdfs:label>
        <rdfs:subClassOf rdf:resource="&m;Empennage_structure_part"/>
        <rdfs:subClassOf>
            <owl:Restriction>
                <owl:onProperty rdf:resource="http://onto.fel.cvut.cz/ontologies/ufo/is_part_of"/>
                <owl:someValuesFrom rdf:resource="&m;Attachment_fitting_(empennage_flight_control_surfaces)"/>
            </owl:Restriction>
        </rdfs:subClassOf>
        <m:generated_time rdf:datatype="&xsd;dateTime">2015-04-12T02:45:54.351+02:00</m:generated_time>
        <m:has_related_eccairs_term rdf:resource="http://onto.fel.cvut.cz/ontologies/2014/ECCAIRS_Aviation_1.3.0.12/eccairs-descriptive-factors#category_11555000"/>
    </owl:Class>
    


    <!-- http://onto.fel.cvut.cz/ontologies/aviation-safety/Attachment_fitting_(nacelle-pylon) -->

    <owl:Class rdf:about="&m;Attachment_fitting_(nacelle-pylon)">
        <rdfs:label>Attachment fitting (nacelle/pylon)</rdfs:label>
        <rdfs:subClassOf rdf:resource="&m;Main_frame_(nacelle-pylon)_part"/>
        <m:generated_time rdf:datatype="&xsd;dateTime">2015-04-09T18:56:27.771+02:00</m:generated_time>
        <rdfs:comment xml:lang="en">(ATA Code:5415) Attachment fitting (nacelle/pylon): The fittings on the nacelles/pylons used for the attachment to its connecting structure, powerplant, thrust reverser and for the support of equipment within the nacelle/pylon.</rdfs:comment>
        <m:has_related_eccairs_term rdf:resource="http://onto.fel.cvut.cz/ontologies/2014/ECCAIRS_Aviation_1.3.0.12/eccairs-descriptive-factors#category_11541500"/>
    </owl:Class>
    


    <!-- http://onto.fel.cvut.cz/ontologies/aviation-safety/Attitude_and_direction_data_system -->

    <owl:Class rdf:about="&m;Attitude_and_direction_data_system">
        <rdfs:label>Attitude and direction data system</rdfs:label>
        <rdfs:subClassOf rdf:resource="&m;Navigation_system"/>
        <m:generated_time rdf:datatype="&xsd;dateTime">2015-04-09T18:56:27.771+02:00</m:generated_time>
        <rdfs:comment xml:lang="en">(ATA Code:3420) Attitude and direction data system: The system components and parts which use magnetic, gyroscopic and inertia forces to indicate an aircraft&apos;s attitude and direction. Includes such items as the inertial reference system.</rdfs:comment>
        <m:has_related_eccairs_term rdf:resource="http://onto.fel.cvut.cz/ontologies/2014/ECCAIRS_Aviation_1.3.0.12/eccairs-descriptive-factors#category_11342000"/>
    </owl:Class>
    


    <!-- http://onto.fel.cvut.cz/ontologies/aviation-safety/Attitude_and_direction_data_system_part -->

    <owl:Class rdf:about="&m;Attitude_and_direction_data_system_part">
        <rdfs:label>Attitude and direction data system part</rdfs:label>
        <rdfs:subClassOf rdf:resource="&m;Navigation_system"/>
        <rdfs:subClassOf>
            <owl:Restriction>
                <owl:onProperty rdf:resource="http://onto.fel.cvut.cz/ontologies/ufo/is_part_of"/>
                <owl:someValuesFrom rdf:resource="&m;Attitude_and_direction_data_system"/>
            </owl:Restriction>
        </rdfs:subClassOf>
        <m:generated_time rdf:datatype="&xsd;dateTime">2015-04-12T02:45:54.351+02:00</m:generated_time>
        <m:has_related_eccairs_term rdf:resource="http://onto.fel.cvut.cz/ontologies/2014/ECCAIRS_Aviation_1.3.0.12/eccairs-descriptive-factors#category_11342000"/>
    </owl:Class>
    


    <!-- http://onto.fel.cvut.cz/ontologies/aviation-safety/Attitude_gyro_and_indicating_system -->

    <owl:Class rdf:about="&m;Attitude_gyro_and_indicating_system">
        <rdfs:label>Attitude gyro and indicating system</rdfs:label>
        <rdfs:subClassOf rdf:resource="&m;Attitude_and_direction_data_system_part"/>
        <m:generated_time rdf:datatype="&xsd;dateTime">2015-04-09T18:56:27.771+02:00</m:generated_time>
        <rdfs:comment xml:lang="en">(ATA Code:3421) Attitude gyro and indicating system: The gyroscopic unit which supplies attitude information to the necessary systems; e.g. vertical reference outputs for use as roll and pitch data to the autopilot computer. Includes the instruments relying on a gyroscope to display their information. Typical parts are vertical gyro and the gyro horizon.</rdfs:comment>
        <m:has_related_eccairs_term rdf:resource="http://onto.fel.cvut.cz/ontologies/2014/ECCAIRS_Aviation_1.3.0.12/eccairs-descriptive-factors#category_11342100"/>
    </owl:Class>
    


    <!-- http://onto.fel.cvut.cz/ontologies/aviation-safety/Audio-video_monitoring -->

    <owl:Class rdf:about="&m;Audio-video_monitoring">
        <rdfs:label>Audio/video monitoring</rdfs:label>
        <rdfs:subClassOf rdf:resource="&m;Aircraft_communication_related_system"/>
        <m:generated_time rdf:datatype="&xsd;dateTime">2015-04-09T18:56:27.771+02:00</m:generated_time>
        <rdfs:comment xml:lang="en">(ATA Code:2370) Audio/video monitoring: Those installations that record, or monitor crew or passenger conversation or movement or provide external monitoring for security or safety purposes. Includes externally mounted cameras, voice and video recorders used for aircraft operations.</rdfs:comment>
        <m:has_related_eccairs_term rdf:resource="http://onto.fel.cvut.cz/ontologies/2014/ECCAIRS_Aviation_1.3.0.12/eccairs-descriptive-factors#category_11237000"/>
    </owl:Class>
    


    <!-- http://onto.fel.cvut.cz/ontologies/aviation-safety/Audio_integrating_system -->

    <owl:Class rdf:about="&m;Audio_integrating_system">
        <rdfs:label>Audio integrating system</rdfs:label>
        <rdfs:subClassOf rdf:resource="&m;Aircraft_communication_related_system"/>
        <m:generated_time rdf:datatype="&xsd;dateTime">2015-04-09T18:56:27.771+02:00</m:generated_time>
        <rdfs:comment xml:lang="en">(ATA Code:2350) Audio integrating system: The system components and parts including the control panel and amplifier which controls output of communications and navigation receivers into flight crew headphones and speakers. Also includes output from microphones into communications transmitters. Typical parts are microphones, cockpit speakers and headphones.</rdfs:comment>
        <m:has_related_eccairs_term rdf:resource="http://onto.fel.cvut.cz/ontologies/2014/ECCAIRS_Aviation_1.3.0.12/eccairs-descriptive-factors#category_11235000"/>
    </owl:Class>
    


    <!-- http://onto.fel.cvut.cz/ontologies/aviation-safety/Auto-throttle_system -->

    <owl:Class rdf:about="&m;Auto-throttle_system">
        <rdfs:subClassOf rdf:resource="&m;autoflight_system"/>
        <all2:has_ATA_code rdf:datatype="&xsd;integer">2230</all2:has_ATA_code>
    </owl:Class>
    


    <!-- http://onto.fel.cvut.cz/ontologies/aviation-safety/Auto_throttle_system -->

    <owl:Class rdf:about="&m;Auto_throttle_system">
        <rdfs:label>Auto throttle system</rdfs:label>
        <rdfs:subClassOf rdf:resource="&m;autoflight_system"/>
        <m:generated_time rdf:datatype="&xsd;dateTime">2015-04-09T18:56:27.771+02:00</m:generated_time>
        <rdfs:comment xml:lang="en">(ATA Code:2230) Auto throttle system: The system that automatically controls the position of the throttles to manage engine power properly during all phases of flight/attitude. This includes engaging, sensing, computing, amplifying, controlling, actuating and warning devices. Typical parts are amplifiers, computers, servos, limit switches, clutches, gearboxes and warning lights.</rdfs:comment>
        <m:has_related_eccairs_term rdf:resource="http://onto.fel.cvut.cz/ontologies/2014/ECCAIRS_Aviation_1.3.0.12/eccairs-descriptive-factors#category_11223000"/>
    </owl:Class>
    


    <!-- http://onto.fel.cvut.cz/ontologies/aviation-safety/Autoflight_system_wiring -->

    <owl:Class rdf:about="&m;Autoflight_system_wiring">
        <rdfs:subClassOf rdf:resource="&m;autoflight_system"/>
    </owl:Class>
    


    <!-- http://onto.fel.cvut.cz/ontologies/aviation-safety/Automatic_direction_finder_system -->

    <owl:Class rdf:about="&m;Automatic_direction_finder_system">
        <rdfs:label>Automatic direction finder system</rdfs:label>
        <rdfs:subClassOf rdf:resource="&m;Dependent_position_determining_system"/>
        <m:generated_time rdf:datatype="&xsd;dateTime">2015-04-09T18:56:27.771+02:00</m:generated_time>
        <rdfs:comment xml:lang="en">(ATA Code:3455) Automatic direction finder system: The low frequency band system which receives a signal from a non-directional radio beacon to determine relative bearing from the beacon location [automatic direction finder system]. Typical parts are antenna, control unit, receiver and coaxial cable.</rdfs:comment>
        <m:has_related_eccairs_term rdf:resource="http://onto.fel.cvut.cz/ontologies/2014/ECCAIRS_Aviation_1.3.0.12/eccairs-descriptive-factors#category_11345500"/>
    </owl:Class>
    


    <!-- http://onto.fel.cvut.cz/ontologies/aviation-safety/Autopilot_computer -->

    <owl:Class rdf:about="&m;Autopilot_computer">
        <rdfs:label>Autopilot computer</rdfs:label>
        <rdfs:subClassOf rdf:resource="&m;Autopilot_system_part"/>
        <rdfs:subClassOf rdf:resource="&m;autoflight_system"/>
        <m:generated_time rdf:datatype="&xsd;dateTime">2015-04-09T18:56:27.771+02:00</m:generated_time>
        <all2:has_ATA_code rdf:datatype="&xsd;integer">2211</all2:has_ATA_code>
        <rdfs:comment xml:lang="en">(ATA Code:2211) Autopilot computer: Typical parts are resistors, circuit board, capacitor and power supply.</rdfs:comment>
        <m:has_related_eccairs_term rdf:resource="http://onto.fel.cvut.cz/ontologies/2014/ECCAIRS_Aviation_1.3.0.12/eccairs-descriptive-factors#category_11221100"/>
    </owl:Class>
    


    <!-- http://onto.fel.cvut.cz/ontologies/aviation-safety/Autopilot_main_servo -->

    <owl:Class rdf:about="&m;Autopilot_main_servo">
        <rdfs:label>Autopilot main servo</rdfs:label>
        <rdfs:subClassOf rdf:resource="&m;Autopilot_system_part"/>
        <rdfs:subClassOf rdf:resource="&m;autoflight_system"/>
        <m:generated_time rdf:datatype="&xsd;dateTime">2015-04-09T18:56:27.771+02:00</m:generated_time>
        <all2:has_ATA_code rdf:datatype="&xsd;integer">2215</all2:has_ATA_code>
        <rdfs:comment xml:lang="en">(ATA Code:2215) Autopilot main servo: The units connected to primary flight control actuating mechanisms which are used to reposition control surfaces mechanically in accordance with electrical or pneumatic signals from a controller.</rdfs:comment>
        <m:has_related_eccairs_term rdf:resource="http://onto.fel.cvut.cz/ontologies/2014/ECCAIRS_Aviation_1.3.0.12/eccairs-descriptive-factors#category_11221500"/>
    </owl:Class>
    


    <!-- http://onto.fel.cvut.cz/ontologies/aviation-safety/Autopilot_system -->

    <owl:Class rdf:about="&m;Autopilot_system">
        <rdfs:subClassOf rdf:resource="&m;autoflight_system"/>
    </owl:Class>
    


    <!-- http://onto.fel.cvut.cz/ontologies/aviation-safety/Autopilot_system_part -->

    <owl:Class rdf:about="&m;Autopilot_system_part">
        <rdfs:label>Autopilot system part</rdfs:label>
        <rdfs:subClassOf rdf:resource="&m;autoflight_system"/>
        <rdfs:subClassOf>
            <owl:Restriction>
                <owl:onProperty rdf:resource="http://onto.fel.cvut.cz/ontologies/ufo/is_part_of"/>
                <owl:someValuesFrom rdf:resource="&m;Autopilot_system"/>
            </owl:Restriction>
        </rdfs:subClassOf>
        <m:generated_time rdf:datatype="&xsd;dateTime">2015-04-12T02:45:54.351+02:00</m:generated_time>
        <m:has_related_eccairs_term rdf:resource="http://onto.fel.cvut.cz/ontologies/2014/ECCAIRS_Aviation_1.3.0.12/eccairs-descriptive-factors#category_11221000"/>
    </owl:Class>
    


    <!-- http://onto.fel.cvut.cz/ontologies/aviation-safety/Autopilot_trim_indicator -->

    <owl:Class rdf:about="&m;Autopilot_trim_indicator">
        <rdfs:subClassOf rdf:resource="&m;Autopilot_system_part"/>
        <rdfs:subClassOf rdf:resource="&m;autoflight_system"/>
    </owl:Class>
    


    <!-- http://onto.fel.cvut.cz/ontologies/aviation-safety/Autopilot_trim_servo -->

    <owl:Class rdf:about="&m;Autopilot_trim_servo">
        <rdfs:label>Autopilot trim servo</rdfs:label>
        <rdfs:subClassOf rdf:resource="&m;Autopilot_system_part"/>
        <rdfs:subClassOf rdf:resource="&m;autoflight_system"/>
        <m:generated_time rdf:datatype="&xsd;dateTime">2015-04-09T18:56:27.771+02:00</m:generated_time>
        <all2:has_ATA_code rdf:datatype="&xsd;integer">2216</all2:has_ATA_code>
        <rdfs:comment xml:lang="en">(ATA Code:2216) Autopilot trim servo: The units that are mechanically connected to flight control cables for making minor corrections in aircraft attitude or direction.</rdfs:comment>
        <m:has_related_eccairs_term rdf:resource="http://onto.fel.cvut.cz/ontologies/2014/ECCAIRS_Aviation_1.3.0.12/eccairs-descriptive-factors#category_11221600"/>
    </owl:Class>
    


    <!-- http://onto.fel.cvut.cz/ontologies/aviation-safety/Auxiliary_power_unit_bleed_air_system -->

    <owl:Class rdf:about="&m;Auxiliary_power_unit_bleed_air_system">
        <rdfs:subClassOf rdf:resource="&m;Airborne_auxiliary_power_unit_system_part"/>
    </owl:Class>
    


    <!-- http://onto.fel.cvut.cz/ontologies/aviation-safety/Auxiliary_power_unit_controls -->

    <owl:Class rdf:about="&m;Auxiliary_power_unit_controls">
        <rdfs:subClassOf rdf:resource="&m;Airborne_auxiliary_power_unit_system_part"/>
    </owl:Class>
    


    <!-- http://onto.fel.cvut.cz/ontologies/aviation-safety/Auxiliary_power_unit_core_engine -->

    <owl:Class rdf:about="&m;Auxiliary_power_unit_core_engine">
        <rdfs:subClassOf rdf:resource="&m;Airborne_auxiliary_power_unit_system_part"/>
    </owl:Class>
    


    <!-- http://onto.fel.cvut.cz/ontologies/aviation-safety/Auxiliary_power_unit_cowling-containment -->

    <owl:Class rdf:about="&m;Auxiliary_power_unit_cowling-containment">
        <rdfs:subClassOf rdf:resource="&m;Airborne_auxiliary_power_unit_system_part"/>
    </owl:Class>
    


    <!-- http://onto.fel.cvut.cz/ontologies/aviation-safety/Auxiliary_power_unit_door -->

    <owl:Class rdf:about="&m;Auxiliary_power_unit_door">
        <rdfs:subClassOf rdf:resource="&m;Service_doors_part"/>
    </owl:Class>
    


    <!-- http://onto.fel.cvut.cz/ontologies/aviation-safety/Auxiliary_power_unit_exhaust_system -->

    <owl:Class rdf:about="&m;Auxiliary_power_unit_exhaust_system">
        <rdfs:subClassOf rdf:resource="&m;Airborne_auxiliary_power_unit_system_part"/>
    </owl:Class>
    


    <!-- http://onto.fel.cvut.cz/ontologies/aviation-safety/Auxiliary_power_unit_fuel_and_control -->

    <owl:Class rdf:about="&m;Auxiliary_power_unit_fuel_and_control">
        <rdfs:subClassOf rdf:resource="&m;Airborne_auxiliary_power_unit_system_part"/>
    </owl:Class>
    


    <!-- http://onto.fel.cvut.cz/ontologies/aviation-safety/Auxiliary_power_unit_indicating_system -->

    <owl:Class rdf:about="&m;Auxiliary_power_unit_indicating_system">
        <rdfs:subClassOf rdf:resource="&m;Airborne_auxiliary_power_unit_system_part"/>
    </owl:Class>
    


    <!-- http://onto.fel.cvut.cz/ontologies/aviation-safety/Auxiliary_power_unit_oil_system -->

    <owl:Class rdf:about="&m;Auxiliary_power_unit_oil_system">
        <rdfs:subClassOf rdf:resource="&m;Airborne_auxiliary_power_unit_system_part"/>
    </owl:Class>
    


    <!-- http://onto.fel.cvut.cz/ontologies/aviation-safety/Auxiliary_power_unit_start-ignition_system -->

    <owl:Class rdf:about="&m;Auxiliary_power_unit_start-ignition_system">
        <rdfs:subClassOf rdf:resource="&m;Airborne_auxiliary_power_unit_system_part"/>
    </owl:Class>
    


    <!-- http://onto.fel.cvut.cz/ontologies/aviation-safety/Balloon-dirigible_components -->

    <owl:Class rdf:about="&m;Balloon-dirigible_components">
        <rdfs:label>Balloon/dirigible components</rdfs:label>
        <rdfs:subClassOf rdf:resource="&m;STANDARD_PRACTICES_AND_STRUCTURES_-_GENERAL_part"/>
        <m:generated_time rdf:datatype="&xsd;dateTime">2015-04-09T18:56:27.771+02:00</m:generated_time>
        <rdfs:comment xml:lang="en">(ATA Code:5102) Balloon/dirigible components: All balloons, airships and dirigible components irrespective of location or component involved. Also includes reports for water ballast which are normally filed under water ballast.</rdfs:comment>
        <m:has_related_eccairs_term rdf:resource="http://onto.fel.cvut.cz/ontologies/2014/ECCAIRS_Aviation_1.3.0.12/eccairs-descriptive-factors#category_11510200"/>
    </owl:Class>
    


    <!-- http://onto.fel.cvut.cz/ontologies/aviation-safety/Barometric_altimeter-encoder -->

    <owl:Class rdf:about="&m;Barometric_altimeter-encoder">
        <rdfs:label>Barometric altimeter/encoder</rdfs:label>
        <rdfs:subClassOf rdf:resource="&m;Flight_environment_data_system"/>
        <m:generated_time rdf:datatype="&xsd;dateTime">2015-04-09T18:56:27.771+02:00</m:generated_time>
        <rdfs:comment xml:lang="en">(ATA Code:3416) The altimeters and barometric encoders used to measure and indicate altitude. Also includes the unit which senses and provides an alert of a change in a pre-selected altitude. Does not include the ground proximity systems. [Code 11344400.] Typical parts are dial, case, pointer and springs.</rdfs:comment>
        <m:has_related_eccairs_term rdf:resource="http://onto.fel.cvut.cz/ontologies/2014/ECCAIRS_Aviation_1.3.0.12/eccairs-descriptive-factors#category_11341600"/>
    </owl:Class>
    


    <!-- http://onto.fel.cvut.cz/ontologies/aviation-safety/Battery-charger_system -->

    <owl:Class rdf:about="&m;Battery-charger_system">
        <rdfs:label>Battery/charger system</rdfs:label>
        <rdfs:subClassOf rdf:resource="&m;Direct_current_generating_system_part"/>
        <m:generated_time rdf:datatype="&xsd;dateTime">2015-04-09T18:56:27.771+02:00</m:generated_time>
        <rdfs:comment xml:lang="en">(ATA Code:2432) Battery/charger system: The component providing a source of direct current voltage and current flow independent of rotating generators and alternators. Typical parts are battery charger, cell, case and post.</rdfs:comment>
        <m:has_related_eccairs_term rdf:resource="http://onto.fel.cvut.cz/ontologies/2014/ECCAIRS_Aviation_1.3.0.12/eccairs-descriptive-factors#category_11243200"/>
    </owl:Class>
    


    <!-- http://onto.fel.cvut.cz/ontologies/aviation-safety/Battery_box_structure -->

    <owl:Class rdf:about="&m;Battery_box_structure">
        <rdfs:label>Battery box structure</rdfs:label>
        <rdfs:subClassOf rdf:resource="&m;Accessory_compartments_part"/>
        <m:generated_time rdf:datatype="&xsd;dateTime">2015-04-09T18:56:27.771+02:00</m:generated_time>
        <rdfs:comment xml:lang="en">(ATA Code:2571) Battery box structure: The supporting structure, vents and overboard drains for aircraft batteries. Typical parts are vent cap, drain tube, insulator and cover.</rdfs:comment>
        <m:has_related_eccairs_term rdf:resource="http://onto.fel.cvut.cz/ontologies/2014/ECCAIRS_Aviation_1.3.0.12/eccairs-descriptive-factors#category_11257100"/>
    </owl:Class>
    


    <!-- http://onto.fel.cvut.cz/ontologies/aviation-safety/Battery_overheat_warning_system -->

    <owl:Class rdf:about="&m;Battery_overheat_warning_system">
        <rdfs:label>Battery overheat warning system</rdfs:label>
        <rdfs:subClassOf rdf:resource="&m;Direct_current_generating_system_part"/>
        <m:generated_time rdf:datatype="&xsd;dateTime">2015-04-09T18:56:27.771+02:00</m:generated_time>
        <rdfs:comment xml:lang="en">(ATA Code:2431) Battery overheat warning system: the system components that sense and indicate, or warn of, a battery over-temperature condition. Typical parts are sensor, lamp and gauge.</rdfs:comment>
        <m:has_related_eccairs_term rdf:resource="http://onto.fel.cvut.cz/ontologies/2014/ECCAIRS_Aviation_1.3.0.12/eccairs-descriptive-factors#category_11243100"/>
    </owl:Class>
    


    <!-- http://onto.fel.cvut.cz/ontologies/aviation-safety/Bleed_air_indicating_system -->

    <owl:Class rdf:about="&m;Bleed_air_indicating_system">
        <rdfs:label>Bleed air indicating system</rdfs:label>
        <rdfs:subClassOf rdf:resource="&m;Engine_bleed_air_system_part"/>
        <m:generated_time rdf:datatype="&xsd;dateTime">2015-04-09T18:56:27.771+02:00</m:generated_time>
        <rdfs:comment xml:lang="en">(ATA Code:7540) Bleed air indicating system: The systems which indicate temperature, pressure, control positions and warning indications of turbine engine compressor bleed air systems in turbine engines. Typical parts are transmitter, sensor, indicator, lamp and pressure switch.</rdfs:comment>
        <m:has_related_eccairs_term rdf:resource="http://onto.fel.cvut.cz/ontologies/2014/ECCAIRS_Aviation_1.3.0.12/eccairs-descriptive-factors#category_11754000"/>
    </owl:Class>
    


    <!-- http://onto.fel.cvut.cz/ontologies/aviation-safety/Buffet-galleys -->

    <owl:Class rdf:about="&m;Buffet-galleys">
        <rdfs:label>Buffet/galleys</rdfs:label>
        <rdfs:subClassOf rdf:resource="&m;Cabin_equipment-furnishings"/>
        <m:generated_time rdf:datatype="&xsd;dateTime">2015-04-09T18:56:27.771+02:00</m:generated_time>
        <rdfs:comment xml:lang="en">(ATA Code:2530) The buffet/galley equipment. Typical components are hot plates, coffee pots, food carts, ovens, trays, relays, switches, connectors and dispensers.</rdfs:comment>
        <m:has_related_eccairs_term rdf:resource="http://onto.fel.cvut.cz/ontologies/2014/ECCAIRS_Aviation_1.3.0.12/eccairs-descriptive-factors#category_11253000"/>
    </owl:Class>
    


    <!-- http://onto.fel.cvut.cz/ontologies/aviation-safety/Bulkhead-firewall_(nacelle-pylon) -->

    <owl:Class rdf:about="&m;Bulkhead-firewall_(nacelle-pylon)">
        <rdfs:label>Bulkhead/firewall (nacelle/pylon)</rdfs:label>
        <rdfs:subClassOf rdf:resource="&m;Main_frame_(nacelle-pylon)_part"/>
        <m:generated_time rdf:datatype="&xsd;dateTime">2015-04-09T18:56:27.771+02:00</m:generated_time>
        <rdfs:comment xml:lang="en">(ATA Code:5412) The bulkhead or firewall structure of the nacelles or pylons.</rdfs:comment>
        <m:has_related_eccairs_term rdf:resource="http://onto.fel.cvut.cz/ontologies/2014/ECCAIRS_Aviation_1.3.0.12/eccairs-descriptive-factors#category_11541200"/>
    </owl:Class>
    


    <!-- http://onto.fel.cvut.cz/ontologies/aviation-safety/Cabin_compressor_system -->

    <owl:Class rdf:about="&m;Cabin_compressor_system">
        <rdfs:label>Cabin compressor system</rdfs:label>
        <rdfs:subClassOf rdf:resource="&m;Air_conditioning_system_part"/>
        <m:generated_time rdf:datatype="&xsd;dateTime">2015-04-09T18:56:27.771+02:00</m:generated_time>
        <all2:has_ATA_code rdf:datatype="&xsd;integer">2110</all2:has_ATA_code>
        <rdfs:comment xml:lang="en">(ATA Code:2110) Cabin compressor system: Includes items such as controls and indicating systems related to the compressors and wiring, but does not include the pressure control and indicating system for the cabin pressurization.</rdfs:comment>
        <m:has_related_eccairs_term rdf:resource="http://onto.fel.cvut.cz/ontologies/2014/ECCAIRS_Aviation_1.3.0.12/eccairs-descriptive-factors#category_11211000"/>
    </owl:Class>
    


    <!-- http://onto.fel.cvut.cz/ontologies/aviation-safety/Cabin_cooling_system -->

    <owl:Class rdf:about="&m;Cabin_cooling_system">
        <rdfs:label>Cabin cooling system</rdfs:label>
        <rdfs:subClassOf rdf:resource="&m;Air_conditioning_system_part"/>
        <m:generated_time rdf:datatype="&xsd;dateTime">2015-04-09T18:56:27.771+02:00</m:generated_time>
        <all2:has_ATA_code rdf:datatype="&xsd;integer">2150</all2:has_ATA_code>
        <rdfs:comment xml:lang="en">(ATA Code:2150) Cabin cooling system: The units and systems supplying cooled air to the cockpit or cabin. Does not include the temperature control and indicating system. Typical parts are flow valve, relay, condenser, ram air sensor, heat exchanger, cooling turbine and air cycle machine.</rdfs:comment>
        <m:has_related_eccairs_term rdf:resource="http://onto.fel.cvut.cz/ontologies/2014/ECCAIRS_Aviation_1.3.0.12/eccairs-descriptive-factors#category_11215000"/>
    </owl:Class>
    


    <!-- http://onto.fel.cvut.cz/ontologies/aviation-safety/Cabin_core_system -->

    <owl:Class rdf:about="&m;Cabin_core_system">
        <rdfs:label>Cabin core system</rdfs:label>
        <rdfs:subClassOf rdf:resource="&m;cabin_system"/>
        <m:generated_time rdf:datatype="&xsd;dateTime">2015-04-09T18:56:27.771+02:00</m:generated_time>
        <rdfs:comment xml:lang="en">(ATA Code:4410) Cabin core system: The portion of the cabin system used to accomplish the integrated functional control, operation, testing and monitoring of cabin systems and to increase cabin comfort (such as active noise control). Includes items such as controllers, cabin control panels, handsets, signs and loudspeakers.</rdfs:comment>
        <m:has_related_eccairs_term rdf:resource="http://onto.fel.cvut.cz/ontologies/2014/ECCAIRS_Aviation_1.3.0.12/eccairs-descriptive-factors#category_11441000"/>
    </owl:Class>
    


    <!-- http://onto.fel.cvut.cz/ontologies/aviation-safety/Cabin_equipment-furnishings -->

    <owl:Class rdf:about="&m;Cabin_equipment-furnishings">
        <rdfs:label>Cabin equipment/furnishings</rdfs:label>
        <rdfs:subClassOf rdf:resource="&m;Aircraft_part"/>
        <m:generated_time rdf:datatype="&xsd;dateTime">2015-04-09T18:56:27.771+02:00</m:generated_time>
        <m:generated_time rdf:datatype="&xsd;dateTime">2015-04-12T02:45:54.351+02:00</m:generated_time>
        <rdfs:comment xml:lang="en">(ATA Code:2500) Cabin equipment/furnishings: The removable items of equipment and furnishings mounted or contained in the flight, passenger, cargo, accessory compartments.</rdfs:comment>
        <m:has_related_eccairs_term rdf:resource="http://onto.fel.cvut.cz/ontologies/2014/ECCAIRS_Aviation_1.3.0.12/eccairs-descriptive-factors#category_11250000"/>
    </owl:Class>
    


    <!-- http://onto.fel.cvut.cz/ontologies/aviation-safety/Cabin_mass_memory_system -->

    <owl:Class rdf:about="&m;Cabin_mass_memory_system">
        <rdfs:label>Cabin mass memory system</rdfs:label>
        <rdfs:subClassOf rdf:resource="&m;cabin_system"/>
        <m:generated_time rdf:datatype="&xsd;dateTime">2015-04-09T18:56:27.771+02:00</m:generated_time>
        <rdfs:comment xml:lang="en">(ATA Code:4440) Cabin mass memory system: That portion of the cabin mass memory system used to store and process cabin related data, such as systems configuration data and multimedia programs. Includes items such as controllers, terminals, keyboards, disk drives, printers and modems.</rdfs:comment>
        <m:has_related_eccairs_term rdf:resource="http://onto.fel.cvut.cz/ontologies/2014/ECCAIRS_Aviation_1.3.0.12/eccairs-descriptive-factors#category_11444000"/>
    </owl:Class>
    


    <!-- http://onto.fel.cvut.cz/ontologies/aviation-safety/Cabin_monitoring_system -->

    <owl:Class rdf:about="&m;Cabin_monitoring_system">
        <rdfs:label>Cabin monitoring system</rdfs:label>
        <rdfs:subClassOf rdf:resource="&m;cabin_system"/>
        <m:generated_time rdf:datatype="&xsd;dateTime">2015-04-09T18:56:27.771+02:00</m:generated_time>
        <rdfs:comment xml:lang="en">(ATA Code:4450) Cabin monitoring system: The portion of the cabin system used to monitor parts of the cabin area. Includes items such as surveillance cameras and monitors. Does not include external anti-hijack devices or external video monitoring.</rdfs:comment>
        <m:has_related_eccairs_term rdf:resource="http://onto.fel.cvut.cz/ontologies/2014/ECCAIRS_Aviation_1.3.0.12/eccairs-descriptive-factors#category_11445000"/>
    </owl:Class>
    


    <!-- http://onto.fel.cvut.cz/ontologies/aviation-safety/Cabin_pressure_control_system -->

    <owl:Class rdf:about="&m;Cabin_pressure_control_system">
        <rdfs:subClassOf rdf:resource="&m;Air_conditioning_system_part"/>
        <rdfs:subClassOf rdf:resource="&m;Pressurization_control_system_part"/>
    </owl:Class>
    


    <!-- http://onto.fel.cvut.cz/ontologies/aviation-safety/Cabin_pressure_controller -->

    <owl:Class rdf:about="&m;Cabin_pressure_controller">
        <rdfs:subClassOf rdf:resource="&m;Air_conditioning_system_part"/>
        <all2:has_ATA_code rdf:datatype="&xsd;integer">2131</all2:has_ATA_code>
    </owl:Class>
    


    <!-- http://onto.fel.cvut.cz/ontologies/aviation-safety/Cabin_pressure_indicator -->

    <owl:Class rdf:about="&m;Cabin_pressure_indicator">
        <rdfs:subClassOf rdf:resource="&m;Air_conditioning_system_part"/>
    </owl:Class>
    


    <!-- http://onto.fel.cvut.cz/ontologies/aviation-safety/Cabin_systems_wiring -->

    <owl:Class rdf:about="&m;Cabin_systems_wiring">
        <rdfs:subClassOf rdf:resource="&m;cabin_system"/>
    </owl:Class>
    


    <!-- http://onto.fel.cvut.cz/ontologies/aviation-safety/Cabin_temperature_control_system -->

    <owl:Class rdf:about="&m;Cabin_temperature_control_system">
        <rdfs:subClassOf rdf:resource="&m;Air_conditioning_system_part"/>
        <rdfs:subClassOf rdf:resource="&m;Temperature_control_system_part"/>
    </owl:Class>
    


    <!-- http://onto.fel.cvut.cz/ontologies/aviation-safety/Cabin_temperature_controller -->

    <owl:Class rdf:about="&m;Cabin_temperature_controller">
        <rdfs:subClassOf rdf:resource="&m;Air_conditioning_system_part"/>
        <all2:has_ATA_code rdf:datatype="&xsd;integer">2161</all2:has_ATA_code>
    </owl:Class>
    


    <!-- http://onto.fel.cvut.cz/ontologies/aviation-safety/Cabin_temperature_indicator -->

    <owl:Class rdf:about="&m;Cabin_temperature_indicator">
        <rdfs:subClassOf rdf:resource="&m;Air_conditioning_system_part"/>
        <rdfs:subClassOf rdf:resource="&m;Temperature_control_system_part"/>
    </owl:Class>
    


    <!-- http://onto.fel.cvut.cz/ontologies/aviation-safety/Cabin_temperature_sensor -->

    <owl:Class rdf:about="&m;Cabin_temperature_sensor">
        <rdfs:label>Cabin temperature sensor</rdfs:label>
        <rdfs:subClassOf rdf:resource="&m;Air_conditioning_system_part"/>
        <rdfs:subClassOf rdf:resource="&m;Temperature_control_system_part"/>
        <m:generated_time rdf:datatype="&xsd;dateTime">2015-04-09T18:56:27.771+02:00</m:generated_time>
        <all2:has_ATA_code rdf:datatype="&xsd;integer">2163</all2:has_ATA_code>
        <rdfs:comment xml:lang="en">(ATA Code:2163) The cabin temperature sensors and associated circuitry which sense the temperature of the air in the cabin and relay a signal to the indicator.</rdfs:comment>
        <m:has_related_eccairs_term rdf:resource="http://onto.fel.cvut.cz/ontologies/2014/ECCAIRS_Aviation_1.3.0.12/eccairs-descriptive-factors#category_11216300"/>
    </owl:Class>
    


    <!-- http://onto.fel.cvut.cz/ontologies/aviation-safety/Cabine_pressure_sensor -->

    <owl:Class rdf:about="&m;Cabine_pressure_sensor">
        <rdfs:subClassOf rdf:resource="&m;Air_conditioning_system_part"/>
        <all2:has_ATA_code rdf:datatype="&xsd;integer">2134</all2:has_ATA_code>
    </owl:Class>
    


    <!-- http://onto.fel.cvut.cz/ontologies/aviation-safety/Canard -->

    <owl:Class rdf:about="&m;Canard">
        <rdfs:label>Canard</rdfs:label>
        <rdfs:subClassOf rdf:resource="&m;Empennage_structure_part"/>
        <m:generated_time rdf:datatype="&xsd;dateTime">2015-04-09T18:56:27.771+02:00</m:generated_time>
        <rdfs:comment xml:lang="en">(ATA Code:5570) Canard: The smaller surface on an aeroplane providing stability or a means of control and placed forward of the main lifting surface.</rdfs:comment>
        <m:has_related_eccairs_term rdf:resource="http://onto.fel.cvut.cz/ontologies/2014/ECCAIRS_Aviation_1.3.0.12/eccairs-descriptive-factors#category_11557000"/>
    </owl:Class>
    


    <!-- http://onto.fel.cvut.cz/ontologies/aviation-safety/Cargo-accessory_compartment_insulation -->

    <owl:Class rdf:about="&m;Cargo-accessory_compartment_insulation">
        <rdfs:subClassOf rdf:resource="&m;Cargo_and_accessory_compartments_part"/>
    </owl:Class>
    


    <!-- http://onto.fel.cvut.cz/ontologies/aviation-safety/Cargo-baggage_doors -->

    <owl:Class rdf:about="&m;Cargo-baggage_doors">
        <rdfs:label>Cargo/baggage doors</rdfs:label>
        <rdfs:subClassOf rdf:resource="&m;Fuselage_doors_part"/>
        <m:generated_time rdf:datatype="&xsd;dateTime">2015-04-09T18:56:27.771+02:00</m:generated_time>
        <rdfs:comment xml:lang="en">(ATA Code:5230) Cargo/baggage doors: The exterior doors used to gain access to cargo or baggage storage areas. Does not include door frames on fuselage, door warning or compartment interior furnishings. Typical parts are door structure, seal, hinge, latch, latch pin, handle and skin.</rdfs:comment>
        <m:has_related_eccairs_term rdf:resource="http://onto.fel.cvut.cz/ontologies/2014/ECCAIRS_Aviation_1.3.0.12/eccairs-descriptive-factors#category_11523000"/>
    </owl:Class>
    


    <!-- http://onto.fel.cvut.cz/ontologies/aviation-safety/Cargo-servicing_compartment_lighting -->

    <owl:Class rdf:about="&m;Cargo-servicing_compartment_lighting">
        <rdfs:label>Cargo/servicing compartment lighting</rdfs:label>
        <rdfs:subClassOf rdf:resource="&m;Lighting_system"/>
        <m:generated_time rdf:datatype="&xsd;dateTime">2015-04-09T18:56:27.771+02:00</m:generated_time>
        <rdfs:comment xml:lang="en">(ATA Code:3330) Cargo/servicing compartment lighting: The lighting systems in the compartments used for storage of cargo, baggage, or aircraft system components which require servicing. Does not include electrical systems, fire or smoke sensing. Typical parts are circuit breaker, lamp, lens and switch.</rdfs:comment>
        <m:has_related_eccairs_term rdf:resource="http://onto.fel.cvut.cz/ontologies/2014/ECCAIRS_Aviation_1.3.0.12/eccairs-descriptive-factors#category_11333000"/>
    </owl:Class>
    


    <!-- http://onto.fel.cvut.cz/ontologies/aviation-safety/Cargo_and_accessory_compartments -->

    <owl:Class rdf:about="&m;Cargo_and_accessory_compartments">
        <rdfs:subClassOf rdf:resource="&m;Aircraft_part"/>
    </owl:Class>
    


    <!-- http://onto.fel.cvut.cz/ontologies/aviation-safety/Cargo_and_accessory_compartments_part -->

    <owl:Class rdf:about="&m;Cargo_and_accessory_compartments_part">
        <rdfs:label>Cargo and accessory compartments part</rdfs:label>
        <rdfs:subClassOf rdf:resource="&m;Aircraft_part"/>
        <rdfs:subClassOf>
            <owl:Restriction>
                <owl:onProperty rdf:resource="http://onto.fel.cvut.cz/ontologies/ufo/is_part_of"/>
                <owl:someValuesFrom rdf:resource="&m;Cargo_and_accessory_compartments"/>
            </owl:Restriction>
        </rdfs:subClassOf>
        <m:generated_time rdf:datatype="&xsd;dateTime">2015-04-12T02:45:54.351+02:00</m:generated_time>
        <m:has_related_eccairs_term rdf:resource="http://onto.fel.cvut.cz/ontologies/2014/ECCAIRS_Aviation_1.3.0.12/eccairs-descriptive-factors#category_11500000"/>
    </owl:Class>
    


    <!-- http://onto.fel.cvut.cz/ontologies/aviation-safety/Cargo_and_accessory_compartments_wiring -->

    <owl:Class rdf:about="&m;Cargo_and_accessory_compartments_wiring">
        <rdfs:subClassOf rdf:resource="&m;Cargo_and_accessory_compartments_part"/>
    </owl:Class>
    


    <!-- http://onto.fel.cvut.cz/ontologies/aviation-safety/Cargo_compartments -->

    <owl:Class rdf:about="&m;Cargo_compartments">
        <rdfs:subClassOf rdf:resource="&m;Cargo_and_accessory_compartments_part"/>
    </owl:Class>
    


    <!-- http://onto.fel.cvut.cz/ontologies/aviation-safety/Cargo_compartments_part -->

    <owl:Class rdf:about="&m;Cargo_compartments_part">
        <rdfs:label>Cargo compartments part</rdfs:label>
        <rdfs:subClassOf rdf:resource="&m;Cargo_and_accessory_compartments_part"/>
        <rdfs:subClassOf>
            <owl:Restriction>
                <owl:onProperty rdf:resource="http://onto.fel.cvut.cz/ontologies/ufo/is_part_of"/>
                <owl:someValuesFrom rdf:resource="&m;Cargo_compartments"/>
            </owl:Restriction>
        </rdfs:subClassOf>
        <m:generated_time rdf:datatype="&xsd;dateTime">2015-04-12T02:45:54.351+02:00</m:generated_time>
        <m:has_related_eccairs_term rdf:resource="http://onto.fel.cvut.cz/ontologies/2014/ECCAIRS_Aviation_1.3.0.12/eccairs-descriptive-factors#category_11501000"/>
    </owl:Class>
    


    <!-- http://onto.fel.cvut.cz/ontologies/aviation-safety/Cargo_loading_system -->

    <owl:Class rdf:about="&m;Cargo_loading_system">
        <rdfs:subClassOf rdf:resource="&m;Cargo_and_accessory_compartments_part"/>
    </owl:Class>
    


    <!-- http://onto.fel.cvut.cz/ontologies/aviation-safety/Cargo_related_systems -->

    <owl:Class rdf:about="&m;Cargo_related_systems">
        <rdfs:subClassOf rdf:resource="&m;Cargo_and_accessory_compartments_part"/>
    </owl:Class>
    


    <!-- http://onto.fel.cvut.cz/ontologies/aviation-safety/Central_Maintenance_System_Wiring -->

    <owl:Class rdf:about="&m;Central_Maintenance_System_Wiring">
        <rdfs:subClassOf rdf:resource="&m;Central_maintenance_computer_part"/>
    </owl:Class>
    


    <!-- http://onto.fel.cvut.cz/ontologies/aviation-safety/Central_maintenance_computer -->

    <owl:Class rdf:about="&m;Central_maintenance_computer">
        <rdfs:label>Central maintenance computer</rdfs:label>
        <rdfs:subClassOf rdf:resource="&m;Aircraft_part"/>
        <m:generated_time rdf:datatype="&xsd;dateTime">2015-04-09T18:56:27.771+02:00</m:generated_time>
        <rdfs:comment xml:lang="en">(ATA Code:4500) Central maintenance computer: The unit, components and associated systems which interface with other airplane systems and provide a convenient way of communicating system problems to aircraft maintenance personnel. The system contains checkout and fault isolation procedures using a central computer to locate a single system or component malfunction. Typical parts are computer, storage devices, controls and display.</rdfs:comment>
        <m:has_related_eccairs_term rdf:resource="http://onto.fel.cvut.cz/ontologies/2014/ECCAIRS_Aviation_1.3.0.12/eccairs-descriptive-factors#category_11450000"/>
    </owl:Class>
    


    <!-- http://onto.fel.cvut.cz/ontologies/aviation-safety/Central_maintenance_computer_part -->

    <owl:Class rdf:about="&m;Central_maintenance_computer_part">
        <rdfs:label>Central maintenance computer part</rdfs:label>
        <rdfs:subClassOf rdf:resource="&m;Aircraft_part"/>
        <rdfs:subClassOf>
            <owl:Restriction>
                <owl:onProperty rdf:resource="http://onto.fel.cvut.cz/ontologies/ufo/is_part_of"/>
                <owl:someValuesFrom rdf:resource="&m;Central_maintenance_computer"/>
            </owl:Restriction>
        </rdfs:subClassOf>
        <m:generated_time rdf:datatype="&xsd;dateTime">2015-04-12T02:45:54.351+02:00</m:generated_time>
        <m:has_related_eccairs_term rdf:resource="http://onto.fel.cvut.cz/ontologies/2014/ECCAIRS_Aviation_1.3.0.12/eccairs-descriptive-factors#category_11450000"/>
    </owl:Class>
    


    <!-- http://onto.fel.cvut.cz/ontologies/aviation-safety/Compressor_bleed_control -->

    <owl:Class rdf:about="&m;Compressor_bleed_control">
        <rdfs:label>Compressor bleed control</rdfs:label>
        <rdfs:subClassOf rdf:resource="&m;Engine_bleed_air_system_part"/>
        <m:generated_time rdf:datatype="&xsd;dateTime">2015-04-09T18:56:27.771+02:00</m:generated_time>
        <rdfs:comment xml:lang="en">(ATA Code:7530) Compressor bleed control: The system, except the valve and governor, which controls the flow of air through turbine engines. Includes the operation of variable stator blades, linkage to the various valves and sense lines. Typical parts are sense line, stator vane, fitting, cable, sense line filter and speed sense valve.</rdfs:comment>
        <m:has_related_eccairs_term rdf:resource="http://onto.fel.cvut.cz/ontologies/2014/ECCAIRS_Aviation_1.3.0.12/eccairs-descriptive-factors#category_11753000"/>
    </owl:Class>
    


    <!-- http://onto.fel.cvut.cz/ontologies/aviation-safety/Compressor_bleed_control_part -->

    <owl:Class rdf:about="&m;Compressor_bleed_control_part">
        <rdfs:label>Compressor bleed control part</rdfs:label>
        <rdfs:subClassOf rdf:resource="&m;Engine_bleed_air_system_part"/>
        <rdfs:subClassOf>
            <owl:Restriction>
                <owl:onProperty rdf:resource="http://onto.fel.cvut.cz/ontologies/ufo/is_part_of"/>
                <owl:someValuesFrom rdf:resource="&m;Compressor_bleed_control"/>
            </owl:Restriction>
        </rdfs:subClassOf>
        <m:generated_time rdf:datatype="&xsd;dateTime">2015-04-12T02:45:54.351+02:00</m:generated_time>
        <m:has_related_eccairs_term rdf:resource="http://onto.fel.cvut.cz/ontologies/2014/ECCAIRS_Aviation_1.3.0.12/eccairs-descriptive-factors#category_11753000"/>
    </owl:Class>
    


    <!-- http://onto.fel.cvut.cz/ontologies/aviation-safety/Compressor_bleed_governor -->

    <owl:Class rdf:about="&m;Compressor_bleed_governor">
        <rdfs:label>Compressor bleed governor</rdfs:label>
        <rdfs:subClassOf rdf:resource="&m;Compressor_bleed_control_part"/>
        <m:generated_time rdf:datatype="&xsd;dateTime">2015-04-09T18:56:27.771+02:00</m:generated_time>
        <rdfs:comment xml:lang="en">(ATA Code:7531) Compressor bleed governor: The unit controlling relative position of the compressor bleed valve in turbine engines for air flow control.</rdfs:comment>
        <m:has_related_eccairs_term rdf:resource="http://onto.fel.cvut.cz/ontologies/2014/ECCAIRS_Aviation_1.3.0.12/eccairs-descriptive-factors#category_11753100"/>
    </owl:Class>
    


    <!-- http://onto.fel.cvut.cz/ontologies/aviation-safety/Compressor_bleed_valve -->

    <owl:Class rdf:about="&m;Compressor_bleed_valve">
        <rdfs:label>Compressor bleed valve</rdfs:label>
        <rdfs:subClassOf rdf:resource="&m;Compressor_bleed_control_part"/>
        <m:generated_time rdf:datatype="&xsd;dateTime">2015-04-09T18:56:27.771+02:00</m:generated_time>
        <rdfs:comment xml:lang="en">(ATA Code:7532) Compressor bleed valve: The component which releases air from turbine engine compressor sections for air flow control. Typical parts are bleed valve, actuator and check valve.</rdfs:comment>
        <m:has_related_eccairs_term rdf:resource="http://onto.fel.cvut.cz/ontologies/2014/ECCAIRS_Aviation_1.3.0.12/eccairs-descriptive-factors#category_11753200"/>
    </owl:Class>
    


    <!-- http://onto.fel.cvut.cz/ontologies/aviation-safety/Control_column_section -->

    <owl:Class rdf:about="&m;Control_column_section">
        <rdfs:label>Control column section</rdfs:label>
        <rdfs:subClassOf rdf:resource="&m;Flight_control_system_part"/>
        <m:generated_time rdf:datatype="&xsd;dateTime">2015-04-09T18:56:27.771+02:00</m:generated_time>
        <rdfs:comment xml:lang="en">(ATA Code:2701) Control column section: The component and associated parts mounted onto the control which transmit pilot input from the cockpit to connecting cables and pushrods, to actuate the ailerons, elevators, stabilator, ruddervator and similar control surfaces. Includes control sticks in aircraft not equipped with control wheels. Typical parts are bearing, socket, guide, bushing, pulley bracket, sprocket, chain and stops.</rdfs:comment>
        <m:has_related_eccairs_term rdf:resource="http://onto.fel.cvut.cz/ontologies/2014/ECCAIRS_Aviation_1.3.0.12/eccairs-descriptive-factors#category_11270100"/>
    </owl:Class>
    


    <!-- http://onto.fel.cvut.cz/ontologies/aviation-safety/Coolant_servicing -->

    <owl:Class rdf:about="&m;Coolant_servicing">
        <rdfs:label>Coolant servicing</rdfs:label>
        <rdfs:subClassOf rdf:resource="&m;Servicing_of_the_aircraft_with_liquids_part"/>
        <m:generated_time rdf:datatype="&xsd;dateTime">2015-04-09T18:56:27.771+02:00</m:generated_time>
        <rdfs:comment xml:lang="en">(ATA Code:1240) Coolant servicing: servicing the aircraft with any type of engine coolant used in aircraft.</rdfs:comment>
        <m:has_related_eccairs_term rdf:resource="http://onto.fel.cvut.cz/ontologies/2014/ECCAIRS_Aviation_1.3.0.12/eccairs-descriptive-factors#category_11124000"/>
    </owl:Class>
    


    <!-- http://onto.fel.cvut.cz/ontologies/aviation-safety/Cooling_fan_system -->

    <owl:Class rdf:about="&m;Cooling_fan_system">
        <rdfs:label>Cooling fan system</rdfs:label>
        <rdfs:subClassOf rdf:resource="&m;Main_rotor_gearbox_part"/>
        <m:generated_time rdf:datatype="&xsd;dateTime">2015-04-09T18:56:27.771+02:00</m:generated_time>
        <rdfs:comment xml:lang="en">(ATA Code:6322) Cooling fan system: The component which provides a cooling air flow to the rotorcraft piston engine cylinders and oil coolers. Typical parts are fan, shroud, blade, impeller, duct, drive belt and stator.</rdfs:comment>
        <m:has_related_eccairs_term rdf:resource="http://onto.fel.cvut.cz/ontologies/2014/ECCAIRS_Aviation_1.3.0.12/eccairs-descriptive-factors#category_11632200"/>
    </owl:Class>
    


    <!-- http://onto.fel.cvut.cz/ontologies/aviation-safety/Cowl_flap_system -->

    <owl:Class rdf:about="&m;Cowl_flap_system">
        <rdfs:label>Cowl flap system</rdfs:label>
        <rdfs:subClassOf rdf:resource="&m;Engine_cowling_system_part"/>
        <m:generated_time rdf:datatype="&xsd;dateTime">2015-04-09T18:56:27.771+02:00</m:generated_time>
        <rdfs:comment xml:lang="en">(ATA Code:7111) Cowl flap system: The moveable flaps mounted in the engine cowling for increasing cooling air flow. Also includes the component which electrically or hydraulically actuates the cowl flaps. Typical parts are actuator, piston, seal and hinge brackets.</rdfs:comment>
        <m:has_related_eccairs_term rdf:resource="http://onto.fel.cvut.cz/ontologies/2014/ECCAIRS_Aviation_1.3.0.12/eccairs-descriptive-factors#category_11711100"/>
    </owl:Class>
    


    <!-- http://onto.fel.cvut.cz/ontologies/aviation-safety/Crew_oxygen_system -->

    <owl:Class rdf:about="&m;Crew_oxygen_system">
        <rdfs:label>Crew oxygen system</rdfs:label>
        <rdfs:subClassOf rdf:resource="&m;Oxygen_system_part"/>
        <m:generated_time rdf:datatype="&xsd;dateTime">2015-04-09T18:56:27.771+02:00</m:generated_time>
        <rdfs:comment xml:lang="en">(ATA Code:3510) Crew oxygen system: The portion of the main system which furnishes oxygen to the crew.</rdfs:comment>
        <m:has_related_eccairs_term rdf:resource="http://onto.fel.cvut.cz/ontologies/2014/ECCAIRS_Aviation_1.3.0.12/eccairs-descriptive-factors#category_11351000"/>
    </owl:Class>
    


    <!-- http://onto.fel.cvut.cz/ontologies/aviation-safety/Cylinder_head_temperature_indicating_system -->

    <owl:Class rdf:about="&m;Cylinder_head_temperature_indicating_system">
        <rdfs:label>Cylinder head temperature indicating system</rdfs:label>
        <rdfs:subClassOf rdf:resource="&m;Engine_temperature_indicating_system_part"/>
        <m:generated_time rdf:datatype="&xsd;dateTime">2015-04-09T18:56:27.771+02:00</m:generated_time>
        <rdfs:comment xml:lang="en">(ATA Code:7721) Cylinder head temperature indicating system: The instruments which indicate temperature measured at reciprocating engine cylinder heads. Typical parts are indicator, case, dial, needle, thermocouple lead, sensor and connector.</rdfs:comment>
        <m:has_related_eccairs_term rdf:resource="http://onto.fel.cvut.cz/ontologies/2014/ECCAIRS_Aviation_1.3.0.12/eccairs-descriptive-factors#category_11772100"/>
    </owl:Class>
    


    <!-- http://onto.fel.cvut.cz/ontologies/aviation-safety/Data_transmission_automatic_call -->

    <owl:Class rdf:about="&m;Data_transmission_automatic_call">
        <rdfs:label>Data transmission automatic call</rdfs:label>
        <rdfs:subClassOf rdf:resource="&m;Aircraft_communication_related_system"/>
        <m:generated_time rdf:datatype="&xsd;dateTime">2015-04-09T18:56:27.771+02:00</m:generated_time>
        <rdfs:comment xml:lang="en">(ATA Code:2320) Data transmission automatic call: That portion of the system which presents information derived from pulse coded transmissions. Includes teleprinter, Selcal, Calsel and ACARS.</rdfs:comment>
        <m:has_related_eccairs_term rdf:resource="http://onto.fel.cvut.cz/ontologies/2014/ECCAIRS_Aviation_1.3.0.12/eccairs-descriptive-factors#category_11232000"/>
    </owl:Class>
    


    <!-- http://onto.fel.cvut.cz/ontologies/aviation-safety/Data_transmission_automatic_call_part -->

    <owl:Class rdf:about="&m;Data_transmission_automatic_call_part">
        <rdfs:label>Data transmission automatic call part</rdfs:label>
        <rdfs:subClassOf rdf:resource="&m;Aircraft_communication_related_system"/>
        <rdfs:subClassOf>
            <owl:Restriction>
                <owl:onProperty rdf:resource="http://onto.fel.cvut.cz/ontologies/ufo/is_part_of"/>
                <owl:someValuesFrom rdf:resource="&m;Data_transmission_automatic_call"/>
            </owl:Restriction>
        </rdfs:subClassOf>
        <m:generated_time rdf:datatype="&xsd;dateTime">2015-04-12T02:45:54.351+02:00</m:generated_time>
        <m:has_related_eccairs_term rdf:resource="http://onto.fel.cvut.cz/ontologies/2014/ECCAIRS_Aviation_1.3.0.12/eccairs-descriptive-factors#category_11232000"/>
    </owl:Class>
    


    <!-- http://onto.fel.cvut.cz/ontologies/aviation-safety/Dependent_position_determining_system -->

    <owl:Class rdf:about="&m;Dependent_position_determining_system">
        <rdfs:label>Dependent position determining system</rdfs:label>
        <rdfs:subClassOf rdf:resource="&m;Navigation_system"/>
        <m:generated_time rdf:datatype="&xsd;dateTime">2015-04-09T18:56:27.771+02:00</m:generated_time>
        <m:generated_time rdf:datatype="&xsd;dateTime">2015-04-12T02:45:54.351+02:00</m:generated_time>
        <rdfs:comment xml:lang="en">(ATA Code:3450) Dependent position determining systems: The system which provides information to determine position and is dependent on ground installations or orbital satellites.</rdfs:comment>
        <m:has_related_eccairs_term rdf:resource="http://onto.fel.cvut.cz/ontologies/2014/ECCAIRS_Aviation_1.3.0.12/eccairs-descriptive-factors#category_11345000"/>
    </owl:Class>
    


    <!-- http://onto.fel.cvut.cz/ontologies/aviation-safety/Direct_current_distribution_system -->

    <owl:Class rdf:about="&m;Direct_current_distribution_system">
        <rdfs:label>Direct current distribution system</rdfs:label>
        <rdfs:subClassOf rdf:resource="&m;Electrical_power_system_part"/>
        <m:generated_time rdf:datatype="&xsd;dateTime">2015-04-09T18:56:27.771+02:00</m:generated_time>
        <rdfs:comment xml:lang="en">(ATA Code:2460) Direct current distribution system: The electrical system which provides for connection of direct current to using systems. Does not include using system. Typical parts are main and secondary system busses, circuit breaker, bus tie breaker, limiter, jumper and load motor switch.</rdfs:comment>
        <m:has_related_eccairs_term rdf:resource="http://onto.fel.cvut.cz/ontologies/2014/ECCAIRS_Aviation_1.3.0.12/eccairs-descriptive-factors#category_11246000"/>
    </owl:Class>
    


    <!-- http://onto.fel.cvut.cz/ontologies/aviation-safety/Direct_current_generating_system -->

    <owl:Class rdf:about="&m;Direct_current_generating_system">
        <rdfs:label>Direct current generating system</rdfs:label>
        <rdfs:subClassOf rdf:resource="&m;Electrical_power_system_part"/>
        <m:generated_time rdf:datatype="&xsd;dateTime">2015-04-09T18:56:27.771+02:00</m:generated_time>
        <rdfs:comment xml:lang="en">(ATA Code:2430) Direct current generating system: The system parts and circuitry other than the generator/alternator and direct current generation system regulator used to generate a direct current; or from an alternator, the output of which is rectified to direct current. Typical parts are relay, switch, connector, terminal, sensor and reverse current relay. Such systems are more prevalent on light single and twin engine aircraft.</rdfs:comment>
        <m:has_related_eccairs_term rdf:resource="http://onto.fel.cvut.cz/ontologies/2014/ECCAIRS_Aviation_1.3.0.12/eccairs-descriptive-factors#category_11243000"/>
    </owl:Class>
    


    <!-- http://onto.fel.cvut.cz/ontologies/aviation-safety/Direct_current_generating_system_part -->

    <owl:Class rdf:about="&m;Direct_current_generating_system_part">
        <rdfs:label>Direct current generating system part</rdfs:label>
        <rdfs:subClassOf rdf:resource="&m;Electrical_power_system_part"/>
        <rdfs:subClassOf>
            <owl:Restriction>
                <owl:onProperty rdf:resource="http://onto.fel.cvut.cz/ontologies/ufo/is_part_of"/>
                <owl:someValuesFrom rdf:resource="&m;Direct_current_generating_system"/>
            </owl:Restriction>
        </rdfs:subClassOf>
        <m:generated_time rdf:datatype="&xsd;dateTime">2015-04-12T02:45:54.351+02:00</m:generated_time>
        <m:has_related_eccairs_term rdf:resource="http://onto.fel.cvut.cz/ontologies/2014/ECCAIRS_Aviation_1.3.0.12/eccairs-descriptive-factors#category_11243000"/>
    </owl:Class>
    


    <!-- http://onto.fel.cvut.cz/ontologies/aviation-safety/Direct_current_generator-alternator -->

    <owl:Class rdf:about="&m;Direct_current_generator-alternator">
        <rdfs:label>Direct current generator-alternator</rdfs:label>
        <rdfs:subClassOf rdf:resource="&m;Direct_current_generating_system_part"/>
        <m:generated_time rdf:datatype="&xsd;dateTime">2015-04-09T18:56:27.771+02:00</m:generated_time>
        <rdfs:comment xml:lang="en">(ATA Code:2434) Direct current generator-alternator: The engine driven component generating a direct current or a rectified alternating current for aircraft with direct current electrical systems. Does not include mounting brackets, drive belts and pulleys external to the unit. Typical parts are bearing, housing, coupling, fan, capacitor, drive, brush, seal, clutch, armature and bell, shaft, field winding, case bolt and ground stud.</rdfs:comment>
        <m:has_related_eccairs_term rdf:resource="http://onto.fel.cvut.cz/ontologies/2014/ECCAIRS_Aviation_1.3.0.12/eccairs-descriptive-factors#category_11243400"/>
    </owl:Class>
    


    <!-- http://onto.fel.cvut.cz/ontologies/aviation-safety/Direct_current_indicating_system -->

    <owl:Class rdf:about="&m;Direct_current_indicating_system">
        <rdfs:label>Direct current indicating system</rdfs:label>
        <rdfs:subClassOf rdf:resource="&m;Direct_current_generating_system_part"/>
        <m:generated_time rdf:datatype="&xsd;dateTime">2015-04-09T18:56:27.771+02:00</m:generated_time>
        <rdfs:comment xml:lang="en">(ATA Code:2437) Direct current indicating system: The system which indicates voltage, current flow and system faults in the direct current power system.</rdfs:comment>
        <m:has_related_eccairs_term rdf:resource="http://onto.fel.cvut.cz/ontologies/2014/ECCAIRS_Aviation_1.3.0.12/eccairs-descriptive-factors#category_11243700"/>
    </owl:Class>
    


    <!-- http://onto.fel.cvut.cz/ontologies/aviation-safety/Direct_current_rectifier-converter -->

    <owl:Class rdf:about="&m;Direct_current_rectifier-converter">
        <rdfs:label>Direct current rectifier-converter</rdfs:label>
        <rdfs:subClassOf rdf:resource="&m;Direct_current_generating_system_part"/>
        <m:generated_time rdf:datatype="&xsd;dateTime">2015-04-09T18:56:27.771+02:00</m:generated_time>
        <rdfs:comment xml:lang="en">(ATA Code:2433) Direct current rectifier-converter: The component which converts alternating current to direct current for the using system(s).</rdfs:comment>
        <m:has_related_eccairs_term rdf:resource="http://onto.fel.cvut.cz/ontologies/2014/ECCAIRS_Aviation_1.3.0.12/eccairs-descriptive-factors#category_11243300"/>
    </owl:Class>
    


    <!-- http://onto.fel.cvut.cz/ontologies/aviation-safety/Direct_current_voltage_regulator -->

    <owl:Class rdf:about="&m;Direct_current_voltage_regulator">
        <rdfs:label>Direct current voltage regulator</rdfs:label>
        <rdfs:subClassOf rdf:resource="&m;Direct_current_generating_system_part"/>
        <m:generated_time rdf:datatype="&xsd;dateTime">2015-04-09T18:56:27.771+02:00</m:generated_time>
        <rdfs:comment xml:lang="en">(ATA Code:2436) Direct current voltage regulator: The component that regulates direct current voltage supplied from a generator or alternator.</rdfs:comment>
        <m:has_related_eccairs_term rdf:resource="http://onto.fel.cvut.cz/ontologies/2014/ECCAIRS_Aviation_1.3.0.12/eccairs-descriptive-factors#category_11243600"/>
    </owl:Class>
    


    <!-- http://onto.fel.cvut.cz/ontologies/aviation-safety/Directional_gyro_and_indicating_system -->

    <owl:Class rdf:about="&m;Directional_gyro_and_indicating_system">
        <rdfs:label>Directional gyro and indicating system</rdfs:label>
        <rdfs:subClassOf rdf:resource="&m;Attitude_and_direction_data_system_part"/>
        <m:generated_time rdf:datatype="&xsd;dateTime">2015-04-09T18:56:27.771+02:00</m:generated_time>
        <rdfs:comment xml:lang="en">(ATA Code:3422) Directional gyro and indicating system: The unit operating by gyroscopic principle and driven by airflow or an electric motor, which provides heading (direction) references relative to a preset heading in degrees of the compass. Also for the flux unit detector which senses the earth&apos;s magnetic field and uses this data to correct for gyro drift. Typical parts are gyro, rotor and bearings.</rdfs:comment>
        <m:has_related_eccairs_term rdf:resource="http://onto.fel.cvut.cz/ontologies/2014/ECCAIRS_Aviation_1.3.0.12/eccairs-descriptive-factors#category_11342200"/>
    </owl:Class>
    


    <!-- http://onto.fel.cvut.cz/ontologies/aviation-safety/Distance_measuring_equipment-ultra_high_frequency_tactical_air_navigation_aid -->

    <owl:Class rdf:about="&m;Distance_measuring_equipment-ultra_high_frequency_tactical_air_navigation_aid">
        <rdfs:label>Distance measuring equipment/ultra high frequency tactical air navigation aid</rdfs:label>
        <rdfs:subClassOf rdf:resource="&m;Dependent_position_determining_system"/>
        <m:generated_time rdf:datatype="&xsd;dateTime">2015-04-09T18:56:27.771+02:00</m:generated_time>
        <rdfs:comment xml:lang="en">(ATA Code:3451) Distance measuring equipment/ultra high frequency tactical air navigation aid: The systems which measure time-to-station, ground speed and distance to a known transmitter location by transmitting and receiving electronic pulse signals e.g. distance measuring equipment; ultra high frequency tactical air navigational aid. Typical parts are antenna, control unit, transceiver and coaxial cables.</rdfs:comment>
        <m:has_related_eccairs_term rdf:resource="http://onto.fel.cvut.cz/ontologies/2014/ECCAIRS_Aviation_1.3.0.12/eccairs-descriptive-factors#category_11345100"/>
    </owl:Class>
    


    <!-- http://onto.fel.cvut.cz/ontologies/aviation-safety/Door_attachment_fittings-hinges__(on_fuselage) -->

    <owl:Class rdf:about="&m;Door_attachment_fittings-hinges__(on_fuselage)">
        <rdfs:label>Door attachment fittings/hinges  (on fuselage)</rdfs:label>
        <rdfs:subClassOf rdf:resource="&m;Fuselage_attachment_fittings_part"/>
        <m:generated_time rdf:datatype="&xsd;dateTime">2015-04-09T18:56:27.771+02:00</m:generated_time>
        <rdfs:comment xml:lang="en">(ATA Code:5344) The fittings on the fuselage used for the attachment of the doors.</rdfs:comment>
        <m:has_related_eccairs_term rdf:resource="http://onto.fel.cvut.cz/ontologies/2014/ECCAIRS_Aviation_1.3.0.12/eccairs-descriptive-factors#category_11534400"/>
    </owl:Class>
    


    <!-- http://onto.fel.cvut.cz/ontologies/aviation-safety/Door_system_wiring -->

    <owl:Class rdf:about="&m;Door_system_wiring">
        <rdfs:label xml:lang="en">Door system wiring</rdfs:label>
        <rdfs:subClassOf rdf:resource="&m;Fuselage_doors_part"/>
        <rdfs:subClassOf rdf:resource="&m;Wiring"/>
        <rdfs:subClassOf>
            <owl:Restriction>
                <owl:onProperty rdf:resource="http://onto.fel.cvut.cz/ontologies/ufo/is_part_of"/>
                <owl:someValuesFrom rdf:resource="&m;Fuselage_doors"/>
            </owl:Restriction>
        </rdfs:subClassOf>
    </owl:Class>
    


    <!-- http://onto.fel.cvut.cz/ontologies/aviation-safety/Door_warning_system -->

    <owl:Class rdf:about="&m;Door_warning_system">
        <rdfs:label>Door warning system</rdfs:label>
        <rdfs:subClassOf rdf:resource="&m;Fuselage_doors_part"/>
        <m:generated_time rdf:datatype="&xsd;dateTime">2015-04-09T18:56:27.771+02:00</m:generated_time>
        <rdfs:comment xml:lang="en">(ATA Code:5270) Door warning system: The system which is used to indicate to the flight crew whether the exterior doors are closed and properly latched. Does not include the landing gear position warning indications [Code 11326000]. Typical parts are switch, lamp, horn and relay.</rdfs:comment>
        <m:has_related_eccairs_term rdf:resource="http://onto.fel.cvut.cz/ontologies/2014/ECCAIRS_Aviation_1.3.0.12/eccairs-descriptive-factors#category_11527000"/>
    </owl:Class>
    


    <!-- http://onto.fel.cvut.cz/ontologies/aviation-safety/Door_windows -->

    <owl:Class rdf:about="&m;Door_windows">
        <rdfs:label>Door windows</rdfs:label>
        <rdfs:subClassOf rdf:resource="&m;Window-windshield_system_part"/>
        <m:generated_time rdf:datatype="&xsd;dateTime">2015-04-09T18:56:27.771+02:00</m:generated_time>
        <rdfs:comment xml:lang="en">(ATA Code:5630) Door windows: The windows mounted in doors. Does not include emergency exit windows [Code 11522000].</rdfs:comment>
        <m:has_related_eccairs_term rdf:resource="http://onto.fel.cvut.cz/ontologies/2014/ECCAIRS_Aviation_1.3.0.12/eccairs-descriptive-factors#category_11563000"/>
    </owl:Class>
    


    <!-- http://onto.fel.cvut.cz/ontologies/aviation-safety/Doppler_system -->

    <owl:Class rdf:about="&m;Doppler_system">
        <rdfs:label>Doppler system</rdfs:label>
        <rdfs:subClassOf rdf:resource="&m;Independent_position_determining_system"/>
        <m:generated_time rdf:datatype="&xsd;dateTime">2015-04-09T18:56:27.771+02:00</m:generated_time>
        <rdfs:comment xml:lang="en">(ATA Code:3443) Doppler system: The airborne radar system which utilizes the doppler effect to measure and display ground speed, drift angle and cross track error.</rdfs:comment>
        <m:has_related_eccairs_term rdf:resource="http://onto.fel.cvut.cz/ontologies/2014/ECCAIRS_Aviation_1.3.0.12/eccairs-descriptive-factors#category_11344300"/>
    </owl:Class>
    


    <!-- http://onto.fel.cvut.cz/ontologies/aviation-safety/Drag_control_actuator -->

    <owl:Class rdf:about="&m;Drag_control_actuator">
        <rdfs:label>Drag control actuator</rdfs:label>
        <rdfs:subClassOf rdf:resource="&m;Drag_control_system_part"/>
        <m:generated_time rdf:datatype="&xsd;dateTime">2015-04-09T18:56:27.771+02:00</m:generated_time>
        <rdfs:comment xml:lang="en">(ATA Code:2761) Drag control actuator: The components that actuate spoiler and speed brake surfaces on the wing for speed and lift reducing purposes. Typical parts are seal, rod end bearing and rod end.</rdfs:comment>
        <m:has_related_eccairs_term rdf:resource="http://onto.fel.cvut.cz/ontologies/2014/ECCAIRS_Aviation_1.3.0.12/eccairs-descriptive-factors#category_11276100"/>
    </owl:Class>
    


    <!-- http://onto.fel.cvut.cz/ontologies/aviation-safety/Drag_control_system -->

    <owl:Class rdf:about="&m;Drag_control_system">
        <rdfs:label>Drag control system</rdfs:label>
        <rdfs:subClassOf rdf:resource="&m;Flight_control_system_part"/>
        <m:generated_time rdf:datatype="&xsd;dateTime">2015-04-09T18:56:27.771+02:00</m:generated_time>
        <rdfs:comment xml:lang="en">(ATA Code:2760) Drag control system: The system components, other than actuator, which control position and movement and indicates relative position of drag devices and variable aerodynamic surfaces on the wing including speed brake systems. Does not include structure and hinges [Code 11575500]. Typical parts are valve, hose, push rod, line, cable and indicator.</rdfs:comment>
        <m:has_related_eccairs_term rdf:resource="http://onto.fel.cvut.cz/ontologies/2014/ECCAIRS_Aviation_1.3.0.12/eccairs-descriptive-factors#category_11276000"/>
    </owl:Class>
    


    <!-- http://onto.fel.cvut.cz/ontologies/aviation-safety/Drag_control_system_part -->

    <owl:Class rdf:about="&m;Drag_control_system_part">
        <rdfs:label>Drag control system part</rdfs:label>
        <rdfs:subClassOf rdf:resource="&m;Flight_control_system_part"/>
        <rdfs:subClassOf>
            <owl:Restriction>
                <owl:onProperty rdf:resource="http://onto.fel.cvut.cz/ontologies/ufo/is_part_of"/>
                <owl:someValuesFrom rdf:resource="&m;Drag_control_system"/>
            </owl:Restriction>
        </rdfs:subClassOf>
        <m:generated_time rdf:datatype="&xsd;dateTime">2015-04-12T02:45:54.351+02:00</m:generated_time>
        <m:has_related_eccairs_term rdf:resource="http://onto.fel.cvut.cz/ontologies/2014/ECCAIRS_Aviation_1.3.0.12/eccairs-descriptive-factors#category_11276000"/>
    </owl:Class>
    


    <!-- http://onto.fel.cvut.cz/ontologies/aviation-safety/ENGINE_TURBINE-TURBO_PROP_DUCTED_FAN-UNDUCTED_FAN -->

    <owl:Class rdf:about="&m;ENGINE_TURBINE-TURBO_PROP_DUCTED_FAN-UNDUCTED_FAN">
        <rdfs:label>ENGINE TURBINE/TURBO PROP DUCTED FAN/UNDUCTED FAN</rdfs:label>
        <rdfs:subClassOf rdf:resource="&m;Aircraft_part"/>
        <m:generated_time rdf:datatype="&xsd;dateTime">2015-04-09T18:56:27.771+02:00</m:generated_time>
        <rdfs:comment xml:lang="en">(ATA Code:7200) Turbine/turboprop engine: The units and components which are used to induce and convert fuel-air mixture into power and to transmit power to the propeller shaft, if any, and accessory drives. Includes bird strikes to engine cowlings.</rdfs:comment>
        <m:has_related_eccairs_term rdf:resource="http://onto.fel.cvut.cz/ontologies/2014/ECCAIRS_Aviation_1.3.0.12/eccairs-descriptive-factors#category_11720000"/>
    </owl:Class>
    


    <!-- http://onto.fel.cvut.cz/ontologies/aviation-safety/ENGINE_TURBINE-TURBO_PROP_DUCTED_FAN-UNDUCTED_FAN_part -->

    <owl:Class rdf:about="&m;ENGINE_TURBINE-TURBO_PROP_DUCTED_FAN-UNDUCTED_FAN_part">
        <rdfs:label>ENGINE TURBINE/TURBO PROP DUCTED FAN/UNDUCTED FAN part</rdfs:label>
        <rdfs:subClassOf rdf:resource="&m;Aircraft_part"/>
        <rdfs:subClassOf>
            <owl:Restriction>
                <owl:onProperty rdf:resource="http://onto.fel.cvut.cz/ontologies/ufo/is_part_of"/>
                <owl:someValuesFrom rdf:resource="&m;ENGINE_TURBINE-TURBO_PROP_DUCTED_FAN-UNDUCTED_FAN"/>
            </owl:Restriction>
        </rdfs:subClassOf>
        <m:generated_time rdf:datatype="&xsd;dateTime">2015-04-12T02:45:54.351+02:00</m:generated_time>
        <m:has_related_eccairs_term rdf:resource="http://onto.fel.cvut.cz/ontologies/2014/ECCAIRS_Aviation_1.3.0.12/eccairs-descriptive-factors#category_11720000"/>
    </owl:Class>
    


    <!-- http://onto.fel.cvut.cz/ontologies/aviation-safety/Electric-electronic_compartment_doors -->

    <owl:Class rdf:about="&m;Electric-electronic_compartment_doors">
        <rdfs:label>Electric/electronic compartment doors</rdfs:label>
        <rdfs:subClassOf rdf:resource="&m;Service_doors_part"/>
        <m:generated_time rdf:datatype="&xsd;dateTime">2015-04-09T18:56:27.771+02:00</m:generated_time>
        <rdfs:comment xml:lang="en">(ATA Code:5242) Electric/electronic compartment doors: The exterior doors used primarily to gain access for servicing the electrical/electronic compartment. Typical parts are hinges, structure and the latch mechanism.</rdfs:comment>
        <m:has_related_eccairs_term rdf:resource="http://onto.fel.cvut.cz/ontologies/2014/ECCAIRS_Aviation_1.3.0.12/eccairs-descriptive-factors#category_11524200"/>
    </owl:Class>
    


    <!-- http://onto.fel.cvut.cz/ontologies/aviation-safety/Electrical_Connectors -->

    <owl:Class rdf:about="&m;Electrical_Connectors">
        <rdfs:label>Electrical Connectors</rdfs:label>
        <rdfs:subClassOf rdf:resource="&m;Miscellaneous_hardware_part"/>
        <m:generated_time rdf:datatype="&xsd;dateTime">2015-04-09T18:56:27.771+02:00</m:generated_time>
        <rdfs:comment xml:lang="en">(ATA Code:1420) Any aircraft or engine electrical connector that is not associated a specific aircraft system.</rdfs:comment>
        <m:has_related_eccairs_term rdf:resource="http://onto.fel.cvut.cz/ontologies/2014/ECCAIRS_Aviation_1.3.0.12/eccairs-descriptive-factors#category_11142000"/>
    </owl:Class>
    


    <!-- http://onto.fel.cvut.cz/ontologies/aviation-safety/Electrical_Power_System_Wiring -->

    <owl:Class rdf:about="&m;Electrical_Power_System_Wiring">
        <rdfs:subClassOf rdf:resource="&m;Electrical_power_system_part"/>
    </owl:Class>
    


    <!-- http://onto.fel.cvut.cz/ontologies/aviation-safety/Electrical_power_system -->

    <owl:Class rdf:about="&m;Electrical_power_system">
        <rdfs:subClassOf rdf:resource="&m;Aircraft_part"/>
    </owl:Class>
    


    <!-- http://onto.fel.cvut.cz/ontologies/aviation-safety/Electrical_power_system_part -->

    <owl:Class rdf:about="&m;Electrical_power_system_part">
        <rdfs:label>Electrical power system part</rdfs:label>
        <rdfs:subClassOf rdf:resource="&m;Aircraft_part"/>
        <rdfs:subClassOf>
            <owl:Restriction>
                <owl:onProperty rdf:resource="http://onto.fel.cvut.cz/ontologies/ufo/is_part_of"/>
                <owl:someValuesFrom rdf:resource="&m;Electrical_power_system"/>
            </owl:Restriction>
        </rdfs:subClassOf>
        <m:generated_time rdf:datatype="&xsd;dateTime">2015-04-12T02:45:54.351+02:00</m:generated_time>
        <m:has_related_eccairs_term rdf:resource="http://onto.fel.cvut.cz/ontologies/2014/ECCAIRS_Aviation_1.3.0.12/eccairs-descriptive-factors#category_11240000"/>
    </owl:Class>
    


    <!-- http://onto.fel.cvut.cz/ontologies/aviation-safety/Electronic_shelf_section -->

    <owl:Class rdf:about="&m;Electronic_shelf_section">
        <rdfs:label>Electronic shelf section</rdfs:label>
        <rdfs:subClassOf rdf:resource="&m;Accessory_compartments_part"/>
        <m:generated_time rdf:datatype="&xsd;dateTime">2015-04-09T18:56:27.771+02:00</m:generated_time>
        <rdfs:comment xml:lang="en">(ATA Code:2572) Electronic shelf section: The shelves and attaching parts supporting the electronic equipment within the fuselage. Does not include the equipment used for equipment cooling such as fans and blower motors.</rdfs:comment>
        <m:has_related_eccairs_term rdf:resource="http://onto.fel.cvut.cz/ontologies/2014/ECCAIRS_Aviation_1.3.0.12/eccairs-descriptive-factors#category_11257200"/>
    </owl:Class>
    


    <!-- http://onto.fel.cvut.cz/ontologies/aviation-safety/Elevator-tab_attachment_fitting -->

    <owl:Class rdf:about="&m;Elevator-tab_attachment_fitting">
        <rdfs:label>Elevator/tab attachment fitting</rdfs:label>
        <rdfs:subClassOf rdf:resource="&m;Attachment_fitting_(empennage_flight_control_surfaces)_part"/>
        <m:generated_time rdf:datatype="&xsd;dateTime">2015-04-09T18:56:27.771+02:00</m:generated_time>
        <rdfs:comment xml:lang="en">(ATA Code:5552) Elevator/tab attachment fitting: The fittings on the elevator or elevator tab which are used to support equipment within the structure.</rdfs:comment>
        <m:has_related_eccairs_term rdf:resource="http://onto.fel.cvut.cz/ontologies/2014/ECCAIRS_Aviation_1.3.0.12/eccairs-descriptive-factors#category_11555200"/>
    </owl:Class>
    


    <!-- http://onto.fel.cvut.cz/ontologies/aviation-safety/Elevator_&amp;_Tab_control_system -->

    <owl:Class rdf:about="&m;Elevator_&amp;_Tab_control_system">
        <rdfs:label>Elevator &amp; Tab control system</rdfs:label>
        <rdfs:subClassOf rdf:resource="&m;Flight_control_system_part"/>
        <m:generated_time rdf:datatype="&xsd;dateTime">2015-04-09T18:56:27.771+02:00</m:generated_time>
        <rdfs:comment xml:lang="en">(ATA Code:2730) Elevator control system: The system components and parts including actuator from the control column to the elevators that cause movement. Includes control actuating mechanism for &quot;ruddervators&quot; installed on &quot;V&quot; tail aircraft. Does not include hinges, structure and balance weights [Code 11552000], or the auto-pilot servo [Code 11221600]. Typical parts are torque tube, cable, rod end, stops, actuator, feel computer, bracket and control valve.</rdfs:comment>
        <m:has_related_eccairs_term rdf:resource="http://onto.fel.cvut.cz/ontologies/2014/ECCAIRS_Aviation_1.3.0.12/eccairs-descriptive-factors#category_11273000"/>
    </owl:Class>
    


    <!-- http://onto.fel.cvut.cz/ontologies/aviation-safety/Elevator_&amp;_Tab_control_system_part -->

    <owl:Class rdf:about="&m;Elevator_&amp;_Tab_control_system_part">
        <rdfs:label>Elevator &amp; Tab control system part</rdfs:label>
        <rdfs:subClassOf rdf:resource="&m;Flight_control_system_part"/>
        <rdfs:subClassOf>
            <owl:Restriction>
                <owl:onProperty rdf:resource="http://onto.fel.cvut.cz/ontologies/ufo/is_part_of"/>
                <owl:someValuesFrom rdf:resource="&m;Elevator_&amp;_Tab_control_system"/>
            </owl:Restriction>
        </rdfs:subClassOf>
        <m:generated_time rdf:datatype="&xsd;dateTime">2015-04-12T02:45:54.351+02:00</m:generated_time>
        <m:has_related_eccairs_term rdf:resource="http://onto.fel.cvut.cz/ontologies/2014/ECCAIRS_Aviation_1.3.0.12/eccairs-descriptive-factors#category_11273000"/>
    </owl:Class>
    


    <!-- http://onto.fel.cvut.cz/ontologies/aviation-safety/Elevator_feel_system -->

    <owl:Class rdf:about="&m;Elevator_feel_system">
        <rdfs:label>Elevator feel system</rdfs:label>
        <rdfs:subClassOf rdf:resource="&m;Elevator_&amp;_Tab_control_system_part"/>
        <m:generated_time rdf:datatype="&xsd;dateTime">2015-04-09T18:56:27.771+02:00</m:generated_time>
        <rdfs:comment xml:lang="en">(ATA Code:2733) Elevator feel system: The system incorporated in the elevator control system which provides artificial resistance to the pilot&apos;s input to the elevators.</rdfs:comment>
        <m:has_related_eccairs_term rdf:resource="http://onto.fel.cvut.cz/ontologies/2014/ECCAIRS_Aviation_1.3.0.12/eccairs-descriptive-factors#category_11273300"/>
    </owl:Class>
    


    <!-- http://onto.fel.cvut.cz/ontologies/aviation-safety/Elevator_structure -->

    <owl:Class rdf:about="&m;Elevator_structure">
        <rdfs:label>Elevator structure</rdfs:label>
        <rdfs:subClassOf rdf:resource="&m;Empennage_structure_part"/>
        <m:generated_time rdf:datatype="&xsd;dateTime">2015-04-09T18:56:27.771+02:00</m:generated_time>
        <rdfs:comment xml:lang="en">(ATA Code:5520) Elevator structure: The aerofoil hinged to the horizontal stabilizer for longitudinal control. Includes the &quot;ruddervator&quot; on V-tail aircraft and balance weights. Does not include the stabilator structure [Code 11551000] or the torque tubes [Code 11273000].</rdfs:comment>
        <m:has_related_eccairs_term rdf:resource="http://onto.fel.cvut.cz/ontologies/2014/ECCAIRS_Aviation_1.3.0.12/eccairs-descriptive-factors#category_11552000"/>
    </owl:Class>
    


    <!-- http://onto.fel.cvut.cz/ontologies/aviation-safety/Elevator_structure_part -->

    <owl:Class rdf:about="&m;Elevator_structure_part">
        <rdfs:label>Elevator structure part</rdfs:label>
        <rdfs:subClassOf rdf:resource="&m;Empennage_structure_part"/>
        <rdfs:subClassOf>
            <owl:Restriction>
                <owl:onProperty rdf:resource="http://onto.fel.cvut.cz/ontologies/ufo/is_part_of"/>
                <owl:someValuesFrom rdf:resource="&m;Elevator_structure"/>
            </owl:Restriction>
        </rdfs:subClassOf>
        <m:generated_time rdf:datatype="&xsd;dateTime">2015-04-12T02:45:54.351+02:00</m:generated_time>
        <m:has_related_eccairs_term rdf:resource="http://onto.fel.cvut.cz/ontologies/2014/ECCAIRS_Aviation_1.3.0.12/eccairs-descriptive-factors#category_11552000"/>
    </owl:Class>
    


    <!-- http://onto.fel.cvut.cz/ontologies/aviation-safety/Elevator_tab_control_system -->

    <owl:Class rdf:about="&m;Elevator_tab_control_system">
        <rdfs:label>Elevator tab control system</rdfs:label>
        <rdfs:subClassOf rdf:resource="&m;Elevator_&amp;_Tab_control_system_part"/>
        <m:generated_time rdf:datatype="&xsd;dateTime">2015-04-09T18:56:27.771+02:00</m:generated_time>
        <rdfs:comment xml:lang="en">(ATA Code:2731) Elevator tab control system: The system components and parts from the cockpit trim control to the elevator, ruddervator or stabilator tab, which controls position and movement of the tab. Includes the manual and electrical trim system parts. Does not include the hinges or structure [Code 11552000] or the balance weights [Code 11552000] or the auto pilot servo [Code 11221600]. Typical parts are jackscrew, cable, actuator, sensor, motor, chain, sprocket and indicator.</rdfs:comment>
        <m:has_related_eccairs_term rdf:resource="http://onto.fel.cvut.cz/ontologies/2014/ECCAIRS_Aviation_1.3.0.12/eccairs-descriptive-factors#category_11273100"/>
    </owl:Class>
    


    <!-- http://onto.fel.cvut.cz/ontologies/aviation-safety/Elevator_tab_structure -->

    <owl:Class rdf:about="&m;Elevator_tab_structure">
        <rdfs:label>Elevator tab structure</rdfs:label>
        <rdfs:subClassOf rdf:resource="&m;Elevator_structure_part"/>
        <m:generated_time rdf:datatype="&xsd;dateTime">2015-04-09T18:56:27.771+02:00</m:generated_time>
        <rdfs:comment xml:lang="en">(ATA Code:5523) Elevator tab structure: The structure of elevator trim surfaces hinged to elevators and &quot;ruddervators.&quot; Includes hinge fittings and associated bearings and bolts. Does not include actuating mechanism [Code 11273100].</rdfs:comment>
        <m:has_related_eccairs_term rdf:resource="http://onto.fel.cvut.cz/ontologies/2014/ECCAIRS_Aviation_1.3.0.12/eccairs-descriptive-factors#category_11552300"/>
    </owl:Class>
    


    <!-- http://onto.fel.cvut.cz/ontologies/aviation-safety/Elevator_trim_system -->

    <owl:Class rdf:about="&m;Elevator_trim_system">
        <rdfs:label>Elevator trim system</rdfs:label>
        <rdfs:subClassOf rdf:resource="&m;Elevator_&amp;_Tab_control_system_part"/>
        <m:generated_time rdf:datatype="&xsd;dateTime">2015-04-09T18:56:27.771+02:00</m:generated_time>
        <rdfs:comment xml:lang="en">(ATA Code:2732) Elevator trim system: The system components and parts from the cockpit trim control to the elevator, ruddervator or stabilator tab, which control position and movement of the trim tab. Includes the manual and electrical trim system parts. Does not include the hinges.</rdfs:comment>
        <m:has_related_eccairs_term rdf:resource="http://onto.fel.cvut.cz/ontologies/2014/ECCAIRS_Aviation_1.3.0.12/eccairs-descriptive-factors#category_11273200"/>
    </owl:Class>
    


    <!-- http://onto.fel.cvut.cz/ontologies/aviation-safety/Emergency_clothing -->

    <owl:Class rdf:about="&m;Emergency_clothing">
        <rdfs:label>Emergency clothing</rdfs:label>
        <rdfs:subClassOf rdf:resource="&m;Cabin_equipment-furnishings"/>
        <m:generated_time rdf:datatype="&xsd;dateTime">2015-04-09T18:56:27.771+02:00</m:generated_time>
        <rdfs:comment xml:lang="en">(ATA Code:2590) Emergency clothing: The clothing stored permanently in the aircraft for use in an emergency.</rdfs:comment>
        <m:has_related_eccairs_term rdf:resource="http://onto.fel.cvut.cz/ontologies/2014/ECCAIRS_Aviation_1.3.0.12/eccairs-descriptive-factors#category_11259000"/>
    </owl:Class>
    


    <!-- http://onto.fel.cvut.cz/ontologies/aviation-safety/Emergency_equipment -->

    <owl:Class rdf:about="&m;Emergency_equipment">
        <rdfs:label>Emergency equipment</rdfs:label>
        <rdfs:subClassOf rdf:resource="&m;Cabin_equipment-furnishings"/>
        <rdfs:subClassOf>
            <owl:Restriction>
                <owl:onProperty rdf:resource="http://onto.fel.cvut.cz/ontologies/ufo/is_part_of"/>
                <owl:someValuesFrom rdf:resource="&m;Emergency_equipment"/>
            </owl:Restriction>
        </rdfs:subClassOf>
        <m:generated_time rdf:datatype="&xsd;dateTime">2015-04-12T02:45:54.351+02:00</m:generated_time>
        <m:has_related_eccairs_term rdf:resource="http://onto.fel.cvut.cz/ontologies/2014/ECCAIRS_Aviation_1.3.0.12/eccairs-descriptive-factors#category_11256000"/>
    </owl:Class>
    


    <!-- http://onto.fel.cvut.cz/ontologies/aviation-safety/Emergency_exits -->

    <owl:Class rdf:about="&m;Emergency_exits">
        <rdfs:label>Emergency exits</rdfs:label>
        <rdfs:subClassOf rdf:resource="&m;Fuselage_doors_part"/>
        <m:generated_time rdf:datatype="&xsd;dateTime">2015-04-09T18:56:27.771+02:00</m:generated_time>
        <rdfs:comment xml:lang="en">(ATA Code:5220) Emergency exits: The emergency exit doors, windows and hatches. Typical parts are pan, hinge, latch and hook.</rdfs:comment>
        <m:has_related_eccairs_term rdf:resource="http://onto.fel.cvut.cz/ontologies/2014/ECCAIRS_Aviation_1.3.0.12/eccairs-descriptive-factors#category_11522000"/>
    </owl:Class>
    


    <!-- http://onto.fel.cvut.cz/ontologies/aviation-safety/Emergency_lighting -->

    <owl:Class rdf:about="&m;Emergency_lighting">
        <rdfs:label>Emergency lighting</rdfs:label>
        <rdfs:subClassOf rdf:resource="&m;Lighting_system"/>
        <m:generated_time rdf:datatype="&xsd;dateTime">2015-04-09T18:56:27.771+02:00</m:generated_time>
        <rdfs:comment xml:lang="en">(ATA Code:3350) Emergency lighting: The cabin, flight compartment and exterior emergency lighting systems, which furnish illumination in event of electrical power failure. Includes items such as inertia flashlights and lanterns.</rdfs:comment>
        <m:has_related_eccairs_term rdf:resource="http://onto.fel.cvut.cz/ontologies/2014/ECCAIRS_Aviation_1.3.0.12/eccairs-descriptive-factors#category_11335000"/>
    </owl:Class>
    


    <!-- http://onto.fel.cvut.cz/ontologies/aviation-safety/Emergency_locator_beacon -->

    <owl:Class rdf:about="&m;Emergency_locator_beacon">
        <rdfs:label>Emergency locator beacon</rdfs:label>
        <rdfs:subClassOf rdf:resource="&m;Emergency_equipment"/>
        <m:generated_time rdf:datatype="&xsd;dateTime">2015-04-09T18:56:27.771+02:00</m:generated_time>
        <rdfs:comment xml:lang="en">(ATA Code:2562) Emergency locator beacon: The components transmitting an electronic signal on an emergency frequency to assist in locating an aircraft which has been involved in an accident. Typical parts are impact switch, antenna and battery pack.ELT: A generic term describing equipment which broadcast distinctive signals on designated frequencies and, depending on application, may be automatically activated by impact or be manually activated.  An ELT may be any of the following:Automatic fixed ELT (ELT(AF)).  An automatically activated ELT which is permanently attached to an aircraft.Automatic portable ELT (ELT(AP)).  An automatically activated ELT which is rigidly attached to an aircraft but readily removable from the aircraft.Automatic deployable ELT (ELT(AD)).  An ELT which is rigidly attached to an aircraft and which is automatically deployed and activated by impact, and, in some cases, also by hydrostatic sensors.  Manual deployment is also provided.Survival ELT (ELT(S)).  An ELT which is removable from an aircraft, stowed so as to facilitate its ready use in an emergency, and manually activated by survivors.(An 6/I, An 6/II, An 6/III, PANS-ABC)</rdfs:comment>
        <m:has_related_eccairs_term rdf:resource="http://onto.fel.cvut.cz/ontologies/2014/ECCAIRS_Aviation_1.3.0.12/eccairs-descriptive-factors#category_11256200"/>
    </owl:Class>
    


    <!-- http://onto.fel.cvut.cz/ontologies/aviation-safety/Empennage_structure -->

    <owl:Class rdf:about="&m;Empennage_structure">
        <rdfs:label>Empennage structure</rdfs:label>
        <rdfs:subClassOf rdf:resource="&m;Aircraft_part"/>
        <m:generated_time rdf:datatype="&xsd;dateTime">2015-04-09T18:56:27.771+02:00</m:generated_time>
        <rdfs:comment xml:lang="en">(ATA Code:5500) Empennage structure: The horizontal and vertical stabilizers include the structure of the elevator and rudder.</rdfs:comment>
        <m:has_related_eccairs_term rdf:resource="http://onto.fel.cvut.cz/ontologies/2014/ECCAIRS_Aviation_1.3.0.12/eccairs-descriptive-factors#category_11550000"/>
    </owl:Class>
    


    <!-- http://onto.fel.cvut.cz/ontologies/aviation-safety/Empennage_structure_part -->

    <owl:Class rdf:about="&m;Empennage_structure_part">
        <rdfs:label>Empennage structure part</rdfs:label>
        <rdfs:subClassOf rdf:resource="&m;Aircraft_part"/>
        <rdfs:subClassOf>
            <owl:Restriction>
                <owl:onProperty rdf:resource="http://onto.fel.cvut.cz/ontologies/ufo/is_part_of"/>
                <owl:someValuesFrom rdf:resource="&m;Empennage_structure"/>
            </owl:Restriction>
        </rdfs:subClassOf>
        <m:generated_time rdf:datatype="&xsd;dateTime">2015-04-12T02:45:54.351+02:00</m:generated_time>
        <m:has_related_eccairs_term rdf:resource="http://onto.fel.cvut.cz/ontologies/2014/ECCAIRS_Aviation_1.3.0.12/eccairs-descriptive-factors#category_11550000"/>
    </owl:Class>
    


    <!-- http://onto.fel.cvut.cz/ontologies/aviation-safety/Engine-transmission_coupling -->

    <owl:Class rdf:about="&m;Engine-transmission_coupling">
        <rdfs:label>Engine/transmission coupling</rdfs:label>
        <rdfs:subClassOf rdf:resource="&m;Main_rotor_drive_system_part"/>
        <m:generated_time rdf:datatype="&xsd;dateTime">2015-04-09T18:56:27.771+02:00</m:generated_time>
        <rdfs:comment xml:lang="en">(ATA Code:6310) Engine/transmission coupling: The drive shaft between the engine and the main gearbox including the clutch and freewheel units (if applicable) and tilt rotor interconnect system. Typical parts are clutch, shaft, coupling, bearing, boot, seal, sync shaft, pulley, pulley bracket and belt.</rdfs:comment>
        <m:has_related_eccairs_term rdf:resource="http://onto.fel.cvut.cz/ontologies/2014/ECCAIRS_Aviation_1.3.0.12/eccairs-descriptive-factors#category_11631000"/>
    </owl:Class>
    


    <!-- http://onto.fel.cvut.cz/ontologies/aviation-safety/Engine_Bleed_Air_System_Wiring -->

    <owl:Class rdf:about="&m;Engine_Bleed_Air_System_Wiring">
        <rdfs:label>Engine Bleed Air System Wiring</rdfs:label>
        <rdfs:subClassOf rdf:resource="&m;Engine_bleed_air_system_part"/>
        <rdfs:subClassOf rdf:resource="&m;Wiring"/>
        <rdfs:subClassOf>
            <owl:Restriction>
                <owl:onProperty rdf:resource="http://onto.fel.cvut.cz/ontologies/ufo/is_part_of"/>
                <owl:someValuesFrom rdf:resource="&m;Engine_bleed_air_system"/>
            </owl:Restriction>
        </rdfs:subClassOf>
        <m:generated_time rdf:datatype="&xsd;dateTime">2015-04-09T18:56:27.771+02:00</m:generated_time>
        <rdfs:comment xml:lang="en">(ATA Code:7597) Wiring specific to the Engine Bleed Air System.</rdfs:comment>
        <m:has_related_eccairs_term rdf:resource="http://onto.fel.cvut.cz/ontologies/2014/ECCAIRS_Aviation_1.3.0.12/eccairs-descriptive-factors#category_11759700"/>
    </owl:Class>
    


    <!-- http://onto.fel.cvut.cz/ontologies/aviation-safety/Engine_Control_System_Wiring -->

    <owl:Class rdf:about="&m;Engine_Control_System_Wiring">
        <rdfs:label>Engine Control System Wiring</rdfs:label>
        <rdfs:subClassOf rdf:resource="&m;Engine_controls_part"/>
        <m:generated_time rdf:datatype="&xsd;dateTime">2015-04-09T18:56:27.771+02:00</m:generated_time>
        <rdfs:comment xml:lang="en">(ATA Code:7697) Wiring specific to the Engine Control System</rdfs:comment>
        <m:has_related_eccairs_term rdf:resource="http://onto.fel.cvut.cz/ontologies/2014/ECCAIRS_Aviation_1.3.0.12/eccairs-descriptive-factors#category_11769700"/>
    </owl:Class>
    


    <!-- http://onto.fel.cvut.cz/ontologies/aviation-safety/Engine_Exhaust_System_Wiring -->

    <owl:Class rdf:about="&m;Engine_Exhaust_System_Wiring">
        <rdfs:label>Engine Exhaust System Wiring</rdfs:label>
        <rdfs:subClassOf rdf:resource="&m;Engine_exhaust_system_part"/>
        <rdfs:subClassOf rdf:resource="&m;Wiring"/>
        <rdfs:subClassOf>
            <owl:Restriction>
                <owl:onProperty rdf:resource="http://onto.fel.cvut.cz/ontologies/ufo/is_part_of"/>
                <owl:someValuesFrom rdf:resource="&m;Engine_exhaust_system"/>
            </owl:Restriction>
        </rdfs:subClassOf>
        <m:generated_time rdf:datatype="&xsd;dateTime">2015-04-09T18:56:27.771+02:00</m:generated_time>
        <rdfs:comment xml:lang="en">(ATA Code:7897) Wiring specific to the Engine Exhaust System</rdfs:comment>
        <m:has_related_eccairs_term rdf:resource="http://onto.fel.cvut.cz/ontologies/2014/ECCAIRS_Aviation_1.3.0.12/eccairs-descriptive-factors#category_11789700"/>
    </owl:Class>
    


    <!-- http://onto.fel.cvut.cz/ontologies/aviation-safety/Engine_Fuel_System_Wiring -->

    <owl:Class rdf:about="&m;Engine_Fuel_System_Wiring">
        <rdfs:label>Engine Fuel System Wiring</rdfs:label>
        <rdfs:subClassOf rdf:resource="&m;Engine_fuel_and_control_systems_part"/>
        <rdfs:subClassOf rdf:resource="&m;Wiring"/>
        <rdfs:subClassOf>
            <owl:Restriction>
                <owl:onProperty rdf:resource="http://onto.fel.cvut.cz/ontologies/ufo/is_part_of"/>
                <owl:someValuesFrom rdf:resource="&m;Engine_fuel_system"/>
            </owl:Restriction>
        </rdfs:subClassOf>
        <m:generated_time rdf:datatype="&xsd;dateTime">2015-04-09T18:56:27.771+02:00</m:generated_time>
        <rdfs:comment xml:lang="en">(ATA Code:7397) Wiring specific to the Engine Fuel System</rdfs:comment>
        <m:has_related_eccairs_term rdf:resource="http://onto.fel.cvut.cz/ontologies/2014/ECCAIRS_Aviation_1.3.0.12/eccairs-descriptive-factors#category_11739700"/>
    </owl:Class>
    


    <!-- http://onto.fel.cvut.cz/ontologies/aviation-safety/Engine_Indicating_System_Wiring -->

    <owl:Class rdf:about="&m;Engine_Indicating_System_Wiring">
        <rdfs:label>Engine Indicating System Wiring</rdfs:label>
        <rdfs:subClassOf rdf:resource="&m;Engine_indicating_system_part"/>
        <rdfs:subClassOf rdf:resource="&m;Wiring"/>
        <rdfs:subClassOf>
            <owl:Restriction>
                <owl:onProperty rdf:resource="http://onto.fel.cvut.cz/ontologies/ufo/is_part_of"/>
                <owl:someValuesFrom rdf:resource="&m;Engine_indicating_system"/>
            </owl:Restriction>
        </rdfs:subClassOf>
        <m:generated_time rdf:datatype="&xsd;dateTime">2015-04-09T18:56:27.771+02:00</m:generated_time>
        <rdfs:comment xml:lang="en">(ATA Code:7797) Wiring specific to the Engine Indication System.</rdfs:comment>
        <m:has_related_eccairs_term rdf:resource="http://onto.fel.cvut.cz/ontologies/2014/ECCAIRS_Aviation_1.3.0.12/eccairs-descriptive-factors#category_11779700"/>
    </owl:Class>
    


    <!-- http://onto.fel.cvut.cz/ontologies/aviation-safety/Engine_Oil_System_Wiring -->

    <owl:Class rdf:about="&m;Engine_Oil_System_Wiring">
        <rdfs:label>Engine Oil System Wiring</rdfs:label>
        <rdfs:subClassOf rdf:resource="&m;Engine_oil_system_(airframe)_part"/>
        <rdfs:subClassOf rdf:resource="&m;Wiring"/>
        <rdfs:subClassOf>
            <owl:Restriction>
                <owl:onProperty rdf:resource="http://onto.fel.cvut.cz/ontologies/ufo/is_part_of"/>
                <owl:someValuesFrom rdf:resource="&m;Engine_oil_system_(airframe)"/>
            </owl:Restriction>
        </rdfs:subClassOf>
        <m:generated_time rdf:datatype="&xsd;dateTime">2015-04-09T18:56:27.771+02:00</m:generated_time>
        <rdfs:comment xml:lang="en">(ATA Code:7997) Wiring specific to the Engine Oil System</rdfs:comment>
        <m:has_related_eccairs_term rdf:resource="http://onto.fel.cvut.cz/ontologies/2014/ECCAIRS_Aviation_1.3.0.12/eccairs-descriptive-factors#category_11799700"/>
    </owl:Class>
    


    <!-- http://onto.fel.cvut.cz/ontologies/aviation-safety/Engine_Starting_System_Wiring -->

    <owl:Class rdf:about="&m;Engine_Starting_System_Wiring">
        <rdfs:label>Engine Starting System Wiring</rdfs:label>
        <rdfs:subClassOf rdf:resource="&m;Engine_starting_system_part"/>
        <rdfs:subClassOf rdf:resource="&m;Wiring"/>
        <rdfs:subClassOf>
            <owl:Restriction>
                <owl:onProperty rdf:resource="http://onto.fel.cvut.cz/ontologies/ufo/is_part_of"/>
                <owl:someValuesFrom rdf:resource="&m;Engine_starting_system"/>
            </owl:Restriction>
        </rdfs:subClassOf>
        <m:generated_time rdf:datatype="&xsd;dateTime">2015-04-09T18:56:27.771+02:00</m:generated_time>
        <rdfs:comment xml:lang="en">(ATA Code:8097) Wiring specific to the Engine Starting System</rdfs:comment>
        <m:has_related_eccairs_term rdf:resource="http://onto.fel.cvut.cz/ontologies/2014/ECCAIRS_Aviation_1.3.0.12/eccairs-descriptive-factors#category_11809700"/>
    </owl:Class>
    


    <!-- http://onto.fel.cvut.cz/ontologies/aviation-safety/Engine_air_baffle_section -->

    <owl:Class rdf:about="&m;Engine_air_baffle_section">
        <rdfs:label>Engine air baffle section</rdfs:label>
        <rdfs:subClassOf rdf:resource="&m;Engine_cowling_system_part"/>
        <m:generated_time rdf:datatype="&xsd;dateTime">2015-04-09T18:56:27.771+02:00</m:generated_time>
        <rdfs:comment xml:lang="en">(ATA Code:7112) Engine air baffle section: The baffles which direct cooling air flow to the engine cylinders and accessories. Does not include cylinder baffles certificated with the engine [Code 11853000]. Typical parts are baffle, shield, bracket, shroud and cooling duct.</rdfs:comment>
        <m:has_related_eccairs_term rdf:resource="http://onto.fel.cvut.cz/ontologies/2014/ECCAIRS_Aviation_1.3.0.12/eccairs-descriptive-factors#category_11711200"/>
    </owl:Class>
    


    <!-- http://onto.fel.cvut.cz/ontologies/aviation-safety/Engine_air_intake_system -->

    <owl:Class rdf:about="&m;Engine_air_intake_system">
        <rdfs:label>Engine air intake system</rdfs:label>
        <rdfs:subClassOf rdf:resource="&m;Powerplant_system_part"/>
        <m:generated_time rdf:datatype="&xsd;dateTime">2015-04-09T18:56:27.771+02:00</m:generated_time>
        <rdfs:comment xml:lang="en">(ATA Code:7160) Engine air intake system: The portion of the powerplant system which directs airflow to the engine. Does not include integral structure with the airframe. Typical parts are carburetor air heat doors, alternate air doors, linkages, controls, filter element, ducts, hose, air box, latch, seals, nose ring cowls, scoops, compressor fan cowls, buried engine ducts, vortex generators, actuators, control handles, cables, wiring, plumbing, doors, warning systems and position indicators.</rdfs:comment>
        <m:has_related_eccairs_term rdf:resource="http://onto.fel.cvut.cz/ontologies/2014/ECCAIRS_Aviation_1.3.0.12/eccairs-descriptive-factors#category_11716000"/>
    </owl:Class>
    


    <!-- http://onto.fel.cvut.cz/ontologies/aviation-safety/Engine_anti-icing_system -->

    <owl:Class rdf:about="&m;Engine_anti-icing_system">
        <rdfs:label>Engine anti-icing system</rdfs:label>
        <rdfs:subClassOf rdf:resource="&m;Engine_bleed_air_system_part"/>
        <m:generated_time rdf:datatype="&xsd;dateTime">2015-04-09T18:56:27.771+02:00</m:generated_time>
        <rdfs:comment xml:lang="en">(ATA Code:7510) Engine anti-icing system: The engine system components and parts used to eliminate and prevent the formation of ice. Includes the control valve and associated actuator, switch and circuitry which controls the flow of turbine engine compressor bleed air to the engine anti-icing system. Does not include anti-icing pertaining to the power plant cowling [Code 11302000]. Typical parts are control valve, actuator, motor, switch, relay, circuit breaker, hose, manifold, coupling, fuel heat duct and fuel heat valve.</rdfs:comment>
        <m:has_related_eccairs_term rdf:resource="http://onto.fel.cvut.cz/ontologies/2014/ECCAIRS_Aviation_1.3.0.12/eccairs-descriptive-factors#category_11751000"/>
    </owl:Class>
    


    <!-- http://onto.fel.cvut.cz/ontologies/aviation-safety/Engine_attachment_fittings -->

    <owl:Class rdf:about="&m;Engine_attachment_fittings">
        <rdfs:label>Engine attachment fittings</rdfs:label>
        <rdfs:subClassOf rdf:resource="&m;Powerplant_system_part"/>
        <m:generated_time rdf:datatype="&xsd;dateTime">2015-04-09T18:56:27.771+02:00</m:generated_time>
        <rdfs:comment xml:lang="en">(ATA Code:7140) The fittings and brackets which are used for the support of equipment in and about the powerplant.</rdfs:comment>
        <m:has_related_eccairs_term rdf:resource="http://onto.fel.cvut.cz/ontologies/2014/ECCAIRS_Aviation_1.3.0.12/eccairs-descriptive-factors#category_11714000"/>
    </owl:Class>
    


    <!-- http://onto.fel.cvut.cz/ontologies/aviation-safety/Engine_bleed_air_system -->

    <owl:Class rdf:about="&m;Engine_bleed_air_system">
        <rdfs:label>Engine bleed air system</rdfs:label>
        <rdfs:subClassOf rdf:resource="&m;Aircraft_part"/>
        <m:generated_time rdf:datatype="&xsd;dateTime">2015-04-09T18:56:27.771+02:00</m:generated_time>
        <rdfs:comment xml:lang="en">(ATA Code:7500) Engine bleed air system: The turbine engine compressor bleed air systems used to control the flow of air through the engine, cooling air systems and heated air for engine anti-icing.</rdfs:comment>
        <m:has_related_eccairs_term rdf:resource="http://onto.fel.cvut.cz/ontologies/2014/ECCAIRS_Aviation_1.3.0.12/eccairs-descriptive-factors#category_11750000"/>
    </owl:Class>
    


    <!-- http://onto.fel.cvut.cz/ontologies/aviation-safety/Engine_bleed_air_system_part -->

    <owl:Class rdf:about="&m;Engine_bleed_air_system_part">
        <rdfs:label>Engine bleed air system part</rdfs:label>
        <rdfs:subClassOf rdf:resource="&m;Aircraft_part"/>
        <rdfs:subClassOf>
            <owl:Restriction>
                <owl:onProperty rdf:resource="http://onto.fel.cvut.cz/ontologies/ufo/is_part_of"/>
                <owl:someValuesFrom rdf:resource="&m;Engine_bleed_air_system"/>
            </owl:Restriction>
        </rdfs:subClassOf>
        <m:generated_time rdf:datatype="&xsd;dateTime">2015-04-12T02:45:54.351+02:00</m:generated_time>
        <m:has_related_eccairs_term rdf:resource="http://onto.fel.cvut.cz/ontologies/2014/ECCAIRS_Aviation_1.3.0.12/eccairs-descriptive-factors#category_11750000"/>
    </owl:Class>
    


    <!-- http://onto.fel.cvut.cz/ontologies/aviation-safety/Engine_brake_mean_effective_pressure-torque_indicating_system -->

    <owl:Class rdf:about="&m;Engine_brake_mean_effective_pressure-torque_indicating_system">
        <rdfs:label>Engine brake mean effective pressure/torque indicating system</rdfs:label>
        <rdfs:subClassOf rdf:resource="&m;Engine_power_indicating_system_part"/>
        <m:generated_time rdf:datatype="&xsd;dateTime">2015-04-09T18:56:27.771+02:00</m:generated_time>
        <rdfs:comment xml:lang="en">(ATA Code:7712) Engine brake mean effective pressure/torque indicating system: The system that senses and measures brake mean effective pressure [BMEP] or engine torque in turbo-prop and piston engines. Does not include internal parts which are type certificated with the engine. Typical parts are indicator, line, sensor, transmitter and pressure switch.</rdfs:comment>
        <m:has_related_eccairs_term rdf:resource="http://onto.fel.cvut.cz/ontologies/2014/ECCAIRS_Aviation_1.3.0.12/eccairs-descriptive-factors#category_11771200"/>
    </owl:Class>
    


    <!-- http://onto.fel.cvut.cz/ontologies/aviation-safety/Engine_controls -->

    <owl:Class rdf:about="&m;Engine_controls">
        <rdfs:label>Engine controls</rdfs:label>
        <rdfs:subClassOf rdf:resource="&m;Aircraft_part"/>
        <m:generated_time rdf:datatype="&xsd;dateTime">2015-04-09T18:56:27.771+02:00</m:generated_time>
        <rdfs:comment xml:lang="en">(ATA Code:7600) Engine controls: The controls which govern operation of the engine. Includes units and components which are interconnected for emergency shutdown. For turbo-prop engines, includes linkages and controls to the coordinator or equivalent to the propeller governor, fuel control unit or other units being controlled. For reciprocating engines, includes controls for blowers.</rdfs:comment>
        <m:has_related_eccairs_term rdf:resource="http://onto.fel.cvut.cz/ontologies/2014/ECCAIRS_Aviation_1.3.0.12/eccairs-descriptive-factors#category_11760000"/>
    </owl:Class>
    


    <!-- http://onto.fel.cvut.cz/ontologies/aviation-safety/Engine_controls_part -->

    <owl:Class rdf:about="&m;Engine_controls_part">
        <rdfs:label>Engine controls part</rdfs:label>
        <rdfs:subClassOf rdf:resource="&m;Aircraft_part"/>
        <rdfs:subClassOf>
            <owl:Restriction>
                <owl:onProperty rdf:resource="http://onto.fel.cvut.cz/ontologies/ufo/is_part_of"/>
                <owl:someValuesFrom rdf:resource="&m;Engine_controls"/>
            </owl:Restriction>
        </rdfs:subClassOf>
        <m:generated_time rdf:datatype="&xsd;dateTime">2015-04-12T02:45:54.351+02:00</m:generated_time>
        <m:has_related_eccairs_term rdf:resource="http://onto.fel.cvut.cz/ontologies/2014/ECCAIRS_Aviation_1.3.0.12/eccairs-descriptive-factors#category_11760000"/>
    </owl:Class>
    


    <!-- http://onto.fel.cvut.cz/ontologies/aviation-safety/Engine_cooling_system -->

    <owl:Class rdf:about="&m;Engine_cooling_system">
        <rdfs:label>Engine cooling system</rdfs:label>
        <rdfs:subClassOf rdf:resource="&m;Engine_bleed_air_system_part"/>
        <m:generated_time rdf:datatype="&xsd;dateTime">2015-04-09T18:56:27.771+02:00</m:generated_time>
        <rdfs:comment xml:lang="en">(ATA Code:7520) Engine cooling system: The portion of the engine compressor bleed air system which is used to ventilate engine compartments and accessories. Does not include the engine bleed control valve [Code 11753200]. Typical parts are jet pumps, vortex generators, valve, actuator and associated parts and circuitry used to control bleed air to engine accessory cooling systems.</rdfs:comment>
        <m:has_related_eccairs_term rdf:resource="http://onto.fel.cvut.cz/ontologies/2014/ECCAIRS_Aviation_1.3.0.12/eccairs-descriptive-factors#category_11752000"/>
    </owl:Class>
    


    <!-- http://onto.fel.cvut.cz/ontologies/aviation-safety/Engine_cowling_system -->

    <owl:Class rdf:about="&m;Engine_cowling_system">
        <rdfs:label>Engine cowling system</rdfs:label>
        <rdfs:subClassOf rdf:resource="&m;Powerplant_system_part"/>
        <m:generated_time rdf:datatype="&xsd;dateTime">2015-04-09T18:56:27.771+02:00</m:generated_time>
        <rdfs:comment xml:lang="en">(ATA Code:7110) Engine cowling system: The enclosure which houses engines for drag reducing and cooling. Includes attachment, structure and access doors. Does not include engine cylinder baffles of fire seals. Typical parts are latch, fastener, lock pin, hook, skin, nose cap, stud, access door, hinge, hinge pin, rivet, bracket and stiffener.</rdfs:comment>
        <m:has_related_eccairs_term rdf:resource="http://onto.fel.cvut.cz/ontologies/2014/ECCAIRS_Aviation_1.3.0.12/eccairs-descriptive-factors#category_11711000"/>
    </owl:Class>
    


    <!-- http://onto.fel.cvut.cz/ontologies/aviation-safety/Engine_cowling_system_part -->

    <owl:Class rdf:about="&m;Engine_cowling_system_part">
        <rdfs:label>Engine cowling system part</rdfs:label>
        <rdfs:subClassOf rdf:resource="&m;Powerplant_system_part"/>
        <rdfs:subClassOf>
            <owl:Restriction>
                <owl:onProperty rdf:resource="http://onto.fel.cvut.cz/ontologies/ufo/is_part_of"/>
                <owl:someValuesFrom rdf:resource="&m;Engine_cowling_system"/>
            </owl:Restriction>
        </rdfs:subClassOf>
        <m:generated_time rdf:datatype="&xsd;dateTime">2015-04-12T02:45:54.351+02:00</m:generated_time>
        <m:has_related_eccairs_term rdf:resource="http://onto.fel.cvut.cz/ontologies/2014/ECCAIRS_Aviation_1.3.0.12/eccairs-descriptive-factors#category_11711000"/>
    </owl:Class>
    


    <!-- http://onto.fel.cvut.cz/ontologies/aviation-safety/Engine_cranking -->

    <owl:Class rdf:about="&m;Engine_cranking">
        <rdfs:label>Engine cranking</rdfs:label>
        <rdfs:subClassOf rdf:resource="&m;Engine_starting_system_part"/>
        <m:generated_time rdf:datatype="&xsd;dateTime">2015-04-09T18:56:27.771+02:00</m:generated_time>
        <rdfs:comment xml:lang="en">(ATA Code:8010) Engine cranking: The portion of the system which is used to perform the cranking functions of the starting operation. Typical parts are plumbing, valve, wiring switch and relay.</rdfs:comment>
        <m:has_related_eccairs_term rdf:resource="http://onto.fel.cvut.cz/ontologies/2014/ECCAIRS_Aviation_1.3.0.12/eccairs-descriptive-factors#category_11801000"/>
    </owl:Class>
    


    <!-- http://onto.fel.cvut.cz/ontologies/aviation-safety/Engine_cranking_part -->

    <owl:Class rdf:about="&m;Engine_cranking_part">
        <rdfs:label>Engine cranking part</rdfs:label>
        <rdfs:subClassOf rdf:resource="&m;Engine_starting_system_part"/>
        <rdfs:subClassOf>
            <owl:Restriction>
                <owl:onProperty rdf:resource="http://onto.fel.cvut.cz/ontologies/ufo/is_part_of"/>
                <owl:someValuesFrom rdf:resource="&m;Engine_cranking"/>
            </owl:Restriction>
        </rdfs:subClassOf>
        <m:generated_time rdf:datatype="&xsd;dateTime">2015-04-12T02:45:54.351+02:00</m:generated_time>
        <m:has_related_eccairs_term rdf:resource="http://onto.fel.cvut.cz/ontologies/2014/ECCAIRS_Aviation_1.3.0.12/eccairs-descriptive-factors#category_11801000"/>
    </owl:Class>
    


    <!-- http://onto.fel.cvut.cz/ontologies/aviation-safety/Engine_drains -->

    <owl:Class rdf:about="&m;Engine_drains">
        <rdfs:label>Engine drains</rdfs:label>
        <rdfs:subClassOf rdf:resource="&m;Powerplant_system_part"/>
        <m:generated_time rdf:datatype="&xsd;dateTime">2015-04-09T18:56:27.771+02:00</m:generated_time>
        <rdfs:comment xml:lang="en">(ATA Code:7170) Engine drains: The components and manifold assemblies which are used to drain off excess fluids from the power plant and its accessories. Includes drain lines, manifolds, flame arrestors and supporting brackets. Also includes components that are an integral part of, or fitted to the power plant cowling.</rdfs:comment>
        <m:has_related_eccairs_term rdf:resource="http://onto.fel.cvut.cz/ontologies/2014/ECCAIRS_Aviation_1.3.0.12/eccairs-descriptive-factors#category_11717000"/>
    </owl:Class>
    


    <!-- http://onto.fel.cvut.cz/ontologies/aviation-safety/Engine_electrical_harness -->

    <owl:Class rdf:about="&m;Engine_electrical_harness">
        <rdfs:label>Engine electrical harness</rdfs:label>
        <rdfs:subClassOf rdf:resource="&m;Powerplant_system_part"/>
        <m:generated_time rdf:datatype="&xsd;dateTime">2015-04-09T18:56:27.771+02:00</m:generated_time>
        <rdfs:comment xml:lang="en">(ATA Code:7150) Engine electrical harness: The electrical cables, conduits, plugs and sockets, which serve several power plant systems, but which are banded together to facilitate removal and installation of the power plant. Does not include the wiring which is specifically covered under another system.</rdfs:comment>
        <m:has_related_eccairs_term rdf:resource="http://onto.fel.cvut.cz/ontologies/2014/ECCAIRS_Aviation_1.3.0.12/eccairs-descriptive-factors#category_11715000"/>
    </owl:Class>
    


    <!-- http://onto.fel.cvut.cz/ontologies/aviation-safety/Engine_emergency_shutdown_system -->

    <owl:Class rdf:about="&m;Engine_emergency_shutdown_system">
        <rdfs:label>Engine emergency shutdown system</rdfs:label>
        <rdfs:subClassOf rdf:resource="&m;Engine_controls_part"/>
        <m:generated_time rdf:datatype="&xsd;dateTime">2015-04-09T18:56:27.771+02:00</m:generated_time>
        <rdfs:comment xml:lang="en">(ATA Code:7620) Engine emergency shutdown system: The system which provides for rapid, complete shut-off of combustible fluids to the engine compartments during emergency procedures. Typical parts are cable, actuator, switch and lever.</rdfs:comment>
        <m:has_related_eccairs_term rdf:resource="http://onto.fel.cvut.cz/ontologies/2014/ECCAIRS_Aviation_1.3.0.12/eccairs-descriptive-factors#category_11762000"/>
    </owl:Class>
    


    <!-- http://onto.fel.cvut.cz/ontologies/aviation-safety/Engine_exhaust_collector-tailpipe-nozzle -->

    <owl:Class rdf:about="&m;Engine_exhaust_collector-tailpipe-nozzle">
        <rdfs:label>Engine exhaust collector/tailpipe/nozzle</rdfs:label>
        <rdfs:subClassOf rdf:resource="&m;Engine_exhaust_system_part"/>
        <m:generated_time rdf:datatype="&xsd;dateTime">2015-04-09T18:56:27.771+02:00</m:generated_time>
        <rdfs:comment xml:lang="en">(ATA Code:7810) Engine exhaust collector/tailpipe/nozzle: The portion of the system which collects the exhaust gases from the cylinders, turbines, or turbochargers and conducts them overboard. Includes variable vanes or nacelle tailpipes used on turboprop powered aircraft and turbo-shaft powered rotorcraft. Typical parts are tailpipe, cone, nozzle, clamp eyebolt, duct and ejector.</rdfs:comment>
        <m:has_related_eccairs_term rdf:resource="http://onto.fel.cvut.cz/ontologies/2014/ECCAIRS_Aviation_1.3.0.12/eccairs-descriptive-factors#category_11781000"/>
    </owl:Class>
    


    <!-- http://onto.fel.cvut.cz/ontologies/aviation-safety/Engine_exhaust_gas_temperature-turbine_inlet_temperature_indicating_system -->

    <owl:Class rdf:about="&m;Engine_exhaust_gas_temperature-turbine_inlet_temperature_indicating_system">
        <rdfs:label>Engine exhaust gas temperature/turbine inlet temperature indicating system</rdfs:label>
        <rdfs:subClassOf rdf:resource="&m;Engine_temperature_indicating_system_part"/>
        <m:generated_time rdf:datatype="&xsd;dateTime">2015-04-09T18:56:27.771+02:00</m:generated_time>
        <rdfs:comment xml:lang="en">(ATA Code:7722) Engine exhaust gas temperature/turbine inlet temperature indicating system: The exhaust gas temperature or turbine inlet temperature, temperature sensing and indicating. Includes the EGT indicators for both reciprocating and turbine engines and the TIT indicators for turbine engines. Typical parts are wiring, turbine outlet temperature (TOT) indicator, EGT indicator, probe, harness, terminal, connector, indicator, sensor, transducer and transmitter.JAR:‘Exhaust Gas Temperature’ (turbine engines) means the average temperature of the exhaust gas stream obtained in an approved manner.</rdfs:comment>
        <m:has_related_eccairs_term rdf:resource="http://onto.fel.cvut.cz/ontologies/2014/ECCAIRS_Aviation_1.3.0.12/eccairs-descriptive-factors#category_11772200"/>
    </owl:Class>
    


    <!-- http://onto.fel.cvut.cz/ontologies/aviation-safety/Engine_exhaust_system -->

    <owl:Class rdf:about="&m;Engine_exhaust_system">
        <rdfs:label>Engine exhaust system</rdfs:label>
        <rdfs:subClassOf rdf:resource="&m;Aircraft_part"/>
        <m:generated_time rdf:datatype="&xsd;dateTime">2015-04-09T18:56:27.771+02:00</m:generated_time>
        <rdfs:comment xml:lang="en">(ATA Code:7800) Engine exhaust system: The units and components which direct the engine exhaust gases overboard.</rdfs:comment>
        <m:has_related_eccairs_term rdf:resource="http://onto.fel.cvut.cz/ontologies/2014/ECCAIRS_Aviation_1.3.0.12/eccairs-descriptive-factors#category_11780000"/>
    </owl:Class>
    


    <!-- http://onto.fel.cvut.cz/ontologies/aviation-safety/Engine_exhaust_system_indication_system -->

    <owl:Class rdf:about="&m;Engine_exhaust_system_indication_system">
        <rdfs:label>Engine exhaust system indication system</rdfs:label>
        <rdfs:subClassOf rdf:resource="&m;Engine_exhaust_system_part"/>
        <m:generated_time rdf:datatype="&xsd;dateTime">2015-04-09T18:56:27.771+02:00</m:generated_time>
        <rdfs:comment xml:lang="en">(ATA Code:7850) Engine exhaust system indication</rdfs:comment>
        <m:has_related_eccairs_term rdf:resource="http://onto.fel.cvut.cz/ontologies/2014/ECCAIRS_Aviation_1.3.0.12/eccairs-descriptive-factors#category_11785000"/>
    </owl:Class>
    


    <!-- http://onto.fel.cvut.cz/ontologies/aviation-safety/Engine_exhaust_system_part -->

    <owl:Class rdf:about="&m;Engine_exhaust_system_part">
        <rdfs:label>Engine exhaust system part</rdfs:label>
        <rdfs:subClassOf rdf:resource="&m;Aircraft_part"/>
        <rdfs:subClassOf>
            <owl:Restriction>
                <owl:onProperty rdf:resource="http://onto.fel.cvut.cz/ontologies/ufo/is_part_of"/>
                <owl:someValuesFrom rdf:resource="&m;Engine_exhaust_system"/>
            </owl:Restriction>
        </rdfs:subClassOf>
        <m:generated_time rdf:datatype="&xsd;dateTime">2015-04-12T02:45:54.351+02:00</m:generated_time>
        <m:has_related_eccairs_term rdf:resource="http://onto.fel.cvut.cz/ontologies/2014/ECCAIRS_Aviation_1.3.0.12/eccairs-descriptive-factors#category_11780000"/>
    </owl:Class>
    


    <!-- http://onto.fel.cvut.cz/ontologies/aviation-safety/Engine_exhaust_thrust_reverser -->

    <owl:Class rdf:about="&m;Engine_exhaust_thrust_reverser">
        <rdfs:label>Engine exhaust thrust reverser</rdfs:label>
        <rdfs:subClassOf rdf:resource="&m;Engine_exhaust_system_part"/>
        <m:generated_time rdf:datatype="&xsd;dateTime">2015-04-09T18:56:27.771+02:00</m:generated_time>
        <rdfs:comment xml:lang="en">(ATA Code:7830) Engine exhaust thrust reverser: The airframe furnished system and components mounted at turbo-jet engine exhaust tailpipes to direct engine thrust forward for deceleration. Does not include the engine tailpipe. Includes items such as clamshells, linkages, levers, actuators, plumbing, wiring, indicators and warning systems.</rdfs:comment>
        <m:has_related_eccairs_term rdf:resource="http://onto.fel.cvut.cz/ontologies/2014/ECCAIRS_Aviation_1.3.0.12/eccairs-descriptive-factors#category_11783000"/>
    </owl:Class>
    


    <!-- http://onto.fel.cvut.cz/ontologies/aviation-safety/Engine_fan -->

    <owl:Class rdf:about="&m;Engine_fan">
        <rdfs:label>Engine fan</rdfs:label>
        <rdfs:subClassOf rdf:resource="&m;Turbine_engine_by-pass_section_part"/>
        <m:generated_time rdf:datatype="&xsd;dateTime">2015-04-09T18:56:27.771+02:00</m:generated_time>
        <rdfs:comment xml:lang="en">(ATA Code:7271) The turbine engine fan.</rdfs:comment>
        <m:has_related_eccairs_term rdf:resource="http://onto.fel.cvut.cz/ontologies/2014/ECCAIRS_Aviation_1.3.0.12/eccairs-descriptive-factors#category_11727100"/>
    </owl:Class>
    


    <!-- http://onto.fel.cvut.cz/ontologies/aviation-safety/Engine_fire_seals -->

    <owl:Class rdf:about="&m;Engine_fire_seals">
        <rdfs:label>Engine fire seals</rdfs:label>
        <rdfs:subClassOf rdf:resource="&m;Powerplant_system_part"/>
        <m:generated_time rdf:datatype="&xsd;dateTime">2015-04-09T18:56:27.771+02:00</m:generated_time>
        <rdfs:comment xml:lang="en">(ATA Code:7130) Engine fire seals: The fire-resistant partitions and seals mounted on or about the powerplant to isolate areas subject to fire. Typical parts are shroud and bracket. Does not include those fire-walls on the nacelle or pylon.</rdfs:comment>
        <m:has_related_eccairs_term rdf:resource="http://onto.fel.cvut.cz/ontologies/2014/ECCAIRS_Aviation_1.3.0.12/eccairs-descriptive-factors#category_11713000"/>
    </owl:Class>
    


    <!-- http://onto.fel.cvut.cz/ontologies/aviation-safety/Engine_fuel_and_control_systems -->

    <owl:Class rdf:about="&m;Engine_fuel_and_control_systems">
        <rdfs:label>Engine fuel and control systems</rdfs:label>
        <rdfs:subClassOf rdf:resource="&m;Aircraft_part"/>
        <m:generated_time rdf:datatype="&xsd;dateTime">2015-04-09T18:56:27.771+02:00</m:generated_time>
        <rdfs:comment xml:lang="en">(ATA Code:7300) Engine fuel and control systems: The turbine engine and reciprocating engine fuel systems.</rdfs:comment>
        <m:has_related_eccairs_term rdf:resource="http://onto.fel.cvut.cz/ontologies/2014/ECCAIRS_Aviation_1.3.0.12/eccairs-descriptive-factors#category_11730000"/>
    </owl:Class>
    


    <!-- http://onto.fel.cvut.cz/ontologies/aviation-safety/Engine_fuel_and_control_systems_part -->

    <owl:Class rdf:about="&m;Engine_fuel_and_control_systems_part">
        <rdfs:label>Engine fuel and control systems part</rdfs:label>
        <rdfs:subClassOf rdf:resource="&m;Aircraft_part"/>
        <rdfs:subClassOf>
            <owl:Restriction>
                <owl:onProperty rdf:resource="http://onto.fel.cvut.cz/ontologies/ufo/is_part_of"/>
                <owl:someValuesFrom rdf:resource="&m;Engine_fuel_and_control_systems"/>
            </owl:Restriction>
        </rdfs:subClassOf>
        <m:generated_time rdf:datatype="&xsd;dateTime">2015-04-12T02:45:54.351+02:00</m:generated_time>
        <m:has_related_eccairs_term rdf:resource="http://onto.fel.cvut.cz/ontologies/2014/ECCAIRS_Aviation_1.3.0.12/eccairs-descriptive-factors#category_11730000"/>
    </owl:Class>
    


    <!-- http://onto.fel.cvut.cz/ontologies/aviation-safety/Engine_fuel_indicating_system -->

    <owl:Class rdf:about="&m;Engine_fuel_indicating_system">
        <rdfs:label>Engine fuel indicating system</rdfs:label>
        <rdfs:subClassOf rdf:resource="&m;Engine_fuel_and_control_systems_part"/>
        <m:generated_time rdf:datatype="&xsd;dateTime">2015-04-09T18:56:27.771+02:00</m:generated_time>
        <rdfs:comment xml:lang="en">(ATA Code:7330) Engine fuel indicating system: The fuel temperature, flow rate or pressure indicating and warning systems other than the indicators, sensors and transmitters. Typical parts are line, hose, lamp, bulb, wiring harness and circuit breaker.</rdfs:comment>
        <m:has_related_eccairs_term rdf:resource="http://onto.fel.cvut.cz/ontologies/2014/ECCAIRS_Aviation_1.3.0.12/eccairs-descriptive-factors#category_11733000"/>
    </owl:Class>
    


    <!-- http://onto.fel.cvut.cz/ontologies/aviation-safety/Engine_fuel_indicating_system_part -->

    <owl:Class rdf:about="&m;Engine_fuel_indicating_system_part">
        <rdfs:label>Engine fuel indicating system part</rdfs:label>
        <rdfs:subClassOf rdf:resource="&m;Engine_fuel_and_control_systems_part"/>
        <rdfs:subClassOf>
            <owl:Restriction>
                <owl:onProperty rdf:resource="http://onto.fel.cvut.cz/ontologies/ufo/is_part_of"/>
                <owl:someValuesFrom rdf:resource="&m;Engine_fuel_indicating_system"/>
            </owl:Restriction>
        </rdfs:subClassOf>
        <m:generated_time rdf:datatype="&xsd;dateTime">2015-04-12T02:45:54.351+02:00</m:generated_time>
        <m:has_related_eccairs_term rdf:resource="http://onto.fel.cvut.cz/ontologies/2014/ECCAIRS_Aviation_1.3.0.12/eccairs-descriptive-factors#category_11733000"/>
    </owl:Class>
    


    <!-- http://onto.fel.cvut.cz/ontologies/aviation-safety/Engine_fuel_pump -->

    <owl:Class rdf:about="&m;Engine_fuel_pump">
        <rdfs:label>Engine fuel pump</rdfs:label>
        <rdfs:subClassOf rdf:resource="&m;Engine_fuel_system_part"/>
        <m:generated_time rdf:datatype="&xsd;dateTime">2015-04-09T18:56:27.771+02:00</m:generated_time>
        <rdfs:comment xml:lang="en">(ATA Code:7314) Engine fuel pump: The powerplant engine fuel pumps: typical parts are housing, spring, rocker, pump, diaphragm, shaft, seal, relief valve, regulator and coupling.</rdfs:comment>
        <m:has_related_eccairs_term rdf:resource="http://onto.fel.cvut.cz/ontologies/2014/ECCAIRS_Aviation_1.3.0.12/eccairs-descriptive-factors#category_11731400"/>
    </owl:Class>
    


    <!-- http://onto.fel.cvut.cz/ontologies/aviation-safety/Engine_fuel_system -->

    <owl:Class rdf:about="&m;Engine_fuel_system">
        <rdfs:label>Engine fuel system</rdfs:label>
        <rdfs:subClassOf rdf:resource="&m;Engine_fuel_and_control_systems_part"/>
        <m:generated_time rdf:datatype="&xsd;dateTime">2015-04-09T18:56:27.771+02:00</m:generated_time>
        <rdfs:comment xml:lang="en">(ATA Code:7310) Engine fuel system: The components and parts of the engine fuel system from the main quick disconnect fitting or airframe fuel system strainer to the fuel control unit. Does not include the controlling or metering aspects [Code 11732200], or the primer systems [Code 11282000] on reciprocating engines or the engine fuel pumps, fuel heater, cooler, divider or injector nozzle (turbine and piston engines). Typical parts are supply lines, hoses, fuel, filters on turbine engines, shutoff and solenoid valves.</rdfs:comment>
        <m:has_related_eccairs_term rdf:resource="http://onto.fel.cvut.cz/ontologies/2014/ECCAIRS_Aviation_1.3.0.12/eccairs-descriptive-factors#category_11731000"/>
    </owl:Class>
    


    <!-- http://onto.fel.cvut.cz/ontologies/aviation-safety/Engine_fuel_system_part -->

    <owl:Class rdf:about="&m;Engine_fuel_system_part">
        <rdfs:label>Engine fuel system part</rdfs:label>
        <rdfs:subClassOf rdf:resource="&m;Engine_fuel_and_control_systems_part"/>
        <rdfs:subClassOf>
            <owl:Restriction>
                <owl:onProperty rdf:resource="http://onto.fel.cvut.cz/ontologies/ufo/is_part_of"/>
                <owl:someValuesFrom rdf:resource="&m;Engine_fuel_system"/>
            </owl:Restriction>
        </rdfs:subClassOf>
        <m:generated_time rdf:datatype="&xsd;dateTime">2015-04-12T02:45:54.351+02:00</m:generated_time>
        <m:has_related_eccairs_term rdf:resource="http://onto.fel.cvut.cz/ontologies/2014/ECCAIRS_Aviation_1.3.0.12/eccairs-descriptive-factors#category_11731000"/>
    </owl:Class>
    


    <!-- http://onto.fel.cvut.cz/ontologies/aviation-safety/Engine_ignition_analyzer -->

    <owl:Class rdf:about="&m;Engine_ignition_analyzer">
        <rdfs:label>Engine ignition analyzer</rdfs:label>
        <rdfs:subClassOf rdf:resource="&m;Engine_ignition_analyzer_system_part"/>
        <m:generated_time rdf:datatype="&xsd;dateTime">2015-04-09T18:56:27.771+02:00</m:generated_time>
        <rdfs:comment xml:lang="en">(ATA Code:7731) Engine ignition analyzer: The unit which interprets and indicates by oscilloscope the condition of ignition systems on reciprocating engines.</rdfs:comment>
        <m:has_related_eccairs_term rdf:resource="http://onto.fel.cvut.cz/ontologies/2014/ECCAIRS_Aviation_1.3.0.12/eccairs-descriptive-factors#category_11773100"/>
    </owl:Class>
    


    <!-- http://onto.fel.cvut.cz/ontologies/aviation-safety/Engine_ignition_analyzer_system -->

    <owl:Class rdf:about="&m;Engine_ignition_analyzer_system">
        <rdfs:label>Engine ignition analyzer system</rdfs:label>
        <rdfs:subClassOf rdf:resource="&m;Engine_indicating_system_part"/>
        <m:generated_time rdf:datatype="&xsd;dateTime">2015-04-09T18:56:27.771+02:00</m:generated_time>
        <rdfs:comment xml:lang="en">(ATA Code:7730) Engine ignition analyzer system</rdfs:comment>
        <m:has_related_eccairs_term rdf:resource="http://onto.fel.cvut.cz/ontologies/2014/ECCAIRS_Aviation_1.3.0.12/eccairs-descriptive-factors#category_11773000"/>
    </owl:Class>
    


    <!-- http://onto.fel.cvut.cz/ontologies/aviation-safety/Engine_ignition_analyzer_system_part -->

    <owl:Class rdf:about="&m;Engine_ignition_analyzer_system_part">
        <rdfs:label>Engine ignition analyzer system part</rdfs:label>
        <rdfs:subClassOf rdf:resource="&m;Engine_indicating_system_part"/>
        <rdfs:subClassOf>
            <owl:Restriction>
                <owl:onProperty rdf:resource="http://onto.fel.cvut.cz/ontologies/ufo/is_part_of"/>
                <owl:someValuesFrom rdf:resource="&m;Engine_ignition_analyzer_system"/>
            </owl:Restriction>
        </rdfs:subClassOf>
        <m:generated_time rdf:datatype="&xsd;dateTime">2015-04-12T02:45:54.351+02:00</m:generated_time>
        <m:has_related_eccairs_term rdf:resource="http://onto.fel.cvut.cz/ontologies/2014/ECCAIRS_Aviation_1.3.0.12/eccairs-descriptive-factors#category_11773000"/>
    </owl:Class>
    


    <!-- http://onto.fel.cvut.cz/ontologies/aviation-safety/Engine_indicating_system -->

    <owl:Class rdf:about="&m;Engine_indicating_system">
        <rdfs:label>Engine indicating system</rdfs:label>
        <rdfs:subClassOf rdf:resource="&m;Aircraft_part"/>
        <m:generated_time rdf:datatype="&xsd;dateTime">2015-04-09T18:56:27.771+02:00</m:generated_time>
        <rdfs:comment xml:lang="en">(ATA Code:7700) Engine indicating system: The engine indicators, transmitters and analyzers.</rdfs:comment>
        <m:has_related_eccairs_term rdf:resource="http://onto.fel.cvut.cz/ontologies/2014/ECCAIRS_Aviation_1.3.0.12/eccairs-descriptive-factors#category_11770000"/>
    </owl:Class>
    


    <!-- http://onto.fel.cvut.cz/ontologies/aviation-safety/Engine_indicating_system_part -->

    <owl:Class rdf:about="&m;Engine_indicating_system_part">
        <rdfs:label>Engine indicating system part</rdfs:label>
        <rdfs:subClassOf rdf:resource="&m;Aircraft_part"/>
        <rdfs:subClassOf>
            <owl:Restriction>
                <owl:onProperty rdf:resource="http://onto.fel.cvut.cz/ontologies/ufo/is_part_of"/>
                <owl:someValuesFrom rdf:resource="&m;Engine_indicating_system"/>
            </owl:Restriction>
        </rdfs:subClassOf>
        <m:generated_time rdf:datatype="&xsd;dateTime">2015-04-12T02:45:54.351+02:00</m:generated_time>
        <m:has_related_eccairs_term rdf:resource="http://onto.fel.cvut.cz/ontologies/2014/ECCAIRS_Aviation_1.3.0.12/eccairs-descriptive-factors#category_11770000"/>
    </owl:Class>
    


    <!-- http://onto.fel.cvut.cz/ontologies/aviation-safety/Engine_integrated_instrument_system -->

    <owl:Class rdf:about="&m;Engine_integrated_instrument_system">
        <rdfs:label>Engine integrated instrument system</rdfs:label>
        <rdfs:subClassOf rdf:resource="&m;Engine_indicating_system_part"/>
        <m:generated_time rdf:datatype="&xsd;dateTime">2015-04-09T18:56:27.771+02:00</m:generated_time>
        <rdfs:comment xml:lang="en">(ATA Code:7740) Engine integrated instrument system: The portion of the system which is an integrated concept receives engine operating parameters and transmits this information to a central processor for flight crew presentation. Typical parts are display units, transmitters, receivers and computers.</rdfs:comment>
        <m:has_related_eccairs_term rdf:resource="http://onto.fel.cvut.cz/ontologies/2014/ECCAIRS_Aviation_1.3.0.12/eccairs-descriptive-factors#category_11774000"/>
    </owl:Class>
    


    <!-- http://onto.fel.cvut.cz/ontologies/aviation-safety/Engine_manifold_pressure_indicating_system -->

    <owl:Class rdf:about="&m;Engine_manifold_pressure_indicating_system">
        <rdfs:label>Engine manifold pressure indicating system</rdfs:label>
        <rdfs:subClassOf rdf:resource="&m;Engine_power_indicating_system_part"/>
        <m:generated_time rdf:datatype="&xsd;dateTime">2015-04-09T18:56:27.771+02:00</m:generated_time>
        <rdfs:comment xml:lang="en">(ATA Code:7713) Engine manifold pressure indicating system: The reciprocating engine manifold pressure indicating system including the indicator and sensor. Typical parts are lines, hoses and fittings.  Manifold pressure means absolute pressure as measured at the appropriate point in the induction system (FAA 14, Part 1)JAR:‘Manifold Pressure’ piston engines means the absolute static pressure measured at the appropriatepoint in the induction system, usually in inches or millimetres of mercury.</rdfs:comment>
        <m:has_related_eccairs_term rdf:resource="http://onto.fel.cvut.cz/ontologies/2014/ECCAIRS_Aviation_1.3.0.12/eccairs-descriptive-factors#category_11771300"/>
    </owl:Class>
    


    <!-- http://onto.fel.cvut.cz/ontologies/aviation-safety/Engine_mount -->

    <owl:Class rdf:about="&m;Engine_mount">
        <rdfs:label>Engine mount</rdfs:label>
        <rdfs:subClassOf rdf:resource="&m;Powerplant_system_part"/>
        <m:generated_time rdf:datatype="&xsd;dateTime">2015-04-09T18:56:27.771+02:00</m:generated_time>
        <rdfs:comment xml:lang="en">(ATA Code:7120) Engine mount: The structural framework which supports the engine on the nacelle, firewall or pylon. Typical parts are mount, bracket, fitting, shock mount, bolt, isolator and hanger.</rdfs:comment>
        <m:has_related_eccairs_term rdf:resource="http://onto.fel.cvut.cz/ontologies/2014/ECCAIRS_Aviation_1.3.0.12/eccairs-descriptive-factors#category_11712000"/>
    </owl:Class>
    


    <!-- http://onto.fel.cvut.cz/ontologies/aviation-safety/Engine_noise_suppressor -->

    <owl:Class rdf:about="&m;Engine_noise_suppressor">
        <rdfs:label>Engine noise suppressor</rdfs:label>
        <rdfs:subClassOf rdf:resource="&m;Engine_exhaust_system_part"/>
        <m:generated_time rdf:datatype="&xsd;dateTime">2015-04-09T18:56:27.771+02:00</m:generated_time>
        <rdfs:comment xml:lang="en">(ATA Code:7820) Engine noise suppressor: The clover leaf shaped unit mounted on turbo-jet engine exhaust tailpipes for sound suppression and components used on reciprocating engines to reduce engine exhaust noise. Does not include the shroud over the muffler used to collect heated fresh air for cabin and carburetor heat [Code 11214000]. Typical parts are baffle, cone, and flame tube.</rdfs:comment>
        <m:has_related_eccairs_term rdf:resource="http://onto.fel.cvut.cz/ontologies/2014/ECCAIRS_Aviation_1.3.0.12/eccairs-descriptive-factors#category_11782000"/>
    </owl:Class>
    


    <!-- http://onto.fel.cvut.cz/ontologies/aviation-safety/Engine_oil_cooler -->

    <owl:Class rdf:about="&m;Engine_oil_cooler">
        <rdfs:label>Engine oil cooler</rdfs:label>
        <rdfs:subClassOf rdf:resource="&m;Engine_oil_distribution_(airframe)_part"/>
        <m:generated_time rdf:datatype="&xsd;dateTime">2015-04-09T18:56:27.771+02:00</m:generated_time>
        <rdfs:comment xml:lang="en">(ATA Code:7921) Engine oil cooler: The component and associated parts that cool engine lubricating oil. Includes brackets, outlet doors, scoops, ducts and louvres, but excludes the temperature regulator. Typical parts are cooler, duct, scoop, door and door actuator.</rdfs:comment>
        <m:has_related_eccairs_term rdf:resource="http://onto.fel.cvut.cz/ontologies/2014/ECCAIRS_Aviation_1.3.0.12/eccairs-descriptive-factors#category_11792100"/>
    </owl:Class>
    


    <!-- http://onto.fel.cvut.cz/ontologies/aviation-safety/Engine_oil_distribution_(airframe) -->

    <owl:Class rdf:about="&m;Engine_oil_distribution_(airframe)">
        <rdfs:label>Engine oil distribution (airframe)</rdfs:label>
        <rdfs:subClassOf rdf:resource="&m;Engine_oil_system_(airframe)_part"/>
        <m:generated_time rdf:datatype="&xsd;dateTime">2015-04-09T18:56:27.771+02:00</m:generated_time>
        <rdfs:comment xml:lang="en">(ATA Code:7920) Engine oil distribution (airframe): The external oil system which distributes engine lubricating oil from the storage tanks to and from the engine. Does not include externally mounted units such as oil coolers, oil filters and shut-off valves. Typical parts are line, hose, coupling, fitting and clamps.Airframe means the fuselage, booms, nacelles, cowlings, fairings, aerofoil surfaces (includingrotors but excluding propellers and rotating aerofoils of engines), and landing gear of an aircraft andtheir accessories and controls.</rdfs:comment>
        <m:has_related_eccairs_term rdf:resource="http://onto.fel.cvut.cz/ontologies/2014/ECCAIRS_Aviation_1.3.0.12/eccairs-descriptive-factors#category_11792000"/>
    </owl:Class>
    


    <!-- http://onto.fel.cvut.cz/ontologies/aviation-safety/Engine_oil_distribution_(airframe)_part -->

    <owl:Class rdf:about="&m;Engine_oil_distribution_(airframe)_part">
        <rdfs:label>Engine oil distribution (airframe) part</rdfs:label>
        <rdfs:subClassOf rdf:resource="&m;Engine_oil_system_(airframe)_part"/>
        <rdfs:subClassOf>
            <owl:Restriction>
                <owl:onProperty rdf:resource="http://onto.fel.cvut.cz/ontologies/ufo/is_part_of"/>
                <owl:someValuesFrom rdf:resource="&m;Engine_oil_distribution_(airframe)"/>
            </owl:Restriction>
        </rdfs:subClassOf>
        <m:generated_time rdf:datatype="&xsd;dateTime">2015-04-12T02:45:54.351+02:00</m:generated_time>
        <m:has_related_eccairs_term rdf:resource="http://onto.fel.cvut.cz/ontologies/2014/ECCAIRS_Aviation_1.3.0.12/eccairs-descriptive-factors#category_11792000"/>
    </owl:Class>
    


    <!-- http://onto.fel.cvut.cz/ontologies/aviation-safety/Engine_oil_indicating_system -->

    <owl:Class rdf:about="&m;Engine_oil_indicating_system">
        <rdfs:label>Engine oil indicating system</rdfs:label>
        <rdfs:subClassOf rdf:resource="&m;Engine_oil_system_(airframe)_part"/>
        <m:generated_time rdf:datatype="&xsd;dateTime">2015-04-09T18:56:27.771+02:00</m:generated_time>
        <rdfs:comment xml:lang="en">(ATA Code:7930) Engine oil indicating system: The portion of the system which is used to indicate the quantity, temperature and pressure of the engine oil.</rdfs:comment>
        <m:has_related_eccairs_term rdf:resource="http://onto.fel.cvut.cz/ontologies/2014/ECCAIRS_Aviation_1.3.0.12/eccairs-descriptive-factors#category_11793000"/>
    </owl:Class>
    


    <!-- http://onto.fel.cvut.cz/ontologies/aviation-safety/Engine_oil_indicating_system_part -->

    <owl:Class rdf:about="&m;Engine_oil_indicating_system_part">
        <rdfs:label>Engine oil indicating system part</rdfs:label>
        <rdfs:subClassOf rdf:resource="&m;Engine_oil_system_(airframe)_part"/>
        <rdfs:subClassOf>
            <owl:Restriction>
                <owl:onProperty rdf:resource="http://onto.fel.cvut.cz/ontologies/ufo/is_part_of"/>
                <owl:someValuesFrom rdf:resource="&m;Engine_oil_indicating_system"/>
            </owl:Restriction>
        </rdfs:subClassOf>
        <m:generated_time rdf:datatype="&xsd;dateTime">2015-04-12T02:45:54.351+02:00</m:generated_time>
        <m:has_related_eccairs_term rdf:resource="http://onto.fel.cvut.cz/ontologies/2014/ECCAIRS_Aviation_1.3.0.12/eccairs-descriptive-factors#category_11793000"/>
    </owl:Class>
    


    <!-- http://onto.fel.cvut.cz/ontologies/aviation-safety/Engine_oil_pressure_indication -->

    <owl:Class rdf:about="&m;Engine_oil_pressure_indication">
        <rdfs:label>Engine oil pressure indication</rdfs:label>
        <rdfs:subClassOf rdf:resource="&m;Engine_oil_indicating_system_part"/>
        <m:generated_time rdf:datatype="&xsd;dateTime">2015-04-09T18:56:27.771+02:00</m:generated_time>
        <rdfs:comment xml:lang="en">(ATA Code:7931) Engine oil pressure indication: The instrument or warning lamp which indicates, senses or transmits the pressure of engine lubricating oil available at the engine or when the pressure is improper for the conditions. Typical parts are transducer, pressure switch, transmitter, indicator, case, dial, needle and lamp.</rdfs:comment>
        <m:has_related_eccairs_term rdf:resource="http://onto.fel.cvut.cz/ontologies/2014/ECCAIRS_Aviation_1.3.0.12/eccairs-descriptive-factors#category_11793100"/>
    </owl:Class>
    


    <!-- http://onto.fel.cvut.cz/ontologies/aviation-safety/Engine_oil_quantity_indicator -->

    <owl:Class rdf:about="&m;Engine_oil_quantity_indicator">
        <rdfs:label>Engine oil quantity indicator</rdfs:label>
        <rdfs:subClassOf rdf:resource="&m;Engine_oil_indicating_system_part"/>
        <m:generated_time rdf:datatype="&xsd;dateTime">2015-04-09T18:56:27.771+02:00</m:generated_time>
        <rdfs:comment xml:lang="en">(ATA Code:7932) Engine oil quantity indicator: The instrument or warning lamp which senses or indicates the quantity of oil in supply tanks or warns of an insufficient quantity. Typical parts are transmitter, indicator, case, lamp.</rdfs:comment>
        <m:has_related_eccairs_term rdf:resource="http://onto.fel.cvut.cz/ontologies/2014/ECCAIRS_Aviation_1.3.0.12/eccairs-descriptive-factors#category_11793200"/>
    </owl:Class>
    


    <!-- http://onto.fel.cvut.cz/ontologies/aviation-safety/Engine_oil_shut-off_valve -->

    <owl:Class rdf:about="&m;Engine_oil_shut-off_valve">
        <rdfs:label>Engine oil shut-off valve</rdfs:label>
        <rdfs:subClassOf rdf:resource="&m;Engine_oil_distribution_(airframe)_part"/>
        <m:generated_time rdf:datatype="&xsd;dateTime">2015-04-09T18:56:27.771+02:00</m:generated_time>
        <rdfs:comment xml:lang="en">(ATA Code:7923) Engine oil shut-off valve: The component and associated controls which stop the flow of lubricating oil to the engine for emergency purposes.</rdfs:comment>
        <m:has_related_eccairs_term rdf:resource="http://onto.fel.cvut.cz/ontologies/2014/ECCAIRS_Aviation_1.3.0.12/eccairs-descriptive-factors#category_11792300"/>
    </owl:Class>
    


    <!-- http://onto.fel.cvut.cz/ontologies/aviation-safety/Engine_oil_storage_(airframe) -->

    <owl:Class rdf:about="&m;Engine_oil_storage_(airframe)">
        <rdfs:label>Engine oil storage (airframe)</rdfs:label>
        <rdfs:subClassOf rdf:resource="&m;Engine_oil_system_(airframe)_part"/>
        <m:generated_time rdf:datatype="&xsd;dateTime">2015-04-09T18:56:27.771+02:00</m:generated_time>
        <rdfs:comment xml:lang="en">(ATA Code:7910) Engine oil storage (airframe): The engine oil storage tank furnished by the airframe manufacturer. Includes attached parts such as filler caps and mount brackets, but excludes engine manufacturer furnished tanks, quantity indication systems and distribution lines. Typical parts are tank, cap, seal, bracket and drain valve.Airframe means the fuselage, booms, nacelles, cowlings, fairings, aerofoil surfaces (includingrotors but excluding propellers and rotating aerofoils of engines), and landing gear of an aircraft andtheir accessories and controls.</rdfs:comment>
        <m:has_related_eccairs_term rdf:resource="http://onto.fel.cvut.cz/ontologies/2014/ECCAIRS_Aviation_1.3.0.12/eccairs-descriptive-factors#category_11791000"/>
    </owl:Class>
    


    <!-- http://onto.fel.cvut.cz/ontologies/aviation-safety/Engine_oil_system_(airframe) -->

    <owl:Class rdf:about="&m;Engine_oil_system_(airframe)">
        <rdfs:label>Engine oil system (airframe)</rdfs:label>
        <rdfs:subClassOf rdf:resource="&m;Aircraft_part"/>
        <m:generated_time rdf:datatype="&xsd;dateTime">2015-04-09T18:56:27.771+02:00</m:generated_time>
        <rdfs:comment xml:lang="en">(ATA Code:7900) Engine oil system (airframe): The system units external to the engine which store and deliver engine lubricating oil to and from both turbine and reciprocating engines. Airframe means the fuselage, booms, nacelles, cowlings, fairings, aerofoil surfaces (includingrotors but excluding propellers and rotating aerofoils of engines), and landing gear of an aircraft andtheir accessories and controls.</rdfs:comment>
        <m:has_related_eccairs_term rdf:resource="http://onto.fel.cvut.cz/ontologies/2014/ECCAIRS_Aviation_1.3.0.12/eccairs-descriptive-factors#category_11790000"/>
    </owl:Class>
    


    <!-- http://onto.fel.cvut.cz/ontologies/aviation-safety/Engine_oil_system_(airframe)_part -->

    <owl:Class rdf:about="&m;Engine_oil_system_(airframe)_part">
        <rdfs:label>Engine oil system (airframe) part</rdfs:label>
        <rdfs:subClassOf rdf:resource="&m;Aircraft_part"/>
        <rdfs:subClassOf>
            <owl:Restriction>
                <owl:onProperty rdf:resource="http://onto.fel.cvut.cz/ontologies/ufo/is_part_of"/>
                <owl:someValuesFrom rdf:resource="&m;Engine_oil_system_(airframe)"/>
            </owl:Restriction>
        </rdfs:subClassOf>
        <m:generated_time rdf:datatype="&xsd;dateTime">2015-04-12T02:45:54.351+02:00</m:generated_time>
        <m:has_related_eccairs_term rdf:resource="http://onto.fel.cvut.cz/ontologies/2014/ECCAIRS_Aviation_1.3.0.12/eccairs-descriptive-factors#category_11790000"/>
    </owl:Class>
    


    <!-- http://onto.fel.cvut.cz/ontologies/aviation-safety/Engine_oil_temperature_indicator -->

    <owl:Class rdf:about="&m;Engine_oil_temperature_indicator">
        <rdfs:label>Engine oil temperature indicator</rdfs:label>
        <rdfs:subClassOf rdf:resource="&m;Engine_oil_indicating_system_part"/>
        <m:generated_time rdf:datatype="&xsd;dateTime">2015-04-09T18:56:27.771+02:00</m:generated_time>
        <rdfs:comment xml:lang="en">(ATA Code:7933) Engine oil temperature indicator: The instrument which senses and indicates temperature of engine oil. Typical parts are sensor, temperature bulb, case, indicator, needle and dial.</rdfs:comment>
        <m:has_related_eccairs_term rdf:resource="http://onto.fel.cvut.cz/ontologies/2014/ECCAIRS_Aviation_1.3.0.12/eccairs-descriptive-factors#category_11793300"/>
    </owl:Class>
    


    <!-- http://onto.fel.cvut.cz/ontologies/aviation-safety/Engine_oil_temperature_regulator -->

    <owl:Class rdf:about="&m;Engine_oil_temperature_regulator">
        <rdfs:label>Engine oil temperature regulator</rdfs:label>
        <rdfs:subClassOf rdf:resource="&m;Engine_oil_distribution_(airframe)_part"/>
        <m:generated_time rdf:datatype="&xsd;dateTime">2015-04-09T18:56:27.771+02:00</m:generated_time>
        <rdfs:comment xml:lang="en">(ATA Code:7922) Engine oil temperature regulator: The unit which is mounted on the airframe oil cooler or the engine for controlling engine lubricating oil temperature. Typical parts are thermostat, thermal valve and regulator.</rdfs:comment>
        <m:has_related_eccairs_term rdf:resource="http://onto.fel.cvut.cz/ontologies/2014/ECCAIRS_Aviation_1.3.0.12/eccairs-descriptive-factors#category_11792200"/>
    </owl:Class>
    


    <!-- http://onto.fel.cvut.cz/ontologies/aviation-safety/Engine_power_control -->

    <owl:Class rdf:about="&m;Engine_power_control">
        <rdfs:label>Engine power control</rdfs:label>
        <rdfs:subClassOf rdf:resource="&m;Engine_controls_part"/>
        <m:generated_time rdf:datatype="&xsd;dateTime">2015-04-09T18:56:27.771+02:00</m:generated_time>
        <rdfs:comment xml:lang="en">(ATA Code:7610) Engine power control: The portion of the system which furnishes a means of controlling the main fuel control or coordinator. Includes controls to the propeller regulator on turboprop engines and items such as linkages, cables, levers, pulleys, switches and wiring. Does not include the units themselves.</rdfs:comment>
        <m:has_related_eccairs_term rdf:resource="http://onto.fel.cvut.cz/ontologies/2014/ECCAIRS_Aviation_1.3.0.12/eccairs-descriptive-factors#category_11761000"/>
    </owl:Class>
    


    <!-- http://onto.fel.cvut.cz/ontologies/aviation-safety/Engine_power_indicating_system -->

    <owl:Class rdf:about="&m;Engine_power_indicating_system">
        <rdfs:label>Engine power indicating system</rdfs:label>
        <rdfs:subClassOf rdf:resource="&m;Engine_indicating_system_part"/>
        <m:generated_time rdf:datatype="&xsd;dateTime">2015-04-09T18:56:27.771+02:00</m:generated_time>
        <rdfs:comment xml:lang="en">(ATA Code:7710) Engine power indicating system: The power indicating systems which directly or indirectly indicates power or thrust e.g. brake mean effective pressure, engine pressure ratio and rpm.</rdfs:comment>
        <m:has_related_eccairs_term rdf:resource="http://onto.fel.cvut.cz/ontologies/2014/ECCAIRS_Aviation_1.3.0.12/eccairs-descriptive-factors#category_11771000"/>
    </owl:Class>
    


    <!-- http://onto.fel.cvut.cz/ontologies/aviation-safety/Engine_power_indicating_system_part -->

    <owl:Class rdf:about="&m;Engine_power_indicating_system_part">
        <rdfs:label>Engine power indicating system part</rdfs:label>
        <rdfs:subClassOf rdf:resource="&m;Engine_indicating_system_part"/>
        <rdfs:subClassOf>
            <owl:Restriction>
                <owl:onProperty rdf:resource="http://onto.fel.cvut.cz/ontologies/ufo/is_part_of"/>
                <owl:someValuesFrom rdf:resource="&m;Engine_power_indicating_system"/>
            </owl:Restriction>
        </rdfs:subClassOf>
        <m:generated_time rdf:datatype="&xsd;dateTime">2015-04-12T02:45:54.351+02:00</m:generated_time>
        <m:has_related_eccairs_term rdf:resource="http://onto.fel.cvut.cz/ontologies/2014/ECCAIRS_Aviation_1.3.0.12/eccairs-descriptive-factors#category_11771000"/>
    </owl:Class>
    


    <!-- http://onto.fel.cvut.cz/ontologies/aviation-safety/Engine_pressure_ratio_(EPR)_indicating_system -->

    <owl:Class rdf:about="&m;Engine_pressure_ratio_(EPR)_indicating_system">
        <rdfs:label>Engine pressure ratio (EPR) indicating system</rdfs:label>
        <rdfs:subClassOf rdf:resource="&m;Engine_power_indicating_system_part"/>
        <m:generated_time rdf:datatype="&xsd;dateTime">2015-04-09T18:56:27.771+02:00</m:generated_time>
        <rdfs:comment xml:lang="en">(ATA Code:7711) Engine pressure ratio indicating system: The system which senses, measures and indicates the engine pressure ratio of a turbine engine. The system measures the difference between the compressor inlet pressure and the turbine discharge pressure. Typical parts are sensor, transducer, transmitter and probe.</rdfs:comment>
        <m:has_related_eccairs_term rdf:resource="http://onto.fel.cvut.cz/ontologies/2014/ECCAIRS_Aviation_1.3.0.12/eccairs-descriptive-factors#category_11771100"/>
    </owl:Class>
    


    <!-- http://onto.fel.cvut.cz/ontologies/aviation-safety/Engine_rpm_indicating_system -->

    <owl:Class rdf:about="&m;Engine_rpm_indicating_system">
        <rdfs:label>Engine rpm indicating system</rdfs:label>
        <rdfs:subClassOf rdf:resource="&m;Engine_power_indicating_system_part"/>
        <m:generated_time rdf:datatype="&xsd;dateTime">2015-04-09T18:56:27.771+02:00</m:generated_time>
        <rdfs:comment xml:lang="en">(ATA Code:7714) Engine rpm indicating system: The system including the indicator and sensor which indicates engine speed in revolutions per minute. Typical parts are cable, connector, tachometer, tachometer generator and N1 indicator.</rdfs:comment>
        <m:has_related_eccairs_term rdf:resource="http://onto.fel.cvut.cz/ontologies/2014/ECCAIRS_Aviation_1.3.0.12/eccairs-descriptive-factors#category_11771400"/>
    </owl:Class>
    


    <!-- http://onto.fel.cvut.cz/ontologies/aviation-safety/Engine_start_valves-controls -->

    <owl:Class rdf:about="&m;Engine_start_valves-controls">
        <rdfs:label>Engine start valves/controls</rdfs:label>
        <rdfs:subClassOf rdf:resource="&m;Engine_cranking_part"/>
        <m:generated_time rdf:datatype="&xsd;dateTime">2015-04-09T18:56:27.771+02:00</m:generated_time>
        <rdfs:comment xml:lang="en">(ATA Code:8012) The valves and controls used for starting engines.</rdfs:comment>
        <m:has_related_eccairs_term rdf:resource="http://onto.fel.cvut.cz/ontologies/2014/ECCAIRS_Aviation_1.3.0.12/eccairs-descriptive-factors#category_11801200"/>
    </owl:Class>
    


    <!-- http://onto.fel.cvut.cz/ontologies/aviation-safety/Engine_starter -->

    <owl:Class rdf:about="&m;Engine_starter">
        <rdfs:label>Engine starter</rdfs:label>
        <rdfs:subClassOf rdf:resource="&m;Engine_cranking_part"/>
        <m:generated_time rdf:datatype="&xsd;dateTime">2015-04-09T18:56:27.771+02:00</m:generated_time>
        <rdfs:comment xml:lang="en">(ATA Code:8011) Engine starter: The component used for starting the engines. Includes parts which are separated from the engine during starter removals, but does not include parts within the engine. Does not include the starter-generator [Code 11243500]. Typical parts are brush, bearing, shaft, clutch, adaptor, back plate, housing, winding and terminal post.</rdfs:comment>
        <m:has_related_eccairs_term rdf:resource="http://onto.fel.cvut.cz/ontologies/2014/ECCAIRS_Aviation_1.3.0.12/eccairs-descriptive-factors#category_11801100"/>
    </owl:Class>
    


    <!-- http://onto.fel.cvut.cz/ontologies/aviation-safety/Engine_starting_system -->

    <owl:Class rdf:about="&m;Engine_starting_system">
        <rdfs:label>Engine starting system</rdfs:label>
        <rdfs:subClassOf rdf:resource="&m;Aircraft_part"/>
        <m:generated_time rdf:datatype="&xsd;dateTime">2015-04-09T18:56:27.771+02:00</m:generated_time>
        <rdfs:comment xml:lang="en">(ATA Code:8000) Engine starting system: The units, components and associated systems used for starting the engine. Includes electrical, inertia, air or other starter systems. Does not include ignition systems.</rdfs:comment>
        <m:has_related_eccairs_term rdf:resource="http://onto.fel.cvut.cz/ontologies/2014/ECCAIRS_Aviation_1.3.0.12/eccairs-descriptive-factors#category_11800000"/>
    </owl:Class>
    


    <!-- http://onto.fel.cvut.cz/ontologies/aviation-safety/Engine_starting_system_part -->

    <owl:Class rdf:about="&m;Engine_starting_system_part">
        <rdfs:label>Engine starting system part</rdfs:label>
        <rdfs:subClassOf rdf:resource="&m;Aircraft_part"/>
        <rdfs:subClassOf>
            <owl:Restriction>
                <owl:onProperty rdf:resource="http://onto.fel.cvut.cz/ontologies/ufo/is_part_of"/>
                <owl:someValuesFrom rdf:resource="&m;Engine_starting_system"/>
            </owl:Restriction>
        </rdfs:subClassOf>
        <m:generated_time rdf:datatype="&xsd;dateTime">2015-04-12T02:45:54.351+02:00</m:generated_time>
        <m:has_related_eccairs_term rdf:resource="http://onto.fel.cvut.cz/ontologies/2014/ECCAIRS_Aviation_1.3.0.12/eccairs-descriptive-factors#category_11800000"/>
    </owl:Class>
    


    <!-- http://onto.fel.cvut.cz/ontologies/aviation-safety/Engine_synchronizing -->

    <owl:Class rdf:about="&m;Engine_synchronizing">
        <rdfs:label>Engine synchronizing</rdfs:label>
        <rdfs:subClassOf rdf:resource="&m;Engine_controls_part"/>
        <m:generated_time rdf:datatype="&xsd;dateTime">2015-04-09T18:56:27.771+02:00</m:generated_time>
        <rdfs:comment xml:lang="en">(ATA Code:7601) The components providing for engine synchronization in multi-engine aircraft.</rdfs:comment>
        <m:has_related_eccairs_term rdf:resource="http://onto.fel.cvut.cz/ontologies/2014/ECCAIRS_Aviation_1.3.0.12/eccairs-descriptive-factors#category_11760100"/>
    </owl:Class>
    


    <!-- http://onto.fel.cvut.cz/ontologies/aviation-safety/Engine_temperature_indicating_system -->

    <owl:Class rdf:about="&m;Engine_temperature_indicating_system">
        <rdfs:label>Engine temperature indicating system</rdfs:label>
        <rdfs:subClassOf rdf:resource="&m;Engine_indicating_system_part"/>
        <m:generated_time rdf:datatype="&xsd;dateTime">2015-04-09T18:56:27.771+02:00</m:generated_time>
        <rdfs:comment xml:lang="en">(ATA Code:7720) Engine temperature indicating system: The system components and parts which indicate engine temperatures.</rdfs:comment>
        <m:has_related_eccairs_term rdf:resource="http://onto.fel.cvut.cz/ontologies/2014/ECCAIRS_Aviation_1.3.0.12/eccairs-descriptive-factors#category_11772000"/>
    </owl:Class>
    


    <!-- http://onto.fel.cvut.cz/ontologies/aviation-safety/Engine_temperature_indicating_system_part -->

    <owl:Class rdf:about="&m;Engine_temperature_indicating_system_part">
        <rdfs:label>Engine temperature indicating system part</rdfs:label>
        <rdfs:subClassOf rdf:resource="&m;Engine_indicating_system_part"/>
        <rdfs:subClassOf>
            <owl:Restriction>
                <owl:onProperty rdf:resource="http://onto.fel.cvut.cz/ontologies/ufo/is_part_of"/>
                <owl:someValuesFrom rdf:resource="&m;Engine_temperature_indicating_system"/>
            </owl:Restriction>
        </rdfs:subClassOf>
        <m:generated_time rdf:datatype="&xsd;dateTime">2015-04-12T02:45:54.351+02:00</m:generated_time>
        <m:has_related_eccairs_term rdf:resource="http://onto.fel.cvut.cz/ontologies/2014/ECCAIRS_Aviation_1.3.0.12/eccairs-descriptive-factors#category_11772000"/>
    </owl:Class>
    


    <!-- http://onto.fel.cvut.cz/ontologies/aviation-safety/Engine_vibration_analyzer -->

    <owl:Class rdf:about="&m;Engine_vibration_analyzer">
        <rdfs:label>Engine vibration analyzer</rdfs:label>
        <rdfs:subClassOf rdf:resource="&m;Engine_ignition_analyzer_system_part"/>
        <m:generated_time rdf:datatype="&xsd;dateTime">2015-04-09T18:56:27.771+02:00</m:generated_time>
        <rdfs:comment xml:lang="en">(ATA Code:7732) The engine vibration analyzer system indicating to the flight crew unusual engine vibration conditions. Typical parts are connector, harness, indicator, monitor, sensor and amplifier.</rdfs:comment>
        <m:has_related_eccairs_term rdf:resource="http://onto.fel.cvut.cz/ontologies/2014/ECCAIRS_Aviation_1.3.0.12/eccairs-descriptive-factors#category_11773200"/>
    </owl:Class>
    


    <!-- http://onto.fel.cvut.cz/ontologies/aviation-safety/Engine_water-methanol_injection -->

    <owl:Class rdf:about="&m;Engine_water-methanol_injection">
        <rdfs:label>Engine water/methanol injection</rdfs:label>
        <rdfs:subClassOf rdf:resource="&m;Water_injection_-_Storage_part"/>
        <m:generated_time rdf:datatype="&xsd;dateTime">2015-04-09T18:56:27.771+02:00</m:generated_time>
        <rdfs:comment xml:lang="en">(ATA Code:8201) Engine water/methanol injection</rdfs:comment>
        <m:has_related_eccairs_term rdf:resource="http://onto.fel.cvut.cz/ontologies/2014/ECCAIRS_Aviation_1.3.0.12/eccairs-descriptive-factors#category_11820100"/>
    </owl:Class>
    


    <!-- http://onto.fel.cvut.cz/ontologies/aviation-safety/Entrance_stairs -->

    <owl:Class rdf:about="&m;Entrance_stairs">
        <rdfs:label>Entrance stairs</rdfs:label>
        <rdfs:subClassOf rdf:resource="&m;Fuselage_doors_part"/>
        <m:generated_time rdf:datatype="&xsd;dateTime">2015-04-09T18:56:27.771+02:00</m:generated_time>
        <rdfs:comment xml:lang="en">(ATA Code:5260) Entrance stairs: The cabin entrance stairs which operate in conjunction with, but are not an integral part of, entrance doors. Typical parts are structure, actuator, controls and handrails, step, cable, bungee, latch hook, latch, bracket and bellcrank.</rdfs:comment>
        <m:has_related_eccairs_term rdf:resource="http://onto.fel.cvut.cz/ontologies/2014/ECCAIRS_Aviation_1.3.0.12/eccairs-descriptive-factors#category_11526000"/>
    </owl:Class>
    


    <!-- http://onto.fel.cvut.cz/ontologies/aviation-safety/Equipment-Furnishings_Wiring -->

    <owl:Class rdf:about="&m;Equipment-Furnishings_Wiring">
        <rdfs:label>Equipment/Furnishings Wiring</rdfs:label>
        <rdfs:subClassOf rdf:resource="&m;Cabin_equipment-furnishings"/>
        <m:generated_time rdf:datatype="&xsd;dateTime">2015-04-09T18:56:27.771+02:00</m:generated_time>
        <rdfs:comment xml:lang="en">(ATA Code:2597) Wiring specific to the Equipment/Furnishing Systems.</rdfs:comment>
        <m:has_related_eccairs_term rdf:resource="http://onto.fel.cvut.cz/ontologies/2014/ECCAIRS_Aviation_1.3.0.12/eccairs-descriptive-factors#category_11259700"/>
    </owl:Class>
    


    <!-- http://onto.fel.cvut.cz/ontologies/aviation-safety/Equipment_attachment_fittings_(on_fuselage) -->

    <owl:Class rdf:about="&m;Equipment_attachment_fittings_(on_fuselage)">
        <rdfs:label>Equipment attachment fittings (on fuselage)</rdfs:label>
        <rdfs:subClassOf rdf:resource="&m;Fuselage_attachment_fittings_part"/>
        <m:generated_time rdf:datatype="&xsd;dateTime">2015-04-09T18:56:27.771+02:00</m:generated_time>
        <rdfs:comment xml:lang="en">(ATA Code:5345) The fittings on the fuselage used for the attachment of equipment.</rdfs:comment>
        <m:has_related_eccairs_term rdf:resource="http://onto.fel.cvut.cz/ontologies/2014/ECCAIRS_Aviation_1.3.0.12/eccairs-descriptive-factors#category_11534500"/>
    </owl:Class>
    


    <!-- http://onto.fel.cvut.cz/ontologies/aviation-safety/Equipment_cooling_system -->

    <owl:Class rdf:about="&m;Equipment_cooling_system">
        <rdfs:subClassOf rdf:resource="&m;Air_conditioning_system_part"/>
    </owl:Class>
    


    <!-- http://onto.fel.cvut.cz/ontologies/aviation-safety/Escape_slide -->

    <owl:Class rdf:about="&m;Escape_slide">
        <rdfs:subClassOf rdf:resource="&m;Emergency_equipment"/>
    </owl:Class>
    


    <!-- http://onto.fel.cvut.cz/ontologies/aviation-safety/Exhaust_turbine_system_(reciprocating) -->

    <owl:Class rdf:about="&m;Exhaust_turbine_system_(reciprocating)">
        <rdfs:label>Exhaust turbine system (reciprocating)</rdfs:label>
        <rdfs:subClassOf rdf:resource="&m;Aircraft_part"/>
        <m:generated_time rdf:datatype="&xsd;dateTime">2015-04-09T18:56:27.771+02:00</m:generated_time>
        <rdfs:comment xml:lang="en">(ATA Code:8100) The exhaust turbine systems for reciprocating engines. Includes power recovery turbine assemblies and turbo-supercharger units when external to the engine.</rdfs:comment>
        <m:has_related_eccairs_term rdf:resource="http://onto.fel.cvut.cz/ontologies/2014/ECCAIRS_Aviation_1.3.0.12/eccairs-descriptive-factors#category_11810000"/>
    </owl:Class>
    


    <!-- http://onto.fel.cvut.cz/ontologies/aviation-safety/Exhaust_turbine_system_(reciprocating)_part -->

    <owl:Class rdf:about="&m;Exhaust_turbine_system_(reciprocating)_part">
        <rdfs:label>Exhaust turbine system (reciprocating) part</rdfs:label>
        <rdfs:subClassOf rdf:resource="&m;Aircraft_part"/>
        <rdfs:subClassOf>
            <owl:Restriction>
                <owl:onProperty rdf:resource="http://onto.fel.cvut.cz/ontologies/ufo/is_part_of"/>
                <owl:someValuesFrom rdf:resource="&m;Exhaust_turbine_system_(reciprocating)"/>
            </owl:Restriction>
        </rdfs:subClassOf>
        <m:generated_time rdf:datatype="&xsd;dateTime">2015-04-12T02:45:54.351+02:00</m:generated_time>
        <m:has_related_eccairs_term rdf:resource="http://onto.fel.cvut.cz/ontologies/2014/ECCAIRS_Aviation_1.3.0.12/eccairs-descriptive-factors#category_11810000"/>
    </owl:Class>
    


    <!-- http://onto.fel.cvut.cz/ontologies/aviation-safety/Exhaust_turbocharger -->

    <owl:Class rdf:about="&m;Exhaust_turbocharger">
        <rdfs:label>Exhaust turbocharger</rdfs:label>
        <rdfs:subClassOf rdf:resource="&m;Exhaust_turbine_system_(reciprocating)_part"/>
        <m:generated_time rdf:datatype="&xsd;dateTime">2015-04-09T18:56:27.771+02:00</m:generated_time>
        <rdfs:comment xml:lang="en">(ATA Code:8120) Exhaust turbocharger: The airframe or engine manufacturer furnished exhaust driven turbocharger systems including the turbocharger unit, density controller and waste gate valve. Does not include the tailpipe. Typical parts are clamp, coupling, rod end, bracket, hose, scroll, bearing, impeller and shaft.</rdfs:comment>
        <m:has_related_eccairs_term rdf:resource="http://onto.fel.cvut.cz/ontologies/2014/ECCAIRS_Aviation_1.3.0.12/eccairs-descriptive-factors#category_11812000"/>
    </owl:Class>
    


    <!-- http://onto.fel.cvut.cz/ontologies/aviation-safety/Explosion_suppression_system -->

    <owl:Class rdf:about="&m;Explosion_suppression_system">
        <rdfs:label>Explosion suppression system</rdfs:label>
        <rdfs:subClassOf rdf:resource="&m;Fire_protection_system_part"/>
        <m:generated_time rdf:datatype="&xsd;dateTime">2015-04-09T18:56:27.771+02:00</m:generated_time>
        <rdfs:comment xml:lang="en">(ATA Code:2630) Explosion suppression system: The system installed to extinguish a flame propagating into the fuel vent or scoop to prevent an explosion in the fuel system.</rdfs:comment>
        <m:has_related_eccairs_term rdf:resource="http://onto.fel.cvut.cz/ontologies/2014/ECCAIRS_Aviation_1.3.0.12/eccairs-descriptive-factors#category_11263000"/>
    </owl:Class>
    


    <!-- http://onto.fel.cvut.cz/ontologies/aviation-safety/Exterior_Color_Schemes_and_Markings -->

    <owl:Class rdf:about="&m;Exterior_Color_Schemes_and_Markings">
        <rdfs:label>Exterior Color Schemes and Markings</rdfs:label>
        <rdfs:subClassOf rdf:resource="&m;Placards_and_markings"/>
        <m:generated_time rdf:datatype="&xsd;dateTime">2015-04-09T18:56:27.771+02:00</m:generated_time>
        <rdfs:comment xml:lang="en">(ATA Code:1110) Exterior Color Schemes and Markings</rdfs:comment>
        <m:has_related_eccairs_term rdf:resource="http://onto.fel.cvut.cz/ontologies/2014/ECCAIRS_Aviation_1.3.0.12/eccairs-descriptive-factors#category_11111000"/>
    </owl:Class>
    


    <!-- http://onto.fel.cvut.cz/ontologies/aviation-safety/Exterior_Placards_and_Markings -->

    <owl:Class rdf:about="&m;Exterior_Placards_and_Markings">
        <rdfs:label>Exterior Placards and Markings</rdfs:label>
        <rdfs:subClassOf rdf:resource="&m;Placards_and_markings"/>
        <m:generated_time rdf:datatype="&xsd;dateTime">2015-04-09T18:56:27.771+02:00</m:generated_time>
        <rdfs:comment xml:lang="en">(ATA Code:1120) Those placards, markings, self-illuminating signs, etc.   required for interior general and emergency information, instructions, cautions, warnings, etc.</rdfs:comment>
        <m:has_related_eccairs_term rdf:resource="http://onto.fel.cvut.cz/ontologies/2014/ECCAIRS_Aviation_1.3.0.12/eccairs-descriptive-factors#category_11112000"/>
    </owl:Class>
    


    <!-- http://onto.fel.cvut.cz/ontologies/aviation-safety/Exterior_lighting -->

    <owl:Class rdf:about="&m;Exterior_lighting">
        <rdfs:label xml:lang="en">Exterior lighting</rdfs:label>
        <rdfs:subClassOf rdf:resource="&m;Lighting_system"/>
    </owl:Class>
    


    <!-- http://onto.fel.cvut.cz/ontologies/aviation-safety/External_electrical_power_system_connection -->

    <owl:Class rdf:about="&m;External_electrical_power_system_connection">
        <rdfs:label>External electrical power system connection</rdfs:label>
        <rdfs:subClassOf rdf:resource="&m;Electrical_power_system_part"/>
        <m:generated_time rdf:datatype="&xsd;dateTime">2015-04-09T18:56:27.771+02:00</m:generated_time>
        <rdfs:comment xml:lang="en">(ATA Code:2440) That portion of the system within the aircraft which connects external electrical power to the aircraft&apos;s electrical system. Includes items such as receptacles, relays, switches, wiring, warning lights, etc.</rdfs:comment>
        <m:has_related_eccairs_term rdf:resource="http://onto.fel.cvut.cz/ontologies/2014/ECCAIRS_Aviation_1.3.0.12/eccairs-descriptive-factors#category_11244000"/>
    </owl:Class>
    


    <!-- http://onto.fel.cvut.cz/ontologies/aviation-safety/Fasteners -->

    <owl:Class rdf:about="&m;Fasteners">
        <rdfs:label>Fasteners</rdfs:label>
        <rdfs:subClassOf rdf:resource="&m;Miscellaneous_hardware_part"/>
        <m:generated_time rdf:datatype="&xsd;dateTime">2015-04-09T18:56:27.771+02:00</m:generated_time>
        <rdfs:comment xml:lang="en">(ATA Code:1430) Any aircraft or engine fastener that are not associated a specific aircraft system.   Typical parts are generic AN bolts, nuts, rivets. etc.</rdfs:comment>
        <m:has_related_eccairs_term rdf:resource="http://onto.fel.cvut.cz/ontologies/2014/ECCAIRS_Aviation_1.3.0.12/eccairs-descriptive-factors#category_11143000"/>
    </owl:Class>
    


    <!-- http://onto.fel.cvut.cz/ontologies/aviation-safety/Fire-smoke-overheat_detection_system -->

    <owl:Class rdf:about="&m;Fire-smoke-overheat_detection_system">
        <rdfs:label>Fire/smoke/overheat detection system</rdfs:label>
        <rdfs:subClassOf rdf:resource="&m;Fire_protection_system_part"/>
        <m:generated_time rdf:datatype="&xsd;dateTime">2015-04-09T18:56:27.771+02:00</m:generated_time>
        <rdfs:comment xml:lang="en">(ATA Code:2610) Fire/smoke/overheat detection system: The system used to sense and indicate the presence of overheat or fire in any of the protected areas.</rdfs:comment>
        <m:has_related_eccairs_term rdf:resource="http://onto.fel.cvut.cz/ontologies/2014/ECCAIRS_Aviation_1.3.0.12/eccairs-descriptive-factors#category_11261000"/>
    </owl:Class>
    


    <!-- http://onto.fel.cvut.cz/ontologies/aviation-safety/Fire-smoke-overheat_detection_system_part -->

    <owl:Class rdf:about="&m;Fire-smoke-overheat_detection_system_part">
        <rdfs:label>Fire/smoke/overheat detection system part</rdfs:label>
        <rdfs:subClassOf rdf:resource="&m;Fire_protection_system_part"/>
        <rdfs:subClassOf>
            <owl:Restriction>
                <owl:onProperty rdf:resource="http://onto.fel.cvut.cz/ontologies/ufo/is_part_of"/>
                <owl:someValuesFrom rdf:resource="&m;Fire-smoke-overheat_detection_system"/>
            </owl:Restriction>
        </rdfs:subClassOf>
        <m:generated_time rdf:datatype="&xsd;dateTime">2015-04-12T02:45:54.351+02:00</m:generated_time>
        <m:has_related_eccairs_term rdf:resource="http://onto.fel.cvut.cz/ontologies/2014/ECCAIRS_Aviation_1.3.0.12/eccairs-descriptive-factors#category_11261000"/>
    </owl:Class>
    


    <!-- http://onto.fel.cvut.cz/ontologies/aviation-safety/Fire_Protection_System_Wiring -->

    <owl:Class rdf:about="&m;Fire_Protection_System_Wiring">
        <rdfs:label>Fire Protection System Wiring</rdfs:label>
        <rdfs:subClassOf rdf:resource="&m;Fire_protection_system_part"/>
        <m:generated_time rdf:datatype="&xsd;dateTime">2015-04-09T18:56:27.771+02:00</m:generated_time>
        <rdfs:comment xml:lang="en">(ATA Code:2697) Wiring specific to the Fire Protection System.</rdfs:comment>
        <m:has_related_eccairs_term rdf:resource="http://onto.fel.cvut.cz/ontologies/2014/ECCAIRS_Aviation_1.3.0.12/eccairs-descriptive-factors#category_11269700"/>
    </owl:Class>
    


    <!-- http://onto.fel.cvut.cz/ontologies/aviation-safety/Fire_bottle,_fixed -->

    <owl:Class rdf:about="&m;Fire_bottle,_fixed">
        <rdfs:label>Fire bottle, fixed</rdfs:label>
        <rdfs:subClassOf rdf:resource="&m;Fire_extinguishing_system_part"/>
        <m:generated_time rdf:datatype="&xsd;dateTime">2015-04-09T18:56:27.771+02:00</m:generated_time>
        <rdfs:comment xml:lang="en">(ATA Code:2621) Fire bottle, fixed: The fixed fire bottle and associated parts that store extinguishing agent under pressure. Typical parts are bottle, cartridge and brackets.</rdfs:comment>
        <m:has_related_eccairs_term rdf:resource="http://onto.fel.cvut.cz/ontologies/2014/ECCAIRS_Aviation_1.3.0.12/eccairs-descriptive-factors#category_11262100"/>
    </owl:Class>
    


    <!-- http://onto.fel.cvut.cz/ontologies/aviation-safety/Fire_bottle,_portable -->

    <owl:Class rdf:about="&m;Fire_bottle,_portable">
        <rdfs:label>Fire bottle, portable</rdfs:label>
        <rdfs:subClassOf rdf:resource="&m;Fire_extinguishing_system_part"/>
        <m:generated_time rdf:datatype="&xsd;dateTime">2015-04-09T18:56:27.771+02:00</m:generated_time>
        <rdfs:comment xml:lang="en">(ATA Code:2622) Fire bottle, portable: The portable fire extinguishes mounted within the flight compartment and cabin.</rdfs:comment>
        <m:has_related_eccairs_term rdf:resource="http://onto.fel.cvut.cz/ontologies/2014/ECCAIRS_Aviation_1.3.0.12/eccairs-descriptive-factors#category_11262200"/>
    </owl:Class>
    


    <!-- http://onto.fel.cvut.cz/ontologies/aviation-safety/Fire_detection_system -->

    <owl:Class rdf:about="&m;Fire_detection_system">
        <rdfs:label>Fire detection system</rdfs:label>
        <rdfs:subClassOf rdf:resource="&m;Fire-smoke-overheat_detection_system_part"/>
        <m:generated_time rdf:datatype="&xsd;dateTime">2015-04-09T18:56:27.771+02:00</m:generated_time>
        <rdfs:comment xml:lang="en">(ATA Code:2612) Fire detection system: The system used to sense and indicate the presence of fire in any of the protected areas of the aircraft. Typical parts are detectors, sensors, wiring, relays, amplifiers and the test circuit.</rdfs:comment>
        <m:has_related_eccairs_term rdf:resource="http://onto.fel.cvut.cz/ontologies/2014/ECCAIRS_Aviation_1.3.0.12/eccairs-descriptive-factors#category_11261200"/>
    </owl:Class>
    


    <!-- http://onto.fel.cvut.cz/ontologies/aviation-safety/Fire_extinguishing_indication_system -->

    <owl:Class rdf:about="&m;Fire_extinguishing_indication_system">
        <rdfs:label>Fire extinguishing indication system</rdfs:label>
        <rdfs:subClassOf rdf:resource="&m;Fire_protection_system_part"/>
        <m:generated_time rdf:datatype="&xsd;dateTime">2015-04-09T18:56:27.771+02:00</m:generated_time>
        <rdfs:comment xml:lang="en">(ATA Code:2640) Fire extinguishing indication system</rdfs:comment>
        <m:has_related_eccairs_term rdf:resource="http://onto.fel.cvut.cz/ontologies/2014/ECCAIRS_Aviation_1.3.0.12/eccairs-descriptive-factors#category_11264000"/>
    </owl:Class>
    


    <!-- http://onto.fel.cvut.cz/ontologies/aviation-safety/Fire_extinguishing_system -->

    <owl:Class rdf:about="&m;Fire_extinguishing_system">
        <rdfs:label>Fire extinguishing system</rdfs:label>
        <rdfs:subClassOf rdf:resource="&m;Fire_protection_system_part"/>
        <m:generated_time rdf:datatype="&xsd;dateTime">2015-04-09T18:56:27.771+02:00</m:generated_time>
        <rdfs:comment xml:lang="en">(ATA Code:2620) Fire extinguishing system: The components and parts other than the fixed or portable bottles used to extinguish any fire in the aircraft. Typical parts are valve, squib, control module, switch and tubing.</rdfs:comment>
        <m:has_related_eccairs_term rdf:resource="http://onto.fel.cvut.cz/ontologies/2014/ECCAIRS_Aviation_1.3.0.12/eccairs-descriptive-factors#category_11262000"/>
    </owl:Class>
    


    <!-- http://onto.fel.cvut.cz/ontologies/aviation-safety/Fire_extinguishing_system_part -->

    <owl:Class rdf:about="&m;Fire_extinguishing_system_part">
        <rdfs:label>Fire extinguishing system part</rdfs:label>
        <rdfs:subClassOf rdf:resource="&m;Fire_protection_system_part"/>
        <rdfs:subClassOf>
            <owl:Restriction>
                <owl:onProperty rdf:resource="http://onto.fel.cvut.cz/ontologies/ufo/is_part_of"/>
                <owl:someValuesFrom rdf:resource="&m;Fire_extinguishing_system"/>
            </owl:Restriction>
        </rdfs:subClassOf>
        <m:generated_time rdf:datatype="&xsd;dateTime">2015-04-12T02:45:54.351+02:00</m:generated_time>
        <m:has_related_eccairs_term rdf:resource="http://onto.fel.cvut.cz/ontologies/2014/ECCAIRS_Aviation_1.3.0.12/eccairs-descriptive-factors#category_11262000"/>
    </owl:Class>
    


    <!-- http://onto.fel.cvut.cz/ontologies/aviation-safety/Fire_protection_system -->

    <owl:Class rdf:about="&m;Fire_protection_system">
        <rdfs:subClassOf rdf:resource="&m;Aircraft_part"/>
    </owl:Class>
    


    <!-- http://onto.fel.cvut.cz/ontologies/aviation-safety/Fire_protection_system_part -->

    <owl:Class rdf:about="&m;Fire_protection_system_part">
        <rdfs:label>Fire protection system part</rdfs:label>
        <rdfs:subClassOf rdf:resource="&m;Aircraft_part"/>
        <rdfs:subClassOf>
            <owl:Restriction>
                <owl:onProperty rdf:resource="http://onto.fel.cvut.cz/ontologies/ufo/is_part_of"/>
                <owl:someValuesFrom rdf:resource="&m;Fire_protection_system"/>
            </owl:Restriction>
        </rdfs:subClassOf>
        <m:generated_time rdf:datatype="&xsd;dateTime">2015-04-12T02:45:54.351+02:00</m:generated_time>
        <m:has_related_eccairs_term rdf:resource="http://onto.fel.cvut.cz/ontologies/2014/ECCAIRS_Aviation_1.3.0.12/eccairs-descriptive-factors#category_11260000"/>
    </owl:Class>
    


    <!-- http://onto.fel.cvut.cz/ontologies/aviation-safety/Fixed_inner_doors -->

    <owl:Class rdf:about="&m;Fixed_inner_doors">
        <rdfs:label>Fixed inner doors</rdfs:label>
        <rdfs:subClassOf rdf:resource="&m;Fuselage_doors_part"/>
        <m:generated_time rdf:datatype="&xsd;dateTime">2015-04-09T18:56:27.771+02:00</m:generated_time>
        <rdfs:comment xml:lang="en">(ATA Code:5250) Fixed inner doors: The doors within the fuselage in fixed partitions but not including doors in movable partitions. Typical parts are structure, hinges, latches and lining.</rdfs:comment>
        <m:has_related_eccairs_term rdf:resource="http://onto.fel.cvut.cz/ontologies/2014/ECCAIRS_Aviation_1.3.0.12/eccairs-descriptive-factors#category_11525000"/>
    </owl:Class>
    


    <!-- http://onto.fel.cvut.cz/ontologies/aviation-safety/Flight_Control_System_Wiring -->

    <owl:Class rdf:about="&m;Flight_Control_System_Wiring">
        <rdfs:label>Flight Control System Wiring</rdfs:label>
        <rdfs:subClassOf rdf:resource="&m;Flight_control_system_part"/>
        <m:generated_time rdf:datatype="&xsd;dateTime">2015-04-09T18:56:27.771+02:00</m:generated_time>
        <rdfs:comment xml:lang="en">(ATA Code:2797) Wiring specific to the Flight Control Systems.</rdfs:comment>
        <m:has_related_eccairs_term rdf:resource="http://onto.fel.cvut.cz/ontologies/2014/ECCAIRS_Aviation_1.3.0.12/eccairs-descriptive-factors#category_11279700"/>
    </owl:Class>
    


    <!-- http://onto.fel.cvut.cz/ontologies/aviation-safety/Flight_compartment_equipment -->

    <owl:Class rdf:about="&m;Flight_compartment_equipment">
        <rdfs:label>Flight compartment equipment</rdfs:label>
        <rdfs:subClassOf rdf:resource="&m;Cabin_equipment-furnishings"/>
        <rdfs:subClassOf>
            <owl:Restriction>
                <owl:onProperty rdf:resource="http://onto.fel.cvut.cz/ontologies/ufo/is_part_of"/>
                <owl:someValuesFrom rdf:resource="&m;Flight_compartment_equipment"/>
            </owl:Restriction>
        </rdfs:subClassOf>
        <m:generated_time rdf:datatype="&xsd;dateTime">2015-04-09T18:56:27.771+02:00</m:generated_time>
        <m:generated_time rdf:datatype="&xsd;dateTime">2015-04-12T02:45:54.351+02:00</m:generated_time>
        <rdfs:comment xml:lang="en">(ATA Code:2510) Flight compartment equipment: The removable equipment and furnishings within the cockpit or crew station of a general nature. Typical parts are seats, shoulder harnesses, take-up harness reels, seat belts, sun visors, panels, map case, attach brackets and hardware.</rdfs:comment>
        <m:has_related_eccairs_term rdf:resource="http://onto.fel.cvut.cz/ontologies/2014/ECCAIRS_Aviation_1.3.0.12/eccairs-descriptive-factors#category_11251000"/>
    </owl:Class>
    


    <!-- http://onto.fel.cvut.cz/ontologies/aviation-safety/Flight_compartment_lighting -->

    <owl:Class rdf:about="&m;Flight_compartment_lighting">
        <rdfs:label>Flight compartment lighting</rdfs:label>
        <rdfs:subClassOf rdf:resource="&m;Lighting_system"/>
        <m:generated_time rdf:datatype="&xsd;dateTime">2015-04-09T18:56:27.771+02:00</m:generated_time>
        <rdfs:comment xml:lang="en">(ATA Code:3310) Flight compartment lighting: The lighting systems and equipment including panel illumination other than inside individual instruments, master warning light systems such as annunciator panels and associated dimming systems located in the flight compartment only. Typical parts are bulb, socket, switch, lamp, lens, relay, rheostat, resistor and ballast.</rdfs:comment>
        <m:has_related_eccairs_term rdf:resource="http://onto.fel.cvut.cz/ontologies/2014/ECCAIRS_Aviation_1.3.0.12/eccairs-descriptive-factors#category_11331000"/>
    </owl:Class>
    


    <!-- http://onto.fel.cvut.cz/ontologies/aviation-safety/Flight_compartment_windows-windshields -->

    <owl:Class rdf:about="&m;Flight_compartment_windows-windshields">
        <rdfs:label>Flight compartment windows/windshields</rdfs:label>
        <rdfs:subClassOf rdf:resource="&m;Window-windshield_system_part"/>
        <m:generated_time rdf:datatype="&xsd;dateTime">2015-04-09T18:56:27.771+02:00</m:generated_time>
        <rdfs:comment xml:lang="en">(ATA Code:5610) Flight compartment windows/windshields: Any cockpit windows, cockpit overhead canopies, observation windows and windshield panels in the flight compartment. Includes attachment and sliding feature of sliding windows. For cockpit windows including the breakage of electrically heated windshield panels regardless of cause. Does not include the heating aspects associated circuitry of heated windshields, [Code 11304000]. Typical parts are windshield, sliding window, seal, frame, panel, latch, hinge and chin bubbles.</rdfs:comment>
        <m:has_related_eccairs_term rdf:resource="http://onto.fel.cvut.cz/ontologies/2014/ECCAIRS_Aviation_1.3.0.12/eccairs-descriptive-factors#category_11561000"/>
    </owl:Class>
    


    <!-- http://onto.fel.cvut.cz/ontologies/aviation-safety/Flight_control_system -->

    <owl:Class rdf:about="&m;Flight_control_system">
        <rdfs:label>Flight control system</rdfs:label>
        <rdfs:subClassOf rdf:resource="&m;Aircraft_part"/>
        <m:generated_time rdf:datatype="&xsd;dateTime">2015-04-09T18:56:27.771+02:00</m:generated_time>
        <rdfs:comment xml:lang="en">(ATA Code:2700) Flight control system: The units and components furnishing a means of manually controlling the flight attitude characteristics of the aircraft. Also includes the functioning and maintenance aspects of the flaps, spoilers and other control surfaces, but does not include the structure. Typical parts are hydraulic boost system, controls and mounting brackets. Includes flight control problems of a general nature involving two or more systems. Does not include rotorcraft flight controls. Typical parts are hydraulic boost system, controls and mounting brackets.</rdfs:comment>
        <m:has_related_eccairs_term rdf:resource="http://onto.fel.cvut.cz/ontologies/2014/ECCAIRS_Aviation_1.3.0.12/eccairs-descriptive-factors#category_11270000"/>
    </owl:Class>
    


    <!-- http://onto.fel.cvut.cz/ontologies/aviation-safety/Flight_control_system_part -->

    <owl:Class rdf:about="&m;Flight_control_system_part">
        <rdfs:label>Flight control system part</rdfs:label>
        <rdfs:subClassOf rdf:resource="&m;Aircraft_part"/>
        <rdfs:subClassOf>
            <owl:Restriction>
                <owl:onProperty rdf:resource="http://onto.fel.cvut.cz/ontologies/ufo/is_part_of"/>
                <owl:someValuesFrom rdf:resource="&m;Flight_control_system"/>
            </owl:Restriction>
        </rdfs:subClassOf>
        <m:generated_time rdf:datatype="&xsd;dateTime">2015-04-12T02:45:54.351+02:00</m:generated_time>
        <m:has_related_eccairs_term rdf:resource="http://onto.fel.cvut.cz/ontologies/2014/ECCAIRS_Aviation_1.3.0.12/eccairs-descriptive-factors#category_11270000"/>
    </owl:Class>
    


    <!-- http://onto.fel.cvut.cz/ontologies/aviation-safety/Flight_controller -->

    <owl:Class rdf:about="&m;Flight_controller">
        <rdfs:label>Flight controller</rdfs:label>
        <rdfs:subClassOf rdf:resource="&m;Autopilot_system_part"/>
        <rdfs:subClassOf rdf:resource="&m;autoflight_system"/>
        <m:generated_time rdf:datatype="&xsd;dateTime">2015-04-09T18:56:27.771+02:00</m:generated_time>
        <all2:has_ATA_code rdf:datatype="&xsd;integer">2213</all2:has_ATA_code>
        <rdfs:comment xml:lang="en">(ATA Code:2213) Flight controller: The command unit of an autopilot system. The unit is manually operated to generate signals which cause the aircraft to climb, dive or perform coordinated turns.</rdfs:comment>
        <m:has_related_eccairs_term rdf:resource="http://onto.fel.cvut.cz/ontologies/2014/ECCAIRS_Aviation_1.3.0.12/eccairs-descriptive-factors#category_11221300"/>
    </owl:Class>
    


    <!-- http://onto.fel.cvut.cz/ontologies/aviation-safety/Flight_crew_documentation -->

    <owl:Class rdf:about="&m;Flight_crew_documentation">
        <rdfs:label>Flight crew documentation</rdfs:label>
        <rdfs:subClassOf rdf:resource="&m;Flight_compartment_equipment"/>
        <m:generated_time rdf:datatype="&xsd;dateTime">2015-04-09T18:56:27.771+02:00</m:generated_time>
        <rdfs:comment xml:lang="en">(ATA Code:2511) Flight crew documentation: The documentation used by the flight crew for reference during the operation of the aircraft, includes maps, charts, manuals and checklists. e.g.: Operations manual. A manual containing procedures, instructions and guidance for use by operational personnel in the execution of their duties.  Minimum equipment list (MEL). A list which provides for the operation of aircraft, subject to specified conditions, with particular equipment inoperative, prepared by an operator in conformity with, or more restrictive than, the MMEL established for the aircraft type.</rdfs:comment>
        <m:has_related_eccairs_term rdf:resource="http://onto.fel.cvut.cz/ontologies/2014/ECCAIRS_Aviation_1.3.0.12/eccairs-descriptive-factors#category_11251100"/>
    </owl:Class>
    


    <!-- http://onto.fel.cvut.cz/ontologies/aviation-safety/Flight_deck_information_systems -->

    <owl:Class rdf:about="&m;Flight_deck_information_systems">
        <rdfs:label>Flight deck information systems</rdfs:label>
        <rdfs:subClassOf rdf:resource="&m;Information_system_part"/>
        <m:generated_time rdf:datatype="&xsd;dateTime">2015-04-09T18:56:27.771+02:00</m:generated_time>
        <rdfs:comment xml:lang="en">(ATA Code:4620) Flight deck information systems: The portion of the onboard information system that supports the flight deck systems, flight crew and flight operations.</rdfs:comment>
        <m:has_related_eccairs_term rdf:resource="http://onto.fel.cvut.cz/ontologies/2014/ECCAIRS_Aviation_1.3.0.12/eccairs-descriptive-factors#category_11462000"/>
    </owl:Class>
    


    <!-- http://onto.fel.cvut.cz/ontologies/aviation-safety/Flight_environment_data_system -->

    <owl:Class rdf:about="&m;Flight_environment_data_system">
        <rdfs:label>Flight environment data system</rdfs:label>
        <rdfs:subClassOf rdf:resource="&m;Navigation_system"/>
        <rdfs:subClassOf>
            <owl:Restriction>
                <owl:onProperty rdf:resource="http://onto.fel.cvut.cz/ontologies/ufo/is_part_of"/>
                <owl:someValuesFrom rdf:resource="&m;Flight_environment_data_system"/>
            </owl:Restriction>
        </rdfs:subClassOf>
        <m:generated_time rdf:datatype="&xsd;dateTime">2015-04-09T18:56:27.771+02:00</m:generated_time>
        <m:generated_time rdf:datatype="&xsd;dateTime">2015-04-12T02:45:54.351+02:00</m:generated_time>
        <rdfs:comment xml:lang="en">(ATA Code:3410) Flight environment data system: The system which senses environmental conditions and uses the data to influence navigation.</rdfs:comment>
        <m:has_related_eccairs_term rdf:resource="http://onto.fel.cvut.cz/ontologies/2014/ECCAIRS_Aviation_1.3.0.12/eccairs-descriptive-factors#category_11341000"/>
    </owl:Class>
    


    <!-- http://onto.fel.cvut.cz/ontologies/aviation-safety/Flight_management_computing_system -->

    <owl:Class rdf:about="&m;Flight_management_computing_system">
        <rdfs:label>Flight management computing system</rdfs:label>
        <rdfs:subClassOf rdf:resource="&m;Navigation_system"/>
        <m:generated_time rdf:datatype="&xsd;dateTime">2015-04-09T18:56:27.771+02:00</m:generated_time>
        <rdfs:comment xml:lang="en">(ATA Code:3460) Flight management computing system: The system which combines navigational data to compute or manage the aircraft&apos;s geographical position or theoretical flight path. Includes items such as course computers, flight management computers, performance data computers and associated control display units and warning annunciators.</rdfs:comment>
        <m:has_related_eccairs_term rdf:resource="http://onto.fel.cvut.cz/ontologies/2014/ECCAIRS_Aviation_1.3.0.12/eccairs-descriptive-factors#category_11346000"/>
    </owl:Class>
    


    <!-- http://onto.fel.cvut.cz/ontologies/aviation-safety/Fluid_service_doors -->

    <owl:Class rdf:about="&m;Fluid_service_doors">
        <rdfs:label>Fluid service doors</rdfs:label>
        <rdfs:subClassOf rdf:resource="&m;Service_doors_part"/>
        <m:generated_time rdf:datatype="&xsd;dateTime">2015-04-09T18:56:27.771+02:00</m:generated_time>
        <rdfs:comment xml:lang="en">(ATA Code:5246) Fluid service doors: The exterior doors used primarily to gain access for servicing the fluid service areas but excluding compartment doors [Code 11524300]. Typical parts are hinges, structure and the latch mechanism.</rdfs:comment>
        <m:has_related_eccairs_term rdf:resource="http://onto.fel.cvut.cz/ontologies/2014/ECCAIRS_Aviation_1.3.0.12/eccairs-descriptive-factors#category_11524600"/>
    </owl:Class>
    


    <!-- http://onto.fel.cvut.cz/ontologies/aviation-safety/Folding_-_Controls_and_Indicating -->

    <owl:Class rdf:about="&m;Folding_-_Controls_and_Indicating">
        <rdfs:label>Folding - Controls and Indicating</rdfs:label>
        <rdfs:subClassOf rdf:resource="&m;Folding_blades-pylon_part"/>
        <m:generated_time rdf:datatype="&xsd;dateTime">2015-04-09T18:56:27.771+02:00</m:generated_time>
        <rdfs:comment xml:lang="en">(ATA Code:6630) Part of the system intended for controlling folding/spreading sequences and for indicating the system operation.   Includes the control units, caption lights, indicators, wiring, etc.</rdfs:comment>
        <m:has_related_eccairs_term rdf:resource="http://onto.fel.cvut.cz/ontologies/2014/ECCAIRS_Aviation_1.3.0.12/eccairs-descriptive-factors#category_11663000"/>
    </owl:Class>
    


    <!-- http://onto.fel.cvut.cz/ontologies/aviation-safety/Folding_blades-pylon -->

    <owl:Class rdf:about="&m;Folding_blades-pylon">
        <rdfs:label>Folding blades/pylon</rdfs:label>
        <rdfs:subClassOf rdf:resource="&m;Aircraft_part"/>
        <m:generated_time rdf:datatype="&xsd;dateTime">2015-04-09T18:56:27.771+02:00</m:generated_time>
        <rdfs:comment xml:lang="en">(ATA Code:6600) Folding blades/pylon: The whole of the system ensuring automatic or manual folding and spreading of the rotor blades and/or tail pylon.</rdfs:comment>
        <m:has_related_eccairs_term rdf:resource="http://onto.fel.cvut.cz/ontologies/2014/ECCAIRS_Aviation_1.3.0.12/eccairs-descriptive-factors#category_11660000"/>
    </owl:Class>
    


    <!-- http://onto.fel.cvut.cz/ontologies/aviation-safety/Folding_blades-pylon_part -->

    <owl:Class rdf:about="&m;Folding_blades-pylon_part">
        <rdfs:label>Folding blades/pylon part</rdfs:label>
        <rdfs:subClassOf rdf:resource="&m;Aircraft_part"/>
        <rdfs:subClassOf>
            <owl:Restriction>
                <owl:onProperty rdf:resource="http://onto.fel.cvut.cz/ontologies/ufo/is_part_of"/>
                <owl:someValuesFrom rdf:resource="&m;Folding_blades-pylon"/>
            </owl:Restriction>
        </rdfs:subClassOf>
        <m:generated_time rdf:datatype="&xsd;dateTime">2015-04-12T02:45:54.351+02:00</m:generated_time>
        <m:has_related_eccairs_term rdf:resource="http://onto.fel.cvut.cz/ontologies/2014/ECCAIRS_Aviation_1.3.0.12/eccairs-descriptive-factors#category_11660000"/>
    </owl:Class>
    


    <!-- http://onto.fel.cvut.cz/ontologies/aviation-safety/Frame-spar-rib_(nacelles-pylon) -->

    <owl:Class rdf:about="&m;Frame-spar-rib_(nacelles-pylon)">
        <rdfs:label>Frame/spar/rib (nacelles/pylon)</rdfs:label>
        <rdfs:subClassOf rdf:resource="&m;Main_frame_(nacelle-pylon)_part"/>
        <m:generated_time rdf:datatype="&xsd;dateTime">2015-04-09T18:56:27.771+02:00</m:generated_time>
        <rdfs:comment xml:lang="en">(ATA Code:5411) The main frame, spar or rib structure on the nacelles or pylons.</rdfs:comment>
        <m:has_related_eccairs_term rdf:resource="http://onto.fel.cvut.cz/ontologies/2014/ECCAIRS_Aviation_1.3.0.12/eccairs-descriptive-factors#category_11541100"/>
    </owl:Class>
    


    <!-- http://onto.fel.cvut.cz/ontologies/aviation-safety/Fuel_Flow_Sensor -->

    <owl:Class rdf:about="&m;Fuel_Flow_Sensor">
        <rdfs:label>Fuel Flow Sensor</rdfs:label>
        <rdfs:subClassOf rdf:resource="&m;Engine_fuel_indicating_system_part"/>
        <m:generated_time rdf:datatype="&xsd;dateTime">2015-04-09T18:56:27.771+02:00</m:generated_time>
        <rdfs:comment xml:lang="en">(ATA Code:7333) The unit and associated circuitry and parts which senses and transmits the rate of fuel flow to the cockpit indicator.  Typical parts are transmitter, sensor, fitting, connector, transducer, etc.</rdfs:comment>
        <m:has_related_eccairs_term rdf:resource="http://onto.fel.cvut.cz/ontologies/2014/ECCAIRS_Aviation_1.3.0.12/eccairs-descriptive-factors#category_100000020"/>
    </owl:Class>
    


    <!-- http://onto.fel.cvut.cz/ontologies/aviation-safety/Fuel_System_Wiring -->

    <owl:Class rdf:about="&m;Fuel_System_Wiring">
        <rdfs:subClassOf rdf:resource="&m;Aircraft_fuel_system_part"/>
    </owl:Class>
    


    <!-- http://onto.fel.cvut.cz/ontologies/aviation-safety/Fuel_control_-_carburetor -->

    <owl:Class rdf:about="&m;Fuel_control_-_carburetor">
        <rdfs:label>Fuel control - carburetor</rdfs:label>
        <rdfs:subClassOf rdf:resource="&m;Fuel_control_system_part"/>
        <m:generated_time rdf:datatype="&xsd;dateTime">2015-04-09T18:56:27.771+02:00</m:generated_time>
        <rdfs:comment xml:lang="en">(ATA Code:7322) Fuel control - carburetor: The component which meters fuel/air mixture for engine combustion, both reciprocating and turbine engines. Includes turbine engines which utilize non-electronic fuel controls. Typical parts are computer, amplifier, synchronization box and carburetor inlet temperature sensor.</rdfs:comment>
        <m:has_related_eccairs_term rdf:resource="http://onto.fel.cvut.cz/ontologies/2014/ECCAIRS_Aviation_1.3.0.12/eccairs-descriptive-factors#category_11732200"/>
    </owl:Class>
    


    <!-- http://onto.fel.cvut.cz/ontologies/aviation-safety/Fuel_control_-_electronic -->

    <owl:Class rdf:about="&m;Fuel_control_-_electronic">
        <rdfs:label>Fuel control - electronic</rdfs:label>
        <rdfs:subClassOf rdf:resource="&m;Fuel_control_system_part"/>
        <m:generated_time rdf:datatype="&xsd;dateTime">2015-04-09T18:56:27.771+02:00</m:generated_time>
        <rdfs:comment xml:lang="en">(ATA Code:7321) Fuel control - electronic: The components which control metered fuel flow electronically under all probable temperature, altitude and barometric pressure conditions. Typical parts are computer, amplifier, synchronizer box and carburetor inlet temperature sensor.</rdfs:comment>
        <m:has_related_eccairs_term rdf:resource="http://onto.fel.cvut.cz/ontologies/2014/ECCAIRS_Aviation_1.3.0.12/eccairs-descriptive-factors#category_11732100"/>
    </owl:Class>
    


    <!-- http://onto.fel.cvut.cz/ontologies/aviation-safety/Fuel_control_system -->

    <owl:Class rdf:about="&m;Fuel_control_system">
        <rdfs:label>Fuel control system</rdfs:label>
        <rdfs:subClassOf rdf:resource="&m;Engine_fuel_and_control_systems_part"/>
        <m:generated_time rdf:datatype="&xsd;dateTime">2015-04-09T18:56:27.771+02:00</m:generated_time>
        <rdfs:comment xml:lang="en">(ATA Code:7320) Fuel control system: The powerplant fuel system components or parts other than the fuel control, amplifier, computer, carburetor and indication systems which control and deliver metered fuel/air to engine cylinders or turbine engine burner cans. Typical parts are sense line, power and drain valve (P &amp; D valve), drain valve and carburetor inlet temperature sensor.</rdfs:comment>
        <m:has_related_eccairs_term rdf:resource="http://onto.fel.cvut.cz/ontologies/2014/ECCAIRS_Aviation_1.3.0.12/eccairs-descriptive-factors#category_11732000"/>
    </owl:Class>
    


    <!-- http://onto.fel.cvut.cz/ontologies/aviation-safety/Fuel_control_system_part -->

    <owl:Class rdf:about="&m;Fuel_control_system_part">
        <rdfs:label>Fuel control system part</rdfs:label>
        <rdfs:subClassOf rdf:resource="&m;Engine_fuel_and_control_systems_part"/>
        <rdfs:subClassOf>
            <owl:Restriction>
                <owl:onProperty rdf:resource="http://onto.fel.cvut.cz/ontologies/ufo/is_part_of"/>
                <owl:someValuesFrom rdf:resource="&m;Fuel_control_system"/>
            </owl:Restriction>
        </rdfs:subClassOf>
        <m:generated_time rdf:datatype="&xsd;dateTime">2015-04-12T02:45:54.351+02:00</m:generated_time>
        <m:has_related_eccairs_term rdf:resource="http://onto.fel.cvut.cz/ontologies/2014/ECCAIRS_Aviation_1.3.0.12/eccairs-descriptive-factors#category_11732000"/>
    </owl:Class>
    


    <!-- http://onto.fel.cvut.cz/ontologies/aviation-safety/Fuel_distribution_system -->

    <owl:Class rdf:about="&m;Fuel_distribution_system">
        <rdfs:label>Fuel distribution system</rdfs:label>
        <rdfs:subClassOf rdf:resource="&m;Aircraft_fuel_system_part"/>
        <m:generated_time rdf:datatype="&xsd;dateTime">2015-04-09T18:56:27.771+02:00</m:generated_time>
        <rdfs:comment xml:lang="en">(ATA Code:2820) Fuel distribution system: The portion of the aircraft fuel system other than selector valves, transfer valves, electric motor driven pumps used to distribute fuel from the tank outlet to the powerplant quick disconnect or up to the strainer unit. Includes the engine primer equipment, the switch that senses failure of a system pump and the switch that automatically activates the boost pump. Typical parts are line, fitting, primer, nozzle, primer pump and actuating linkage for the fuel selector/shutoff valve.</rdfs:comment>
        <m:has_related_eccairs_term rdf:resource="http://onto.fel.cvut.cz/ontologies/2014/ECCAIRS_Aviation_1.3.0.12/eccairs-descriptive-factors#category_11282000"/>
    </owl:Class>
    


    <!-- http://onto.fel.cvut.cz/ontologies/aviation-safety/Fuel_distribution_system_part -->

    <owl:Class rdf:about="&m;Fuel_distribution_system_part">
        <rdfs:label>Fuel distribution system part</rdfs:label>
        <rdfs:subClassOf rdf:resource="&m;Aircraft_fuel_system_part"/>
        <rdfs:subClassOf>
            <owl:Restriction>
                <owl:onProperty rdf:resource="http://onto.fel.cvut.cz/ontologies/ufo/is_part_of"/>
                <owl:someValuesFrom rdf:resource="&m;Fuel_distribution_system"/>
            </owl:Restriction>
        </rdfs:subClassOf>
        <m:generated_time rdf:datatype="&xsd;dateTime">2015-04-12T02:45:54.351+02:00</m:generated_time>
        <m:has_related_eccairs_term rdf:resource="http://onto.fel.cvut.cz/ontologies/2014/ECCAIRS_Aviation_1.3.0.12/eccairs-descriptive-factors#category_11282000"/>
    </owl:Class>
    


    <!-- http://onto.fel.cvut.cz/ontologies/aviation-safety/Fuel_divider -->

    <owl:Class rdf:about="&m;Fuel_divider">
        <rdfs:label>Fuel divider</rdfs:label>
        <rdfs:subClassOf rdf:resource="&m;Fuel_control_system_part"/>
        <m:generated_time rdf:datatype="&xsd;dateTime">2015-04-09T18:56:27.771+02:00</m:generated_time>
        <rdfs:comment xml:lang="en">(ATA Code:7324) Fuel divider: The unit in metered fuel lines which directs fuel to individual cylinders or burner cans.</rdfs:comment>
        <m:has_related_eccairs_term rdf:resource="http://onto.fel.cvut.cz/ontologies/2014/ECCAIRS_Aviation_1.3.0.12/eccairs-descriptive-factors#category_11732400"/>
    </owl:Class>
    


    <!-- http://onto.fel.cvut.cz/ontologies/aviation-safety/Fuel_dump_system -->

    <owl:Class rdf:about="&m;Fuel_dump_system">
        <rdfs:label>Fuel dump system</rdfs:label>
        <rdfs:subClassOf rdf:resource="&m;Aircraft_fuel_system_part"/>
        <m:generated_time rdf:datatype="&xsd;dateTime">2015-04-09T18:56:27.771+02:00</m:generated_time>
        <rdfs:comment xml:lang="en">(ATA Code:2830) Fuel dump system: The system and components which provide for the jettison of fuel during flight. Typical parts are valve, switch and dump chutes.Fuel dumping: The intentional airborne release of usable fuel. This does not include the dropping of fuel tanks.</rdfs:comment>
        <m:has_related_eccairs_term rdf:resource="http://onto.fel.cvut.cz/ontologies/2014/ECCAIRS_Aviation_1.3.0.12/eccairs-descriptive-factors#category_11283000"/>
    </owl:Class>
    


    <!-- http://onto.fel.cvut.cz/ontologies/aviation-safety/Fuel_filter-strainer -->

    <owl:Class rdf:about="&m;Fuel_filter-strainer">
        <rdfs:label>Fuel filter/strainer</rdfs:label>
        <rdfs:subClassOf rdf:resource="&m;Fuel_distribution_system_part"/>
        <m:generated_time rdf:datatype="&xsd;dateTime">2015-04-09T18:56:27.771+02:00</m:generated_time>
        <rdfs:comment xml:lang="en">(ATA Code:2821) Fuel filter/strainer: The component that filters unmetered fuel upstream of the engine fuel control/carburetor. Does not include the engine fuel metered control system filters [Code 11730000]. Typical parts are screen, housing, bowl, gasket, plunger and stand pipe.</rdfs:comment>
        <m:has_related_eccairs_term rdf:resource="http://onto.fel.cvut.cz/ontologies/2014/ECCAIRS_Aviation_1.3.0.12/eccairs-descriptive-factors#category_11282100"/>
    </owl:Class>
    


    <!-- http://onto.fel.cvut.cz/ontologies/aviation-safety/Fuel_flow_indicating_system -->

    <owl:Class rdf:about="&m;Fuel_flow_indicating_system">
        <rdfs:label>Fuel flow indicating system</rdfs:label>
        <rdfs:subClassOf rdf:resource="&m;Engine_fuel_indicating_system_part"/>
        <m:generated_time rdf:datatype="&xsd;dateTime">2015-04-09T18:56:27.771+02:00</m:generated_time>
        <rdfs:comment xml:lang="en">(ATA Code:7331) Fuel flow indicating system: The instrument which indicates the flow rate of metered fuel to the engine. Does not include the transmitter. Typical parts are indicator, power supply, needle and dial.</rdfs:comment>
        <m:has_related_eccairs_term rdf:resource="http://onto.fel.cvut.cz/ontologies/2014/ECCAIRS_Aviation_1.3.0.12/eccairs-descriptive-factors#category_11733100"/>
    </owl:Class>
    


    <!-- http://onto.fel.cvut.cz/ontologies/aviation-safety/Fuel_heater -->

    <owl:Class rdf:about="&m;Fuel_heater">
        <rdfs:label>Fuel heater</rdfs:label>
        <rdfs:subClassOf rdf:resource="&m;Engine_fuel_system_part"/>
        <m:generated_time rdf:datatype="&xsd;dateTime">2015-04-09T18:56:27.771+02:00</m:generated_time>
        <rdfs:comment xml:lang="en">(ATA Code:7312) Fuel heater: The powerplant fuel unit which heats fuel flowing to the engine to prevent freezing of entrapped water. Does not include connecting lines or the heat source.</rdfs:comment>
        <m:has_related_eccairs_term rdf:resource="http://onto.fel.cvut.cz/ontologies/2014/ECCAIRS_Aviation_1.3.0.12/eccairs-descriptive-factors#category_11731200"/>
    </owl:Class>
    


    <!-- http://onto.fel.cvut.cz/ontologies/aviation-safety/Fuel_indicating_system -->

    <owl:Class rdf:about="&m;Fuel_indicating_system">
        <rdfs:label>Fuel indicating system</rdfs:label>
        <rdfs:subClassOf rdf:resource="&m;Aircraft_fuel_system_part"/>
        <m:generated_time rdf:datatype="&xsd;dateTime">2015-04-09T18:56:27.771+02:00</m:generated_time>
        <rdfs:comment xml:lang="en">(ATA Code:2840) Fuel indicating system: The portion of the system which is used to indicate the quantity, temperature and pressure of the fuel. Includes pressure warning systems for pumping systems within the tank. Does not include engine fuel pressure reports [Code 11733200] or flow indication system [Code 11733100]. Typical parts are circuit breaker, connector, pressure switch, indicator lights and dipstick.</rdfs:comment>
        <m:has_related_eccairs_term rdf:resource="http://onto.fel.cvut.cz/ontologies/2014/ECCAIRS_Aviation_1.3.0.12/eccairs-descriptive-factors#category_11284000"/>
    </owl:Class>
    


    <!-- http://onto.fel.cvut.cz/ontologies/aviation-safety/Fuel_indicating_system_part -->

    <owl:Class rdf:about="&m;Fuel_indicating_system_part">
        <rdfs:label>Fuel indicating system part</rdfs:label>
        <rdfs:subClassOf rdf:resource="&m;Aircraft_fuel_system_part"/>
        <rdfs:subClassOf>
            <owl:Restriction>
                <owl:onProperty rdf:resource="http://onto.fel.cvut.cz/ontologies/ufo/is_part_of"/>
                <owl:someValuesFrom rdf:resource="&m;Fuel_indicating_system"/>
            </owl:Restriction>
        </rdfs:subClassOf>
        <m:generated_time rdf:datatype="&xsd;dateTime">2015-04-12T02:45:54.351+02:00</m:generated_time>
        <m:has_related_eccairs_term rdf:resource="http://onto.fel.cvut.cz/ontologies/2014/ECCAIRS_Aviation_1.3.0.12/eccairs-descriptive-factors#category_11284000"/>
    </owl:Class>
    


    <!-- http://onto.fel.cvut.cz/ontologies/aviation-safety/Fuel_injection_nozzle -->

    <owl:Class rdf:about="&m;Fuel_injection_nozzle">
        <rdfs:label>Fuel injection nozzle</rdfs:label>
        <rdfs:subClassOf rdf:resource="&m;Engine_fuel_system_part"/>
        <m:generated_time rdf:datatype="&xsd;dateTime">2015-04-09T18:56:27.771+02:00</m:generated_time>
        <rdfs:comment xml:lang="en">(ATA Code:7313) Fuel injection nozzle: The powerplant fuel unit which injects metered fuel into piston engine cylinders and burner cans in turbine engines.</rdfs:comment>
        <m:has_related_eccairs_term rdf:resource="http://onto.fel.cvut.cz/ontologies/2014/ECCAIRS_Aviation_1.3.0.12/eccairs-descriptive-factors#category_11731300"/>
    </owl:Class>
    


    <!-- http://onto.fel.cvut.cz/ontologies/aviation-safety/Fuel_oil_cooler -->

    <owl:Class rdf:about="&m;Fuel_oil_cooler">
        <rdfs:label>Fuel oil cooler</rdfs:label>
        <rdfs:subClassOf rdf:resource="&m;Engine_fuel_system_part"/>
        <m:generated_time rdf:datatype="&xsd;dateTime">2015-04-09T18:56:27.771+02:00</m:generated_time>
        <rdfs:comment xml:lang="en">(ATA Code:7311) Fuel oil cooler: The powerplant fuel unit in which aircraft fuel flows to cool the turbine engine lubricating oil. Does not include the connecting lines.</rdfs:comment>
        <m:has_related_eccairs_term rdf:resource="http://onto.fel.cvut.cz/ontologies/2014/ECCAIRS_Aviation_1.3.0.12/eccairs-descriptive-factors#category_11731100"/>
    </owl:Class>
    


    <!-- http://onto.fel.cvut.cz/ontologies/aviation-safety/Fuel_press_sensor -->

    <owl:Class rdf:about="&m;Fuel_press_sensor">
        <rdfs:label>Fuel press sensor</rdfs:label>
        <rdfs:subClassOf rdf:resource="&m;Engine_fuel_indicating_system_part"/>
        <m:generated_time rdf:datatype="&xsd;dateTime">2015-04-09T18:56:27.771+02:00</m:generated_time>
        <rdfs:comment xml:lang="en">(ATA Code:7334) Fuel press sensor: The units which sense and transmit to the cockpit indicator or indicator lamps, the pressure of fuel available at the engine fuel control/carburetor. Includes pressure switch and circuitry for warning indication. Typical parts are transducer and transmitter.</rdfs:comment>
        <m:has_related_eccairs_term rdf:resource="http://onto.fel.cvut.cz/ontologies/2014/ECCAIRS_Aviation_1.3.0.12/eccairs-descriptive-factors#category_11733201"/>
    </owl:Class>
    


    <!-- http://onto.fel.cvut.cz/ontologies/aviation-safety/Fuel_pressure_indicating_system -->

    <owl:Class rdf:about="&m;Fuel_pressure_indicating_system">
        <rdfs:label>Fuel pressure indicating system</rdfs:label>
        <rdfs:subClassOf rdf:resource="&m;Engine_fuel_indicating_system_part"/>
        <m:generated_time rdf:datatype="&xsd;dateTime">2015-04-09T18:56:27.771+02:00</m:generated_time>
        <rdfs:comment xml:lang="en">(ATA Code:7332) Fuel pressure indicating system: The instrument which indicates the pressure of fuel at the fuel control/carburetor as provided by the engine driven, or motor driven, pumps. Includes the pressure warning indicating lamps. Typical parts are indicator, bourdon tube, diaphragm, needle and case.</rdfs:comment>
        <m:has_related_eccairs_term rdf:resource="http://onto.fel.cvut.cz/ontologies/2014/ECCAIRS_Aviation_1.3.0.12/eccairs-descriptive-factors#category_11733200"/>
    </owl:Class>
    


    <!-- http://onto.fel.cvut.cz/ontologies/aviation-safety/Fuel_pressure_indicator -->

    <owl:Class rdf:about="&m;Fuel_pressure_indicator">
        <rdfs:label>Fuel pressure indicator</rdfs:label>
        <rdfs:subClassOf rdf:resource="&m;Fuel_indicating_system_part"/>
        <m:generated_time rdf:datatype="&xsd;dateTime">2015-04-09T18:56:27.771+02:00</m:generated_time>
        <rdfs:comment xml:lang="en">(ATA Code:2844) Fuel pressure indicator: The tank unit which measures the pressure of fuel in that tank and indicates it on a gauge on the flight deck. Typical parts are the pressure switch and indicator lights.</rdfs:comment>
        <m:has_related_eccairs_term rdf:resource="http://onto.fel.cvut.cz/ontologies/2014/ECCAIRS_Aviation_1.3.0.12/eccairs-descriptive-factors#category_11284400"/>
    </owl:Class>
    


    <!-- http://onto.fel.cvut.cz/ontologies/aviation-safety/Fuel_pumps -->

    <owl:Class rdf:about="&m;Fuel_pumps">
        <rdfs:label>Fuel pumps</rdfs:label>
        <rdfs:subClassOf rdf:resource="&m;Fuel_distribution_system_part"/>
        <m:generated_time rdf:datatype="&xsd;dateTime">2015-04-09T18:56:27.771+02:00</m:generated_time>
        <rdfs:comment xml:lang="en">(ATA Code:2822) Fuel pumps</rdfs:comment>
        <m:has_related_eccairs_term rdf:resource="http://onto.fel.cvut.cz/ontologies/2014/ECCAIRS_Aviation_1.3.0.12/eccairs-descriptive-factors#category_11282200"/>
    </owl:Class>
    


    <!-- http://onto.fel.cvut.cz/ontologies/aviation-safety/Fuel_quantity_indicator -->

    <owl:Class rdf:about="&m;Fuel_quantity_indicator">
        <rdfs:label>Fuel quantity indicator</rdfs:label>
        <rdfs:subClassOf rdf:resource="&m;Fuel_indicating_system_part"/>
        <m:generated_time rdf:datatype="&xsd;dateTime">2015-04-09T18:56:27.771+02:00</m:generated_time>
        <rdfs:comment xml:lang="en">(ATA Code:2841) Fuel quantity indicator: The indicator and low level warning system used to indicate the quantity of fuel in the tanks. Typical parts are indicator, lamp and bulbs.</rdfs:comment>
        <m:has_related_eccairs_term rdf:resource="http://onto.fel.cvut.cz/ontologies/2014/ECCAIRS_Aviation_1.3.0.12/eccairs-descriptive-factors#category_11284100"/>
    </owl:Class>
    


    <!-- http://onto.fel.cvut.cz/ontologies/aviation-safety/Fuel_quantity_sensor -->

    <owl:Class rdf:about="&m;Fuel_quantity_sensor">
        <rdfs:label>Fuel quantity sensor</rdfs:label>
        <rdfs:subClassOf rdf:resource="&m;Fuel_indicating_system_part"/>
        <m:generated_time rdf:datatype="&xsd;dateTime">2015-04-09T18:56:27.771+02:00</m:generated_time>
        <rdfs:comment xml:lang="en">(ATA Code:2842) Fuel quantity sensor: The tank unit which measures and transmits a signal to the cockpit indicator. Typical parts are transmitter, float switch, probe, sensor, totalizer, tank unit float and gaskets.</rdfs:comment>
        <m:has_related_eccairs_term rdf:resource="http://onto.fel.cvut.cz/ontologies/2014/ECCAIRS_Aviation_1.3.0.12/eccairs-descriptive-factors#category_11284200"/>
    </owl:Class>
    


    <!-- http://onto.fel.cvut.cz/ontologies/aviation-safety/Fuel_selector-shutoff_valve -->

    <owl:Class rdf:about="&m;Fuel_selector-shutoff_valve">
        <rdfs:label>Fuel selector/shutoff valve</rdfs:label>
        <rdfs:subClassOf rdf:resource="&m;Fuel_distribution_system_part"/>
        <m:generated_time rdf:datatype="&xsd;dateTime">2015-04-09T18:56:27.771+02:00</m:generated_time>
        <rdfs:comment xml:lang="en">(ATA Code:2823) Fuel selector/shutoff valve: The component and associated controls and position indication units which provides for specific tank selection or shutting off of flow to the engine. Typical parts are housing, rotor, handle, guard, seat, seal, selector valve, shutoff valve and springs.</rdfs:comment>
        <m:has_related_eccairs_term rdf:resource="http://onto.fel.cvut.cz/ontologies/2014/ECCAIRS_Aviation_1.3.0.12/eccairs-descriptive-factors#category_11282300"/>
    </owl:Class>
    


    <!-- http://onto.fel.cvut.cz/ontologies/aviation-safety/Fuel_storage_system -->

    <owl:Class rdf:about="&m;Fuel_storage_system">
        <rdfs:label>Fuel storage system</rdfs:label>
        <rdfs:subClassOf rdf:resource="&m;Aircraft_fuel_system_part"/>
        <m:generated_time rdf:datatype="&xsd;dateTime">2015-04-09T18:56:27.771+02:00</m:generated_time>
        <rdfs:comment xml:lang="en">(ATA Code:2810) Fuel storage system: The portion of the fuel system used for the storage of fuel. Does not include defects in the wing primary structure of integral tanks. Typical parts are removable metal tank, tip tank, header tank, bladder fuel cell, tank interconnect lines, vent line, vent valve, drain valve, filler cap, filler neck, check valve, vent tube, cap seal, filler adapter, outlet fitting, screen, fuelling panel, tank strap and sealant.</rdfs:comment>
        <m:has_related_eccairs_term rdf:resource="http://onto.fel.cvut.cz/ontologies/2014/ECCAIRS_Aviation_1.3.0.12/eccairs-descriptive-factors#category_11281000"/>
    </owl:Class>
    


    <!-- http://onto.fel.cvut.cz/ontologies/aviation-safety/Fuel_temperature_indicating -->

    <owl:Class rdf:about="&m;Fuel_temperature_indicating">
        <rdfs:label>Fuel temperature indicating</rdfs:label>
        <rdfs:subClassOf rdf:resource="&m;Fuel_indicating_system_part"/>
        <m:generated_time rdf:datatype="&xsd;dateTime">2015-04-09T18:56:27.771+02:00</m:generated_time>
        <rdfs:comment xml:lang="en">(ATA Code:2843) Fuel temperature indicating: The system which measures the temperature of fuel in each tank and indicates that temperature on a gauge located on the flight deck.</rdfs:comment>
        <m:has_related_eccairs_term rdf:resource="http://onto.fel.cvut.cz/ontologies/2014/ECCAIRS_Aviation_1.3.0.12/eccairs-descriptive-factors#category_11284300"/>
    </owl:Class>
    


    <!-- http://onto.fel.cvut.cz/ontologies/aviation-safety/Fuel_transfer_valve -->

    <owl:Class rdf:about="&m;Fuel_transfer_valve">
        <rdfs:label>Fuel transfer valve</rdfs:label>
        <rdfs:subClassOf rdf:resource="&m;Fuel_distribution_system_part"/>
        <m:generated_time rdf:datatype="&xsd;dateTime">2015-04-09T18:56:27.771+02:00</m:generated_time>
        <rdfs:comment xml:lang="en">(ATA Code:2824) Fuel transfer valve: The component and associated control linkage which provides for the transfer of fuel between tanks for crossfeeding to alternate engine fuel systems. Typical parts are seal, housing, rotor, handle and transfer valves.</rdfs:comment>
        <m:has_related_eccairs_term rdf:resource="http://onto.fel.cvut.cz/ontologies/2014/ECCAIRS_Aviation_1.3.0.12/eccairs-descriptive-factors#category_11282400"/>
    </owl:Class>
    


    <!-- http://onto.fel.cvut.cz/ontologies/aviation-safety/Fuselage_attachment_fittings -->

    <owl:Class rdf:about="&m;Fuselage_attachment_fittings">
        <rdfs:label>Fuselage attachment fittings</rdfs:label>
        <rdfs:subClassOf rdf:resource="&m;Fuselage_structure_(general)_part"/>
        <m:generated_time rdf:datatype="&xsd;dateTime">2015-04-09T18:56:27.771+02:00</m:generated_time>
        <rdfs:comment xml:lang="en">(ATA Code:5340) Fuselage attachment fittings: The fittings on the fuselage used for the attachment of doors, wings, stabilizers, landing gear, engine and rotor pylons and the support of equipment within the fuselage.</rdfs:comment>
        <m:has_related_eccairs_term rdf:resource="http://onto.fel.cvut.cz/ontologies/2014/ECCAIRS_Aviation_1.3.0.12/eccairs-descriptive-factors#category_11534000"/>
    </owl:Class>
    


    <!-- http://onto.fel.cvut.cz/ontologies/aviation-safety/Fuselage_attachment_fittings_part -->

    <owl:Class rdf:about="&m;Fuselage_attachment_fittings_part">
        <rdfs:label>Fuselage attachment fittings part</rdfs:label>
        <rdfs:subClassOf rdf:resource="&m;Fuselage_structure_(general)_part"/>
        <rdfs:subClassOf>
            <owl:Restriction>
                <owl:onProperty rdf:resource="http://onto.fel.cvut.cz/ontologies/ufo/is_part_of"/>
                <owl:someValuesFrom rdf:resource="&m;Fuselage_attachment_fittings"/>
            </owl:Restriction>
        </rdfs:subClassOf>
        <m:generated_time rdf:datatype="&xsd;dateTime">2015-04-12T02:45:54.351+02:00</m:generated_time>
        <m:has_related_eccairs_term rdf:resource="http://onto.fel.cvut.cz/ontologies/2014/ECCAIRS_Aviation_1.3.0.12/eccairs-descriptive-factors#category_11534000"/>
    </owl:Class>
    


    <!-- http://onto.fel.cvut.cz/ontologies/aviation-safety/Fuselage_doors -->

    <owl:Class rdf:about="&m;Fuselage_doors">
        <rdfs:label>Fuselage doors</rdfs:label>
        <rdfs:subClassOf rdf:resource="&m;Aircraft_part"/>
        <m:generated_time rdf:datatype="&xsd;dateTime">2015-04-09T18:56:27.771+02:00</m:generated_time>
        <rdfs:comment xml:lang="en">(ATA Code:5200) Fuselage doors: The removable units used for entrance or exit and for enclosing other structure contained within the fuselage. Includes passenger and crew doors, cargo doors and emergency exits. Includes electrical and hydraulic systems associated with door control as appropriate.</rdfs:comment>
        <m:has_related_eccairs_term rdf:resource="http://onto.fel.cvut.cz/ontologies/2014/ECCAIRS_Aviation_1.3.0.12/eccairs-descriptive-factors#category_11520000"/>
    </owl:Class>
    


    <!-- http://onto.fel.cvut.cz/ontologies/aviation-safety/Fuselage_doors_part -->

    <owl:Class rdf:about="&m;Fuselage_doors_part">
        <rdfs:label>Fuselage doors part</rdfs:label>
        <rdfs:subClassOf rdf:resource="&m;Aircraft_part"/>
        <rdfs:subClassOf>
            <owl:Restriction>
                <owl:onProperty rdf:resource="http://onto.fel.cvut.cz/ontologies/ufo/is_part_of"/>
                <owl:someValuesFrom rdf:resource="&m;Fuselage_doors"/>
            </owl:Restriction>
        </rdfs:subClassOf>
        <m:generated_time rdf:datatype="&xsd;dateTime">2015-04-12T02:45:54.351+02:00</m:generated_time>
        <m:has_related_eccairs_term rdf:resource="http://onto.fel.cvut.cz/ontologies/2014/ECCAIRS_Aviation_1.3.0.12/eccairs-descriptive-factors#category_11520000"/>
    </owl:Class>
    


    <!-- http://onto.fel.cvut.cz/ontologies/aviation-safety/Fuselage_fairings -->

    <owl:Class rdf:about="&m;Fuselage_fairings">
        <rdfs:label>Fuselage fairings</rdfs:label>
        <rdfs:subClassOf rdf:resource="&m;Fuselage_structure_(general)_part"/>
        <m:generated_time rdf:datatype="&xsd;dateTime">2015-04-09T18:56:27.771+02:00</m:generated_time>
        <rdfs:comment xml:lang="en">(ATA Code:5350) Fuselage fairings: The fixed and removable aerodynamic fairings between the fuselage and wing/empennage/nacelle attachment points, tail cones and radomes. Also includes the rings on rotorcraft tail cones. Typical parts are tail, radome, fairing, stiffener, screw, fillet and skin.</rdfs:comment>
        <m:has_related_eccairs_term rdf:resource="http://onto.fel.cvut.cz/ontologies/2014/ECCAIRS_Aviation_1.3.0.12/eccairs-descriptive-factors#category_11535000"/>
    </owl:Class>
    


    <!-- http://onto.fel.cvut.cz/ontologies/aviation-safety/Fuselage_fixed_partitions -->

    <owl:Class rdf:about="&m;Fuselage_fixed_partitions">
        <rdfs:label>Fuselage fixed partitions</rdfs:label>
        <rdfs:subClassOf rdf:resource="&m;Fuselage_miscellaneous_structure_part"/>
        <m:generated_time rdf:datatype="&xsd;dateTime">2015-04-09T18:56:27.771+02:00</m:generated_time>
        <rdfs:comment xml:lang="en">(ATA Code:5324) Fuselage fixed partitions: The fixed partitions which are part of the fuselage structure.</rdfs:comment>
        <m:has_related_eccairs_term rdf:resource="http://onto.fel.cvut.cz/ontologies/2014/ECCAIRS_Aviation_1.3.0.12/eccairs-descriptive-factors#category_11532400"/>
    </owl:Class>
    


    <!-- http://onto.fel.cvut.cz/ontologies/aviation-safety/Fuselage_floor_panel -->

    <owl:Class rdf:about="&m;Fuselage_floor_panel">
        <rdfs:label>Fuselage floor panel</rdfs:label>
        <rdfs:subClassOf rdf:resource="&m;Fuselage_miscellaneous_structure_part"/>
        <m:generated_time rdf:datatype="&xsd;dateTime">2015-04-09T18:56:27.771+02:00</m:generated_time>
        <rdfs:comment xml:lang="en">(ATA Code:5321) Fuselage floor panel: The interior floor panels within the main fuselage auxiliary structure.</rdfs:comment>
        <m:has_related_eccairs_term rdf:resource="http://onto.fel.cvut.cz/ontologies/2014/ECCAIRS_Aviation_1.3.0.12/eccairs-descriptive-factors#category_11532100"/>
    </owl:Class>
    


    <!-- http://onto.fel.cvut.cz/ontologies/aviation-safety/Fuselage_internal_mounting_structure -->

    <owl:Class rdf:about="&m;Fuselage_internal_mounting_structure">
        <rdfs:label>Fuselage internal mounting structure</rdfs:label>
        <rdfs:subClassOf rdf:resource="&m;Fuselage_miscellaneous_structure_part"/>
        <m:generated_time rdf:datatype="&xsd;dateTime">2015-04-09T18:56:27.771+02:00</m:generated_time>
        <rdfs:comment xml:lang="en">(ATA Code:5322) Fuselage internal mounting structure: The internal mounting auxiliary structure which aids in the support of the fuselage structure.</rdfs:comment>
        <m:has_related_eccairs_term rdf:resource="http://onto.fel.cvut.cz/ontologies/2014/ECCAIRS_Aviation_1.3.0.12/eccairs-descriptive-factors#category_11532200"/>
    </owl:Class>
    


    <!-- http://onto.fel.cvut.cz/ontologies/aviation-safety/Fuselage_internal_stairs -->

    <owl:Class rdf:about="&m;Fuselage_internal_stairs">
        <rdfs:label>Fuselage internal stairs</rdfs:label>
        <rdfs:subClassOf rdf:resource="&m;Fuselage_miscellaneous_structure_part"/>
        <m:generated_time rdf:datatype="&xsd;dateTime">2015-04-09T18:56:27.771+02:00</m:generated_time>
        <rdfs:comment xml:lang="en">(ATA Code:5323) Fuselage internal stairs: The internal stairs which are part of the fuselage auxiliary structure.</rdfs:comment>
        <m:has_related_eccairs_term rdf:resource="http://onto.fel.cvut.cz/ontologies/2014/ECCAIRS_Aviation_1.3.0.12/eccairs-descriptive-factors#category_11532300"/>
    </owl:Class>
    


    <!-- http://onto.fel.cvut.cz/ontologies/aviation-safety/Fuselage_main_bulkheads -->

    <owl:Class rdf:about="&m;Fuselage_main_bulkheads">
        <rdfs:label>Fuselage main bulkheads</rdfs:label>
        <rdfs:subClassOf rdf:resource="&m;Fuselage_main_structure_part"/>
        <m:generated_time rdf:datatype="&xsd;dateTime">2015-04-09T18:56:27.771+02:00</m:generated_time>
        <rdfs:comment xml:lang="en">(ATA Code:5312) The main fuselage bulkheads and the associated attachment fittings.</rdfs:comment>
        <m:has_related_eccairs_term rdf:resource="http://onto.fel.cvut.cz/ontologies/2014/ECCAIRS_Aviation_1.3.0.12/eccairs-descriptive-factors#category_11531200"/>
    </owl:Class>
    


    <!-- http://onto.fel.cvut.cz/ontologies/aviation-safety/Fuselage_main_floor_beam -->

    <owl:Class rdf:about="&m;Fuselage_main_floor_beam">
        <rdfs:label>Fuselage main floor beam</rdfs:label>
        <rdfs:subClassOf rdf:resource="&m;Fuselage_main_structure_part"/>
        <m:generated_time rdf:datatype="&xsd;dateTime">2015-04-09T18:56:27.771+02:00</m:generated_time>
        <rdfs:comment xml:lang="en">(ATA Code:5315) The main fuselage floor beams and the associated attach fittings.</rdfs:comment>
        <m:has_related_eccairs_term rdf:resource="http://onto.fel.cvut.cz/ontologies/2014/ECCAIRS_Aviation_1.3.0.12/eccairs-descriptive-factors#category_11531500"/>
    </owl:Class>
    


    <!-- http://onto.fel.cvut.cz/ontologies/aviation-safety/Fuselage_main_frames -->

    <owl:Class rdf:about="&m;Fuselage_main_frames">
        <rdfs:label>Fuselage main frames</rdfs:label>
        <rdfs:subClassOf rdf:resource="&m;Fuselage_main_structure_part"/>
        <m:generated_time rdf:datatype="&xsd;dateTime">2015-04-09T18:56:27.771+02:00</m:generated_time>
        <rdfs:comment xml:lang="en">(ATA Code:5311) The main fuselage frames: The associated attachment fittings are covered in &quot;Fuselage miscellaneous structure&quot;.</rdfs:comment>
        <m:has_related_eccairs_term rdf:resource="http://onto.fel.cvut.cz/ontologies/2014/ECCAIRS_Aviation_1.3.0.12/eccairs-descriptive-factors#category_11531100"/>
    </owl:Class>
    


    <!-- http://onto.fel.cvut.cz/ontologies/aviation-safety/Fuselage_main_keel -->

    <owl:Class rdf:about="&m;Fuselage_main_keel">
        <rdfs:label>Fuselage main keel</rdfs:label>
        <rdfs:subClassOf rdf:resource="&m;Fuselage_main_structure_part"/>
        <m:generated_time rdf:datatype="&xsd;dateTime">2015-04-09T18:56:27.771+02:00</m:generated_time>
        <rdfs:comment xml:lang="en">(ATA Code:5314) The main fuselage keel beams and the associated attachment fittings.</rdfs:comment>
        <m:has_related_eccairs_term rdf:resource="http://onto.fel.cvut.cz/ontologies/2014/ECCAIRS_Aviation_1.3.0.12/eccairs-descriptive-factors#category_11531400"/>
    </owl:Class>
    


    <!-- http://onto.fel.cvut.cz/ontologies/aviation-safety/Fuselage_main_longeron-stringer -->

    <owl:Class rdf:about="&m;Fuselage_main_longeron-stringer">
        <rdfs:label>Fuselage main longeron/stringer</rdfs:label>
        <rdfs:subClassOf rdf:resource="&m;Fuselage_main_structure_part"/>
        <m:generated_time rdf:datatype="&xsd;dateTime">2015-04-09T18:56:27.771+02:00</m:generated_time>
        <rdfs:comment xml:lang="en">(ATA Code:5313) The main fuselage longerons/stringers and the associated attachment fittings.</rdfs:comment>
        <m:has_related_eccairs_term rdf:resource="http://onto.fel.cvut.cz/ontologies/2014/ECCAIRS_Aviation_1.3.0.12/eccairs-descriptive-factors#category_11531300"/>
    </owl:Class>
    


    <!-- http://onto.fel.cvut.cz/ontologies/aviation-safety/Fuselage_main_structure -->

    <owl:Class rdf:about="&m;Fuselage_main_structure">
        <rdfs:label>Fuselage main structure</rdfs:label>
        <rdfs:subClassOf rdf:resource="&m;Fuselage_structure_(general)_part"/>
        <m:generated_time rdf:datatype="&xsd;dateTime">2015-04-09T18:56:27.771+02:00</m:generated_time>
        <rdfs:comment xml:lang="en">(ATA Code:5310) Fuselage main structure: The fuselage structure defects which affect two or more related parts.</rdfs:comment>
        <m:has_related_eccairs_term rdf:resource="http://onto.fel.cvut.cz/ontologies/2014/ECCAIRS_Aviation_1.3.0.12/eccairs-descriptive-factors#category_11531000"/>
    </owl:Class>
    


    <!-- http://onto.fel.cvut.cz/ontologies/aviation-safety/Fuselage_main_structure_part -->

    <owl:Class rdf:about="&m;Fuselage_main_structure_part">
        <rdfs:label>Fuselage main structure part</rdfs:label>
        <rdfs:subClassOf rdf:resource="&m;Fuselage_structure_(general)_part"/>
        <rdfs:subClassOf>
            <owl:Restriction>
                <owl:onProperty rdf:resource="http://onto.fel.cvut.cz/ontologies/ufo/is_part_of"/>
                <owl:someValuesFrom rdf:resource="&m;Fuselage_main_structure"/>
            </owl:Restriction>
        </rdfs:subClassOf>
        <m:generated_time rdf:datatype="&xsd;dateTime">2015-04-12T02:45:54.351+02:00</m:generated_time>
        <m:has_related_eccairs_term rdf:resource="http://onto.fel.cvut.cz/ontologies/2014/ECCAIRS_Aviation_1.3.0.12/eccairs-descriptive-factors#category_11531000"/>
    </owl:Class>
    


    <!-- http://onto.fel.cvut.cz/ontologies/aviation-safety/Fuselage_miscellaneous_structure -->

    <owl:Class rdf:about="&m;Fuselage_miscellaneous_structure">
        <rdfs:label>Fuselage miscellaneous structure</rdfs:label>
        <rdfs:subClassOf rdf:resource="&m;Fuselage_structure_(general)_part"/>
        <m:generated_time rdf:datatype="&xsd;dateTime">2015-04-09T18:56:27.771+02:00</m:generated_time>
        <rdfs:comment xml:lang="en">(ATA Code:5320) The miscellaneous structures of the main fuselage that aid in the support of the primary structure. Includes such items as brackets, channels, stiffeners and clips. Does not include movable partitions.</rdfs:comment>
        <m:has_related_eccairs_term rdf:resource="http://onto.fel.cvut.cz/ontologies/2014/ECCAIRS_Aviation_1.3.0.12/eccairs-descriptive-factors#category_11532000"/>
    </owl:Class>
    


    <!-- http://onto.fel.cvut.cz/ontologies/aviation-safety/Fuselage_miscellaneous_structure_part -->

    <owl:Class rdf:about="&m;Fuselage_miscellaneous_structure_part">
        <rdfs:label>Fuselage miscellaneous structure part</rdfs:label>
        <rdfs:subClassOf rdf:resource="&m;Fuselage_structure_(general)_part"/>
        <rdfs:subClassOf>
            <owl:Restriction>
                <owl:onProperty rdf:resource="http://onto.fel.cvut.cz/ontologies/ufo/is_part_of"/>
                <owl:someValuesFrom rdf:resource="&m;Fuselage_miscellaneous_structure"/>
            </owl:Restriction>
        </rdfs:subClassOf>
        <m:generated_time rdf:datatype="&xsd;dateTime">2015-04-12T02:45:54.351+02:00</m:generated_time>
        <m:has_related_eccairs_term rdf:resource="http://onto.fel.cvut.cz/ontologies/2014/ECCAIRS_Aviation_1.3.0.12/eccairs-descriptive-factors#category_11532000"/>
    </owl:Class>
    


    <!-- http://onto.fel.cvut.cz/ontologies/aviation-safety/Fuselage_plate-skin -->

    <owl:Class rdf:about="&m;Fuselage_plate-skin">
        <rdfs:label>Fuselage plate/skin</rdfs:label>
        <rdfs:subClassOf rdf:resource="&m;Fuselage_structure_(general)_part"/>
        <m:generated_time rdf:datatype="&xsd;dateTime">2015-04-09T18:56:27.771+02:00</m:generated_time>
        <rdfs:comment xml:lang="en">(ATA Code:5330) Fuselage plate/skin: The exterior covering of the fuselage including access covers and skin doublers.</rdfs:comment>
        <m:has_related_eccairs_term rdf:resource="http://onto.fel.cvut.cz/ontologies/2014/ECCAIRS_Aviation_1.3.0.12/eccairs-descriptive-factors#category_11533000"/>
    </owl:Class>
    


    <!-- http://onto.fel.cvut.cz/ontologies/aviation-safety/Fuselage_structure_(general) -->

    <owl:Class rdf:about="&m;Fuselage_structure_(general)">
        <rdfs:label>Fuselage structure (general)</rdfs:label>
        <rdfs:subClassOf rdf:resource="&m;Aircraft_part"/>
        <m:generated_time rdf:datatype="&xsd;dateTime">2015-04-09T18:56:27.771+02:00</m:generated_time>
        <rdfs:comment xml:lang="en">(ATA Code:5300) Fuselage structure (general): The structural units and associated components and members which make up the compartments for crew, passengers, equipment and cargo.</rdfs:comment>
        <m:has_related_eccairs_term rdf:resource="http://onto.fel.cvut.cz/ontologies/2014/ECCAIRS_Aviation_1.3.0.12/eccairs-descriptive-factors#category_11530000"/>
    </owl:Class>
    


    <!-- http://onto.fel.cvut.cz/ontologies/aviation-safety/Fuselage_structure_(general)_part -->

    <owl:Class rdf:about="&m;Fuselage_structure_(general)_part">
        <rdfs:label>Fuselage structure (general) part</rdfs:label>
        <rdfs:subClassOf rdf:resource="&m;Aircraft_part"/>
        <rdfs:subClassOf>
            <owl:Restriction>
                <owl:onProperty rdf:resource="http://onto.fel.cvut.cz/ontologies/ufo/is_part_of"/>
                <owl:someValuesFrom rdf:resource="&m;Fuselage_structure_(general)"/>
            </owl:Restriction>
        </rdfs:subClassOf>
        <m:generated_time rdf:datatype="&xsd;dateTime">2015-04-12T02:45:54.351+02:00</m:generated_time>
        <m:has_related_eccairs_term rdf:resource="http://onto.fel.cvut.cz/ontologies/2014/ECCAIRS_Aviation_1.3.0.12/eccairs-descriptive-factors#category_11530000"/>
    </owl:Class>
    


    <!-- http://onto.fel.cvut.cz/ontologies/aviation-safety/Galley_doors -->

    <owl:Class rdf:about="&m;Galley_doors">
        <rdfs:label>Galley doors</rdfs:label>
        <rdfs:subClassOf rdf:resource="&m;Service_doors_part"/>
        <m:generated_time rdf:datatype="&xsd;dateTime">2015-04-09T18:56:27.771+02:00</m:generated_time>
        <rdfs:comment xml:lang="en">(ATA Code:5241) Galley doors: The exterior doors used primarily to gain access for servicing the aircraft galley. Typical parts are hinges, structure and the latch mechanism.</rdfs:comment>
        <m:has_related_eccairs_term rdf:resource="http://onto.fel.cvut.cz/ontologies/2014/ECCAIRS_Aviation_1.3.0.12/eccairs-descriptive-factors#category_11524100"/>
    </owl:Class>
    


    <!-- http://onto.fel.cvut.cz/ontologies/aviation-safety/Glide_slope_system -->

    <owl:Class rdf:about="&m;Glide_slope_system">
        <rdfs:label>Glide slope system</rdfs:label>
        <rdfs:subClassOf rdf:resource="&m;ILS_aircraft_equipment"/>
        <m:generated_time rdf:datatype="&xsd;dateTime">2015-04-09T18:56:27.771+02:00</m:generated_time>
        <rdfs:comment xml:lang="en">(ATA Code:3432) Glide slope system: The system which provides an instrument needle reference from an electronic signal radiated from a ground transmitter to enable the pilot to fly the proper glide path for landing under instrument meteorological conditions. Typical parts are circuit breaker, switch, receiver, antenna and indicator.</rdfs:comment>
        <m:has_related_eccairs_term rdf:resource="http://onto.fel.cvut.cz/ontologies/2014/ECCAIRS_Aviation_1.3.0.12/eccairs-descriptive-factors#category_11343200"/>
    </owl:Class>
    


    <!-- http://onto.fel.cvut.cz/ontologies/aviation-safety/Global_positioning_system -->

    <owl:Class rdf:about="&m;Global_positioning_system">
        <rdfs:label>Global positioning system</rdfs:label>
        <rdfs:subClassOf rdf:resource="&m;Dependent_position_determining_system"/>
        <m:generated_time rdf:datatype="&xsd;dateTime">2015-04-09T18:56:27.771+02:00</m:generated_time>
        <rdfs:comment xml:lang="en">(ATA Code:3457) Global positioning system: The systems which are mainly dependent upon signals from ground transmitters or orbital satellites for their operations; systems such as VHF omni-directional radio range, automatic direction finding, and distance measuring equipment. Typical parts are antenna, control unit, receiver, remote switches, connectors and coaxial cable.</rdfs:comment>
        <m:has_related_eccairs_term rdf:resource="http://onto.fel.cvut.cz/ontologies/2014/ECCAIRS_Aviation_1.3.0.12/eccairs-descriptive-factors#category_11345700"/>
    </owl:Class>
    


    <!-- http://onto.fel.cvut.cz/ontologies/aviation-safety/Ground_proximity_warning_system-terrain_avoidance_warning_system -->

    <owl:Class rdf:about="&m;Ground_proximity_warning_system-terrain_avoidance_warning_system">
        <rdfs:label>Ground proximity warning system/terrain avoidance warning system</rdfs:label>
        <rdfs:subClassOf rdf:resource="&m;Independent_position_determining_system"/>
        <m:generated_time rdf:datatype="&xsd;dateTime">2015-04-09T18:56:27.771+02:00</m:generated_time>
        <rdfs:comment xml:lang="en">(ATA Code:3444) Ground proximity warning system/terrain avoidance warning system: The system which detects and alerts flight crew to potential terrain hazards. Includes the antenna which transmits and receives an electronic signal for the radio altimeter equipment used for terrain-to-aircraft distance. Also includes the component which interprets a radio signal reflected back to a receiver to determine distance from the nearest terrain and the component which process the warning computer input signals from various sources in order to determine if and when the crew should be alerted to a terrain hazard.</rdfs:comment>
        <m:has_related_eccairs_term rdf:resource="http://onto.fel.cvut.cz/ontologies/2014/ECCAIRS_Aviation_1.3.0.12/eccairs-descriptive-factors#category_11344400"/>
    </owl:Class>
    


    <!-- http://onto.fel.cvut.cz/ontologies/aviation-safety/Gust_lock_and_damper_system -->

    <owl:Class rdf:about="&m;Gust_lock_and_damper_system">
        <rdfs:label>Gust lock and damper system</rdfs:label>
        <rdfs:subClassOf rdf:resource="&m;Flight_control_system_part"/>
        <m:generated_time rdf:datatype="&xsd;dateTime">2015-04-09T18:56:27.771+02:00</m:generated_time>
        <rdfs:comment xml:lang="en">(ATA Code:2770) Gust lock and damper system: The system and components protecting flight control surfaces from movement and damage by wind gusts while the aircraft is on the ground. Includes cockpit controlled surface locks common in light aircraft and independent hydraulic gust damper units mounted at each flight control surface on large jet powered aircraft. Does not include the damping feature of the flight control power boost systems. Typical parts are damper, cylinder, seal, rod end and lock pin cable.</rdfs:comment>
        <m:has_related_eccairs_term rdf:resource="http://onto.fel.cvut.cz/ontologies/2014/ECCAIRS_Aviation_1.3.0.12/eccairs-descriptive-factors#category_11277000"/>
    </owl:Class>
    


    <!-- http://onto.fel.cvut.cz/ontologies/aviation-safety/HF_radio_telephony -->

    <owl:Class rdf:about="&m;HF_radio_telephony">
        <rdfs:label xml:lang="en">High frequency radio telephony</rdfs:label>
        <rdfs:subClassOf>
            <owl:Class>
                <owl:intersectionOf rdf:parseType="Collection">
                    <rdf:Description rdf:about="&m;Radio_communication_equipment"/>
                    <owl:Restriction>
                        <owl:onProperty rdf:resource="&m;relates_to"/>
                        <owl:someValuesFrom rdf:resource="&m;High_frequency_communication_system"/>
                    </owl:Restriction>
                </owl:intersectionOf>
            </owl:Class>
        </rdfs:subClassOf>
        <m:generated_time rdf:datatype="&xsd;dateTime">2015-04-17T16:49:10.062+02:00</m:generated_time>
        <m:has_abbreviation xml:lang="en">HF</m:has_abbreviation>
        <m:has_related_eccairs_term rdf:resource="http://onto.fel.cvut.cz/ontologies/2014/ECCAIRS_Aviation_1.3.0.12/eccairs-descriptive-factors#category_21010300"/>
    </owl:Class>
    


    <!-- http://onto.fel.cvut.cz/ontologies/aviation-safety/Hand_pump,_main_system -->

    <owl:Class rdf:about="&m;Hand_pump,_main_system">
        <rdfs:label>Hand pump, main system</rdfs:label>
        <rdfs:subClassOf rdf:resource="&m;Hydraulic,_main_system_part"/>
        <m:generated_time rdf:datatype="&xsd;dateTime">2015-04-09T18:56:27.771+02:00</m:generated_time>
        <rdfs:comment xml:lang="en">(ATA Code:2914) and pump, main system: Any manually actuated pump for emergency system pressure. Typical parts are handle, lever and seals.</rdfs:comment>
        <m:has_related_eccairs_term rdf:resource="http://onto.fel.cvut.cz/ontologies/2014/ECCAIRS_Aviation_1.3.0.12/eccairs-descriptive-factors#category_11291400"/>
    </owl:Class>
    


    <!-- http://onto.fel.cvut.cz/ontologies/aviation-safety/Head_up_display_system -->

    <owl:Class rdf:about="&m;Head_up_display_system">
        <rdfs:label>Head up display system</rdfs:label>
        <rdfs:subClassOf rdf:resource="&m;Landing_and_taxi_aid"/>
        <m:generated_time rdf:datatype="&xsd;dateTime">2015-04-09T18:56:27.771+02:00</m:generated_time>
        <rdfs:comment xml:lang="en">(ATA Code:3435) Head up display system: The flight instrument system that allows the pilot of an aircraft to watch the flight instruments while looking ahead of the aircraft. Includes the display screen which allows information to be visually presented to the pilot while looking through the windscreen or at the control panel.</rdfs:comment>
        <m:has_related_eccairs_term rdf:resource="http://onto.fel.cvut.cz/ontologies/2014/ECCAIRS_Aviation_1.3.0.12/eccairs-descriptive-factors#category_11343500"/>
    </owl:Class>
    


    <!-- http://onto.fel.cvut.cz/ontologies/aviation-safety/Heating_system -->

    <owl:Class rdf:about="&m;Heating_system">
        <rdfs:label>Heating system</rdfs:label>
        <rdfs:subClassOf rdf:resource="&m;Air_conditioning_system_part"/>
        <m:generated_time rdf:datatype="&xsd;dateTime">2015-04-09T18:56:27.771+02:00</m:generated_time>
        <all2:has_ATA_code rdf:datatype="&xsd;integer">2140</all2:has_ATA_code>
        <rdfs:comment xml:lang="en">(ATA Code:2140) Heating system: The units and systems supplying heated air to the cockpit or cabin. Includes the heat source (heater), controlling aspects and temperature sensors/indicators. Typical parts are fuel pump, filter, plumbing, circuitry, relay, heat exchanger and igniter.</rdfs:comment>
        <m:has_related_eccairs_term rdf:resource="http://onto.fel.cvut.cz/ontologies/2014/ECCAIRS_Aviation_1.3.0.12/eccairs-descriptive-factors#category_11214000"/>
    </owl:Class>
    


    <!-- http://onto.fel.cvut.cz/ontologies/aviation-safety/Helicopter_Vibration_System_Wiring -->

    <owl:Class rdf:about="&m;Helicopter_Vibration_System_Wiring">
        <rdfs:subClassOf rdf:resource="&m;Helicopter_vibration_analysis_part"/>
    </owl:Class>
    


    <!-- http://onto.fel.cvut.cz/ontologies/aviation-safety/Helicopter_noise_analysis -->

    <owl:Class rdf:about="&m;Helicopter_noise_analysis">
        <rdfs:subClassOf rdf:resource="&m;Helicopter_vibration_analysis_part"/>
    </owl:Class>
    


    <!-- http://onto.fel.cvut.cz/ontologies/aviation-safety/Helicopter_vibration_analysis -->

    <owl:Class rdf:about="&m;Helicopter_vibration_analysis">
        <rdfs:subClassOf rdf:resource="&m;Helicopter_vibration_analysis_part"/>
    </owl:Class>
    


    <!-- http://onto.fel.cvut.cz/ontologies/aviation-safety/Helicopter_vibration_analysis_part -->

    <owl:Class rdf:about="&m;Helicopter_vibration_analysis_part">
        <rdfs:label>Helicopter vibration analysis part</rdfs:label>
        <rdfs:subClassOf rdf:resource="&m;Aircraft_part"/>
        <rdfs:subClassOf>
            <owl:Restriction>
                <owl:onProperty rdf:resource="http://onto.fel.cvut.cz/ontologies/ufo/is_part_of"/>
                <owl:someValuesFrom rdf:resource="&m;Helicopter_vibration_analysis"/>
            </owl:Restriction>
        </rdfs:subClassOf>
        <m:generated_time rdf:datatype="&xsd;dateTime">2015-04-12T02:45:54.351+02:00</m:generated_time>
        <m:has_related_eccairs_term rdf:resource="http://onto.fel.cvut.cz/ontologies/2014/ECCAIRS_Aviation_1.3.0.12/eccairs-descriptive-factors#category_11180000"/>
    </owl:Class>
    


    <!-- http://onto.fel.cvut.cz/ontologies/aviation-safety/High_frequency_communication_system -->

    <owl:Class rdf:about="&m;High_frequency_communication_system">
        <rdfs:label>High frequency communication system</rdfs:label>
        <rdfs:subClassOf rdf:resource="&m;speech_communication_system"/>
        <m:generated_time rdf:datatype="&xsd;dateTime">2015-04-09T18:56:27.771+02:00</m:generated_time>
        <rdfs:comment xml:lang="en">(ATA Code:2316) HF communication system: The system parts and circuitry including the receiver, transmitter and antenna used exclusively in the high frequency communications.</rdfs:comment>
        <m:has_related_eccairs_term rdf:resource="http://onto.fel.cvut.cz/ontologies/2014/ECCAIRS_Aviation_1.3.0.12/eccairs-descriptive-factors#category_11231600"/>
    </owl:Class>
    


    <!-- http://onto.fel.cvut.cz/ontologies/aviation-safety/High_speed_warning_system -->

    <owl:Class rdf:about="&m;High_speed_warning_system">
        <rdfs:label>High speed warning system</rdfs:label>
        <rdfs:subClassOf rdf:resource="&m;Flight_environment_data_system"/>
        <m:generated_time rdf:datatype="&xsd;dateTime">2015-04-09T18:56:27.771+02:00</m:generated_time>
        <rdfs:comment xml:lang="en">(ATA Code:3415) High speed warning system: The system components, including the computer, which sense, transmit and provide warning when operating air speed limits are exceeded. Typical parts are transducer, stall warning detector, switch, vane, horn, lamp, warning unit computer and module.</rdfs:comment>
        <m:has_related_eccairs_term rdf:resource="http://onto.fel.cvut.cz/ontologies/2014/ECCAIRS_Aviation_1.3.0.12/eccairs-descriptive-factors#category_11341500"/>
    </owl:Class>
    


    <!-- http://onto.fel.cvut.cz/ontologies/aviation-safety/Horizontal_stabilizer_actuator -->

    <owl:Class rdf:about="&m;Horizontal_stabilizer_actuator">
        <rdfs:label>Horizontal stabilizer actuator</rdfs:label>
        <rdfs:subClassOf rdf:resource="&m;Horizontal_stabilizer_control_system_part"/>
        <m:generated_time rdf:datatype="&xsd;dateTime">2015-04-09T18:56:27.771+02:00</m:generated_time>
        <rdfs:comment xml:lang="en">(ATA Code:2742) Horizontal stabilizer actuator: The component which actuates the horizontal stabilizer to finite angles of incidence to provide pitch trim. Includes both manual and power assist types. Typical parts are actuator, actuator bracket, clutch, motor and seals.</rdfs:comment>
        <m:has_related_eccairs_term rdf:resource="http://onto.fel.cvut.cz/ontologies/2014/ECCAIRS_Aviation_1.3.0.12/eccairs-descriptive-factors#category_11274200"/>
    </owl:Class>
    


    <!-- http://onto.fel.cvut.cz/ontologies/aviation-safety/Horizontal_stabilizer_attachment_fitting -->

    <owl:Class rdf:about="&m;Horizontal_stabilizer_attachment_fitting">
        <rdfs:label>Horizontal stabilizer attachment fitting</rdfs:label>
        <rdfs:subClassOf rdf:resource="&m;Attachment_fitting_(empennage_flight_control_surfaces)_part"/>
        <m:generated_time rdf:datatype="&xsd;dateTime">2015-04-09T18:56:27.771+02:00</m:generated_time>
        <rdfs:comment xml:lang="en">(ATA Code:5551) Horizontal stabilizer attachment fitting: The fittings on the horizontal stabilizer which are used to support equipment within the structure.</rdfs:comment>
        <m:has_related_eccairs_term rdf:resource="http://onto.fel.cvut.cz/ontologies/2014/ECCAIRS_Aviation_1.3.0.12/eccairs-descriptive-factors#category_11555100"/>
    </owl:Class>
    


    <!-- http://onto.fel.cvut.cz/ontologies/aviation-safety/Horizontal_stabilizer_control_system -->

    <owl:Class rdf:about="&m;Horizontal_stabilizer_control_system">
        <rdfs:label>Horizontal stabilizer control system</rdfs:label>
        <rdfs:subClassOf rdf:resource="&m;Flight_control_system_part"/>
        <m:generated_time rdf:datatype="&xsd;dateTime">2015-04-09T18:56:27.771+02:00</m:generated_time>
        <rdfs:comment xml:lang="en">(ATA Code:2740) Horizontal stabilizer control system: The system components and parts from the cockpit control to the stabilizer, except the actuator which controls position of the horizontal stabilizer for pitch trim (usually found on high performance turbine powered aircraft). Also for stabilator control systems on aircraft utilizing a single horizontal tail surface for both the stabilizer and elevator. Typical parts are cable, bellcrank, pulley, control valve and indicator.</rdfs:comment>
        <m:has_related_eccairs_term rdf:resource="http://onto.fel.cvut.cz/ontologies/2014/ECCAIRS_Aviation_1.3.0.12/eccairs-descriptive-factors#category_11274000"/>
    </owl:Class>
    


    <!-- http://onto.fel.cvut.cz/ontologies/aviation-safety/Horizontal_stabilizer_control_system_part -->

    <owl:Class rdf:about="&m;Horizontal_stabilizer_control_system_part">
        <rdfs:label>Horizontal stabilizer control system part</rdfs:label>
        <rdfs:subClassOf rdf:resource="&m;Flight_control_system_part"/>
        <rdfs:subClassOf>
            <owl:Restriction>
                <owl:onProperty rdf:resource="http://onto.fel.cvut.cz/ontologies/ufo/is_part_of"/>
                <owl:someValuesFrom rdf:resource="&m;Horizontal_stabilizer_control_system"/>
            </owl:Restriction>
        </rdfs:subClassOf>
        <m:generated_time rdf:datatype="&xsd;dateTime">2015-04-12T02:45:54.351+02:00</m:generated_time>
        <m:has_related_eccairs_term rdf:resource="http://onto.fel.cvut.cz/ontologies/2014/ECCAIRS_Aviation_1.3.0.12/eccairs-descriptive-factors#category_11274000"/>
    </owl:Class>
    


    <!-- http://onto.fel.cvut.cz/ontologies/aviation-safety/Horizontal_stabilizer_structure -->

    <owl:Class rdf:about="&m;Horizontal_stabilizer_structure">
        <rdfs:label>Horizontal stabilizer structure</rdfs:label>
        <rdfs:subClassOf rdf:resource="&m;Empennage_structure_part"/>
        <m:generated_time rdf:datatype="&xsd;dateTime">2015-04-09T18:56:27.771+02:00</m:generated_time>
        <rdfs:comment xml:lang="en">(ATA Code:5510) Horizontal stabilizer structure: The structural aspects of horizontal stabilizer and stabilators or canard. Includes fuselage and boom-to-surface attachment fittings. Does not include any actuating mechanism [Code 11274200].</rdfs:comment>
        <m:has_related_eccairs_term rdf:resource="http://onto.fel.cvut.cz/ontologies/2014/ECCAIRS_Aviation_1.3.0.12/eccairs-descriptive-factors#category_11551000"/>
    </owl:Class>
    


    <!-- http://onto.fel.cvut.cz/ontologies/aviation-safety/Horizontal_stabilizer_structure_part -->

    <owl:Class rdf:about="&m;Horizontal_stabilizer_structure_part">
        <rdfs:label>Horizontal stabilizer structure part</rdfs:label>
        <rdfs:subClassOf rdf:resource="&m;Empennage_structure_part"/>
        <rdfs:subClassOf>
            <owl:Restriction>
                <owl:onProperty rdf:resource="http://onto.fel.cvut.cz/ontologies/ufo/is_part_of"/>
                <owl:someValuesFrom rdf:resource="&m;Horizontal_stabilizer_structure"/>
            </owl:Restriction>
        </rdfs:subClassOf>
        <m:generated_time rdf:datatype="&xsd;dateTime">2015-04-12T02:45:54.351+02:00</m:generated_time>
        <m:has_related_eccairs_term rdf:resource="http://onto.fel.cvut.cz/ontologies/2014/ECCAIRS_Aviation_1.3.0.12/eccairs-descriptive-factors#category_11551000"/>
    </owl:Class>
    


    <!-- http://onto.fel.cvut.cz/ontologies/aviation-safety/Horizontal_stabilizer_tab_structure -->

    <owl:Class rdf:about="&m;Horizontal_stabilizer_tab_structure">
        <rdfs:label>Horizontal stabilizer tab structure</rdfs:label>
        <rdfs:subClassOf rdf:resource="&m;Horizontal_stabilizer_structure_part"/>
        <m:generated_time rdf:datatype="&xsd;dateTime">2015-04-09T18:56:27.771+02:00</m:generated_time>
        <rdfs:comment xml:lang="en">(ATA Code:5513) Horizontal stabilizer tab structure: The structure and attachment of the tab surface mounted on movable stabilizers and stabilators. Includes hinge brackets and bearings/bushings. Does not include the actuating mechanism [Code 11274000]. Typical parts are hinge, skin, rib and spar.</rdfs:comment>
        <m:has_related_eccairs_term rdf:resource="http://onto.fel.cvut.cz/ontologies/2014/ECCAIRS_Aviation_1.3.0.12/eccairs-descriptive-factors#category_11551300"/>
    </owl:Class>
    


    <!-- http://onto.fel.cvut.cz/ontologies/aviation-safety/Hoses_and_tubes -->

    <owl:Class rdf:about="&m;Hoses_and_tubes">
        <rdfs:label>Hoses and tubes</rdfs:label>
        <rdfs:subClassOf rdf:resource="&m;Miscellaneous_hardware_part"/>
        <m:generated_time rdf:datatype="&xsd;dateTime">2015-04-09T18:56:27.771+02:00</m:generated_time>
        <rdfs:comment xml:lang="en">(ATA Code:1410) Any aircraft or engine hose or that are not associated a specific aircraft system.</rdfs:comment>
        <m:has_related_eccairs_term rdf:resource="http://onto.fel.cvut.cz/ontologies/2014/ECCAIRS_Aviation_1.3.0.12/eccairs-descriptive-factors#category_11141000"/>
    </owl:Class>
    


    <!-- http://onto.fel.cvut.cz/ontologies/aviation-safety/Humidity_control_system -->

    <owl:Class rdf:about="&m;Humidity_control_system">
        <rdfs:subClassOf rdf:resource="&m;Air_conditioning_system_part"/>
    </owl:Class>
    


    <!-- http://onto.fel.cvut.cz/ontologies/aviation-safety/Hydraulic,_main_system -->

    <owl:Class rdf:about="&m;Hydraulic,_main_system">
        <rdfs:label>Hydraulic, main system</rdfs:label>
        <rdfs:subClassOf rdf:resource="&m;Hydraulic_power_system_part"/>
        <m:generated_time rdf:datatype="&xsd;dateTime">2015-04-09T18:56:27.771+02:00</m:generated_time>
        <rdfs:comment xml:lang="en">(ATA Code:2910) Hydraulic, main system: The portion of the system which is used to store and deliver hydraulic fluid to using systems. Includes all hydraulic systems other than those designated emergency or standby. Does not include the supply valves to the using systems. Typical parts are tanks, accumulators, valves, pumps, levers, cables, line, hose, relief, shutoff valves, check valves, wiring, switches and external connectors.</rdfs:comment>
        <m:has_related_eccairs_term rdf:resource="http://onto.fel.cvut.cz/ontologies/2014/ECCAIRS_Aviation_1.3.0.12/eccairs-descriptive-factors#category_11291000"/>
    </owl:Class>
    


    <!-- http://onto.fel.cvut.cz/ontologies/aviation-safety/Hydraulic,_main_system_part -->

    <owl:Class rdf:about="&m;Hydraulic,_main_system_part">
        <rdfs:label>Hydraulic, main system part</rdfs:label>
        <rdfs:subClassOf rdf:resource="&m;Hydraulic_power_system_part"/>
        <rdfs:subClassOf>
            <owl:Restriction>
                <owl:onProperty rdf:resource="http://onto.fel.cvut.cz/ontologies/ufo/is_part_of"/>
                <owl:someValuesFrom rdf:resource="&m;Hydraulic,_main_system"/>
            </owl:Restriction>
        </rdfs:subClassOf>
        <m:generated_time rdf:datatype="&xsd;dateTime">2015-04-12T02:45:54.351+02:00</m:generated_time>
        <m:has_related_eccairs_term rdf:resource="http://onto.fel.cvut.cz/ontologies/2014/ECCAIRS_Aviation_1.3.0.12/eccairs-descriptive-factors#category_11291000"/>
    </owl:Class>
    


    <!-- http://onto.fel.cvut.cz/ontologies/aviation-safety/Hydraulic_Power_System_Wiring -->

    <owl:Class rdf:about="&m;Hydraulic_Power_System_Wiring">
        <rdfs:label>Hydraulic Power System Wiring</rdfs:label>
        <rdfs:subClassOf rdf:resource="&m;Hydraulic_power_system_part"/>
        <m:generated_time rdf:datatype="&xsd;dateTime">2015-04-09T18:56:27.771+02:00</m:generated_time>
        <rdfs:comment xml:lang="en">(ATA Code:2997) Wiring specific to the Hydraulic Power System.</rdfs:comment>
        <m:has_related_eccairs_term rdf:resource="http://onto.fel.cvut.cz/ontologies/2014/ECCAIRS_Aviation_1.3.0.12/eccairs-descriptive-factors#category_11299700"/>
    </owl:Class>
    


    <!-- http://onto.fel.cvut.cz/ontologies/aviation-safety/Hydraulic_accumulator,_auxiliary -->

    <owl:Class rdf:about="&m;Hydraulic_accumulator,_auxiliary">
        <rdfs:label>Hydraulic accumulator, auxiliary</rdfs:label>
        <rdfs:subClassOf rdf:resource="&m;Hydraulic_auxiliary_system_part"/>
        <m:generated_time rdf:datatype="&xsd;dateTime">2015-04-09T18:56:27.771+02:00</m:generated_time>
        <rdfs:comment xml:lang="en">(ATA Code:2921) Hydraulic accumulator, auxiliary: The component which absorbs pressure surges to maintain a constant pressure in the auxiliary hydraulic system. Typical parts are accumulator, seal, end cap and air valves.</rdfs:comment>
        <m:has_related_eccairs_term rdf:resource="http://onto.fel.cvut.cz/ontologies/2014/ECCAIRS_Aviation_1.3.0.12/eccairs-descriptive-factors#category_11292100"/>
    </owl:Class>
    


    <!-- http://onto.fel.cvut.cz/ontologies/aviation-safety/Hydraulic_auxiliary_system -->

    <owl:Class rdf:about="&m;Hydraulic_auxiliary_system">
        <rdfs:label>Hydraulic auxiliary system</rdfs:label>
        <rdfs:subClassOf rdf:resource="&m;Hydraulic_power_system_part"/>
        <m:generated_time rdf:datatype="&xsd;dateTime">2015-04-09T18:56:27.771+02:00</m:generated_time>
        <rdfs:comment xml:lang="en">(ATA Code:2920) Hydraulic auxiliary system: The portion of the main hydraulic system which is classified as auxiliary, emergency or standby and which is used to supplement or take the place of the main hydraulic fluid to the using system. Does not include the supply valves to the using systems. Typical parts are tank, accumulator, valve, pump, lever, cables, switch, plumbing, wiring, external connectors and miscellaneous auxiliary system parts.</rdfs:comment>
        <m:has_related_eccairs_term rdf:resource="http://onto.fel.cvut.cz/ontologies/2014/ECCAIRS_Aviation_1.3.0.12/eccairs-descriptive-factors#category_11292000"/>
    </owl:Class>
    


    <!-- http://onto.fel.cvut.cz/ontologies/aviation-safety/Hydraulic_auxiliary_system_part -->

    <owl:Class rdf:about="&m;Hydraulic_auxiliary_system_part">
        <rdfs:label>Hydraulic auxiliary system part</rdfs:label>
        <rdfs:subClassOf rdf:resource="&m;Hydraulic_power_system_part"/>
        <rdfs:subClassOf>
            <owl:Restriction>
                <owl:onProperty rdf:resource="http://onto.fel.cvut.cz/ontologies/ufo/is_part_of"/>
                <owl:someValuesFrom rdf:resource="&m;Hydraulic_auxiliary_system"/>
            </owl:Restriction>
        </rdfs:subClassOf>
        <m:generated_time rdf:datatype="&xsd;dateTime">2015-04-12T02:45:54.351+02:00</m:generated_time>
        <m:has_related_eccairs_term rdf:resource="http://onto.fel.cvut.cz/ontologies/2014/ECCAIRS_Aviation_1.3.0.12/eccairs-descriptive-factors#category_11292000"/>
    </owl:Class>
    


    <!-- http://onto.fel.cvut.cz/ontologies/aviation-safety/Hydraulic_auxiliary_system_ram_air_turbine -->

    <owl:Class rdf:about="&m;Hydraulic_auxiliary_system_ram_air_turbine">
        <rdfs:label>Hydraulic auxiliary system ram air turbine</rdfs:label>
        <rdfs:subClassOf rdf:resource="&m;Hydraulic_auxiliary_system_part"/>
        <m:generated_time rdf:datatype="&xsd;dateTime">2015-04-09T18:56:27.771+02:00</m:generated_time>
        <rdfs:comment xml:lang="en">(ATA Code:2928) Hydraulic auxiliary system ram air turbine: The emergency air driven hydraulic pump which is lowered into the air stream in an emergency to generate pressure in the aircraft&apos;s hydraulic system.</rdfs:comment>
        <m:has_related_eccairs_term rdf:resource="http://onto.fel.cvut.cz/ontologies/2014/ECCAIRS_Aviation_1.3.0.12/eccairs-descriptive-factors#category_11292800"/>
    </owl:Class>
    


    <!-- http://onto.fel.cvut.cz/ontologies/aviation-safety/Hydraulic_compartment_doors -->

    <owl:Class rdf:about="&m;Hydraulic_compartment_doors">
        <rdfs:label>Hydraulic compartment doors</rdfs:label>
        <rdfs:subClassOf rdf:resource="&m;Service_doors_part"/>
        <m:generated_time rdf:datatype="&xsd;dateTime">2015-04-09T18:56:27.771+02:00</m:generated_time>
        <rdfs:comment xml:lang="en">(ATA Code:5243) Hydraulic compartment doors: The exterior doors used primarily to gain access for servicing the hydraulic compartment. Typical parts are hinges, structure and the latch mechanism.</rdfs:comment>
        <m:has_related_eccairs_term rdf:resource="http://onto.fel.cvut.cz/ontologies/2014/ECCAIRS_Aviation_1.3.0.12/eccairs-descriptive-factors#category_11524300"/>
    </owl:Class>
    


    <!-- http://onto.fel.cvut.cz/ontologies/aviation-safety/Hydraulic_filter,_auxiliary -->

    <owl:Class rdf:about="&m;Hydraulic_filter,_auxiliary">
        <rdfs:label>Hydraulic filter, auxiliary</rdfs:label>
        <rdfs:subClassOf rdf:resource="&m;Hydraulic_auxiliary_system_part"/>
        <m:generated_time rdf:datatype="&xsd;dateTime">2015-04-09T18:56:27.771+02:00</m:generated_time>
        <rdfs:comment xml:lang="en">(ATA Code:2922) Hydraulic filter, auxiliary: The component which filters sediment from the hydraulic fluid in the auxiliary system. Typical parts are seal, gasket, housing, element and packings.</rdfs:comment>
        <m:has_related_eccairs_term rdf:resource="http://onto.fel.cvut.cz/ontologies/2014/ECCAIRS_Aviation_1.3.0.12/eccairs-descriptive-factors#category_11292200"/>
    </owl:Class>
    


    <!-- http://onto.fel.cvut.cz/ontologies/aviation-safety/Hydraulic_hand_pump,_auxiliary -->

    <owl:Class rdf:about="&m;Hydraulic_hand_pump,_auxiliary">
        <rdfs:label>Hydraulic hand pump, auxiliary</rdfs:label>
        <rdfs:subClassOf rdf:resource="&m;Hydraulic_auxiliary_system_part"/>
        <m:generated_time rdf:datatype="&xsd;dateTime">2015-04-09T18:56:27.771+02:00</m:generated_time>
        <rdfs:comment xml:lang="en">(ATA Code:2924) Hydraulic hand pump, auxiliary: The manually actuated pump for emergency system pressure. Typical parts are handle, lever and seals.</rdfs:comment>
        <m:has_related_eccairs_term rdf:resource="http://onto.fel.cvut.cz/ontologies/2014/ECCAIRS_Aviation_1.3.0.12/eccairs-descriptive-factors#category_11292400"/>
    </owl:Class>
    


    <!-- http://onto.fel.cvut.cz/ontologies/aviation-safety/Hydraulic_main_system_filter -->

    <owl:Class rdf:about="&m;Hydraulic_main_system_filter">
        <rdfs:label>Hydraulic main system filter</rdfs:label>
        <rdfs:subClassOf rdf:resource="&m;Hydraulic,_main_system_part"/>
        <m:generated_time rdf:datatype="&xsd;dateTime">2015-04-09T18:56:27.771+02:00</m:generated_time>
        <rdfs:comment xml:lang="en">Hydraulic main system filter: The component which filters sediment from the hydraulic fluid in the main system. Typical parts are seal, gasket, housing, element and packing.</rdfs:comment>
        <m:has_related_eccairs_term rdf:resource="http://onto.fel.cvut.cz/ontologies/2014/ECCAIRS_Aviation_1.3.0.12/eccairs-descriptive-factors#category_11291002"/>
    </owl:Class>
    


    <!-- http://onto.fel.cvut.cz/ontologies/aviation-safety/Hydraulic_power_accumulator,_main_system_ -->

    <owl:Class rdf:about="&m;Hydraulic_power_accumulator,_main_system_">
        <rdfs:label>Hydraulic power accumulator, main system </rdfs:label>
        <rdfs:subClassOf rdf:resource="&m;Hydraulic,_main_system_part"/>
        <m:generated_time rdf:datatype="&xsd;dateTime">2015-04-09T18:56:27.771+02:00</m:generated_time>
        <rdfs:comment xml:lang="en">(ATA Code:2911) Hydraulic power accumulator, main system: The component that absorbs pressure surges to maintain a constant pressure in the system. Typical parts are accumulator, seal, end cap and air valve.</rdfs:comment>
        <m:has_related_eccairs_term rdf:resource="http://onto.fel.cvut.cz/ontologies/2014/ECCAIRS_Aviation_1.3.0.12/eccairs-descriptive-factors#category_11291100"/>
    </owl:Class>
    


    <!-- http://onto.fel.cvut.cz/ontologies/aviation-safety/Hydraulic_power_system -->

    <owl:Class rdf:about="&m;Hydraulic_power_system">
        <rdfs:label>Hydraulic power system</rdfs:label>
        <rdfs:subClassOf rdf:resource="&m;Aircraft_part"/>
        <m:generated_time rdf:datatype="&xsd;dateTime">2015-04-09T18:56:27.771+02:00</m:generated_time>
        <rdfs:comment xml:lang="en">(ATA Code:2900) Hydraulic power system: The units and components which furnish hydraulic fluid under pressure to a common point (manifold) for re-distribution to other defined systems.</rdfs:comment>
        <m:has_related_eccairs_term rdf:resource="http://onto.fel.cvut.cz/ontologies/2014/ECCAIRS_Aviation_1.3.0.12/eccairs-descriptive-factors#category_11290000"/>
    </owl:Class>
    


    <!-- http://onto.fel.cvut.cz/ontologies/aviation-safety/Hydraulic_power_system_part -->

    <owl:Class rdf:about="&m;Hydraulic_power_system_part">
        <rdfs:label>Hydraulic power system part</rdfs:label>
        <rdfs:subClassOf rdf:resource="&m;Aircraft_part"/>
        <rdfs:subClassOf>
            <owl:Restriction>
                <owl:onProperty rdf:resource="http://onto.fel.cvut.cz/ontologies/ufo/is_part_of"/>
                <owl:someValuesFrom rdf:resource="&m;Hydraulic_power_system"/>
            </owl:Restriction>
        </rdfs:subClassOf>
        <m:generated_time rdf:datatype="&xsd;dateTime">2015-04-12T02:45:54.351+02:00</m:generated_time>
        <m:has_related_eccairs_term rdf:resource="http://onto.fel.cvut.cz/ontologies/2014/ECCAIRS_Aviation_1.3.0.12/eccairs-descriptive-factors#category_11290000"/>
    </owl:Class>
    


    <!-- http://onto.fel.cvut.cz/ontologies/aviation-safety/Hydraulic_pressure_indicator -->

    <owl:Class rdf:about="&m;Hydraulic_pressure_indicator">
        <rdfs:label>Hydraulic pressure indicator</rdfs:label>
        <rdfs:subClassOf rdf:resource="&m;Hydraulic_system_indicating_system_part"/>
        <m:generated_time rdf:datatype="&xsd;dateTime">2015-04-09T18:56:27.771+02:00</m:generated_time>
        <rdfs:comment xml:lang="en">(ATA Code:2931) Hydraulic pressure indicator: The instrument and associated low pressure warning system which registers system pressure. Typical parts are indicator, warning lamp and bulb.</rdfs:comment>
        <m:has_related_eccairs_term rdf:resource="http://onto.fel.cvut.cz/ontologies/2014/ECCAIRS_Aviation_1.3.0.12/eccairs-descriptive-factors#category_11293100"/>
    </owl:Class>
    


    <!-- http://onto.fel.cvut.cz/ontologies/aviation-safety/Hydraulic_pressure_regulator,_auxiliary -->

    <owl:Class rdf:about="&m;Hydraulic_pressure_regulator,_auxiliary">
        <rdfs:label>Hydraulic pressure regulator, auxiliary</rdfs:label>
        <rdfs:subClassOf rdf:resource="&m;Hydraulic_auxiliary_system_part"/>
        <m:generated_time rdf:datatype="&xsd;dateTime">2015-04-09T18:56:27.771+02:00</m:generated_time>
        <rdfs:comment xml:lang="en">(ATA Code:2927) Hydraulic pressure regulator, auxiliary: The unit which maintains a preset operating system pressure to the using auxiliary hydraulic system. Typical parts are regulator, seal and case.</rdfs:comment>
        <m:has_related_eccairs_term rdf:resource="http://onto.fel.cvut.cz/ontologies/2014/ECCAIRS_Aviation_1.3.0.12/eccairs-descriptive-factors#category_11292700"/>
    </owl:Class>
    


    <!-- http://onto.fel.cvut.cz/ontologies/aviation-safety/Hydraulic_pressure_regulator_-_system -->

    <owl:Class rdf:about="&m;Hydraulic_pressure_regulator_-_system">
        <rdfs:label>Hydraulic pressure regulator - system</rdfs:label>
        <rdfs:subClassOf rdf:resource="&m;Hydraulic,_main_system_part"/>
        <m:generated_time rdf:datatype="&xsd;dateTime">2015-04-09T18:56:27.771+02:00</m:generated_time>
        <rdfs:comment xml:lang="en">(ATA Code:2917) Hydraulic pressure regulator - system: The unit which maintains a preset operating system pressure to the using systems. Typical parts are regulator, seals and the case.</rdfs:comment>
        <m:has_related_eccairs_term rdf:resource="http://onto.fel.cvut.cz/ontologies/2014/ECCAIRS_Aviation_1.3.0.12/eccairs-descriptive-factors#category_11291700"/>
    </owl:Class>
    


    <!-- http://onto.fel.cvut.cz/ontologies/aviation-safety/Hydraulic_pressure_relief,_auxiliary -->

    <owl:Class rdf:about="&m;Hydraulic_pressure_relief,_auxiliary">
        <rdfs:label>Hydraulic pressure relief, auxiliary</rdfs:label>
        <rdfs:subClassOf rdf:resource="&m;Hydraulic_auxiliary_system_part"/>
        <m:generated_time rdf:datatype="&xsd;dateTime">2015-04-09T18:56:27.771+02:00</m:generated_time>
        <rdfs:comment xml:lang="en">(ATA Code:2925) Hydraulic pressure relief, auxiliary: The unit which prevents auxiliary system pressure from exceeding a maximum specified pressure. Typical parts are seal, spring, housing and relief valves.</rdfs:comment>
        <m:has_related_eccairs_term rdf:resource="http://onto.fel.cvut.cz/ontologies/2014/ECCAIRS_Aviation_1.3.0.12/eccairs-descriptive-factors#category_11292500"/>
    </owl:Class>
    


    <!-- http://onto.fel.cvut.cz/ontologies/aviation-safety/Hydraulic_pressure_relief_valve-main_system -->

    <owl:Class rdf:about="&m;Hydraulic_pressure_relief_valve-main_system">
        <rdfs:label>Hydraulic pressure relief valve-main system</rdfs:label>
        <rdfs:subClassOf rdf:resource="&m;Hydraulic,_main_system_part"/>
        <m:generated_time rdf:datatype="&xsd;dateTime">2015-04-09T18:56:27.771+02:00</m:generated_time>
        <rdfs:comment xml:lang="en">(ATA Code:2915) Hydraulic pressure relief valve-main system: The unit which relieves main hydraulic system pressure to prevent it exceeding a preset pressure. Typical parts are seal, spring, housing and relief valve.</rdfs:comment>
        <m:has_related_eccairs_term rdf:resource="http://onto.fel.cvut.cz/ontologies/2014/ECCAIRS_Aviation_1.3.0.12/eccairs-descriptive-factors#category_11291500"/>
    </owl:Class>
    


    <!-- http://onto.fel.cvut.cz/ontologies/aviation-safety/Hydraulic_pressure_sensor -->

    <owl:Class rdf:about="&m;Hydraulic_pressure_sensor">
        <rdfs:label>Hydraulic pressure sensor</rdfs:label>
        <rdfs:subClassOf rdf:resource="&m;Hydraulic_system_indicating_system_part"/>
        <m:generated_time rdf:datatype="&xsd;dateTime">2015-04-09T18:56:27.771+02:00</m:generated_time>
        <rdfs:comment xml:lang="en">(ATA Code:2932) Hydraulic pressure sensor: The components which sense system pressure and transmit a signal to the cockpit indicator or low pressure warning lamp. Typical parts are transmitter, pressure switch and sensor.</rdfs:comment>
        <m:has_related_eccairs_term rdf:resource="http://onto.fel.cvut.cz/ontologies/2014/ECCAIRS_Aviation_1.3.0.12/eccairs-descriptive-factors#category_11293200"/>
    </owl:Class>
    


    <!-- http://onto.fel.cvut.cz/ontologies/aviation-safety/Hydraulic_pump,_auxiliary -->

    <owl:Class rdf:about="&m;Hydraulic_pump,_auxiliary">
        <rdfs:label>Hydraulic pump, auxiliary</rdfs:label>
        <rdfs:subClassOf rdf:resource="&m;Hydraulic_auxiliary_system_part"/>
        <m:generated_time rdf:datatype="&xsd;dateTime">2015-04-09T18:56:27.771+02:00</m:generated_time>
        <rdfs:comment xml:lang="en">(ATA Code:2923) Hydraulic pump, auxiliary: The component which provides hydraulic fluid pressure to the using auxiliary system. Typical parts are pump, motor, shaft, brushes, case, seal and switches.</rdfs:comment>
        <m:has_related_eccairs_term rdf:resource="http://onto.fel.cvut.cz/ontologies/2014/ECCAIRS_Aviation_1.3.0.12/eccairs-descriptive-factors#category_11292300"/>
    </owl:Class>
    


    <!-- http://onto.fel.cvut.cz/ontologies/aviation-safety/Hydraulic_reservoir,_auxiliary -->

    <owl:Class rdf:about="&m;Hydraulic_reservoir,_auxiliary">
        <rdfs:label>Hydraulic reservoir, auxiliary</rdfs:label>
        <rdfs:subClassOf rdf:resource="&m;Hydraulic_auxiliary_system_part"/>
        <m:generated_time rdf:datatype="&xsd;dateTime">2015-04-09T18:56:27.771+02:00</m:generated_time>
        <rdfs:comment xml:lang="en">(ATA Code:2926) Hydraulic reservoir, auxiliary: The unit which stores hydraulic fluid for the auxiliary system. Typical parts are reservoir, filler cap, filler neck and sight gauge.</rdfs:comment>
        <m:has_related_eccairs_term rdf:resource="http://onto.fel.cvut.cz/ontologies/2014/ECCAIRS_Aviation_1.3.0.12/eccairs-descriptive-factors#category_11292600"/>
    </owl:Class>
    


    <!-- http://onto.fel.cvut.cz/ontologies/aviation-safety/Hydraulic_reservoir-main -->

    <owl:Class rdf:about="&m;Hydraulic_reservoir-main">
        <rdfs:label>Hydraulic reservoir-main</rdfs:label>
        <rdfs:subClassOf rdf:resource="&m;Hydraulic,_main_system_part"/>
        <m:generated_time rdf:datatype="&xsd;dateTime">2015-04-09T18:56:27.771+02:00</m:generated_time>
        <rdfs:comment xml:lang="en">(ATA Code:2916) Hydraulic reservoir-main: The component which stores hydraulic fluid. Typical parts are reservoir, filler cap, filler neck, sight gauge and seal.</rdfs:comment>
        <m:has_related_eccairs_term rdf:resource="http://onto.fel.cvut.cz/ontologies/2014/ECCAIRS_Aviation_1.3.0.12/eccairs-descriptive-factors#category_11291600"/>
    </owl:Class>
    


    <!-- http://onto.fel.cvut.cz/ontologies/aviation-safety/Hydraulic_system_-_quantity_indicator -->

    <owl:Class rdf:about="&m;Hydraulic_system_-_quantity_indicator">
        <rdfs:label>Hydraulic system - quantity indicator</rdfs:label>
        <rdfs:subClassOf rdf:resource="&m;Hydraulic_system_indicating_system_part"/>
        <m:generated_time rdf:datatype="&xsd;dateTime">2015-04-09T18:56:27.771+02:00</m:generated_time>
        <rdfs:comment xml:lang="en">(ATA Code:2933) Hydraulic system - quantity indicator: The instrument and associated low level warning system which registers reservoir fluid quantity. Typical parts are indicator, lamp, bulb and sight gauge.</rdfs:comment>
        <m:has_related_eccairs_term rdf:resource="http://onto.fel.cvut.cz/ontologies/2014/ECCAIRS_Aviation_1.3.0.12/eccairs-descriptive-factors#category_11293300"/>
    </owl:Class>
    


    <!-- http://onto.fel.cvut.cz/ontologies/aviation-safety/Hydraulic_system_-_quantity_sensor -->

    <owl:Class rdf:about="&m;Hydraulic_system_-_quantity_sensor">
        <rdfs:label>Hydraulic system - quantity sensor</rdfs:label>
        <rdfs:subClassOf rdf:resource="&m;Hydraulic_system_indicating_system_part"/>
        <m:generated_time rdf:datatype="&xsd;dateTime">2015-04-09T18:56:27.771+02:00</m:generated_time>
        <rdfs:comment xml:lang="en">(ATA Code:2934) Hydraulic system - quantity sensor: The components which sense the fluid level and low level warning and transmit a signal to the quantity indicator. Typical parts are transmitter, sensor and float switch.</rdfs:comment>
        <m:has_related_eccairs_term rdf:resource="http://onto.fel.cvut.cz/ontologies/2014/ECCAIRS_Aviation_1.3.0.12/eccairs-descriptive-factors#category_11293400"/>
    </owl:Class>
    


    <!-- http://onto.fel.cvut.cz/ontologies/aviation-safety/Hydraulic_system_indicating_system -->

    <owl:Class rdf:about="&m;Hydraulic_system_indicating_system">
        <rdfs:label>Hydraulic system indicating system</rdfs:label>
        <rdfs:subClassOf rdf:resource="&m;Hydraulic_power_system_part"/>
        <m:generated_time rdf:datatype="&xsd;dateTime">2015-04-09T18:56:27.771+02:00</m:generated_time>
        <rdfs:comment xml:lang="en">(ATA Code:2930) Hydraulic system indicating system: The hydraulic pressure and quantity indicating system parts other than the indicator or sensor or for parts common to both pressure and quantity systems.</rdfs:comment>
        <m:has_related_eccairs_term rdf:resource="http://onto.fel.cvut.cz/ontologies/2014/ECCAIRS_Aviation_1.3.0.12/eccairs-descriptive-factors#category_11293000"/>
    </owl:Class>
    


    <!-- http://onto.fel.cvut.cz/ontologies/aviation-safety/Hydraulic_system_indicating_system_part -->

    <owl:Class rdf:about="&m;Hydraulic_system_indicating_system_part">
        <rdfs:label>Hydraulic system indicating system part</rdfs:label>
        <rdfs:subClassOf rdf:resource="&m;Hydraulic_power_system_part"/>
        <rdfs:subClassOf>
            <owl:Restriction>
                <owl:onProperty rdf:resource="http://onto.fel.cvut.cz/ontologies/ufo/is_part_of"/>
                <owl:someValuesFrom rdf:resource="&m;Hydraulic_system_indicating_system"/>
            </owl:Restriction>
        </rdfs:subClassOf>
        <m:generated_time rdf:datatype="&xsd;dateTime">2015-04-12T02:45:54.351+02:00</m:generated_time>
        <m:has_related_eccairs_term rdf:resource="http://onto.fel.cvut.cz/ontologies/2014/ECCAIRS_Aviation_1.3.0.12/eccairs-descriptive-factors#category_11293000"/>
    </owl:Class>
    


    <!-- http://onto.fel.cvut.cz/ontologies/aviation-safety/ILS_aircraft_equipment -->

    <owl:Class rdf:about="&m;ILS_aircraft_equipment">
        <rdfs:label>ILS aircraft equipment</rdfs:label>
        <rdfs:subClassOf>
            <owl:Class>
                <owl:intersectionOf rdf:parseType="Collection">
                    <rdf:Description rdf:about="&m;Landing_and_taxi_aid"/>
                    <owl:Restriction>
                        <owl:onProperty rdf:resource="&m;communicates_with"/>
                        <owl:someValuesFrom rdf:resource="&m;instrument_landing_system_ground_system"/>
                    </owl:Restriction>
                </owl:intersectionOf>
            </owl:Class>
        </rdfs:subClassOf>
    </owl:Class>
    


    <!-- http://onto.fel.cvut.cz/ontologies/aviation-safety/I_Buss_cable -->

    <owl:Class rdf:about="&m;I_Buss_cable">
        <rdfs:subClassOf rdf:resource="&m;Trailing_edge_flap_control_system_part"/>
    </owl:Class>
    


    <!-- http://onto.fel.cvut.cz/ontologies/aviation-safety/I_Bypass_valve -->

    <owl:Class rdf:about="&m;I_Bypass_valve">
        <rdfs:subClassOf rdf:resource="&m;Trailing_edge_flap_control_system_part"/>
    </owl:Class>
    


    <!-- http://onto.fel.cvut.cz/ontologies/aviation-safety/I_Cable -->

    <owl:Class rdf:about="&m;I_Cable">
        <rdfs:subClassOf rdf:resource="&m;Trailing_edge_flap_control_system_part"/>
    </owl:Class>
    


    <!-- http://onto.fel.cvut.cz/ontologies/aviation-safety/I_Control_system_switch -->

    <owl:Class rdf:about="&m;I_Control_system_switch">
        <rdfs:subClassOf rdf:resource="&m;Trailing_edge_flap_control_system_part"/>
    </owl:Class>
    


    <!-- http://onto.fel.cvut.cz/ontologies/aviation-safety/I_Control_valve -->

    <owl:Class rdf:about="&m;I_Control_valve">
        <rdfs:subClassOf rdf:resource="&m;Trailing_edge_flap_control_system_part"/>
    </owl:Class>
    


    <!-- http://onto.fel.cvut.cz/ontologies/aviation-safety/I_Flow_limiter -->

    <owl:Class rdf:about="&m;I_Flow_limiter">
        <rdfs:subClassOf rdf:resource="&m;Trailing_edge_flap_control_system_part"/>
    </owl:Class>
    


    <!-- http://onto.fel.cvut.cz/ontologies/aviation-safety/I_Jackscrew -->

    <owl:Class rdf:about="&m;I_Jackscrew">
        <rdfs:subClassOf rdf:resource="&m;Trailing_edge_flap_control_system_part"/>
    </owl:Class>
    


    <!-- http://onto.fel.cvut.cz/ontologies/aviation-safety/I_Limit_switch -->

    <owl:Class rdf:about="&m;I_Limit_switch">
        <rdfs:subClassOf rdf:resource="&m;Trailing_edge_flap_control_system_part"/>
    </owl:Class>
    


    <!-- http://onto.fel.cvut.cz/ontologies/aviation-safety/I_Return_spring -->

    <owl:Class rdf:about="&m;I_Return_spring">
        <rdfs:subClassOf rdf:resource="&m;Trailing_edge_flap_control_system_part"/>
    </owl:Class>
    


    <!-- http://onto.fel.cvut.cz/ontologies/aviation-safety/I_Torque_tube -->

    <owl:Class rdf:about="&m;I_Torque_tube">
        <rdfs:subClassOf rdf:resource="&m;Trailing_edge_flap_control_system_part"/>
    </owl:Class>
    


    <!-- http://onto.fel.cvut.cz/ontologies/aviation-safety/I_Transmission -->

    <owl:Class rdf:about="&m;I_Transmission">
        <rdfs:subClassOf rdf:resource="&m;Trailing_edge_flap_control_system_part"/>
    </owl:Class>
    


    <!-- http://onto.fel.cvut.cz/ontologies/aviation-safety/I_not(actuator) -->

    <owl:Class rdf:about="&m;I_not(actuator)">
        <rdfs:subClassOf rdf:resource="&m;Trailing_edge_flap_control_system_part"/>
    </owl:Class>
    


    <!-- http://onto.fel.cvut.cz/ontologies/aviation-safety/I_not(position_indicator_which_controls_position_and_movement_of_wing_trailing_edge_flaps) -->

    <owl:Class rdf:about="&m;I_not(position_indicator_which_controls_position_and_movement_of_wing_trailing_edge_flaps)">
        <rdfs:subClassOf rdf:resource="&m;Trailing_edge_flap_control_system_part"/>
    </owl:Class>
    


    <!-- http://onto.fel.cvut.cz/ontologies/aviation-safety/Ice-Rain_Protection_System_Wiring -->

    <owl:Class rdf:about="&m;Ice-Rain_Protection_System_Wiring">
        <rdfs:label>Ice/Rain Protection System Wiring</rdfs:label>
        <rdfs:subClassOf rdf:resource="&m;Ice-rain_protection_systems"/>
        <m:generated_time rdf:datatype="&xsd;dateTime">2015-04-09T18:56:27.771+02:00</m:generated_time>
        <rdfs:comment xml:lang="en">(ATA Code:3097) Wiring specific to the Ice/Rain Protection System</rdfs:comment>
        <m:has_related_eccairs_term rdf:resource="http://onto.fel.cvut.cz/ontologies/2014/ECCAIRS_Aviation_1.3.0.12/eccairs-descriptive-factors#category_11309700"/>
    </owl:Class>
    


    <!-- http://onto.fel.cvut.cz/ontologies/aviation-safety/Ice-rain_protection_system_indication -->

    <owl:Class rdf:about="&m;Ice-rain_protection_system_indication">
        <rdfs:label>Ice/rain protection system indication</rdfs:label>
        <rdfs:subClassOf rdf:resource="&m;Ice-rain_protection_systems"/>
        <m:generated_time rdf:datatype="&xsd;dateTime">2015-04-09T18:56:27.771+02:00</m:generated_time>
        <rdfs:comment xml:lang="en">(ATA Code:3090) Ice/rain protection system indication: The system which is used to detect and indicate the presence of rain or the formation of ice. Typical parts are panels and detectors.</rdfs:comment>
        <m:has_related_eccairs_term rdf:resource="http://onto.fel.cvut.cz/ontologies/2014/ECCAIRS_Aviation_1.3.0.12/eccairs-descriptive-factors#category_11309000"/>
    </owl:Class>
    


    <!-- http://onto.fel.cvut.cz/ontologies/aviation-safety/Ice-rain_protection_systems -->

    <owl:Class rdf:about="&m;Ice-rain_protection_systems">
        <rdfs:label xml:lang="en">Ice/rain protection system</rdfs:label>
        <rdfs:subClassOf rdf:resource="&m;Aircraft_part"/>
        <rdfs:subClassOf>
            <owl:Restriction>
                <owl:onProperty rdf:resource="http://onto.fel.cvut.cz/ontologies/ufo/is_part_of"/>
                <owl:someValuesFrom rdf:resource="&m;Ice-rain_protection_systems"/>
            </owl:Restriction>
        </rdfs:subClassOf>
        <m:generated_time rdf:datatype="&xsd;dateTime">2015-04-09T18:56:27.771+02:00</m:generated_time>
        <m:generated_time rdf:datatype="&xsd;dateTime">2015-04-12T02:45:54.351+02:00</m:generated_time>
        <rdfs:comment xml:lang="en">(ATA Code:3000) Ice/rain protection systems: Those units and components which provide a means of preventing or disposing of formation of ice and rain on various parts of the aircraft other than turbine power plants. Includes alcohol pump, valves, tanks, propeller/rotor anti-icing system, wing heaters, water line heaters, pitot heaters, scoop heaters, windshield wipers and the electrical and heated air portion of windshield ice control. Does not include the basic windshield panel.</rdfs:comment>
        <m:has_related_eccairs_term rdf:resource="http://onto.fel.cvut.cz/ontologies/2014/ECCAIRS_Aviation_1.3.0.12/eccairs-descriptive-factors#category_11300000"/>
    </owl:Class>
    


    <!-- http://onto.fel.cvut.cz/ontologies/aviation-safety/Ice_detection_system -->

    <owl:Class rdf:about="&m;Ice_detection_system">
        <rdfs:subClassOf rdf:resource="&m;Ice-rain_protection_systems"/>
    </owl:Class>
    


    <!-- http://onto.fel.cvut.cz/ontologies/aviation-safety/Ignition_harness -->

    <owl:Class rdf:about="&m;Ignition_harness">
        <rdfs:label>Ignition harness</rdfs:label>
        <rdfs:subClassOf rdf:resource="&m;Ignition_system_part"/>
        <m:generated_time rdf:datatype="&xsd;dateTime">2015-04-09T18:56:27.771+02:00</m:generated_time>
        <rdfs:comment xml:lang="en">(ATA Code:7420) Ignition harness: The high tension insulated wiring from the magneto to the spark plug which provides a spark for combustion in reciprocating engines. For turbine engine, the high tension leads to burner can igniters used for starting. Typical parts are lead, shielding, sleeve, ignition cable, terminal and ferrule.</rdfs:comment>
        <m:has_related_eccairs_term rdf:resource="http://onto.fel.cvut.cz/ontologies/2014/ECCAIRS_Aviation_1.3.0.12/eccairs-descriptive-factors#category_11742000"/>
    </owl:Class>
    


    <!-- http://onto.fel.cvut.cz/ontologies/aviation-safety/Ignition_harness_part -->

    <owl:Class rdf:about="&m;Ignition_harness_part">
        <rdfs:label>Ignition harness part</rdfs:label>
        <rdfs:subClassOf rdf:resource="&m;Ignition_system_part"/>
        <rdfs:subClassOf>
            <owl:Restriction>
                <owl:onProperty rdf:resource="http://onto.fel.cvut.cz/ontologies/ufo/is_part_of"/>
                <owl:someValuesFrom rdf:resource="&m;Ignition_harness"/>
            </owl:Restriction>
        </rdfs:subClassOf>
        <m:generated_time rdf:datatype="&xsd;dateTime">2015-04-12T02:45:54.351+02:00</m:generated_time>
        <m:has_related_eccairs_term rdf:resource="http://onto.fel.cvut.cz/ontologies/2014/ECCAIRS_Aviation_1.3.0.12/eccairs-descriptive-factors#category_11742000"/>
    </owl:Class>
    


    <!-- http://onto.fel.cvut.cz/ontologies/aviation-safety/Ignition_indication -->

    <owl:Class rdf:about="&m;Ignition_indication">
        <rdfs:label>Ignition indication</rdfs:label>
        <rdfs:subClassOf rdf:resource="&m;Ignition_system_part"/>
        <m:generated_time rdf:datatype="&xsd;dateTime">2015-04-09T18:56:27.771+02:00</m:generated_time>
        <rdfs:comment xml:lang="en">(ATA Code:7440) Ignition indication</rdfs:comment>
        <m:has_related_eccairs_term rdf:resource="http://onto.fel.cvut.cz/ontologies/2014/ECCAIRS_Aviation_1.3.0.12/eccairs-descriptive-factors#category_11744000"/>
    </owl:Class>
    


    <!-- http://onto.fel.cvut.cz/ontologies/aviation-safety/Ignition_power_supply -->

    <owl:Class rdf:about="&m;Ignition_power_supply">
        <rdfs:label>Ignition power supply</rdfs:label>
        <rdfs:subClassOf rdf:resource="&m;Ignition_system_part"/>
        <m:generated_time rdf:datatype="&xsd;dateTime">2015-04-09T18:56:27.771+02:00</m:generated_time>
        <rdfs:comment xml:lang="en">(ATA Code:7410) Ignition power supply: The units and components which generate, control, furnish or distribute an electrical current to ignite the fuel air mixture in cylinders of reciprocating engines or in the combustion chambers or thrust augmenters of turbine engines.</rdfs:comment>
        <m:has_related_eccairs_term rdf:resource="http://onto.fel.cvut.cz/ontologies/2014/ECCAIRS_Aviation_1.3.0.12/eccairs-descriptive-factors#category_11741000"/>
    </owl:Class>
    


    <!-- http://onto.fel.cvut.cz/ontologies/aviation-safety/Ignition_power_supply_part -->

    <owl:Class rdf:about="&m;Ignition_power_supply_part">
        <rdfs:label>Ignition power supply part</rdfs:label>
        <rdfs:subClassOf rdf:resource="&m;Ignition_system_part"/>
        <rdfs:subClassOf>
            <owl:Restriction>
                <owl:onProperty rdf:resource="http://onto.fel.cvut.cz/ontologies/ufo/is_part_of"/>
                <owl:someValuesFrom rdf:resource="&m;Ignition_power_supply"/>
            </owl:Restriction>
        </rdfs:subClassOf>
        <m:generated_time rdf:datatype="&xsd;dateTime">2015-04-12T02:45:54.351+02:00</m:generated_time>
        <m:has_related_eccairs_term rdf:resource="http://onto.fel.cvut.cz/ontologies/2014/ECCAIRS_Aviation_1.3.0.12/eccairs-descriptive-factors#category_11741000"/>
    </owl:Class>
    


    <!-- http://onto.fel.cvut.cz/ontologies/aviation-safety/Ignition_switching -->

    <owl:Class rdf:about="&m;Ignition_switching">
        <rdfs:label>Ignition switching</rdfs:label>
        <rdfs:subClassOf rdf:resource="&m;Ignition_system_part"/>
        <m:generated_time rdf:datatype="&xsd;dateTime">2015-04-09T18:56:27.771+02:00</m:generated_time>
        <rdfs:comment xml:lang="en">(ATA Code:7430) Ignition switching: The unit which provides a means of rendering the ignition power supply (magneto) inoperative. Also used to direct electrical current to the engine starter motor. Typical parts are start button, switch, back plate and contacts.</rdfs:comment>
        <m:has_related_eccairs_term rdf:resource="http://onto.fel.cvut.cz/ontologies/2014/ECCAIRS_Aviation_1.3.0.12/eccairs-descriptive-factors#category_11743000"/>
    </owl:Class>
    


    <!-- http://onto.fel.cvut.cz/ontologies/aviation-safety/Ignition_system -->

    <owl:Class rdf:about="&m;Ignition_system">
        <rdfs:label>Ignition system</rdfs:label>
        <rdfs:subClassOf rdf:resource="&m;Aircraft_part"/>
        <m:generated_time rdf:datatype="&xsd;dateTime">2015-04-09T18:56:27.771+02:00</m:generated_time>
        <rdfs:comment xml:lang="en">(ATA Code:7400) Ignition system: The units which ignite the fuel air mixture in the cylinders of reciprocating engines or in the combustion chambers or thrust augmenters of turbine engines.</rdfs:comment>
        <m:has_related_eccairs_term rdf:resource="http://onto.fel.cvut.cz/ontologies/2014/ECCAIRS_Aviation_1.3.0.12/eccairs-descriptive-factors#category_11740000"/>
    </owl:Class>
    


    <!-- http://onto.fel.cvut.cz/ontologies/aviation-safety/Ignition_system_-_other -->

    <owl:Class rdf:about="&m;Ignition_system_-_other">
        <rdfs:label>Ignition system - other</rdfs:label>
        <rdfs:subClassOf rdf:resource="&m;Ignition_system_part"/>
        <m:generated_time rdf:datatype="&xsd;dateTime">2015-04-09T18:56:27.771+02:00</m:generated_time>
        <rdfs:comment xml:lang="en">(ATA Code:7498) Ignition system - other: Components of the ignition system - other than those listed above.</rdfs:comment>
        <m:has_related_eccairs_term rdf:resource="http://onto.fel.cvut.cz/ontologies/2014/ECCAIRS_Aviation_1.3.0.12/eccairs-descriptive-factors#category_11749800"/>
    </owl:Class>
    


    <!-- http://onto.fel.cvut.cz/ontologies/aviation-safety/Ignition_system_exciter -->

    <owl:Class rdf:about="&m;Ignition_system_exciter">
        <rdfs:label>Ignition system exciter</rdfs:label>
        <rdfs:subClassOf rdf:resource="&m;Ignition_power_supply_part"/>
        <m:generated_time rdf:datatype="&xsd;dateTime">2015-04-09T18:56:27.771+02:00</m:generated_time>
        <rdfs:comment xml:lang="en">(ATA Code:7412) Ignition system exciter: The unit used with turbine engine ignition systems for starting engines. Typical parts are exciter box, bracket and relay.</rdfs:comment>
        <m:has_related_eccairs_term rdf:resource="http://onto.fel.cvut.cz/ontologies/2014/ECCAIRS_Aviation_1.3.0.12/eccairs-descriptive-factors#category_11741200"/>
    </owl:Class>
    


    <!-- http://onto.fel.cvut.cz/ontologies/aviation-safety/Ignition_system_part -->

    <owl:Class rdf:about="&m;Ignition_system_part">
        <rdfs:label>Ignition system part</rdfs:label>
        <rdfs:subClassOf rdf:resource="&m;Aircraft_part"/>
        <rdfs:subClassOf>
            <owl:Restriction>
                <owl:onProperty rdf:resource="http://onto.fel.cvut.cz/ontologies/ufo/is_part_of"/>
                <owl:someValuesFrom rdf:resource="&m;Ignition_system"/>
            </owl:Restriction>
        </rdfs:subClassOf>
        <m:generated_time rdf:datatype="&xsd;dateTime">2015-04-12T02:45:54.351+02:00</m:generated_time>
        <m:has_related_eccairs_term rdf:resource="http://onto.fel.cvut.cz/ontologies/2014/ECCAIRS_Aviation_1.3.0.12/eccairs-descriptive-factors#category_11740000"/>
    </owl:Class>
    


    <!-- http://onto.fel.cvut.cz/ontologies/aviation-safety/In-flight_entertainment_system -->

    <owl:Class rdf:about="&m;In-flight_entertainment_system">
        <rdfs:label>In-flight entertainment system</rdfs:label>
        <rdfs:subClassOf rdf:resource="&m;cabin_system"/>
        <m:generated_time rdf:datatype="&xsd;dateTime">2015-04-09T18:56:27.771+02:00</m:generated_time>
        <rdfs:comment xml:lang="en">(ATA Code:4420) In-flight entertainment system: The portion of the cabin system used to entertain the passengers with music, video, information and games. Includes items such as controllers, cabin control panels, audio and video equipment.</rdfs:comment>
        <m:has_related_eccairs_term rdf:resource="http://onto.fel.cvut.cz/ontologies/2014/ECCAIRS_Aviation_1.3.0.12/eccairs-descriptive-factors#category_11442000"/>
    </owl:Class>
    


    <!-- http://onto.fel.cvut.cz/ontologies/aviation-safety/Independent_position_determining_system -->

    <owl:Class rdf:about="&m;Independent_position_determining_system">
        <rdfs:label>Independent position determining system</rdfs:label>
        <rdfs:subClassOf rdf:resource="&m;Navigation_system"/>
        <rdfs:subClassOf>
            <owl:Restriction>
                <owl:onProperty rdf:resource="http://onto.fel.cvut.cz/ontologies/ufo/is_part_of"/>
                <owl:someValuesFrom rdf:resource="&m;Independent_position_determining_system"/>
            </owl:Restriction>
        </rdfs:subClassOf>
        <m:generated_time rdf:datatype="&xsd;dateTime">2015-04-09T18:56:27.771+02:00</m:generated_time>
        <m:generated_time rdf:datatype="&xsd;dateTime">2015-04-12T02:45:54.351+02:00</m:generated_time>
        <rdfs:comment xml:lang="en">(ATA Code:3440) Independent position determining system: The system which provides information to determine position and is primarily independent of ground installations. Typical parts are star tracker and sextants/octants.</rdfs:comment>
        <m:has_related_eccairs_term rdf:resource="http://onto.fel.cvut.cz/ontologies/2014/ECCAIRS_Aviation_1.3.0.12/eccairs-descriptive-factors#category_11344000"/>
    </owl:Class>
    


    <!-- http://onto.fel.cvut.cz/ontologies/aviation-safety/Induction_vibrator -->

    <owl:Class rdf:about="&m;Induction_vibrator">
        <rdfs:label>Induction vibrator</rdfs:label>
        <rdfs:subClassOf rdf:resource="&m;Ignition_power_supply_part"/>
        <m:generated_time rdf:datatype="&xsd;dateTime">2015-04-09T18:56:27.771+02:00</m:generated_time>
        <rdfs:comment xml:lang="en">(ATA Code:7413) Induction vibrator: The unit which provides a high tension spark to reciprocating engine spark plugs for starting.</rdfs:comment>
        <m:has_related_eccairs_term rdf:resource="http://onto.fel.cvut.cz/ontologies/2014/ECCAIRS_Aviation_1.3.0.12/eccairs-descriptive-factors#category_11741300"/>
    </owl:Class>
    


    <!-- http://onto.fel.cvut.cz/ontologies/aviation-safety/Inertial_guidance_system -->

    <owl:Class rdf:about="&m;Inertial_guidance_system">
        <rdfs:label>Inertial guidance system</rdfs:label>
        <rdfs:subClassOf rdf:resource="&m;Independent_position_determining_system"/>
        <m:generated_time rdf:datatype="&xsd;dateTime">2015-04-09T18:56:27.771+02:00</m:generated_time>
        <rdfs:comment xml:lang="en">(ATA Code:3441) Inertial guidance system: The navigation system which relies upon gyro platforms and accelerometers for its operation. Includes the control panel for the inertial navigation system; the instruments which receives their signal from the inertial navigation unit and the unit containing the inertial platform and digital computer portion of the system. Typical parts are mode selector unit, control display unit and remote display unit.</rdfs:comment>
        <m:has_related_eccairs_term rdf:resource="http://onto.fel.cvut.cz/ontologies/2014/ECCAIRS_Aviation_1.3.0.12/eccairs-descriptive-factors#category_11344100"/>
    </owl:Class>
    


    <!-- http://onto.fel.cvut.cz/ontologies/aviation-safety/Information_system -->

    <owl:Class rdf:about="&m;Information_system">
        <rdfs:label>Information system</rdfs:label>
        <rdfs:subClassOf rdf:resource="&m;Aircraft_part"/>
        <m:generated_time rdf:datatype="&xsd;dateTime">2015-04-09T18:56:27.771+02:00</m:generated_time>
        <rdfs:comment xml:lang="en">(ATA Code:4600) Information system: The units and components which furnish a means of storing, updating and retrieving digital information traditionally provided on paper, microfilm or microfiche. Includes units that are dedicated to the information storage and retrieval function such as the electronic library mass storage and controller. Does not include units or components installed for other uses and shared with other systems, such as flight deck printer or general use display.</rdfs:comment>
        <m:has_related_eccairs_term rdf:resource="http://onto.fel.cvut.cz/ontologies/2014/ECCAIRS_Aviation_1.3.0.12/eccairs-descriptive-factors#category_11460000"/>
    </owl:Class>
    


    <!-- http://onto.fel.cvut.cz/ontologies/aviation-safety/Information_system_part -->

    <owl:Class rdf:about="&m;Information_system_part">
        <rdfs:label>Information system part</rdfs:label>
        <rdfs:subClassOf rdf:resource="&m;Aircraft_part"/>
        <rdfs:subClassOf>
            <owl:Restriction>
                <owl:onProperty rdf:resource="http://onto.fel.cvut.cz/ontologies/ufo/is_part_of"/>
                <owl:someValuesFrom rdf:resource="&m;Information_system"/>
            </owl:Restriction>
        </rdfs:subClassOf>
        <m:generated_time rdf:datatype="&xsd;dateTime">2015-04-12T02:45:54.351+02:00</m:generated_time>
        <m:has_related_eccairs_term rdf:resource="http://onto.fel.cvut.cz/ontologies/2014/ECCAIRS_Aviation_1.3.0.12/eccairs-descriptive-factors#category_11460000"/>
    </owl:Class>
    


    <!-- http://onto.fel.cvut.cz/ontologies/aviation-safety/Inspection_and_observation_windows -->

    <owl:Class rdf:about="&m;Inspection_and_observation_windows">
        <rdfs:label>Inspection and observation windows</rdfs:label>
        <rdfs:subClassOf rdf:resource="&m;Window-windshield_system_part"/>
        <m:generated_time rdf:datatype="&xsd;dateTime">2015-04-09T18:56:27.771+02:00</m:generated_time>
        <rdfs:comment xml:lang="en">(ATA Code:5640) Inspection and observation windows: The windows used for examining compartments and equipment in and about the aeroplane such as door latches and cargo bays.</rdfs:comment>
        <m:has_related_eccairs_term rdf:resource="http://onto.fel.cvut.cz/ontologies/2014/ECCAIRS_Aviation_1.3.0.12/eccairs-descriptive-factors#category_11564000"/>
    </owl:Class>
    


    <!-- http://onto.fel.cvut.cz/ontologies/aviation-safety/Insulation_blankets -->

    <owl:Class rdf:about="&m;Insulation_blankets">
        <rdfs:label>Insulation blankets</rdfs:label>
        <rdfs:subClassOf rdf:resource="&m;Cabin_equipment-furnishings"/>
        <m:generated_time rdf:datatype="&xsd;dateTime">2015-04-09T18:56:27.771+02:00</m:generated_time>
        <rdfs:comment xml:lang="en">(ATA Code:2580) The insulation blankets which are used for heat and sound insulation. Includes flight crew compartments, passenger compartment and additional compartment insulation.</rdfs:comment>
        <m:has_related_eccairs_term rdf:resource="http://onto.fel.cvut.cz/ontologies/2014/ECCAIRS_Aviation_1.3.0.12/eccairs-descriptive-factors#category_11258000"/>
    </owl:Class>
    


    <!-- http://onto.fel.cvut.cz/ontologies/aviation-safety/Integrated_automatic_tuning -->

    <owl:Class rdf:about="&m;Integrated_automatic_tuning">
        <rdfs:label>Integrated automatic tuning</rdfs:label>
        <rdfs:subClassOf rdf:resource="&m;Aircraft_communication_related_system"/>
        <m:generated_time rdf:datatype="&xsd;dateTime">2015-04-09T18:56:27.771+02:00</m:generated_time>
        <rdfs:comment xml:lang="en">(ATA Code:2380) Integrated auto tuning: That portion of the system which maintains integrated control of the operating frequencies of communication and navigation transmitter/receivers after either a manually inserted command or a pre-programmed integrated flight system command. Includes such items as integrated frequency selector panels, digital frequency control computers and integrated frequency display panels.</rdfs:comment>
        <m:has_related_eccairs_term rdf:resource="http://onto.fel.cvut.cz/ontologies/2014/ECCAIRS_Aviation_1.3.0.12/eccairs-descriptive-factors#category_11238000"/>
    </owl:Class>
    


    <!-- http://onto.fel.cvut.cz/ontologies/aviation-safety/Integrated_flight_director_system -->

    <owl:Class rdf:about="&m;Integrated_flight_director_system">
        <rdfs:label>Integrated flight director system</rdfs:label>
        <rdfs:subClassOf rdf:resource="&m;Attitude_and_direction_data_system_part"/>
        <m:generated_time rdf:datatype="&xsd;dateTime">2015-04-09T18:56:27.771+02:00</m:generated_time>
        <rdfs:comment xml:lang="en">(ATA Code:3425) Integrated flight director system: The system which computes, interrogates, and continuously displays basic attitude, position and steering information in order to maintain a particular course, heading or attitude. Does not include flight management system components [Code 11346000]. Typical parts are integrated flight annunciator, integrated flight comparator, integrated flight computer/amplifier, integrated flight control and integrated flight indicators (i.e. horizontal situation indicator, attitude and direction indicator, attitude direction unit, heading and direction indicator, radio direction indicator, course direction indicator, flight director indicator, pictorial navigation indicator, flight command indicator, steering computer utilized in the integrated flight instrument systems and other components such as cables and connectors.</rdfs:comment>
        <m:has_related_eccairs_term rdf:resource="http://onto.fel.cvut.cz/ontologies/2014/ECCAIRS_Aviation_1.3.0.12/eccairs-descriptive-factors#category_11342500"/>
    </owl:Class>
    


    <!-- http://onto.fel.cvut.cz/ontologies/aviation-safety/Interior_Placards -->

    <owl:Class rdf:about="&m;Interior_Placards">
        <rdfs:label>Interior Placards</rdfs:label>
        <rdfs:subClassOf rdf:resource="&m;Placards_and_markings"/>
        <m:generated_time rdf:datatype="&xsd;dateTime">2015-04-09T18:56:27.771+02:00</m:generated_time>
        <rdfs:comment xml:lang="en">(ATA Code:1130) Those placards, markings, self-illuminating signs, etc.   required for interior general and emergency information, instructions, cautions, warnings, etc.</rdfs:comment>
        <m:has_related_eccairs_term rdf:resource="http://onto.fel.cvut.cz/ontologies/2014/ECCAIRS_Aviation_1.3.0.12/eccairs-descriptive-factors#category_11113000"/>
    </owl:Class>
    


    <!-- http://onto.fel.cvut.cz/ontologies/aviation-safety/Interphone_system -->

    <owl:Class rdf:about="&m;Interphone_system">
        <rdfs:label>Interphone system</rdfs:label>
        <rdfs:subClassOf rdf:resource="&m;Aircraft_communication_related_system"/>
        <m:generated_time rdf:datatype="&xsd;dateTime">2015-04-09T18:56:27.771+02:00</m:generated_time>
        <rdfs:comment xml:lang="en">(ATA Code:2340) Interphone system</rdfs:comment>
        <m:has_related_eccairs_term rdf:resource="http://onto.fel.cvut.cz/ontologies/2014/ECCAIRS_Aviation_1.3.0.12/eccairs-descriptive-factors#category_11234000"/>
    </owl:Class>
    


    <!-- http://onto.fel.cvut.cz/ontologies/aviation-safety/Jacking -->

    <owl:Class rdf:about="&m;Jacking">
        <rdfs:label>Jacking</rdfs:label>
        <rdfs:subClassOf rdf:resource="&m;Lifting_and_shoring_part"/>
        <m:generated_time rdf:datatype="&xsd;dateTime">2015-04-09T18:56:27.771+02:00</m:generated_time>
        <rdfs:comment xml:lang="en">(ATA Code:0710) Provides information relative to jack points, adapters, tail supports, balance weights, jacks and jacking procedures utilized during aircraft maintenance and repair.</rdfs:comment>
        <m:has_related_eccairs_term rdf:resource="http://onto.fel.cvut.cz/ontologies/2014/ECCAIRS_Aviation_1.3.0.12/eccairs-descriptive-factors#category_11071000"/>
    </owl:Class>
    


    <!-- http://onto.fel.cvut.cz/ontologies/aviation-safety/Landing_and_taxi_aid -->

    <owl:Class rdf:about="&m;Landing_and_taxi_aid">
        <rdfs:label>Landing and taxi aid</rdfs:label>
        <rdfs:subClassOf rdf:resource="&m;Navigation_system"/>
        <rdfs:subClassOf>
            <owl:Restriction>
                <owl:onProperty rdf:resource="http://onto.fel.cvut.cz/ontologies/ufo/is_part_of"/>
                <owl:someValuesFrom rdf:resource="&m;Landing_and_taxi_aid"/>
            </owl:Restriction>
        </rdfs:subClassOf>
        <m:generated_time rdf:datatype="&xsd;dateTime">2015-04-09T18:56:27.771+02:00</m:generated_time>
        <m:generated_time rdf:datatype="&xsd;dateTime">2015-04-12T02:45:54.351+02:00</m:generated_time>
        <rdfs:comment xml:lang="en">(ATA Code:3430) Landing and taxi aids: The system providing guidance during approach, landing and taxiing. Includes such items as, ILS, paravisual director, ground guidance systems and markers.</rdfs:comment>
        <m:has_related_eccairs_term rdf:resource="http://onto.fel.cvut.cz/ontologies/2014/ECCAIRS_Aviation_1.3.0.12/eccairs-descriptive-factors#category_11343000"/>
    </owl:Class>
    


    <!-- http://onto.fel.cvut.cz/ontologies/aviation-safety/Landing_gear_attachment_fittings_(on_fuselage) -->

    <owl:Class rdf:about="&m;Landing_gear_attachment_fittings_(on_fuselage)">
        <rdfs:label>Landing gear attachment fittings (on fuselage)</rdfs:label>
        <rdfs:subClassOf rdf:resource="&m;Fuselage_attachment_fittings_part"/>
        <m:generated_time rdf:datatype="&xsd;dateTime">2015-04-09T18:56:27.771+02:00</m:generated_time>
        <rdfs:comment xml:lang="en">(ATA Code:5343) Landing gear attachment fittings (on fuselage): The fittings on the fuselage used for the attachment of the landing gear.</rdfs:comment>
        <m:has_related_eccairs_term rdf:resource="http://onto.fel.cvut.cz/ontologies/2014/ECCAIRS_Aviation_1.3.0.12/eccairs-descriptive-factors#category_11534300"/>
    </owl:Class>
    


    <!-- http://onto.fel.cvut.cz/ontologies/aviation-safety/Landing_gear_doors -->

    <owl:Class rdf:about="&m;Landing_gear_doors">
        <rdfs:label>Landing gear doors</rdfs:label>
        <rdfs:subClassOf rdf:resource="&m;Fuselage_doors_part"/>
        <m:generated_time rdf:datatype="&xsd;dateTime">2015-04-09T18:56:27.771+02:00</m:generated_time>
        <rdfs:comment xml:lang="en">(ATA Code:5280) Landing gear doors: The structural aspects of landing gear doors including hinges and seals on the wing, landing gear, and fuselage mounted doors. Does not include the operating mechanism or position indicating or warning system [Codes 11323100 or 11326000].</rdfs:comment>
        <m:has_related_eccairs_term rdf:resource="http://onto.fel.cvut.cz/ontologies/2014/ECCAIRS_Aviation_1.3.0.12/eccairs-descriptive-factors#category_11528000"/>
    </owl:Class>
    


    <!-- http://onto.fel.cvut.cz/ontologies/aviation-safety/Leading_edge_devices -->

    <owl:Class rdf:about="&m;Leading_edge_devices">
        <rdfs:label>Leading edge devices</rdfs:label>
        <rdfs:subClassOf rdf:resource="&m;Wing_flight_control_surface_part"/>
        <m:generated_time rdf:datatype="&xsd;dateTime">2015-04-09T18:56:27.771+02:00</m:generated_time>
        <rdfs:comment xml:lang="en">(ATA Code:5754) Leading edge devices: The structural aspects of the wing leading edge device control surface. Includes hinge, brackets and bolts but does not include actuators or actuator mounting brackets [Code 11278200]. Typical parts are skin, rib, track, roller, bearing and carriage.</rdfs:comment>
        <m:has_related_eccairs_term rdf:resource="http://onto.fel.cvut.cz/ontologies/2014/ECCAIRS_Aviation_1.3.0.12/eccairs-descriptive-factors#category_11575400"/>
    </owl:Class>
    


    <!-- http://onto.fel.cvut.cz/ontologies/aviation-safety/Leading_edge_flap_actuator -->

    <owl:Class rdf:about="&m;Leading_edge_flap_actuator">
        <rdfs:label>Leading edge flap actuator</rdfs:label>
        <rdfs:subClassOf rdf:resource="&m;Lift_Augmenting_-_Leading_edge_slat_control_system_part"/>
        <m:generated_time rdf:datatype="&xsd;dateTime">2015-04-09T18:56:27.771+02:00</m:generated_time>
        <rdfs:comment xml:lang="en">(ATA Code:2782) Leading edge flap actuator: The components which cause movement of the wing leading edge device control surfaces. Does not include related system or position indicating. Typical parts are actuator, actuator bracket and seal.</rdfs:comment>
        <m:has_related_eccairs_term rdf:resource="http://onto.fel.cvut.cz/ontologies/2014/ECCAIRS_Aviation_1.3.0.12/eccairs-descriptive-factors#category_11278200"/>
    </owl:Class>
    


    <!-- http://onto.fel.cvut.cz/ontologies/aviation-safety/Leading_edge_flap_position_indicating_system -->

    <owl:Class rdf:about="&m;Leading_edge_flap_position_indicating_system">
        <rdfs:label>Leading edge flap position indicating system</rdfs:label>
        <rdfs:subClassOf rdf:resource="&m;Lift_Augmenting_-_Leading_edge_slat_control_system_part"/>
        <m:generated_time rdf:datatype="&xsd;dateTime">2015-04-09T18:56:27.771+02:00</m:generated_time>
        <rdfs:comment xml:lang="en">(ATA Code:2781) Leading edge flap position indicating system: The transmitter, indicator, warning lamps and associated circuitry providing relative position information of wing leading edge devices to the flight crew.</rdfs:comment>
        <m:has_related_eccairs_term rdf:resource="http://onto.fel.cvut.cz/ontologies/2014/ECCAIRS_Aviation_1.3.0.12/eccairs-descriptive-factors#category_11278100"/>
    </owl:Class>
    


    <!-- http://onto.fel.cvut.cz/ontologies/aviation-safety/Leveling -->

    <owl:Class rdf:about="&m;Leveling">
        <rdfs:label>Leveling</rdfs:label>
        <rdfs:subClassOf rdf:resource="&m;Leveling_and_weighting_part"/>
        <m:generated_time rdf:datatype="&xsd;dateTime">2015-04-09T18:56:27.771+02:00</m:generated_time>
        <rdfs:comment xml:lang="en">(ATA Code:0820) Those units or components dedicated to the specific function of leveling the aircraft.</rdfs:comment>
        <m:has_related_eccairs_term rdf:resource="http://onto.fel.cvut.cz/ontologies/2014/ECCAIRS_Aviation_1.3.0.12/eccairs-descriptive-factors#category_11082000"/>
    </owl:Class>
    


    <!-- http://onto.fel.cvut.cz/ontologies/aviation-safety/Leveling_and_weighting -->

    <owl:Class rdf:about="&m;Leveling_and_weighting">
        <rdfs:label>Leveling and weighting</rdfs:label>
        <rdfs:subClassOf rdf:resource="&m;Aircraft_part"/>
        <m:generated_time rdf:datatype="&xsd;dateTime">2015-04-09T18:56:27.771+02:00</m:generated_time>
        <rdfs:comment xml:lang="en">(ATA Code:0800) Data to properly level the aircraft for any of the various maintenance, overhaul or major repairs which might become necessary during the life of the aircraft. It shall also include those units or components which are specifically dedicated to record, store or compute weight and balance data. Includes those maintenance practices necessary to prepare the aircraft for weighing.</rdfs:comment>
        <m:has_related_eccairs_term rdf:resource="http://onto.fel.cvut.cz/ontologies/2014/ECCAIRS_Aviation_1.3.0.12/eccairs-descriptive-factors#category_11080000"/>
    </owl:Class>
    


    <!-- http://onto.fel.cvut.cz/ontologies/aviation-safety/Leveling_and_weighting_part -->

    <owl:Class rdf:about="&m;Leveling_and_weighting_part">
        <rdfs:label>Leveling and weighting part</rdfs:label>
        <rdfs:subClassOf rdf:resource="&m;Aircraft_part"/>
        <rdfs:subClassOf>
            <owl:Restriction>
                <owl:onProperty rdf:resource="http://onto.fel.cvut.cz/ontologies/ufo/is_part_of"/>
                <owl:someValuesFrom rdf:resource="&m;Leveling_and_weighting"/>
            </owl:Restriction>
        </rdfs:subClassOf>
        <m:generated_time rdf:datatype="&xsd;dateTime">2015-04-12T02:45:54.351+02:00</m:generated_time>
        <m:has_related_eccairs_term rdf:resource="http://onto.fel.cvut.cz/ontologies/2014/ECCAIRS_Aviation_1.3.0.12/eccairs-descriptive-factors#category_11080000"/>
    </owl:Class>
    


    <!-- http://onto.fel.cvut.cz/ontologies/aviation-safety/Life-jacket -->

    <owl:Class rdf:about="&m;Life-jacket">
        <rdfs:label>Life-jacket</rdfs:label>
        <rdfs:subClassOf rdf:resource="&m;Emergency_equipment"/>
        <m:generated_time rdf:datatype="&xsd;dateTime">2015-04-09T18:56:27.771+02:00</m:generated_time>
        <rdfs:comment xml:lang="en">(ATA Code:2561) Life-jacket: The buoyant jackets used to float incapacitated individuals in a face up attitude.</rdfs:comment>
        <m:has_related_eccairs_term rdf:resource="http://onto.fel.cvut.cz/ontologies/2014/ECCAIRS_Aviation_1.3.0.12/eccairs-descriptive-factors#category_11256100"/>
    </owl:Class>
    


    <!-- http://onto.fel.cvut.cz/ontologies/aviation-safety/Life-raft -->

    <owl:Class rdf:about="&m;Life-raft">
        <rdfs:label>Life-raft</rdfs:label>
        <rdfs:subClassOf rdf:resource="&m;Emergency_equipment"/>
        <m:generated_time rdf:datatype="&xsd;dateTime">2015-04-09T18:56:27.771+02:00</m:generated_time>
        <rdfs:comment xml:lang="en">(ATA Code:2564) Life-raft: The inflatable raft which provides emergency flotation for one or more persons in event of an aircraft ditching. Typical parts are the gas bottle, valve and manual pump.</rdfs:comment>
        <m:has_related_eccairs_term rdf:resource="http://onto.fel.cvut.cz/ontologies/2014/ECCAIRS_Aviation_1.3.0.12/eccairs-descriptive-factors#category_11256400"/>
    </owl:Class>
    


    <!-- http://onto.fel.cvut.cz/ontologies/aviation-safety/Lift_Augmenting_-_Leading_edge_slat_control_system -->

    <owl:Class rdf:about="&m;Lift_Augmenting_-_Leading_edge_slat_control_system">
        <rdfs:label>Lift Augmenting - Leading edge slat control system</rdfs:label>
        <rdfs:subClassOf rdf:resource="&m;Flight_control_system_part"/>
        <m:generated_time rdf:datatype="&xsd;dateTime">2015-04-09T18:56:27.771+02:00</m:generated_time>
        <rdfs:comment xml:lang="en">(ATA Code:2780) Leading edge flap control system: That portion of the systems which controls the position and movement of variable opening wings slots, leading edge wing flaps, and other similar auxiliary devices used for increasing aerodynamic lift. Includes items such as control handles, cables, actuators, linkages, warning systems, control surfaces, position indicators, etc. Does not include trailing edge flaps.</rdfs:comment>
        <m:has_related_eccairs_term rdf:resource="http://onto.fel.cvut.cz/ontologies/2014/ECCAIRS_Aviation_1.3.0.12/eccairs-descriptive-factors#category_11278000"/>
    </owl:Class>
    


    <!-- http://onto.fel.cvut.cz/ontologies/aviation-safety/Lift_Augmenting_-_Leading_edge_slat_control_system_part -->

    <owl:Class rdf:about="&m;Lift_Augmenting_-_Leading_edge_slat_control_system_part">
        <rdfs:label>Lift Augmenting - Leading edge slat control system part</rdfs:label>
        <rdfs:subClassOf rdf:resource="&m;Flight_control_system_part"/>
        <rdfs:subClassOf>
            <owl:Restriction>
                <owl:onProperty rdf:resource="http://onto.fel.cvut.cz/ontologies/ufo/is_part_of"/>
                <owl:someValuesFrom rdf:resource="&m;Lift_Augmenting_-_Leading_edge_slat_control_system"/>
            </owl:Restriction>
        </rdfs:subClassOf>
        <m:generated_time rdf:datatype="&xsd;dateTime">2015-04-12T02:45:54.351+02:00</m:generated_time>
        <m:has_related_eccairs_term rdf:resource="http://onto.fel.cvut.cz/ontologies/2014/ECCAIRS_Aviation_1.3.0.12/eccairs-descriptive-factors#category_11278000"/>
    </owl:Class>
    


    <!-- http://onto.fel.cvut.cz/ontologies/aviation-safety/Lifting_and_shoring -->

    <owl:Class rdf:about="&m;Lifting_and_shoring">
        <rdfs:label>Lifting and shoring</rdfs:label>
        <rdfs:subClassOf rdf:resource="&m;Aircraft_part"/>
        <m:generated_time rdf:datatype="&xsd;dateTime">2015-04-09T18:56:27.771+02:00</m:generated_time>
        <rdfs:comment xml:lang="en">(ATA Code:0700) This chapter shall include the necessary procedures to lift &amp; shore aircraft in any of the conditions to which it may be subjected.   Includes lifting and shoring procedures that may be employed during aircraft maintenance and repair.</rdfs:comment>
        <m:has_related_eccairs_term rdf:resource="http://onto.fel.cvut.cz/ontologies/2014/ECCAIRS_Aviation_1.3.0.12/eccairs-descriptive-factors#category_11070000"/>
    </owl:Class>
    


    <!-- http://onto.fel.cvut.cz/ontologies/aviation-safety/Lifting_and_shoring_part -->

    <owl:Class rdf:about="&m;Lifting_and_shoring_part">
        <rdfs:label>Lifting and shoring part</rdfs:label>
        <rdfs:subClassOf rdf:resource="&m;Aircraft_part"/>
        <rdfs:subClassOf>
            <owl:Restriction>
                <owl:onProperty rdf:resource="http://onto.fel.cvut.cz/ontologies/ufo/is_part_of"/>
                <owl:someValuesFrom rdf:resource="&m;Lifting_and_shoring"/>
            </owl:Restriction>
        </rdfs:subClassOf>
        <m:generated_time rdf:datatype="&xsd;dateTime">2015-04-12T02:45:54.351+02:00</m:generated_time>
        <m:has_related_eccairs_term rdf:resource="http://onto.fel.cvut.cz/ontologies/2014/ECCAIRS_Aviation_1.3.0.12/eccairs-descriptive-factors#category_11070000"/>
    </owl:Class>
    


    <!-- http://onto.fel.cvut.cz/ontologies/aviation-safety/Lighting_System_Wiring -->

    <owl:Class rdf:about="&m;Lighting_System_Wiring">
        <rdfs:label>Lighting System Wiring</rdfs:label>
        <rdfs:subClassOf rdf:resource="&m;Lighting_system"/>
        <rdfs:subClassOf rdf:resource="&m;Wiring"/>
        <rdfs:subClassOf>
            <owl:Restriction>
                <owl:onProperty rdf:resource="http://onto.fel.cvut.cz/ontologies/ufo/is_part_of"/>
                <owl:someValuesFrom rdf:resource="&m;Lighting_system"/>
            </owl:Restriction>
        </rdfs:subClassOf>
        <m:generated_time rdf:datatype="&xsd;dateTime">2015-04-09T18:56:27.771+02:00</m:generated_time>
        <rdfs:comment xml:lang="en">(ATA Code:3397) Wiring specific to the Lighting Systems</rdfs:comment>
        <m:has_related_eccairs_term rdf:resource="http://onto.fel.cvut.cz/ontologies/2014/ECCAIRS_Aviation_1.3.0.12/eccairs-descriptive-factors#category_11339700"/>
    </owl:Class>
    


    <!-- http://onto.fel.cvut.cz/ontologies/aviation-safety/Lighting_system -->

    <owl:Class rdf:about="&m;Lighting_system">
        <rdfs:label>Lighting system</rdfs:label>
        <rdfs:subClassOf rdf:resource="&m;Aircraft_part"/>
        <rdfs:subClassOf>
            <owl:Restriction>
                <owl:onProperty rdf:resource="http://onto.fel.cvut.cz/ontologies/ufo/is_part_of"/>
                <owl:someValuesFrom rdf:resource="&m;Lighting_system"/>
            </owl:Restriction>
        </rdfs:subClassOf>
        <m:generated_time rdf:datatype="&xsd;dateTime">2015-04-09T18:56:27.771+02:00</m:generated_time>
        <m:generated_time rdf:datatype="&xsd;dateTime">2015-04-12T02:45:54.351+02:00</m:generated_time>
        <rdfs:comment xml:lang="en">(ATA Code:3300) Lighting system: The units and components which provide for external and internal illumination. Includes light fixtures, switches and wiring. Does not include warning lights for individual systems.</rdfs:comment>
        <m:has_related_eccairs_term rdf:resource="http://onto.fel.cvut.cz/ontologies/2014/ECCAIRS_Aviation_1.3.0.12/eccairs-descriptive-factors#category_11330000"/>
    </owl:Class>
    


    <!-- http://onto.fel.cvut.cz/ontologies/aviation-safety/Localizer-very_high_frequency_omni_directional_radio_range_system -->

    <owl:Class rdf:about="&m;Localizer-very_high_frequency_omni_directional_radio_range_system">
        <rdfs:label>Localizer/very high frequency omni directional radio range system</rdfs:label>
        <rdfs:subClassOf rdf:resource="&m;ILS_aircraft_equipment"/>
        <m:generated_time rdf:datatype="&xsd;dateTime">2015-04-09T18:56:27.771+02:00</m:generated_time>
        <rdfs:comment xml:lang="en">(ATA Code:3431) Localizer/very high frequency omni directional radio range system: The electronic portion of an instrument landing system that indicates the centreline of the runway to the pilot. Includes localizer/very high frequency omni directional radio range systems. Typical parts are receiver, antenna, indicator, circuit breaker, switch and antenna coaxial cable.</rdfs:comment>
        <m:has_related_eccairs_term rdf:resource="http://onto.fel.cvut.cz/ontologies/2014/ECCAIRS_Aviation_1.3.0.12/eccairs-descriptive-factors#category_11343100"/>
    </owl:Class>
    


    <!-- http://onto.fel.cvut.cz/ontologies/aviation-safety/Long_range_navigation_system -->

    <owl:Class rdf:about="&m;Long_range_navigation_system">
        <rdfs:label>Long range navigation system</rdfs:label>
        <rdfs:subClassOf rdf:resource="&m;Dependent_position_determining_system"/>
        <m:generated_time rdf:datatype="&xsd;dateTime">2015-04-09T18:56:27.771+02:00</m:generated_time>
        <rdfs:comment xml:lang="en">(ATA Code:3453) Long range navigation system: The radio navigation system and associated components and parts which provides for long range navigation en route when operating on signals from ground based master and slave transmitting stations. Typical parts are antenna, coupler, CPU and receiver.</rdfs:comment>
        <m:has_related_eccairs_term rdf:resource="http://onto.fel.cvut.cz/ontologies/2014/ECCAIRS_Aviation_1.3.0.12/eccairs-descriptive-factors#category_11345300"/>
    </owl:Class>
    


    <!-- http://onto.fel.cvut.cz/ontologies/aviation-safety/Longeron-stringers_(nacelle-pylon) -->

    <owl:Class rdf:about="&m;Longeron-stringers_(nacelle-pylon)">
        <rdfs:label>Longeron/stringers (nacelle/pylon)</rdfs:label>
        <rdfs:subClassOf rdf:resource="&m;Main_frame_(nacelle-pylon)_part"/>
        <m:generated_time rdf:datatype="&xsd;dateTime">2015-04-09T18:56:27.771+02:00</m:generated_time>
        <rdfs:comment xml:lang="en">(ATA Code:5413) The longeron or stringer structure on the nacelles or pylons.</rdfs:comment>
        <m:has_related_eccairs_term rdf:resource="http://onto.fel.cvut.cz/ontologies/2014/ECCAIRS_Aviation_1.3.0.12/eccairs-descriptive-factors#category_11541300"/>
    </owl:Class>
    


    <!-- http://onto.fel.cvut.cz/ontologies/aviation-safety/Low_tension_coil -->

    <owl:Class rdf:about="&m;Low_tension_coil">
        <rdfs:label>Low tension coil</rdfs:label>
        <rdfs:subClassOf rdf:resource="&m;Ignition_power_supply_part"/>
        <m:generated_time rdf:datatype="&xsd;dateTime">2015-04-09T18:56:27.771+02:00</m:generated_time>
        <rdfs:comment xml:lang="en">(ATA Code:7411) Low tension coil: The magneto coils used on select engines such as the Pratt and Whitney, model R2800, to generate a low tension voltage for high tension voltage coil mounted at each engine cylinder. Not generally used on modern light aircraft reciprocating engines.</rdfs:comment>
        <m:has_related_eccairs_term rdf:resource="http://onto.fel.cvut.cz/ontologies/2014/ECCAIRS_Aviation_1.3.0.12/eccairs-descriptive-factors#category_11741100"/>
    </owl:Class>
    


    <!-- http://onto.fel.cvut.cz/ontologies/aviation-safety/Mach_trim -->

    <owl:Class rdf:about="&m;Mach_trim">
        <rdfs:label>Mach trim</rdfs:label>
        <rdfs:subClassOf rdf:resource="&m;Elevator_&amp;_Tab_control_system_part"/>
        <m:generated_time rdf:datatype="&xsd;dateTime">2015-04-09T18:56:27.771+02:00</m:generated_time>
        <rdfs:comment xml:lang="en">(ATA Code:2736) Mach trim: The electronic/mechanical system for relieving the pilot of task of correcting progressive deficiency in aircraft pitch trim and longitudinal stability at high Mach numbers. Sensitive to Mach number and vertical acceleration and automatically feeds primary pitch-trim demand to keep aircraft level or in desired attitude while leaving pilot authority to feed manual trim.</rdfs:comment>
        <m:has_related_eccairs_term rdf:resource="http://onto.fel.cvut.cz/ontologies/2014/ECCAIRS_Aviation_1.3.0.12/eccairs-descriptive-factors#category_11273600"/>
    </owl:Class>
    


    <!-- http://onto.fel.cvut.cz/ontologies/aviation-safety/Magnetic_compass -->

    <owl:Class rdf:about="&m;Magnetic_compass">
        <rdfs:label>Magnetic compass</rdfs:label>
        <rdfs:subClassOf rdf:resource="&m;Attitude_and_direction_data_system_part"/>
        <m:generated_time rdf:datatype="&xsd;dateTime">2015-04-09T18:56:27.771+02:00</m:generated_time>
        <rdfs:comment xml:lang="en">(ATA Code:3423) Magnetic compass: The instrument which indicates the magnetic heading of an aircraft by self contained magnetized needles. Typical parts are compensator, adjusting screw, gasket, float and case.</rdfs:comment>
        <m:has_related_eccairs_term rdf:resource="http://onto.fel.cvut.cz/ontologies/2014/ECCAIRS_Aviation_1.3.0.12/eccairs-descriptive-factors#category_11342300"/>
    </owl:Class>
    


    <!-- http://onto.fel.cvut.cz/ontologies/aviation-safety/Magneto-distributor -->

    <owl:Class rdf:about="&m;Magneto-distributor">
        <rdfs:label>Magneto/distributor</rdfs:label>
        <rdfs:subClassOf rdf:resource="&m;Ignition_power_supply_part"/>
        <m:generated_time rdf:datatype="&xsd;dateTime">2015-04-09T18:56:27.771+02:00</m:generated_time>
        <rdfs:comment xml:lang="en">(ATA Code:7414) Magneto/distributor: The components which generate and distribute a high voltage to spark plugs in reciprocating engines for fuel/air combustion. Typical parts are coil, breaker points, gear, bearing, contact finger, distributor block, frame, impulse coupling, condenser, rotor, cam, electrode and seal.</rdfs:comment>
        <m:has_related_eccairs_term rdf:resource="http://onto.fel.cvut.cz/ontologies/2014/ECCAIRS_Aviation_1.3.0.12/eccairs-descriptive-factors#category_11741400"/>
    </owl:Class>
    


    <!-- http://onto.fel.cvut.cz/ontologies/aviation-safety/Main_Rotor_Drive_System_Wiring -->

    <owl:Class rdf:about="&m;Main_Rotor_Drive_System_Wiring">
        <rdfs:label>Main Rotor Drive System Wiring</rdfs:label>
        <rdfs:subClassOf rdf:resource="&m;Main_rotor_drive_system_part"/>
        <rdfs:subClassOf rdf:resource="&m;Wiring"/>
        <rdfs:subClassOf>
            <owl:Restriction>
                <owl:onProperty rdf:resource="http://onto.fel.cvut.cz/ontologies/ufo/is_part_of"/>
                <owl:someValuesFrom rdf:resource="&m;Main_rotor_drive_system"/>
            </owl:Restriction>
        </rdfs:subClassOf>
        <m:generated_time rdf:datatype="&xsd;dateTime">2015-04-09T18:56:27.771+02:00</m:generated_time>
        <rdfs:comment xml:lang="en">(ATA Code:6397) Wiring specific to the Main Rotor Drive System.</rdfs:comment>
        <m:has_related_eccairs_term rdf:resource="http://onto.fel.cvut.cz/ontologies/2014/ECCAIRS_Aviation_1.3.0.12/eccairs-descriptive-factors#category_11639700"/>
    </owl:Class>
    


    <!-- http://onto.fel.cvut.cz/ontologies/aviation-safety/Main_Rotor_System_Wiring -->

    <owl:Class rdf:about="&m;Main_Rotor_System_Wiring">
        <rdfs:subClassOf rdf:resource="&m;Rotorcraft_main_rotor_system_part"/>
    </owl:Class>
    


    <!-- http://onto.fel.cvut.cz/ontologies/aviation-safety/Main_frame_(nacelle-pylon) -->

    <owl:Class rdf:about="&m;Main_frame_(nacelle-pylon)">
        <rdfs:label>Main frame (nacelle/pylon)</rdfs:label>
        <rdfs:subClassOf rdf:resource="&m;Nacelle-pylon_structure_part"/>
        <m:generated_time rdf:datatype="&xsd;dateTime">2015-04-09T18:56:27.771+02:00</m:generated_time>
        <rdfs:comment xml:lang="en">(ATA Code:5410) Main frame (nacelle/pylon): The structure which houses and supports powerplants. Includes the firewall and all structure aft on multi-engine aircraft and firewalls on single engine aircraft. Does not include engine mounting or cowling.</rdfs:comment>
        <m:has_related_eccairs_term rdf:resource="http://onto.fel.cvut.cz/ontologies/2014/ECCAIRS_Aviation_1.3.0.12/eccairs-descriptive-factors#category_11541000"/>
    </owl:Class>
    


    <!-- http://onto.fel.cvut.cz/ontologies/aviation-safety/Main_frame_(nacelle-pylon)_part -->

    <owl:Class rdf:about="&m;Main_frame_(nacelle-pylon)_part">
        <rdfs:label>Main frame (nacelle/pylon) part</rdfs:label>
        <rdfs:subClassOf rdf:resource="&m;Nacelle-pylon_structure_part"/>
        <rdfs:subClassOf>
            <owl:Restriction>
                <owl:onProperty rdf:resource="http://onto.fel.cvut.cz/ontologies/ufo/is_part_of"/>
                <owl:someValuesFrom rdf:resource="&m;Main_frame_(nacelle-pylon)"/>
            </owl:Restriction>
        </rdfs:subClassOf>
        <m:generated_time rdf:datatype="&xsd;dateTime">2015-04-12T02:45:54.351+02:00</m:generated_time>
        <m:has_related_eccairs_term rdf:resource="http://onto.fel.cvut.cz/ontologies/2014/ECCAIRS_Aviation_1.3.0.12/eccairs-descriptive-factors#category_11541000"/>
    </owl:Class>
    


    <!-- http://onto.fel.cvut.cz/ontologies/aviation-safety/Main_rotor_blades -->

    <owl:Class rdf:about="&m;Main_rotor_blades">
        <rdfs:label>Main rotor blades</rdfs:label>
        <rdfs:subClassOf rdf:resource="&m;Rotorcraft_main_rotor_system_part"/>
        <m:generated_time rdf:datatype="&xsd;dateTime">2015-04-09T18:56:27.771+02:00</m:generated_time>
        <rdfs:comment xml:lang="en">(ATA Code:6210) The main rotor blades including attachment to the rotor head and heating mats on the blades for anti-icing. Also includes tilt rotor blades. Does not include the anti-icing system [Code 11306000], or the rotor head [Code 11622000]. Typical parts are blade, attachment bolt and bushing,</rdfs:comment>
        <m:has_related_eccairs_term rdf:resource="http://onto.fel.cvut.cz/ontologies/2014/ECCAIRS_Aviation_1.3.0.12/eccairs-descriptive-factors#category_11621000"/>
    </owl:Class>
    


    <!-- http://onto.fel.cvut.cz/ontologies/aviation-safety/Main_rotor_brake -->

    <owl:Class rdf:about="&m;Main_rotor_brake">
        <rdfs:label>Main rotor brake</rdfs:label>
        <rdfs:subClassOf rdf:resource="&m;Main_rotor_gearbox_part"/>
        <m:generated_time rdf:datatype="&xsd;dateTime">2015-04-09T18:56:27.771+02:00</m:generated_time>
        <rdfs:comment xml:lang="en">(ATA Code:6321) Main rotor brake: The system which reduces rundown time or stops rotor rotation during engine power-off conditions. Typical parts are brake, calliper, lining, seal and check valve.</rdfs:comment>
        <m:has_related_eccairs_term rdf:resource="http://onto.fel.cvut.cz/ontologies/2014/ECCAIRS_Aviation_1.3.0.12/eccairs-descriptive-factors#category_11632100"/>
    </owl:Class>
    


    <!-- http://onto.fel.cvut.cz/ontologies/aviation-safety/Main_rotor_control -->

    <owl:Class rdf:about="&m;Main_rotor_control">
        <rdfs:label>Main rotor control</rdfs:label>
        <rdfs:subClassOf rdf:resource="&m;Rotorcraft_flight_control_part"/>
        <m:generated_time rdf:datatype="&xsd;dateTime">2015-04-09T18:56:27.771+02:00</m:generated_time>
        <rdfs:comment xml:lang="en">(ATA Code:6710) Main rotor control: The system components and parts, other than the servo control system, which control and indicate the attitude or the angle of attack of the rotor blades. Typical parts are collective pitch lever, cyclic pitch stick, coupling and mixing units and position indicators.</rdfs:comment>
        <m:has_related_eccairs_term rdf:resource="http://onto.fel.cvut.cz/ontologies/2014/ECCAIRS_Aviation_1.3.0.12/eccairs-descriptive-factors#category_11671000"/>
    </owl:Class>
    


    <!-- http://onto.fel.cvut.cz/ontologies/aviation-safety/Main_rotor_drive_system -->

    <owl:Class rdf:about="&m;Main_rotor_drive_system">
        <rdfs:label>Main rotor drive system</rdfs:label>
        <rdfs:subClassOf rdf:resource="&m;Aircraft_part"/>
        <m:generated_time rdf:datatype="&xsd;dateTime">2015-04-09T18:56:27.771+02:00</m:generated_time>
        <rdfs:comment xml:lang="en">(ATA Code:6300) Main rotor drive system</rdfs:comment>
        <m:has_related_eccairs_term rdf:resource="http://onto.fel.cvut.cz/ontologies/2014/ECCAIRS_Aviation_1.3.0.12/eccairs-descriptive-factors#category_11630000"/>
    </owl:Class>
    


    <!-- http://onto.fel.cvut.cz/ontologies/aviation-safety/Main_rotor_drive_system_part -->

    <owl:Class rdf:about="&m;Main_rotor_drive_system_part">
        <rdfs:label>Main rotor drive system part</rdfs:label>
        <rdfs:subClassOf rdf:resource="&m;Aircraft_part"/>
        <rdfs:subClassOf>
            <owl:Restriction>
                <owl:onProperty rdf:resource="http://onto.fel.cvut.cz/ontologies/ufo/is_part_of"/>
                <owl:someValuesFrom rdf:resource="&m;Main_rotor_drive_system"/>
            </owl:Restriction>
        </rdfs:subClassOf>
        <m:generated_time rdf:datatype="&xsd;dateTime">2015-04-12T02:45:54.351+02:00</m:generated_time>
        <m:has_related_eccairs_term rdf:resource="http://onto.fel.cvut.cz/ontologies/2014/ECCAIRS_Aviation_1.3.0.12/eccairs-descriptive-factors#category_11630000"/>
    </owl:Class>
    


    <!-- http://onto.fel.cvut.cz/ontologies/aviation-safety/Main_rotor_gearbox -->

    <owl:Class rdf:about="&m;Main_rotor_gearbox">
        <rdfs:label>Main rotor gearbox</rdfs:label>
        <rdfs:subClassOf rdf:resource="&m;Main_rotor_drive_system_part"/>
        <m:generated_time rdf:datatype="&xsd;dateTime">2015-04-09T18:56:27.771+02:00</m:generated_time>
        <rdfs:comment xml:lang="en">(ATA Code:6320) Main rotor gearbox: The component which transmits engine power to rotary motion in the main rotor mast. Includes the mechanical power take-off(s) and accessory drives but does not include the accessories themselves such as alternators and hydraulic pumps. Includes the gearbox lubricating system(s). Typical parts are gearbox, case, shaft, gear, pump, seal and sun gear.</rdfs:comment>
        <m:has_related_eccairs_term rdf:resource="http://onto.fel.cvut.cz/ontologies/2014/ECCAIRS_Aviation_1.3.0.12/eccairs-descriptive-factors#category_11632000"/>
    </owl:Class>
    


    <!-- http://onto.fel.cvut.cz/ontologies/aviation-safety/Main_rotor_gearbox_part -->

    <owl:Class rdf:about="&m;Main_rotor_gearbox_part">
        <rdfs:label>Main rotor gearbox part</rdfs:label>
        <rdfs:subClassOf rdf:resource="&m;Main_rotor_drive_system_part"/>
        <rdfs:subClassOf>
            <owl:Restriction>
                <owl:onProperty rdf:resource="http://onto.fel.cvut.cz/ontologies/ufo/is_part_of"/>
                <owl:someValuesFrom rdf:resource="&m;Main_rotor_gearbox"/>
            </owl:Restriction>
        </rdfs:subClassOf>
        <m:generated_time rdf:datatype="&xsd;dateTime">2015-04-12T02:45:54.351+02:00</m:generated_time>
        <m:has_related_eccairs_term rdf:resource="http://onto.fel.cvut.cz/ontologies/2014/ECCAIRS_Aviation_1.3.0.12/eccairs-descriptive-factors#category_11632000"/>
    </owl:Class>
    


    <!-- http://onto.fel.cvut.cz/ontologies/aviation-safety/Main_rotor_head -->

    <owl:Class rdf:about="&m;Main_rotor_head">
        <rdfs:label>Main rotor head</rdfs:label>
        <rdfs:subClassOf rdf:resource="&m;Rotorcraft_main_rotor_system_part"/>
        <m:generated_time rdf:datatype="&xsd;dateTime">2015-04-09T18:56:27.771+02:00</m:generated_time>
        <rdfs:comment xml:lang="en">(ATA Code:6220) Main rotor head: The rotating assembly which supports the main rotor blades including blade folding system and the swashplate if it is an integral part of the mast head assembly. Also includes the head mechanism on tilt rotor craft. Typical parts are sleeve, spindle, damper and fairing. Does not include the controlling aspects [Code 11671000].</rdfs:comment>
        <m:has_related_eccairs_term rdf:resource="http://onto.fel.cvut.cz/ontologies/2014/ECCAIRS_Aviation_1.3.0.12/eccairs-descriptive-factors#category_11622000"/>
    </owl:Class>
    


    <!-- http://onto.fel.cvut.cz/ontologies/aviation-safety/Main_rotor_indicating_system -->

    <owl:Class rdf:about="&m;Main_rotor_indicating_system">
        <rdfs:label>Main rotor indicating system</rdfs:label>
        <rdfs:subClassOf rdf:resource="&m;Rotorcraft_main_rotor_system_part"/>
        <m:generated_time rdf:datatype="&xsd;dateTime">2015-04-09T18:56:27.771+02:00</m:generated_time>
        <rdfs:comment xml:lang="en">(ATA Code:6240) Main rotor indicating system: The system used to indicate the operation or activation of the main rotor. Includes lights, gauges, switches and wiring.</rdfs:comment>
        <m:has_related_eccairs_term rdf:resource="http://onto.fel.cvut.cz/ontologies/2014/ECCAIRS_Aviation_1.3.0.12/eccairs-descriptive-factors#category_11624000"/>
    </owl:Class>
    


    <!-- http://onto.fel.cvut.cz/ontologies/aviation-safety/Main_rotor_mast-swashplate -->

    <owl:Class rdf:about="&m;Main_rotor_mast-swashplate">
        <rdfs:label>Main rotor mast/swashplate</rdfs:label>
        <rdfs:subClassOf rdf:resource="&m;Rotorcraft_main_rotor_system_part"/>
        <m:generated_time rdf:datatype="&xsd;dateTime">2015-04-09T18:56:27.771+02:00</m:generated_time>
        <rdfs:comment xml:lang="en">(ATA Code:6230) Main rotor mast/swashplate: The vertical shaft which supports the main rotor head. Typical parts are shaft, bearing, guide, mast, seal and swashplate.</rdfs:comment>
        <m:has_related_eccairs_term rdf:resource="http://onto.fel.cvut.cz/ontologies/2014/ECCAIRS_Aviation_1.3.0.12/eccairs-descriptive-factors#category_11623000"/>
    </owl:Class>
    


    <!-- http://onto.fel.cvut.cz/ontologies/aviation-safety/Main_rotor_transmission_mount -->

    <owl:Class rdf:about="&m;Main_rotor_transmission_mount">
        <rdfs:label>Main rotor transmission mount</rdfs:label>
        <rdfs:subClassOf rdf:resource="&m;Main_rotor_drive_system_part"/>
        <m:generated_time rdf:datatype="&xsd;dateTime">2015-04-09T18:56:27.771+02:00</m:generated_time>
        <rdfs:comment xml:lang="en">(ATA Code:6330) Main rotor transmission mount: The suspension system for the transmission mounting in the airframe. Typical parts are suspension bars and isolation mount.</rdfs:comment>
        <m:has_related_eccairs_term rdf:resource="http://onto.fel.cvut.cz/ontologies/2014/ECCAIRS_Aviation_1.3.0.12/eccairs-descriptive-factors#category_11633000"/>
    </owl:Class>
    


    <!-- http://onto.fel.cvut.cz/ontologies/aviation-safety/Main_system_electric_or_engine_driven_hydraulic_pump -->

    <owl:Class rdf:about="&m;Main_system_electric_or_engine_driven_hydraulic_pump">
        <rdfs:label>Main system electric or engine driven hydraulic pump</rdfs:label>
        <rdfs:subClassOf rdf:resource="&m;Hydraulic,_main_system_part"/>
        <m:generated_time rdf:datatype="&xsd;dateTime">2015-04-09T18:56:27.771+02:00</m:generated_time>
        <rdfs:comment xml:lang="en">(ATA Code:2913) Main system electric or engine driven hydraulic pump: The component which provides hydraulic fluid pressure to using systems, but does not include the using systems. Includes power packs incorporating integral pumps, electric motors and solenoids used in certain light aircraft models. Also includes pumps such as those used in flight control systems on large aircraft. Typical parts are pump, motor, shaft, brush, solenoid, case, power pack, seals and switches.</rdfs:comment>
        <m:has_related_eccairs_term rdf:resource="http://onto.fel.cvut.cz/ontologies/2014/ECCAIRS_Aviation_1.3.0.12/eccairs-descriptive-factors#category_11291300"/>
    </owl:Class>
    


    <!-- http://onto.fel.cvut.cz/ontologies/aviation-safety/Maintenance_information_system -->

    <owl:Class rdf:about="&m;Maintenance_information_system">
        <rdfs:label>Maintenance information system</rdfs:label>
        <rdfs:subClassOf rdf:resource="&m;Information_system_part"/>
        <m:generated_time rdf:datatype="&xsd;dateTime">2015-04-09T18:56:27.771+02:00</m:generated_time>
        <rdfs:comment xml:lang="en">(ATA Code:4630) Maintenance information system: The portion of the onboard flight information system that supports all onboard maintenance system functions, maintenance technicians, and any ground based maintenance activity. Maintenance. The performance of tasks required to ensure the continuing airworthiness of an aircraft, including any one or combination of overhaul, inspection, replacement, defect rectification, and the embodiment of a modification or repair. (Annex 8)</rdfs:comment>
        <m:has_related_eccairs_term rdf:resource="http://onto.fel.cvut.cz/ontologies/2014/ECCAIRS_Aviation_1.3.0.12/eccairs-descriptive-factors#category_11463000"/>
    </owl:Class>
    


    <!-- http://onto.fel.cvut.cz/ontologies/aviation-safety/Marker_beacon_system -->

    <owl:Class rdf:about="&m;Marker_beacon_system">
        <rdfs:label>Marker beacon system</rdfs:label>
        <rdfs:subClassOf rdf:resource="&m;Landing_and_taxi_aid"/>
        <rdfs:subClassOf>
            <owl:Restriction>
                <owl:onProperty rdf:resource="&m;communicates_with"/>
                <owl:someValuesFrom rdf:resource="&m;Navaids_marker_beacon"/>
            </owl:Restriction>
        </rdfs:subClassOf>
        <m:generated_time rdf:datatype="&xsd;dateTime">2015-04-09T18:56:27.771+02:00</m:generated_time>
        <rdfs:comment xml:lang="en">(ATA Code:3434) Marker beacon system: The system which provides an aural and visual indication of passage over specified points on the glide path for landing under instrument meteorological conditions. Does not includes control panel when it is an integral portion of the audio control panel [Code 11235000]. Typical parts are marker beacon antenna, receivers, visual/aural indication units, marker light and control panel.</rdfs:comment>
        <m:has_related_eccairs_term rdf:resource="http://onto.fel.cvut.cz/ontologies/2014/ECCAIRS_Aviation_1.3.0.12/eccairs-descriptive-factors#category_11343400"/>
    </owl:Class>
    


    <!-- http://onto.fel.cvut.cz/ontologies/aviation-safety/Marking -->

    <owl:Class rdf:about="&m;Marking"/>
    


    <!-- http://onto.fel.cvut.cz/ontologies/aviation-safety/Microwave_landing_system -->

    <owl:Class rdf:about="&m;Microwave_landing_system">
        <rdfs:label>Microwave landing system aircraft equipment</rdfs:label>
        <rdfs:subClassOf rdf:resource="&m;Landing_and_taxi_aid"/>
        <rdfs:subClassOf>
            <owl:Restriction>
                <owl:onProperty rdf:resource="&m;communicates_with"/>
                <owl:someValuesFrom rdf:resource="&m;microwave_landing_system_ground_system"/>
            </owl:Restriction>
        </rdfs:subClassOf>
    </owl:Class>
    


    <!-- http://onto.fel.cvut.cz/ontologies/aviation-safety/Miscellaneous_Wiring -->

    <owl:Class rdf:about="&m;Miscellaneous_Wiring">
        <rdfs:subClassOf rdf:resource="&m;Miscellaneous_hardware_part"/>
    </owl:Class>
    


    <!-- http://onto.fel.cvut.cz/ontologies/aviation-safety/Miscellaneous_cabin_system -->

    <owl:Class rdf:about="&m;Miscellaneous_cabin_system">
        <rdfs:label>Miscellaneous cabin system</rdfs:label>
        <rdfs:subClassOf rdf:resource="&m;cabin_system"/>
        <m:generated_time rdf:datatype="&xsd;dateTime">2015-04-09T18:56:27.771+02:00</m:generated_time>
        <rdfs:comment xml:lang="en">(ATA Code:4460) Miscellaneous cabin system: The portion of the cabin system used to support miscellaneous cabin functions.</rdfs:comment>
        <m:has_related_eccairs_term rdf:resource="http://onto.fel.cvut.cz/ontologies/2014/ECCAIRS_Aviation_1.3.0.12/eccairs-descriptive-factors#category_11446000"/>
    </owl:Class>
    


    <!-- http://onto.fel.cvut.cz/ontologies/aviation-safety/Miscellaneous_hardware -->

    <owl:Class rdf:about="&m;Miscellaneous_hardware">
        <rdfs:label>Miscellaneous hardware</rdfs:label>
        <rdfs:subClassOf rdf:resource="&m;Aircraft_part"/>
        <m:generated_time rdf:datatype="&xsd;dateTime">2015-04-09T18:56:27.771+02:00</m:generated_time>
        <rdfs:comment xml:lang="en">(ATA Code:1400) For miscellaneous parts that are not associated with an installed aircraft component or system.</rdfs:comment>
        <m:has_related_eccairs_term rdf:resource="http://onto.fel.cvut.cz/ontologies/2014/ECCAIRS_Aviation_1.3.0.12/eccairs-descriptive-factors#category_11140000"/>
    </owl:Class>
    


    <!-- http://onto.fel.cvut.cz/ontologies/aviation-safety/Miscellaneous_hardware_part -->

    <owl:Class rdf:about="&m;Miscellaneous_hardware_part">
        <rdfs:label>Miscellaneous hardware part</rdfs:label>
        <rdfs:subClassOf rdf:resource="&m;Aircraft_part"/>
        <rdfs:subClassOf>
            <owl:Restriction>
                <owl:onProperty rdf:resource="http://onto.fel.cvut.cz/ontologies/ufo/is_part_of"/>
                <owl:someValuesFrom rdf:resource="&m;Miscellaneous_hardware"/>
            </owl:Restriction>
        </rdfs:subClassOf>
        <m:generated_time rdf:datatype="&xsd;dateTime">2015-04-12T02:45:54.351+02:00</m:generated_time>
        <m:has_related_eccairs_term rdf:resource="http://onto.fel.cvut.cz/ontologies/2014/ECCAIRS_Aviation_1.3.0.12/eccairs-descriptive-factors#category_11140000"/>
    </owl:Class>
    


    <!-- http://onto.fel.cvut.cz/ontologies/aviation-safety/Miscellaneous_information_system -->

    <owl:Class rdf:about="&m;Miscellaneous_information_system">
        <rdfs:label>Miscellaneous information system</rdfs:label>
        <rdfs:subClassOf rdf:resource="&m;Information_system_part"/>
        <m:generated_time rdf:datatype="&xsd;dateTime">2015-04-09T18:56:27.771+02:00</m:generated_time>
        <rdfs:comment xml:lang="en">(ATA Code:4650) Miscellaneous information system: The portion of the onboard information system that supports other functions, as defined by the user, that cannot be related to the flight deck, passenger cabin, or maintenance.</rdfs:comment>
        <m:has_related_eccairs_term rdf:resource="http://onto.fel.cvut.cz/ontologies/2014/ECCAIRS_Aviation_1.3.0.12/eccairs-descriptive-factors#category_11465000"/>
    </owl:Class>
    


    <!-- http://onto.fel.cvut.cz/ontologies/aviation-safety/Mixture_control -->

    <owl:Class rdf:about="&m;Mixture_control">
        <rdfs:label>Mixture control</rdfs:label>
        <rdfs:subClassOf rdf:resource="&m;Engine_controls_part"/>
        <m:generated_time rdf:datatype="&xsd;dateTime">2015-04-09T18:56:27.771+02:00</m:generated_time>
        <rdfs:comment xml:lang="en">(ATA Code:7602) Mixture control: The control for adjusting fuel-air mixture in piston engines. Includes linkage from the cockpit lever to the carburetor or fuel injector servo but does not include the arm on mixture control shafts. Typical parts are cable, rod, bellcrank, rod end, housing, clamp and cockpit control lever/knob.</rdfs:comment>
        <m:has_related_eccairs_term rdf:resource="http://onto.fel.cvut.cz/ontologies/2014/ECCAIRS_Aviation_1.3.0.12/eccairs-descriptive-factors#category_11760200"/>
    </owl:Class>
    


    <!-- http://onto.fel.cvut.cz/ontologies/aviation-safety/Moisture-Air_Contaminant_Control -->

    <owl:Class rdf:about="&m;Moisture-Air_Contaminant_Control">
        <rdfs:label>Moisture/Air Contaminant Control</rdfs:label>
        <rdfs:subClassOf rdf:resource="&m;Air_conditioning_system_part"/>
        <m:generated_time rdf:datatype="&xsd;dateTime">2015-04-09T18:56:27.771+02:00</m:generated_time>
        <rdfs:comment xml:lang="en">(ATA Code:2170) That portion of the system used to control moisture in the air, to control ozone concentrations, to filter radioactive debris from conditioned air, and to treat the air with deodorizers, insecticides, etc.</rdfs:comment>
        <m:has_related_eccairs_term rdf:resource="http://onto.fel.cvut.cz/ontologies/2014/ECCAIRS_Aviation_1.3.0.12/eccairs-descriptive-factors#category_11217000"/>
    </owl:Class>
    


    <!-- http://onto.fel.cvut.cz/ontologies/aviation-safety/Mooring -->

    <owl:Class rdf:about="&m;Mooring">
        <rdfs:subClassOf rdf:resource="&m;Aircraft_operation"/>
    </owl:Class>
    


    <!-- http://onto.fel.cvut.cz/ontologies/aviation-safety/Nacelle-Pylon,_Miscellaneous_Structure -->

    <owl:Class rdf:about="&m;Nacelle-Pylon,_Miscellaneous_Structure">
        <rdfs:label>Nacelle/Pylon, Miscellaneous Structure</rdfs:label>
        <rdfs:subClassOf rdf:resource="&m;Nacelle-pylon_structure_part"/>
        <m:generated_time rdf:datatype="&xsd;dateTime">2015-04-09T18:56:27.771+02:00</m:generated_time>
        <rdfs:comment xml:lang="en">(ATA Code:5420) Miscellaneous structure on the nacelle/pylon structure which aids in the support of the primary structure.   Includes such items as brackets, channels, stiffeners, doublers, clips, etc.</rdfs:comment>
        <m:has_related_eccairs_term rdf:resource="http://onto.fel.cvut.cz/ontologies/2014/ECCAIRS_Aviation_1.3.0.12/eccairs-descriptive-factors#category_11542000"/>
    </owl:Class>
    


    <!-- http://onto.fel.cvut.cz/ontologies/aviation-safety/Nacelle-Pylon,_System_Wiring -->

    <owl:Class rdf:about="&m;Nacelle-Pylon,_System_Wiring">
        <rdfs:label>Nacelle/Pylon, System Wiring</rdfs:label>
        <rdfs:subClassOf rdf:resource="&m;Nacelle-pylon_structure_part"/>
        <m:generated_time rdf:datatype="&xsd;dateTime">2015-04-09T18:56:27.771+02:00</m:generated_time>
        <rdfs:comment xml:lang="en">(ATA Code:5497) Wiring specific to the Nacelle/Pylon System</rdfs:comment>
        <m:has_related_eccairs_term rdf:resource="http://onto.fel.cvut.cz/ontologies/2014/ECCAIRS_Aviation_1.3.0.12/eccairs-descriptive-factors#category_11549700"/>
    </owl:Class>
    


    <!-- http://onto.fel.cvut.cz/ontologies/aviation-safety/Nacelle-pylon_attachment_fitting_(wing) -->

    <owl:Class rdf:about="&m;Nacelle-pylon_attachment_fitting_(wing)">
        <rdfs:label>Nacelle/pylon attachment fitting [wing)</rdfs:label>
        <rdfs:subClassOf rdf:resource="&m;Wing_attachment_fitting_part"/>
        <m:generated_time rdf:datatype="&xsd;dateTime">2015-04-09T18:56:27.771+02:00</m:generated_time>
        <rdfs:comment xml:lang="en">(ATA Code:5742) The fittings on the wing used for attachment of the nacelle/pylon.</rdfs:comment>
        <m:has_related_eccairs_term rdf:resource="http://onto.fel.cvut.cz/ontologies/2014/ECCAIRS_Aviation_1.3.0.12/eccairs-descriptive-factors#category_11574200"/>
    </owl:Class>
    


    <!-- http://onto.fel.cvut.cz/ontologies/aviation-safety/Nacelle-pylon_fairing -->

    <owl:Class rdf:about="&m;Nacelle-pylon_fairing">
        <rdfs:label>Nacelle/pylon fairing</rdfs:label>
        <rdfs:subClassOf rdf:resource="&m;Main_frame_(nacelle-pylon)_part"/>
        <m:generated_time rdf:datatype="&xsd;dateTime">2015-04-09T18:56:27.771+02:00</m:generated_time>
        <rdfs:comment xml:lang="en">(ATA Code:5416) Nacelle/pylon fairing: The panels mounted on the nacelle/pylon to optimize the airflow around these structures.</rdfs:comment>
        <m:has_related_eccairs_term rdf:resource="http://onto.fel.cvut.cz/ontologies/2014/ECCAIRS_Aviation_1.3.0.12/eccairs-descriptive-factors#category_11541600"/>
    </owl:Class>
    


    <!-- http://onto.fel.cvut.cz/ontologies/aviation-safety/Nacelle-pylon_structure -->

    <owl:Class rdf:about="&m;Nacelle-pylon_structure">
        <rdfs:label>Nacelle/pylon structure</rdfs:label>
        <rdfs:subClassOf rdf:resource="&m;Aircraft_part"/>
        <m:generated_time rdf:datatype="&xsd;dateTime">2015-04-09T18:56:27.771+02:00</m:generated_time>
        <rdfs:comment xml:lang="en">(ATA Code:5400) Nacelle/pylon structure: The structural units and associated components and members which furnish a means of mounting and housing the power plant or rotor assembly. Includes skins, longerons, belt frames, stringers, clamshells, scuppers, doors, nacelle fillets, attachment fittings and the structure of power plant cowling inclusive of the structural portion of the inlet whether or not integral with the aircraft. Structural portions of the exhaust system are excluded where they are not integral with the airframe.</rdfs:comment>
        <m:has_related_eccairs_term rdf:resource="http://onto.fel.cvut.cz/ontologies/2014/ECCAIRS_Aviation_1.3.0.12/eccairs-descriptive-factors#category_11540000"/>
    </owl:Class>
    


    <!-- http://onto.fel.cvut.cz/ontologies/aviation-safety/Nacelle-pylon_structure_part -->

    <owl:Class rdf:about="&m;Nacelle-pylon_structure_part">
        <rdfs:label>Nacelle/pylon structure part</rdfs:label>
        <rdfs:subClassOf rdf:resource="&m;Aircraft_part"/>
        <rdfs:subClassOf>
            <owl:Restriction>
                <owl:onProperty rdf:resource="http://onto.fel.cvut.cz/ontologies/ufo/is_part_of"/>
                <owl:someValuesFrom rdf:resource="&m;Nacelle-pylon_structure"/>
            </owl:Restriction>
        </rdfs:subClassOf>
        <m:generated_time rdf:datatype="&xsd;dateTime">2015-04-12T02:45:54.351+02:00</m:generated_time>
        <m:has_related_eccairs_term rdf:resource="http://onto.fel.cvut.cz/ontologies/2014/ECCAIRS_Aviation_1.3.0.12/eccairs-descriptive-factors#category_11540000"/>
    </owl:Class>
    


    <!-- http://onto.fel.cvut.cz/ontologies/aviation-safety/Navaids_marker_beacon -->

    <owl:Class rdf:about="&m;Navaids_marker_beacon"/>
    


    <!-- http://onto.fel.cvut.cz/ontologies/aviation-safety/Navigation_System_Wiring -->

    <owl:Class rdf:about="&m;Navigation_System_Wiring">
        <rdfs:label>Navigation System Wiring</rdfs:label>
        <rdfs:subClassOf rdf:resource="&m;Navigation_system"/>
        <rdfs:subClassOf rdf:resource="&m;Wiring"/>
        <rdfs:subClassOf>
            <owl:Restriction>
                <owl:onProperty rdf:resource="http://onto.fel.cvut.cz/ontologies/ufo/is_part_of"/>
                <owl:someValuesFrom rdf:resource="&m;Navigation_system"/>
            </owl:Restriction>
        </rdfs:subClassOf>
        <m:generated_time rdf:datatype="&xsd;dateTime">2015-04-09T18:56:27.771+02:00</m:generated_time>
        <rdfs:comment xml:lang="en">(ATA Code:3497) Wiring specific to the Navigation Systems.</rdfs:comment>
        <m:has_related_eccairs_term rdf:resource="http://onto.fel.cvut.cz/ontologies/2014/ECCAIRS_Aviation_1.3.0.12/eccairs-descriptive-factors#category_11349700"/>
    </owl:Class>
    


    <!-- http://onto.fel.cvut.cz/ontologies/aviation-safety/Navigation_system -->

    <owl:Class rdf:about="&m;Navigation_system">
        <rdfs:label>Navigation system</rdfs:label>
        <rdfs:subClassOf rdf:resource="&m;Aircraft_part"/>
        <m:generated_time rdf:datatype="&xsd;dateTime">2015-04-09T18:56:27.771+02:00</m:generated_time>
        <rdfs:comment xml:lang="en">(ATA Code:3400) Navigation system: The units and components which provide aircraft navigational information.</rdfs:comment>
        <m:has_related_eccairs_term rdf:resource="http://onto.fel.cvut.cz/ontologies/2014/ECCAIRS_Aviation_1.3.0.12/eccairs-descriptive-factors#category_11340000"/>
    </owl:Class>
    


    <!-- http://onto.fel.cvut.cz/ontologies/aviation-safety/Non-radar_weather_system -->

    <owl:Class rdf:about="&m;Non-radar_weather_system">
        <rdfs:label>Non-radar weather system</rdfs:label>
        <rdfs:subClassOf rdf:resource="&m;Independent_position_determining_system"/>
        <m:generated_time rdf:datatype="&xsd;dateTime">2015-04-09T18:56:27.771+02:00</m:generated_time>
        <rdfs:comment xml:lang="en">(ATA Code:3446) Non-radar weather system: The non-radar weather system and components which sense the electrostatic charges accumulated around a storm cell in order to &quot;map out&quot; that cell on an indicator.</rdfs:comment>
        <m:has_related_eccairs_term rdf:resource="http://onto.fel.cvut.cz/ontologies/2014/ECCAIRS_Aviation_1.3.0.12/eccairs-descriptive-factors#category_11344600"/>
    </owl:Class>
    


    <!-- http://onto.fel.cvut.cz/ontologies/aviation-safety/Not_used -->

    <owl:Class rdf:about="&m;Not_used">
        <rdfs:label>Not used</rdfs:label>
        <rdfs:subClassOf rdf:resource="&m;Cargo_and_accessory_compartments_part"/>
        <m:generated_time rdf:datatype="&xsd;dateTime">2015-04-09T18:56:27.771+02:00</m:generated_time>
        <rdfs:comment xml:lang="en">(ATA Code:5040) This group is not in use at present</rdfs:comment>
        <m:has_related_eccairs_term rdf:resource="http://onto.fel.cvut.cz/ontologies/2014/ECCAIRS_Aviation_1.3.0.12/eccairs-descriptive-factors#category_11504000"/>
    </owl:Class>
    


    <!-- http://onto.fel.cvut.cz/ontologies/aviation-safety/Omega_navigation_system -->

    <owl:Class rdf:about="&m;Omega_navigation_system">
        <rdfs:label>Omega navigation system</rdfs:label>
        <rdfs:subClassOf rdf:resource="&m;Dependent_position_determining_system"/>
        <m:generated_time rdf:datatype="&xsd;dateTime">2015-04-09T18:56:27.771+02:00</m:generated_time>
        <rdfs:comment xml:lang="en">(ATA Code:3456) Omega navigation system: The navigation system which provides for geographical location of the aircraft down to sea level on a worldwide basis when operating on signals from eight ground-based OMEGA very low frequency transmitting stations. Typical parts are antenna, control unit or receiver, coaxial connecting cable, remote switches and connectors.</rdfs:comment>
        <m:has_related_eccairs_term rdf:resource="http://onto.fel.cvut.cz/ontologies/2014/ECCAIRS_Aviation_1.3.0.12/eccairs-descriptive-factors#category_11345600"/>
    </owl:Class>
    


    <!-- http://onto.fel.cvut.cz/ontologies/aviation-safety/Other_navigation_systems -->

    <owl:Class rdf:about="&m;Other_navigation_systems">
        <rdfs:label>Other navigation systems</rdfs:label>
        <rdfs:subClassOf rdf:resource="&m;Navigation_system"/>
        <m:generated_time rdf:datatype="&xsd;dateTime">2015-04-09T18:56:27.771+02:00</m:generated_time>
        <rdfs:comment xml:lang="en">(ATA Code:3470) Other navigation systems: The navigation systems other than those mentioned above.</rdfs:comment>
        <m:has_related_eccairs_term rdf:resource="http://onto.fel.cvut.cz/ontologies/2014/ECCAIRS_Aviation_1.3.0.12/eccairs-descriptive-factors#category_11347000"/>
    </owl:Class>
    


    <!-- http://onto.fel.cvut.cz/ontologies/aviation-safety/Outside_air_temperature_indicator-sensor -->

    <owl:Class rdf:about="&m;Outside_air_temperature_indicator-sensor">
        <rdfs:label>Outside air temperature indicator/sensor</rdfs:label>
        <rdfs:subClassOf rdf:resource="&m;Flight_environment_data_system"/>
        <m:generated_time rdf:datatype="&xsd;dateTime">2015-04-09T18:56:27.771+02:00</m:generated_time>
        <rdfs:comment xml:lang="en">(ATA Code:3412) Outside air temperature indicator/sensor: The unit mounted in the engine induction air intake to sense and transmit temperature to the cockpit indicator. Also for the sensors and instruments which measure and indicate the temperature of ambient air outside the aircraft. Includes associated circuitry and related parts. Typical parts are sensor, indicator and case.</rdfs:comment>
        <m:has_related_eccairs_term rdf:resource="http://onto.fel.cvut.cz/ontologies/2014/ECCAIRS_Aviation_1.3.0.12/eccairs-descriptive-factors#category_11341200"/>
    </owl:Class>
    


    <!-- http://onto.fel.cvut.cz/ontologies/aviation-safety/Overheat_detection_system -->

    <owl:Class rdf:about="&m;Overheat_detection_system">
        <rdfs:label>Overheat detection system</rdfs:label>
        <rdfs:subClassOf rdf:resource="&m;Fire-smoke-overheat_detection_system_part"/>
        <m:generated_time rdf:datatype="&xsd;dateTime">2015-04-09T18:56:27.771+02:00</m:generated_time>
        <rdfs:comment xml:lang="en">(ATA Code:2613) Overheat detection system: The system used to sense and indicate the presence of an overheat condition in any of the protected areas of the aircraft. Typical parts are detectors, sensors, wiring, relays, amplifiers and test circuits.</rdfs:comment>
        <m:has_related_eccairs_term rdf:resource="http://onto.fel.cvut.cz/ontologies/2014/ECCAIRS_Aviation_1.3.0.12/eccairs-descriptive-factors#category_11261300"/>
    </owl:Class>
    


    <!-- http://onto.fel.cvut.cz/ontologies/aviation-safety/Oxygen_System_Wiring -->

    <owl:Class rdf:about="&m;Oxygen_System_Wiring">
        <rdfs:label>Oxygen System Wiring</rdfs:label>
        <rdfs:subClassOf rdf:resource="&m;Oxygen_system_part"/>
        <m:generated_time rdf:datatype="&xsd;dateTime">2015-04-09T18:56:27.771+02:00</m:generated_time>
        <rdfs:comment xml:lang="en">(ATA Code:3597) Wiring specific to the Oxygen System.</rdfs:comment>
        <m:has_related_eccairs_term rdf:resource="http://onto.fel.cvut.cz/ontologies/2014/ECCAIRS_Aviation_1.3.0.12/eccairs-descriptive-factors#category_11359700"/>
    </owl:Class>
    


    <!-- http://onto.fel.cvut.cz/ontologies/aviation-safety/Oxygen_system -->

    <owl:Class rdf:about="&m;Oxygen_system">
        <rdfs:label>Oxygen system</rdfs:label>
        <rdfs:subClassOf rdf:resource="&m;Aircraft_part"/>
        <m:generated_time rdf:datatype="&xsd;dateTime">2015-04-09T18:56:27.771+02:00</m:generated_time>
        <rdfs:comment xml:lang="en">(ATA Code:3500) Oxygen system: The units and components which store, regulate, and deliver breathing oxygen to the passengers and crew. Typical parts are bottles, relief valves, shut-off valves, outlets, regulators, masks and walk-around bottles.</rdfs:comment>
        <m:has_related_eccairs_term rdf:resource="http://onto.fel.cvut.cz/ontologies/2014/ECCAIRS_Aviation_1.3.0.12/eccairs-descriptive-factors#category_11350000"/>
    </owl:Class>
    


    <!-- http://onto.fel.cvut.cz/ontologies/aviation-safety/Oxygen_system_part -->

    <owl:Class rdf:about="&m;Oxygen_system_part">
        <rdfs:label>Oxygen system part</rdfs:label>
        <rdfs:subClassOf rdf:resource="&m;Aircraft_part"/>
        <rdfs:subClassOf>
            <owl:Restriction>
                <owl:onProperty rdf:resource="http://onto.fel.cvut.cz/ontologies/ufo/is_part_of"/>
                <owl:someValuesFrom rdf:resource="&m;Oxygen_system"/>
            </owl:Restriction>
        </rdfs:subClassOf>
        <m:generated_time rdf:datatype="&xsd;dateTime">2015-04-12T02:45:54.351+02:00</m:generated_time>
        <m:has_related_eccairs_term rdf:resource="http://onto.fel.cvut.cz/ontologies/2014/ECCAIRS_Aviation_1.3.0.12/eccairs-descriptive-factors#category_11350000"/>
    </owl:Class>
    


    <!-- http://onto.fel.cvut.cz/ontologies/aviation-safety/Parachute -->

    <owl:Class rdf:about="&m;Parachute">
        <rdfs:label>Parachute</rdfs:label>
        <rdfs:subClassOf rdf:resource="&m;Emergency_equipment"/>
        <m:generated_time rdf:datatype="&xsd;dateTime">2015-04-09T18:56:27.771+02:00</m:generated_time>
        <rdfs:comment xml:lang="en">(ATA Code:2563) The parachutes used for aircraft occupants to escape from the aircraft while it is airborne.</rdfs:comment>
        <m:has_related_eccairs_term rdf:resource="http://onto.fel.cvut.cz/ontologies/2014/ECCAIRS_Aviation_1.3.0.12/eccairs-descriptive-factors#category_11256300"/>
    </owl:Class>
    


    <!-- http://onto.fel.cvut.cz/ontologies/aviation-safety/Parking_mooring_storage_and_return_to_service -->

    <owl:Class rdf:about="&m;Parking_mooring_storage_and_return_to_service">
        <rdfs:label xml:lang="en">Parking, mooring, storage and return to service instructions</rdfs:label>
        <rdfs:subClassOf rdf:resource="&m;Aircraft_part"/>
        <rdfs:subClassOf>
            <owl:Class>
                <owl:intersectionOf rdf:parseType="Collection">
                    <rdf:Description rdf:about="&m;regulation"/>
                    <owl:Restriction>
                        <owl:onProperty rdf:resource="&m;prescribes"/>
                        <owl:someValuesFrom>
                            <owl:Class>
                                <owl:intersectionOf rdf:parseType="Collection">
                                    <rdf:Description rdf:about="&m;Operation"/>
                                    <owl:Restriction>
                                        <owl:onProperty rdf:resource="http://onto.fel.cvut.cz/ontologies/ufo/is_performed_by"/>
                                        <owl:someValuesFrom rdf:resource="&m;Aircraft"/>
                                    </owl:Restriction>
                                </owl:intersectionOf>
                            </owl:Class>
                        </owl:someValuesFrom>
                    </owl:Restriction>
                </owl:intersectionOf>
            </owl:Class>
        </rdfs:subClassOf>
        <m:generated_time rdf:datatype="&xsd;dateTime">2015-04-09T18:56:27.771+02:00</m:generated_time>
        <m:generated_time rdf:datatype="&xsd;dateTime">2015-04-12T02:45:54.351+02:00</m:generated_time>
        <rdfs:comment xml:lang="en">(ATA Code:1000) Those instructions necessary to park, store, moor and prepare the aircraft for service in any of the conditions to which it may be subjected. Charts showing location of landing gear and control surface locks, blanking plugs and covers, mooring points, etc., shall be included. Includes those maintenance practices necessary to prepare the aircraft for parking, mooring, or storage.</rdfs:comment>
        <m:has_related_eccairs_term rdf:resource="http://onto.fel.cvut.cz/ontologies/2014/ECCAIRS_Aviation_1.3.0.12/eccairs-descriptive-factors#category_11100000"/>
    </owl:Class>
    


    <!-- http://onto.fel.cvut.cz/ontologies/aviation-safety/Passenger-crew_doors -->

    <owl:Class rdf:about="&m;Passenger-crew_doors">
        <rdfs:label>Passenger/crew doors</rdfs:label>
        <rdfs:subClassOf rdf:resource="&m;Fuselage_doors_part"/>
        <m:generated_time rdf:datatype="&xsd;dateTime">2015-04-09T18:56:27.771+02:00</m:generated_time>
        <rdfs:comment xml:lang="en">(ATA Code:5210) Passenger/crew doors: The cabin entrance doors not including door frames, warning systems, or cabin emergency exit doors/hatches. Typical parts are hinges, actuators, latches, handle, seals, structure, spring, cable, bellcrank and skin.</rdfs:comment>
        <m:has_related_eccairs_term rdf:resource="http://onto.fel.cvut.cz/ontologies/2014/ECCAIRS_Aviation_1.3.0.12/eccairs-descriptive-factors#category_11521000"/>
    </owl:Class>
    


    <!-- http://onto.fel.cvut.cz/ontologies/aviation-safety/Passenger_Address,_Entertainment_and_Comfort -->

    <owl:Class rdf:about="&m;Passenger_Address,_Entertainment_and_Comfort">
        <rdfs:label>Passenger Address, Entertainment and Comfort</rdfs:label>
        <rdfs:subClassOf rdf:resource="&m;Aircraft_communication_related_system"/>
        <m:generated_time rdf:datatype="&xsd;dateTime">2015-04-09T18:56:27.771+02:00</m:generated_time>
        <rdfs:comment xml:lang="en">(ATA Code:2330) Passenger entertainment system or components such as amplifier, cassette recorder player, control panel, speaker, video equipment, etc.</rdfs:comment>
        <m:has_related_eccairs_term rdf:resource="http://onto.fel.cvut.cz/ontologies/2014/ECCAIRS_Aviation_1.3.0.12/eccairs-descriptive-factors#category_11233000"/>
    </owl:Class>
    


    <!-- http://onto.fel.cvut.cz/ontologies/aviation-safety/Passenger_address,_entertainment_and_comfort_systems -->

    <owl:Class rdf:about="&m;Passenger_address,_entertainment_and_comfort_systems">
        <rdfs:label>Passenger address, entertainment and comfort systems</rdfs:label>
        <rdfs:subClassOf rdf:resource="&m;cabin_system"/>
        <m:generated_time rdf:datatype="&xsd;dateTime">2015-04-09T18:56:27.771+02:00</m:generated_time>
        <rdfs:comment xml:lang="en">(ATA Code:4430) The passenger address, comfort and entertainment systems or components such as amplifier, cassette recorder player, control panel, speaker and video equipment.</rdfs:comment>
        <m:has_related_eccairs_term rdf:resource="http://onto.fel.cvut.cz/ontologies/2014/ECCAIRS_Aviation_1.3.0.12/eccairs-descriptive-factors#category_11443000"/>
    </owl:Class>
    


    <!-- http://onto.fel.cvut.cz/ontologies/aviation-safety/Passenger_cabin_information_system -->

    <owl:Class rdf:about="&m;Passenger_cabin_information_system">
        <rdfs:label>Passenger cabin information system</rdfs:label>
        <rdfs:subClassOf rdf:resource="&m;Information_system_part"/>
        <m:generated_time rdf:datatype="&xsd;dateTime">2015-04-09T18:56:27.771+02:00</m:generated_time>
        <rdfs:comment xml:lang="en">(ATA Code:4640) Passenger cabin information system: The portion of the onboard information system that supports passenger cabin information systems.</rdfs:comment>
        <m:has_related_eccairs_term rdf:resource="http://onto.fel.cvut.cz/ontologies/2014/ECCAIRS_Aviation_1.3.0.12/eccairs-descriptive-factors#category_11464000"/>
    </owl:Class>
    


    <!-- http://onto.fel.cvut.cz/ontologies/aviation-safety/Passenger_compartment_equipment -->

    <owl:Class rdf:about="&m;Passenger_compartment_equipment">
        <rdfs:label>Passenger compartment equipment</rdfs:label>
        <rdfs:subClassOf rdf:resource="&m;Cabin_equipment-furnishings"/>
        <m:generated_time rdf:datatype="&xsd;dateTime">2015-04-09T18:56:27.771+02:00</m:generated_time>
        <rdfs:comment xml:lang="en">(ATA Code:2520) Passenger compartment equipment: The removable general equipment and furnishings within the cabin. Typical parts are seats, seat belts, hat rack, coat closet, panels and passenger comfort items such as personal blankets and pillows.</rdfs:comment>
        <m:has_related_eccairs_term rdf:resource="http://onto.fel.cvut.cz/ontologies/2014/ECCAIRS_Aviation_1.3.0.12/eccairs-descriptive-factors#category_11252000"/>
    </owl:Class>
    


    <!-- http://onto.fel.cvut.cz/ontologies/aviation-safety/Passenger_compartment_lighting -->

    <owl:Class rdf:about="&m;Passenger_compartment_lighting">
        <rdfs:label>Passenger compartment lighting</rdfs:label>
        <rdfs:subClassOf rdf:resource="&m;Lighting_system"/>
        <m:generated_time rdf:datatype="&xsd;dateTime">2015-04-09T18:56:27.771+02:00</m:generated_time>
        <rdfs:comment xml:lang="en">(ATA Code:3320) Passenger compartment lighting: The lighting systems in the passenger seating compartment, lavatories, buffet/galley compartments and cabin carry-on baggage/coat areas. Includes lamps for illumination of cabin, reading lamps, seat belt/no-smoking signs and passenger call systems. Does not include emergency lighting [Code 11335000]. Typical parts are ballast, switch, transformer and lamps.</rdfs:comment>
        <m:has_related_eccairs_term rdf:resource="http://onto.fel.cvut.cz/ontologies/2014/ECCAIRS_Aviation_1.3.0.12/eccairs-descriptive-factors#category_11332000"/>
    </owl:Class>
    


    <!-- http://onto.fel.cvut.cz/ontologies/aviation-safety/Passenger_compartment_windows -->

    <owl:Class rdf:about="&m;Passenger_compartment_windows">
        <rdfs:label>Passenger compartment windows</rdfs:label>
        <rdfs:subClassOf rdf:resource="&m;Window-windshield_system_part"/>
        <m:generated_time rdf:datatype="&xsd;dateTime">2015-04-09T18:56:27.771+02:00</m:generated_time>
        <rdfs:comment xml:lang="en">(ATA Code:5620) Passenger compartment windows: The cabin mounted windows in the passenger compartments. Includes the inner and outer windows, frame attaching hardware, picture windows. Does not include the windows in the escape hatches [Code 11522000].</rdfs:comment>
        <m:has_related_eccairs_term rdf:resource="http://onto.fel.cvut.cz/ontologies/2014/ECCAIRS_Aviation_1.3.0.12/eccairs-descriptive-factors#category_11562000"/>
    </owl:Class>
    


    <!-- http://onto.fel.cvut.cz/ontologies/aviation-safety/Passenger_oxygen_system -->

    <owl:Class rdf:about="&m;Passenger_oxygen_system">
        <rdfs:label>Passenger oxygen system</rdfs:label>
        <rdfs:subClassOf rdf:resource="&m;Oxygen_system_part"/>
        <m:generated_time rdf:datatype="&xsd;dateTime">2015-04-09T18:56:27.771+02:00</m:generated_time>
        <rdfs:comment xml:lang="en">(ATA Code:3520) Passenger oxygen system: The portion of the main system which furnishes oxygen to the passengers.</rdfs:comment>
        <m:has_related_eccairs_term rdf:resource="http://onto.fel.cvut.cz/ontologies/2014/ECCAIRS_Aviation_1.3.0.12/eccairs-descriptive-factors#category_11352000"/>
    </owl:Class>
    


    <!-- http://onto.fel.cvut.cz/ontologies/aviation-safety/Phase_adapter -->

    <owl:Class rdf:about="&m;Phase_adapter">
        <rdfs:label>Phase adapter</rdfs:label>
        <rdfs:subClassOf rdf:resource="&m;Alternating_current_generation_system_part"/>
        <m:generated_time rdf:datatype="&xsd;dateTime">2015-04-09T18:56:27.771+02:00</m:generated_time>
        <rdfs:comment xml:lang="en">(ATA Code:2423) Phase adapter: The component used to change the alternating current phase of output for specific equipment.</rdfs:comment>
        <m:has_related_eccairs_term rdf:resource="http://onto.fel.cvut.cz/ontologies/2014/ECCAIRS_Aviation_1.3.0.12/eccairs-descriptive-factors#category_11242300"/>
    </owl:Class>
    


    <!-- http://onto.fel.cvut.cz/ontologies/aviation-safety/Pitot-static_anti-ice_system -->

    <owl:Class rdf:about="&m;Pitot-static_anti-ice_system">
        <rdfs:label>Pitot/static anti-ice system</rdfs:label>
        <rdfs:subClassOf rdf:resource="&m;Ice-rain_protection_systems"/>
        <m:generated_time rdf:datatype="&xsd;dateTime">2015-04-09T18:56:27.771+02:00</m:generated_time>
        <rdfs:comment xml:lang="en">(ATA Code:3030) Pitot/static anti-ice system: The heating elements in the pitot-static heads installed to remove or prevent the formation of ice. Typical parts are element, switch and wiring.</rdfs:comment>
        <m:has_related_eccairs_term rdf:resource="http://onto.fel.cvut.cz/ontologies/2014/ECCAIRS_Aviation_1.3.0.12/eccairs-descriptive-factors#category_11303000"/>
    </owl:Class>
    


    <!-- http://onto.fel.cvut.cz/ontologies/aviation-safety/Pitot-static_system -->

    <owl:Class rdf:about="&m;Pitot-static_system">
        <rdfs:label>Pitot/static system</rdfs:label>
        <rdfs:subClassOf rdf:resource="&m;Flight_environment_data_system"/>
        <m:generated_time rdf:datatype="&xsd;dateTime">2015-04-09T18:56:27.771+02:00</m:generated_time>
        <rdfs:comment xml:lang="en">(ATA Code:3411) Pitot/static system: The system which provides a source of ram or static air for distribution to using instruments and pressure differential units such as automatic landing gear extender, altimeter, airspeed and rate of climb indicator. Does not include the using units, instruments, the anti-ice heating elements, or the associated circuitry and switches [Code 11303000]. Typical parts are air pick up heads, lines, fittings, drain valves, static port and selector valves.</rdfs:comment>
        <m:has_related_eccairs_term rdf:resource="http://onto.fel.cvut.cz/ontologies/2014/ECCAIRS_Aviation_1.3.0.12/eccairs-descriptive-factors#category_11341100"/>
    </owl:Class>
    


    <!-- http://onto.fel.cvut.cz/ontologies/aviation-safety/Placards_and_markings -->

    <owl:Class rdf:about="&m;Placards_and_markings">
        <rdfs:label>Placards and markings</rdfs:label>
        <rdfs:subClassOf rdf:resource="&m;Aircraft_part"/>
        <rdfs:subClassOf rdf:resource="&m;Marking"/>
        <m:generated_time rdf:datatype="&xsd;dateTime">2015-04-09T18:56:27.771+02:00</m:generated_time>
        <m:generated_time rdf:datatype="&xsd;dateTime">2015-04-12T02:45:54.351+02:00</m:generated_time>
        <rdfs:comment xml:lang="en">(ATA Code:1100) Placards and markings: Those installed by the manufacturer including those required by government regulations.</rdfs:comment>
        <m:has_related_eccairs_term rdf:resource="http://onto.fel.cvut.cz/ontologies/2014/ECCAIRS_Aviation_1.3.0.12/eccairs-descriptive-factors#category_11110000"/>
    </owl:Class>
    


    <!-- http://onto.fel.cvut.cz/ontologies/aviation-safety/Plate_skin_(nacelle-pylons) -->

    <owl:Class rdf:about="&m;Plate_skin_(nacelle-pylons)">
        <rdfs:label>Plate skin (nacelle/pylons)</rdfs:label>
        <rdfs:subClassOf rdf:resource="&m;Main_frame_(nacelle-pylon)_part"/>
        <m:generated_time rdf:datatype="&xsd;dateTime">2015-04-09T18:56:27.771+02:00</m:generated_time>
        <rdfs:comment xml:lang="en">(ATA Code:5414) The plates or skins on the nacelles or pylons.</rdfs:comment>
        <m:has_related_eccairs_term rdf:resource="http://onto.fel.cvut.cz/ontologies/2014/ECCAIRS_Aviation_1.3.0.12/eccairs-descriptive-factors#category_11541400"/>
    </owl:Class>
    


    <!-- http://onto.fel.cvut.cz/ontologies/aviation-safety/Plates-skins_(horizontal_stabilizer) -->

    <owl:Class rdf:about="&m;Plates-skins_(horizontal_stabilizer)">
        <rdfs:label>Plates/skins (horizontal stabilizer)</rdfs:label>
        <rdfs:subClassOf rdf:resource="&m;Horizontal_stabilizer_structure_part"/>
        <m:generated_time rdf:datatype="&xsd;dateTime">2015-04-09T18:56:27.771+02:00</m:generated_time>
        <rdfs:comment xml:lang="en">(ATA Code:5512) The plates/skins on the horizontal stabilizer.</rdfs:comment>
        <m:has_related_eccairs_term rdf:resource="http://onto.fel.cvut.cz/ontologies/2014/ECCAIRS_Aviation_1.3.0.12/eccairs-descriptive-factors#category_11551200"/>
    </owl:Class>
    


    <!-- http://onto.fel.cvut.cz/ontologies/aviation-safety/Plates-skins_(rudder) -->

    <owl:Class rdf:about="&m;Plates-skins_(rudder)">
        <rdfs:label>Plates/skins (rudder)</rdfs:label>
        <rdfs:subClassOf rdf:resource="&m;Rudder_structure_part"/>
        <m:generated_time rdf:datatype="&xsd;dateTime">2015-04-09T18:56:27.771+02:00</m:generated_time>
        <rdfs:comment xml:lang="en">(ATA Code:5542) The plates or skins on the rudder structure.</rdfs:comment>
        <m:has_related_eccairs_term rdf:resource="http://onto.fel.cvut.cz/ontologies/2014/ECCAIRS_Aviation_1.3.0.12/eccairs-descriptive-factors#category_11554200"/>
    </owl:Class>
    


    <!-- http://onto.fel.cvut.cz/ontologies/aviation-safety/Pneumatic_System_Wiring -->

    <owl:Class rdf:about="&m;Pneumatic_System_Wiring">
        <rdfs:label>Pneumatic System Wiring</rdfs:label>
        <rdfs:subClassOf rdf:resource="&m;Pneumatic_system_part"/>
        <m:generated_time rdf:datatype="&xsd;dateTime">2015-04-09T18:56:27.771+02:00</m:generated_time>
        <rdfs:comment xml:lang="en">(ATA Code:3697) Wiring specific to the Pneumatic System.</rdfs:comment>
        <m:has_related_eccairs_term rdf:resource="http://onto.fel.cvut.cz/ontologies/2014/ECCAIRS_Aviation_1.3.0.12/eccairs-descriptive-factors#category_11369700"/>
    </owl:Class>
    


    <!-- http://onto.fel.cvut.cz/ontologies/aviation-safety/Pneumatic_distribution_system -->

    <owl:Class rdf:about="&m;Pneumatic_distribution_system">
        <rdfs:label>Pneumatic distribution system</rdfs:label>
        <rdfs:subClassOf rdf:resource="&m;Pneumatic_system_part"/>
        <m:generated_time rdf:datatype="&xsd;dateTime">2015-04-09T18:56:27.771+02:00</m:generated_time>
        <rdfs:comment xml:lang="en">(ATA Code:3610) Pneumatic distribution system: The components and parts other than the regulator and shut-off valves delivering large volumes of compressed air from a power source to the control valves of using systems such as conditioning and pressurization. Does not include engine and aerofoil anti-icing/de-icing. Typical parts are regulator valve, actuator, duct, ducts valves, manifold, clamp, flow venturi, bellows, &quot;Y&quot; duct and check valve.</rdfs:comment>
        <m:has_related_eccairs_term rdf:resource="http://onto.fel.cvut.cz/ontologies/2014/ECCAIRS_Aviation_1.3.0.12/eccairs-descriptive-factors#category_11361000"/>
    </owl:Class>
    


    <!-- http://onto.fel.cvut.cz/ontologies/aviation-safety/Pneumatic_indicating_system -->

    <owl:Class rdf:about="&m;Pneumatic_indicating_system">
        <rdfs:label>Pneumatic indicating system</rdfs:label>
        <rdfs:subClassOf rdf:resource="&m;Pneumatic_system_part"/>
        <m:generated_time rdf:datatype="&xsd;dateTime">2015-04-09T18:56:27.771+02:00</m:generated_time>
        <rdfs:comment xml:lang="en">(ATA Code:3620) Pneumatic indicating system: The system components and parts which sense, transmit and indicate the temperature and pressure of air in the distribution system. Includes the instrument which indicates air pressure in the pneumatic distribution system. Does not include the using systems.</rdfs:comment>
        <m:has_related_eccairs_term rdf:resource="http://onto.fel.cvut.cz/ontologies/2014/ECCAIRS_Aviation_1.3.0.12/eccairs-descriptive-factors#category_11362000"/>
    </owl:Class>
    


    <!-- http://onto.fel.cvut.cz/ontologies/aviation-safety/Pneumatic_system -->

    <owl:Class rdf:about="&m;Pneumatic_system">
        <rdfs:label>Pneumatic system</rdfs:label>
        <rdfs:subClassOf rdf:resource="&m;Aircraft_part"/>
        <m:generated_time rdf:datatype="&xsd;dateTime">2015-04-09T18:56:27.771+02:00</m:generated_time>
        <rdfs:comment xml:lang="en">(ATA Code:3600) Pneumatic system: The units and components which deliver large volumes of compressed air from a power source to connecting points for other systems such as air conditioning, pressurization and de-icing.</rdfs:comment>
        <m:has_related_eccairs_term rdf:resource="http://onto.fel.cvut.cz/ontologies/2014/ECCAIRS_Aviation_1.3.0.12/eccairs-descriptive-factors#category_11360000"/>
    </owl:Class>
    


    <!-- http://onto.fel.cvut.cz/ontologies/aviation-safety/Pneumatic_system_part -->

    <owl:Class rdf:about="&m;Pneumatic_system_part">
        <rdfs:label>Pneumatic system part</rdfs:label>
        <rdfs:subClassOf rdf:resource="&m;Aircraft_part"/>
        <rdfs:subClassOf>
            <owl:Restriction>
                <owl:onProperty rdf:resource="http://onto.fel.cvut.cz/ontologies/ufo/is_part_of"/>
                <owl:someValuesFrom rdf:resource="&m;Pneumatic_system"/>
            </owl:Restriction>
        </rdfs:subClassOf>
        <m:generated_time rdf:datatype="&xsd;dateTime">2015-04-12T02:45:54.351+02:00</m:generated_time>
        <m:has_related_eccairs_term rdf:resource="http://onto.fel.cvut.cz/ontologies/2014/ECCAIRS_Aviation_1.3.0.12/eccairs-descriptive-factors#category_11360000"/>
    </owl:Class>
    


    <!-- http://onto.fel.cvut.cz/ontologies/aviation-safety/Portable_oxygen_system -->

    <owl:Class rdf:about="&m;Portable_oxygen_system">
        <rdfs:label>Portable oxygen system</rdfs:label>
        <rdfs:subClassOf rdf:resource="&m;Oxygen_system_part"/>
        <m:generated_time rdf:datatype="&xsd;dateTime">2015-04-09T18:56:27.771+02:00</m:generated_time>
        <rdfs:comment xml:lang="en">(ATA Code:3530) Portable oxygen system: The equipment attached to the portable bottle to regulate and dispense breathing oxygen, including the storage bottle for the portable oxygen system.</rdfs:comment>
        <m:has_related_eccairs_term rdf:resource="http://onto.fel.cvut.cz/ontologies/2014/ECCAIRS_Aviation_1.3.0.12/eccairs-descriptive-factors#category_11353000"/>
    </owl:Class>
    


    <!-- http://onto.fel.cvut.cz/ontologies/aviation-safety/Potable_water_system -->

    <owl:Class rdf:about="&m;Potable_water_system">
        <rdfs:label>Potable water system</rdfs:label>
        <rdfs:subClassOf rdf:resource="&m;Water_and_waste_system_part"/>
        <m:generated_time rdf:datatype="&xsd;dateTime">2015-04-09T18:56:27.771+02:00</m:generated_time>
        <rdfs:comment xml:lang="en">(ATA Code:3810) Water and waste system: The system which is used to store and deliver fresh drinking water.</rdfs:comment>
        <m:has_related_eccairs_term rdf:resource="http://onto.fel.cvut.cz/ontologies/2014/ECCAIRS_Aviation_1.3.0.12/eccairs-descriptive-factors#category_11381000"/>
    </owl:Class>
    


    <!-- http://onto.fel.cvut.cz/ontologies/aviation-safety/Power_lever -->

    <owl:Class rdf:about="&m;Power_lever">
        <rdfs:label>Power lever</rdfs:label>
        <rdfs:subClassOf rdf:resource="&m;Engine_controls_part"/>
        <m:generated_time rdf:datatype="&xsd;dateTime">2015-04-09T18:56:27.771+02:00</m:generated_time>
        <rdfs:comment xml:lang="en">(ATA Code:7603) Power lever: The system which provides for control of carburetor or fuel injectors on piston engines; fuel controls or coordinator on turbine engines and propeller regulator turboprop engines. Typical parts are cable, rod, rod end, bellcrank, bracket, clamp, actuator, shaft pin and knob.</rdfs:comment>
        <m:has_related_eccairs_term rdf:resource="http://onto.fel.cvut.cz/ontologies/2014/ECCAIRS_Aviation_1.3.0.12/eccairs-descriptive-factors#category_11760300"/>
    </owl:Class>
    


    <!-- http://onto.fel.cvut.cz/ontologies/aviation-safety/Power_recovery_turbine -->

    <owl:Class rdf:about="&m;Power_recovery_turbine">
        <rdfs:label>Power recovery turbine</rdfs:label>
        <rdfs:subClassOf rdf:resource="&m;Exhaust_turbine_system_(reciprocating)_part"/>
        <m:generated_time rdf:datatype="&xsd;dateTime">2015-04-09T18:56:27.771+02:00</m:generated_time>
        <rdfs:comment xml:lang="en">(ATA Code:8110) Power recovery turbine: The turbines which extract energy from the exhaust gases and are coupled to the crankshaft on reciprocating engines. Includes the power recovery turbine and supercharger unit when external to the engine. Does not include the drive shaft, coupling, and gears [Code 11854000].</rdfs:comment>
        <m:has_related_eccairs_term rdf:resource="http://onto.fel.cvut.cz/ontologies/2014/ECCAIRS_Aviation_1.3.0.12/eccairs-descriptive-factors#category_11811000"/>
    </owl:Class>
    


    <!-- http://onto.fel.cvut.cz/ontologies/aviation-safety/Powerplant_System_Wiring -->

    <owl:Class rdf:about="&m;Powerplant_System_Wiring">
        <rdfs:label>Powerplant System Wiring</rdfs:label>
        <rdfs:subClassOf rdf:resource="&m;Powerplant_system_part"/>
        <m:generated_time rdf:datatype="&xsd;dateTime">2015-04-09T18:56:27.771+02:00</m:generated_time>
        <rdfs:comment xml:lang="en">(ATA Code:7197) Wiring specific to the Powerplant System.</rdfs:comment>
        <m:has_related_eccairs_term rdf:resource="http://onto.fel.cvut.cz/ontologies/2014/ECCAIRS_Aviation_1.3.0.12/eccairs-descriptive-factors#category_11719700"/>
    </owl:Class>
    


    <!-- http://onto.fel.cvut.cz/ontologies/aviation-safety/Powerplant_attachment_fittings_(on_fuselage) -->

    <owl:Class rdf:about="&m;Powerplant_attachment_fittings_(on_fuselage)">
        <rdfs:label>Powerplant attachment fittings (on fuselage)</rdfs:label>
        <rdfs:subClassOf rdf:resource="&m;Fuselage_attachment_fittings_part"/>
        <m:generated_time rdf:datatype="&xsd;dateTime">2015-04-09T18:56:27.771+02:00</m:generated_time>
        <rdfs:comment xml:lang="en">(ATA Code:5346) Powerplant attachment fittings (on fuselage): The fittings on the fuselage used for the attachment of the powerplant e.g. the centre engine on tri-engine airplanes.</rdfs:comment>
        <m:has_related_eccairs_term rdf:resource="http://onto.fel.cvut.cz/ontologies/2014/ECCAIRS_Aviation_1.3.0.12/eccairs-descriptive-factors#category_11534600"/>
    </owl:Class>
    


    <!-- http://onto.fel.cvut.cz/ontologies/aviation-safety/Powerplant_installation_indications -->

    <owl:Class rdf:about="&m;Powerplant_installation_indications">
        <rdfs:label>Powerplant installation indications</rdfs:label>
        <rdfs:subClassOf rdf:resource="&m;Powerplant_system_part"/>
        <m:generated_time rdf:datatype="&xsd;dateTime">2015-04-09T18:56:27.771+02:00</m:generated_time>
        <rdfs:comment xml:lang="en">(ATA Code:7180) Powerplant installation indications: The system installed to provide continuous indication to the flight deck of the functioning of the power plant.</rdfs:comment>
        <m:has_related_eccairs_term rdf:resource="http://onto.fel.cvut.cz/ontologies/2014/ECCAIRS_Aviation_1.3.0.12/eccairs-descriptive-factors#category_11718000"/>
    </owl:Class>
    


    <!-- http://onto.fel.cvut.cz/ontologies/aviation-safety/Powerplant_system -->

    <owl:Class rdf:about="&m;Powerplant_system">
        <rdfs:label>Powerplant system</rdfs:label>
        <rdfs:subClassOf rdf:resource="&m;Aircraft_part"/>
        <m:generated_time rdf:datatype="&xsd;dateTime">2015-04-09T18:56:27.771+02:00</m:generated_time>
        <rdfs:comment xml:lang="en">(ATA Code:7100) The complete powerplant.</rdfs:comment>
        <m:has_related_eccairs_term rdf:resource="http://onto.fel.cvut.cz/ontologies/2014/ECCAIRS_Aviation_1.3.0.12/eccairs-descriptive-factors#category_11710000"/>
    </owl:Class>
    


    <!-- http://onto.fel.cvut.cz/ontologies/aviation-safety/Powerplant_system_part -->

    <owl:Class rdf:about="&m;Powerplant_system_part">
        <rdfs:label>Powerplant system part</rdfs:label>
        <rdfs:subClassOf rdf:resource="&m;Aircraft_part"/>
        <rdfs:subClassOf>
            <owl:Restriction>
                <owl:onProperty rdf:resource="http://onto.fel.cvut.cz/ontologies/ufo/is_part_of"/>
                <owl:someValuesFrom rdf:resource="&m;Powerplant_system"/>
            </owl:Restriction>
        </rdfs:subClassOf>
        <m:generated_time rdf:datatype="&xsd;dateTime">2015-04-12T02:45:54.351+02:00</m:generated_time>
        <m:has_related_eccairs_term rdf:resource="http://onto.fel.cvut.cz/ontologies/2014/ECCAIRS_Aviation_1.3.0.12/eccairs-descriptive-factors#category_11710000"/>
    </owl:Class>
    


    <!-- http://onto.fel.cvut.cz/ontologies/aviation-safety/Pressure_indicator -->

    <owl:Class rdf:about="&m;Pressure_indicator">
        <rdfs:subClassOf rdf:resource="&m;Pressurization_control_system_part"/>
    </owl:Class>
    


    <!-- http://onto.fel.cvut.cz/ontologies/aviation-safety/Pressure_regulator -->

    <owl:Class rdf:about="&m;Pressure_regulator">
        <rdfs:subClassOf rdf:resource="&m;Air_conditioning_system_part"/>
        <all2:has_ATA_code rdf:datatype="&xsd;integer">2133</all2:has_ATA_code>
    </owl:Class>
    


    <!-- http://onto.fel.cvut.cz/ontologies/aviation-safety/Pressure_regulator,_outflow_valve -->

    <owl:Class rdf:about="&m;Pressure_regulator,_outflow_valve">
        <rdfs:label>Pressure regulator, outflow valve</rdfs:label>
        <rdfs:subClassOf rdf:resource="&m;Pressurization_control_system_part"/>
        <m:generated_time rdf:datatype="&xsd;dateTime">2015-04-09T18:56:27.771+02:00</m:generated_time>
        <rdfs:comment xml:lang="en">(ATA Code:2133) Pressure regulator, outflow valve: The pressure regulating outflow/dump valves and associated parts such as linkage, filter and diaphragm.</rdfs:comment>
        <m:has_related_eccairs_term rdf:resource="http://onto.fel.cvut.cz/ontologies/2014/ECCAIRS_Aviation_1.3.0.12/eccairs-descriptive-factors#category_11213300"/>
    </owl:Class>
    


    <!-- http://onto.fel.cvut.cz/ontologies/aviation-safety/Pressure_sensor -->

    <owl:Class rdf:about="&m;Pressure_sensor">
        <rdfs:label>Pressure sensor</rdfs:label>
        <rdfs:subClassOf rdf:resource="&m;Pressurization_control_system_part"/>
        <m:generated_time rdf:datatype="&xsd;dateTime">2015-04-09T18:56:27.771+02:00</m:generated_time>
        <rdfs:comment xml:lang="en">(ATA Code:2134) Pressure sensor: The units and systems which measure differential pressure and transmit a signal. Typical parts are pressure switch and transducer.</rdfs:comment>
        <m:has_related_eccairs_term rdf:resource="http://onto.fel.cvut.cz/ontologies/2014/ECCAIRS_Aviation_1.3.0.12/eccairs-descriptive-factors#category_11213400"/>
    </owl:Class>
    


    <!-- http://onto.fel.cvut.cz/ontologies/aviation-safety/Pressurization_control_system -->

    <owl:Class rdf:about="&m;Pressurization_control_system">
        <rdfs:label>Pressurization control system</rdfs:label>
        <rdfs:subClassOf rdf:resource="&m;Air_conditioning_system_part"/>
        <m:generated_time rdf:datatype="&xsd;dateTime">2015-04-09T18:56:27.771+02:00</m:generated_time>
        <rdfs:comment xml:lang="en">(ATA Code:2130) Pressurization control system: The miscellaneous system components or parts other than the controller, indicator, sensor, regulator, or outflow valves. Typical parts are the amplifier, switches and electrical connectors.</rdfs:comment>
        <m:has_related_eccairs_term rdf:resource="http://onto.fel.cvut.cz/ontologies/2014/ECCAIRS_Aviation_1.3.0.12/eccairs-descriptive-factors#category_11213000"/>
    </owl:Class>
    


    <!-- http://onto.fel.cvut.cz/ontologies/aviation-safety/Pressurization_control_system_part -->

    <owl:Class rdf:about="&m;Pressurization_control_system_part">
        <rdfs:label>Pressurization control system part</rdfs:label>
        <rdfs:subClassOf rdf:resource="&m;Air_conditioning_system_part"/>
        <rdfs:subClassOf>
            <owl:Restriction>
                <owl:onProperty rdf:resource="http://onto.fel.cvut.cz/ontologies/ufo/is_part_of"/>
                <owl:someValuesFrom rdf:resource="&m;Pressurization_control_system"/>
            </owl:Restriction>
        </rdfs:subClassOf>
        <m:generated_time rdf:datatype="&xsd;dateTime">2015-04-12T02:45:54.351+02:00</m:generated_time>
        <m:has_related_eccairs_term rdf:resource="http://onto.fel.cvut.cz/ontologies/2014/ECCAIRS_Aviation_1.3.0.12/eccairs-descriptive-factors#category_11213000"/>
    </owl:Class>
    


    <!-- http://onto.fel.cvut.cz/ontologies/aviation-safety/Primary_and_Secondary_Power -->

    <owl:Class rdf:about="&m;Primary_and_Secondary_Power">
        <rdfs:label>Primary and Secondary Power</rdfs:label>
        <rdfs:subClassOf rdf:resource="&m;Electrical_power_system_part"/>
        <m:generated_time rdf:datatype="&xsd;dateTime">2015-04-09T18:56:27.771+02:00</m:generated_time>
        <rdfs:comment xml:lang="en">(ATA Code:2470) That portion of the system which provides for connection of AC and DC power to using systems. Includes items such as main and secondary busses, main system circuit breakers, power system devices, specific interface for computer-aided maintenance action etc.</rdfs:comment>
        <m:has_related_eccairs_term rdf:resource="http://onto.fel.cvut.cz/ontologies/2014/ECCAIRS_Aviation_1.3.0.12/eccairs-descriptive-factors#category_11247000"/>
    </owl:Class>
    


    <!-- http://onto.fel.cvut.cz/ontologies/aviation-safety/Propeller-Propulsor_System_Wiring -->

    <owl:Class rdf:about="&m;Propeller-Propulsor_System_Wiring">
        <rdfs:label>Propeller/Propulsor System Wiring</rdfs:label>
        <rdfs:subClassOf rdf:resource="&m;Propeller_system_part"/>
        <m:generated_time rdf:datatype="&xsd;dateTime">2015-04-09T18:56:27.771+02:00</m:generated_time>
        <rdfs:comment xml:lang="en">(ATA Code:6197) Wiring specific to the Propeller/Propulsor Systems</rdfs:comment>
        <m:has_related_eccairs_term rdf:resource="http://onto.fel.cvut.cz/ontologies/2014/ECCAIRS_Aviation_1.3.0.12/eccairs-descriptive-factors#category_11619700"/>
    </owl:Class>
    


    <!-- http://onto.fel.cvut.cz/ontologies/aviation-safety/Propeller_-_rotor_anti-ice-de-ice_system -->

    <owl:Class rdf:about="&m;Propeller_-_rotor_anti-ice-de-ice_system">
        <rdfs:label>Propeller / rotor anti-ice/de-ice system</rdfs:label>
        <rdfs:subClassOf rdf:resource="&m;Ice-rain_protection_systems"/>
        <m:generated_time rdf:datatype="&xsd;dateTime">2015-04-09T18:56:27.771+02:00</m:generated_time>
        <rdfs:comment xml:lang="en">(ATA Code:3060) Propeller / rotor anti-ice/de-ice system: The system components and parts which are used to eliminate or prevent the formation of ice on propellers and rotors. Includes electrically heated systems, and alcohol spray systems. Does not include the system parts on the rotating portion of the propeller [Code 11611200] or the heating mats on the rotating portion of the rotor [Code 11621000 or code 11641000]. Typical parts are brush block, timer, switch, relay, harness and terminal block.</rdfs:comment>
        <m:has_related_eccairs_term rdf:resource="http://onto.fel.cvut.cz/ontologies/2014/ECCAIRS_Aviation_1.3.0.12/eccairs-descriptive-factors#category_11306000"/>
    </owl:Class>
    


    <!-- http://onto.fel.cvut.cz/ontologies/aviation-safety/Propeller_assembly -->

    <owl:Class rdf:about="&m;Propeller_assembly">
        <rdfs:label>Propeller assembly</rdfs:label>
        <rdfs:subClassOf rdf:resource="&m;Propeller_system_part"/>
        <m:generated_time rdf:datatype="&xsd;dateTime">2015-04-09T18:56:27.771+02:00</m:generated_time>
        <rdfs:comment xml:lang="en">(ATA Code:6110) The propeller assembly excluding controlling aspects or conditions which affect two or more parts of the propeller such as hub and blades.</rdfs:comment>
        <m:has_related_eccairs_term rdf:resource="http://onto.fel.cvut.cz/ontologies/2014/ECCAIRS_Aviation_1.3.0.12/eccairs-descriptive-factors#category_11611000"/>
    </owl:Class>
    


    <!-- http://onto.fel.cvut.cz/ontologies/aviation-safety/Propeller_assembly_part -->

    <owl:Class rdf:about="&m;Propeller_assembly_part">
        <rdfs:label>Propeller assembly part</rdfs:label>
        <rdfs:subClassOf rdf:resource="&m;Propeller_system_part"/>
        <rdfs:subClassOf>
            <owl:Restriction>
                <owl:onProperty rdf:resource="http://onto.fel.cvut.cz/ontologies/ufo/is_part_of"/>
                <owl:someValuesFrom rdf:resource="&m;Propeller_assembly"/>
            </owl:Restriction>
        </rdfs:subClassOf>
        <m:generated_time rdf:datatype="&xsd;dateTime">2015-04-12T02:45:54.351+02:00</m:generated_time>
        <m:has_related_eccairs_term rdf:resource="http://onto.fel.cvut.cz/ontologies/2014/ECCAIRS_Aviation_1.3.0.12/eccairs-descriptive-factors#category_11611000"/>
    </owl:Class>
    


    <!-- http://onto.fel.cvut.cz/ontologies/aviation-safety/Propeller_blade_section -->

    <owl:Class rdf:about="&m;Propeller_blade_section">
        <rdfs:label>Propeller blade section</rdfs:label>
        <rdfs:subClassOf rdf:resource="&m;Propeller_assembly_part"/>
        <m:generated_time rdf:datatype="&xsd;dateTime">2015-04-09T18:56:27.771+02:00</m:generated_time>
        <rdfs:comment xml:lang="en">(ATA Code:6111) Propeller blade section: The propeller blade but not the de-ice boots. Includes retaining clamps and blade pitch change actuating mechanism which rotates with the propeller. Typical parts are blade, clamp, link, motor, counterweight and bearings.</rdfs:comment>
        <m:has_related_eccairs_term rdf:resource="http://onto.fel.cvut.cz/ontologies/2014/ECCAIRS_Aviation_1.3.0.12/eccairs-descriptive-factors#category_11611100"/>
    </owl:Class>
    


    <!-- http://onto.fel.cvut.cz/ontologies/aviation-safety/Propeller_braking -->

    <owl:Class rdf:about="&m;Propeller_braking">
        <rdfs:label>Propeller braking</rdfs:label>
        <rdfs:subClassOf rdf:resource="&m;Propeller_system_part"/>
        <m:generated_time rdf:datatype="&xsd;dateTime">2015-04-09T18:56:27.771+02:00</m:generated_time>
        <rdfs:comment xml:lang="en">(ATA Code:6130) Propeller braking: The portion of the system which is used to decrease run-down time or stop propeller rotation during engine power-off conditions.</rdfs:comment>
        <m:has_related_eccairs_term rdf:resource="http://onto.fel.cvut.cz/ontologies/2014/ECCAIRS_Aviation_1.3.0.12/eccairs-descriptive-factors#category_11613000"/>
    </owl:Class>
    


    <!-- http://onto.fel.cvut.cz/ontologies/aviation-safety/Propeller_control_system -->

    <owl:Class rdf:about="&m;Propeller_control_system">
        <rdfs:label>Propeller control system</rdfs:label>
        <rdfs:subClassOf rdf:resource="&m;Propeller_system_part"/>
        <m:generated_time rdf:datatype="&xsd;dateTime">2015-04-09T18:56:27.771+02:00</m:generated_time>
        <rdfs:comment xml:lang="en">(ATA Code:6120) Propeller control system: The propeller speed controlling system other than the governor unit or the synchronizer. Includes the controlling systems of propellers regardless of the propeller type. (Includes propeller regulator, negative torque switch and the rigging mechanism). Also includes governor control linkage, levers, cable and associated brackets from the cockpit to the governor and the feather and unfeathering systems except the pump and accumulator. Typical parts are cable, bellcrank, lever, rod end, pressure switch, solenoid valve and beta switch.</rdfs:comment>
        <m:has_related_eccairs_term rdf:resource="http://onto.fel.cvut.cz/ontologies/2014/ECCAIRS_Aviation_1.3.0.12/eccairs-descriptive-factors#category_11612000"/>
    </owl:Class>
    


    <!-- http://onto.fel.cvut.cz/ontologies/aviation-safety/Propeller_control_system_part -->

    <owl:Class rdf:about="&m;Propeller_control_system_part">
        <rdfs:label>Propeller control system part</rdfs:label>
        <rdfs:subClassOf rdf:resource="&m;Propeller_system_part"/>
        <rdfs:subClassOf>
            <owl:Restriction>
                <owl:onProperty rdf:resource="http://onto.fel.cvut.cz/ontologies/ufo/is_part_of"/>
                <owl:someValuesFrom rdf:resource="&m;Propeller_control_system"/>
            </owl:Restriction>
        </rdfs:subClassOf>
        <m:generated_time rdf:datatype="&xsd;dateTime">2015-04-12T02:45:54.351+02:00</m:generated_time>
        <m:has_related_eccairs_term rdf:resource="http://onto.fel.cvut.cz/ontologies/2014/ECCAIRS_Aviation_1.3.0.12/eccairs-descriptive-factors#category_11612000"/>
    </owl:Class>
    


    <!-- http://onto.fel.cvut.cz/ontologies/aviation-safety/Propeller_de-ice_boot -->

    <owl:Class rdf:about="&m;Propeller_de-ice_boot">
        <rdfs:label>Propeller de-ice boot</rdfs:label>
        <rdfs:subClassOf rdf:resource="&m;Propeller_assembly_part"/>
        <m:generated_time rdf:datatype="&xsd;dateTime">2015-04-09T18:56:27.771+02:00</m:generated_time>
        <rdfs:comment xml:lang="en">(ATA Code:6112) Propeller de-ice boot: The de-ice/anti-ice system parts on the rotating parts of the propeller such as blades or spinner. Does not include the power source, controls or other non-rotating system parts [Code 11306000]. Typical parts are boot and cuff, heat element and slip ring.</rdfs:comment>
        <m:has_related_eccairs_term rdf:resource="http://onto.fel.cvut.cz/ontologies/2014/ECCAIRS_Aviation_1.3.0.12/eccairs-descriptive-factors#category_11611200"/>
    </owl:Class>
    


    <!-- http://onto.fel.cvut.cz/ontologies/aviation-safety/Propeller_feather-reversing -->

    <owl:Class rdf:about="&m;Propeller_feather-reversing">
        <rdfs:label>Propeller feather/reversing</rdfs:label>
        <rdfs:subClassOf rdf:resource="&m;Propeller_control_system_part"/>
        <m:generated_time rdf:datatype="&xsd;dateTime">2015-04-09T18:56:27.771+02:00</m:generated_time>
        <rdfs:comment xml:lang="en">(ATA Code:6123) Propeller feather/reversing: The system component and parts which store and deliver an energy charge for propeller feathering and unfeathering. Includes the pump and associated motor, switch, circuitry and plumbing which provides the force for feathering the propeller blades for stopping the engine&apos;s rotation. Typical parts are pump, motor, switch, accumulator, air valve and seal.</rdfs:comment>
        <m:has_related_eccairs_term rdf:resource="http://onto.fel.cvut.cz/ontologies/2014/ECCAIRS_Aviation_1.3.0.12/eccairs-descriptive-factors#category_11612300"/>
    </owl:Class>
    


    <!-- http://onto.fel.cvut.cz/ontologies/aviation-safety/Propeller_governor -->

    <owl:Class rdf:about="&m;Propeller_governor">
        <rdfs:label>Propeller governor</rdfs:label>
        <rdfs:subClassOf rdf:resource="&m;Propeller_control_system_part"/>
        <m:generated_time rdf:datatype="&xsd;dateTime">2015-04-09T18:56:27.771+02:00</m:generated_time>
        <rdfs:comment xml:lang="en">(ATA Code:6122) Propeller governor: The unit which controls the propeller blade angle, but is limited to parts in and on the governor. Does not include airframe furnished control linkage from the cockpit [Code 11612000]. Typical parts are shaft, flyweight, governor, spring, arm, seal, beta valve, pilot valve and head.</rdfs:comment>
        <m:has_related_eccairs_term rdf:resource="http://onto.fel.cvut.cz/ontologies/2014/ECCAIRS_Aviation_1.3.0.12/eccairs-descriptive-factors#category_11612200"/>
    </owl:Class>
    


    <!-- http://onto.fel.cvut.cz/ontologies/aviation-safety/Propeller_hub_section -->

    <owl:Class rdf:about="&m;Propeller_hub_section">
        <rdfs:label>Propeller hub section</rdfs:label>
        <rdfs:subClassOf rdf:resource="&m;Propeller_assembly_part"/>
        <m:generated_time rdf:datatype="&xsd;dateTime">2015-04-09T18:56:27.771+02:00</m:generated_time>
        <rdfs:comment xml:lang="en">(ATA Code:6114) Propeller hub section: The hubs which house and support the rotating blades. Includes the dome, but not the blade actuating mechanism [Code 11611000] or the attachment to the engine flange [Code 11611001].</rdfs:comment>
        <m:has_related_eccairs_term rdf:resource="http://onto.fel.cvut.cz/ontologies/2014/ECCAIRS_Aviation_1.3.0.12/eccairs-descriptive-factors#category_11611400"/>
    </owl:Class>
    


    <!-- http://onto.fel.cvut.cz/ontologies/aviation-safety/Propeller_indicating_system -->

    <owl:Class rdf:about="&m;Propeller_indicating_system">
        <rdfs:label>Propeller indicating system</rdfs:label>
        <rdfs:subClassOf rdf:resource="&m;Propeller_system_part"/>
        <m:generated_time rdf:datatype="&xsd;dateTime">2015-04-09T18:56:27.771+02:00</m:generated_time>
        <rdfs:comment xml:lang="en">(ATA Code:6140) Propeller indicating system: The system components and parts which indicate the operation or activation of propeller systems. Typical parts are switch, lamp, connector, harness and indicators.</rdfs:comment>
        <m:has_related_eccairs_term rdf:resource="http://onto.fel.cvut.cz/ontologies/2014/ECCAIRS_Aviation_1.3.0.12/eccairs-descriptive-factors#category_11614000"/>
    </owl:Class>
    


    <!-- http://onto.fel.cvut.cz/ontologies/aviation-safety/Propeller_spinner_section -->

    <owl:Class rdf:about="&m;Propeller_spinner_section">
        <rdfs:label>Propeller spinner section</rdfs:label>
        <rdfs:subClassOf rdf:resource="&m;Propeller_assembly_part"/>
        <m:generated_time rdf:datatype="&xsd;dateTime">2015-04-09T18:56:27.771+02:00</m:generated_time>
        <rdfs:comment xml:lang="en">(ATA Code:6113) Propeller spinner section: The propeller spinner assemblies. Typical parts are shell, back plate, bulkhead, rivets, screw, nut plate and brackets.</rdfs:comment>
        <m:has_related_eccairs_term rdf:resource="http://onto.fel.cvut.cz/ontologies/2014/ECCAIRS_Aviation_1.3.0.12/eccairs-descriptive-factors#category_11611300"/>
    </owl:Class>
    


    <!-- http://onto.fel.cvut.cz/ontologies/aviation-safety/Propeller_synchronizer_section -->

    <owl:Class rdf:about="&m;Propeller_synchronizer_section">
        <rdfs:label>Propeller synchronizer section</rdfs:label>
        <rdfs:subClassOf rdf:resource="&m;Propeller_control_system_part"/>
        <m:generated_time rdf:datatype="&xsd;dateTime">2015-04-09T18:56:27.771+02:00</m:generated_time>
        <rdfs:comment xml:lang="en">(ATA Code:6121) Propeller synchronizer section: The unit which controls the synchronization of propellers on multi-engine aircraft. Typical parts are synchronizer actuator, computer, synchrophaser and control unit.</rdfs:comment>
        <m:has_related_eccairs_term rdf:resource="http://onto.fel.cvut.cz/ontologies/2014/ECCAIRS_Aviation_1.3.0.12/eccairs-descriptive-factors#category_11612100"/>
    </owl:Class>
    


    <!-- http://onto.fel.cvut.cz/ontologies/aviation-safety/Propeller_system -->

    <owl:Class rdf:about="&m;Propeller_system">
        <rdfs:label>Propeller system</rdfs:label>
        <rdfs:subClassOf rdf:resource="&m;Aircraft_part"/>
        <m:generated_time rdf:datatype="&xsd;dateTime">2015-04-09T18:56:27.771+02:00</m:generated_time>
        <rdfs:comment xml:lang="en">(ATA Code:6100) Propeller system: The complete mechanical or electrical propeller, pumps, motors, governor, alternators and those units and components external to or integral with the engine used to control the propeller blade angle. Includes the propulsor duct assemblies, aerodynamic fairing of mechanical components, stators and vectoring systems.  Propeller: a device for propelling an aircraft that has blades on an engine-driven shaft and that, when rotated, produces by its action on the air, a thrust approximately perpendicular to its plane of rotation. (FAA)</rdfs:comment>
        <m:has_related_eccairs_term rdf:resource="http://onto.fel.cvut.cz/ontologies/2014/ECCAIRS_Aviation_1.3.0.12/eccairs-descriptive-factors#category_11610000"/>
    </owl:Class>
    


    <!-- http://onto.fel.cvut.cz/ontologies/aviation-safety/Propeller_system_part -->

    <owl:Class rdf:about="&m;Propeller_system_part">
        <rdfs:label>Propeller system part</rdfs:label>
        <rdfs:subClassOf rdf:resource="&m;Aircraft_part"/>
        <rdfs:subClassOf>
            <owl:Restriction>
                <owl:onProperty rdf:resource="http://onto.fel.cvut.cz/ontologies/ufo/is_part_of"/>
                <owl:someValuesFrom rdf:resource="&m;Propeller_system"/>
            </owl:Restriction>
        </rdfs:subClassOf>
        <m:generated_time rdf:datatype="&xsd;dateTime">2015-04-12T02:45:54.351+02:00</m:generated_time>
        <m:has_related_eccairs_term rdf:resource="http://onto.fel.cvut.cz/ontologies/2014/ECCAIRS_Aviation_1.3.0.12/eccairs-descriptive-factors#category_11610000"/>
    </owl:Class>
    


    <!-- http://onto.fel.cvut.cz/ontologies/aviation-safety/Propulsor_Duct -->

    <owl:Class rdf:about="&m;Propulsor_Duct">
        <rdfs:label>Propulsor Duct</rdfs:label>
        <rdfs:subClassOf rdf:resource="&m;Propeller_system_part"/>
        <m:generated_time rdf:datatype="&xsd;dateTime">2015-04-09T18:56:27.771+02:00</m:generated_time>
        <rdfs:comment xml:lang="en">(ATA Code:6150) The complete duct assembly including vector drive attachment, fairings, stators, gearbox covers, etc.</rdfs:comment>
        <m:has_related_eccairs_term rdf:resource="http://onto.fel.cvut.cz/ontologies/2014/ECCAIRS_Aviation_1.3.0.12/eccairs-descriptive-factors#category_11615000"/>
    </owl:Class>
    


    <!-- http://onto.fel.cvut.cz/ontologies/aviation-safety/Radio_communication_equipment -->

    <owl:Class rdf:about="&m;Radio_communication_equipment"/>
    


    <!-- http://onto.fel.cvut.cz/ontologies/aviation-safety/Rain_repellent_system -->

    <owl:Class rdf:about="&m;Rain_repellent_system">
        <rdfs:label>Rain repellent system</rdfs:label>
        <rdfs:subClassOf rdf:resource="&m;Windshield-door_rain-ice_removal_part"/>
        <m:generated_time rdf:datatype="&xsd;dateTime">2015-04-09T18:56:27.771+02:00</m:generated_time>
        <rdfs:comment xml:lang="en">(ATA Code:3041) Rain repellent system: The system and components used to prevent the build up of rain on the aircraft windshield. Typical parts are motor, actuator and storage tank.</rdfs:comment>
        <m:has_related_eccairs_term rdf:resource="http://onto.fel.cvut.cz/ontologies/2014/ECCAIRS_Aviation_1.3.0.12/eccairs-descriptive-factors#category_11304100"/>
    </owl:Class>
    


    <!-- http://onto.fel.cvut.cz/ontologies/aviation-safety/Rate_of_climb_indication -->

    <owl:Class rdf:about="&m;Rate_of_climb_indication">
        <rdfs:label>Rate of climb indication</rdfs:label>
        <rdfs:subClassOf rdf:resource="&m;Flight_environment_data_system"/>
        <m:generated_time rdf:datatype="&xsd;dateTime">2015-04-09T18:56:27.771+02:00</m:generated_time>
        <rdfs:comment xml:lang="en">(ATA Code:3413) Rate of climb indicator: The instrument which senses and indicates the rate of climb or descent of an aircraft. Does not include the associated static system. Includes the instantaneous vertical speed indicator (IVSI).</rdfs:comment>
        <m:has_related_eccairs_term rdf:resource="http://onto.fel.cvut.cz/ontologies/2014/ECCAIRS_Aviation_1.3.0.12/eccairs-descriptive-factors#category_11341300"/>
    </owl:Class>
    


    <!-- http://onto.fel.cvut.cz/ontologies/aviation-safety/Reciprocating_Engine_Liquid_Cooling -->

    <owl:Class rdf:about="&m;Reciprocating_Engine_Liquid_Cooling">
        <rdfs:label>Reciprocating Engine Liquid Cooling</rdfs:label>
        <rdfs:subClassOf rdf:resource="&m;Reciprocating_engine_part"/>
        <m:generated_time rdf:datatype="&xsd;dateTime">2015-04-09T18:56:27.771+02:00</m:generated_time>
        <rdfs:comment xml:lang="en">(ATA Code:8570) The components and parts that provide cooling liquid to the engine. Includes the plumbing leading to and from the engine. Typical parts are radiator, hoses, pump, drive belt, pulleys, bearings, seals, overflow line, overflow tank, pressure cap, thermostat.</rdfs:comment>
        <m:has_related_eccairs_term rdf:resource="http://onto.fel.cvut.cz/ontologies/2014/ECCAIRS_Aviation_1.3.0.12/eccairs-descriptive-factors#category_11857000"/>
    </owl:Class>
    


    <!-- http://onto.fel.cvut.cz/ontologies/aviation-safety/Reciprocating_Engine_Supercharger -->

    <owl:Class rdf:about="&m;Reciprocating_Engine_Supercharger">
        <rdfs:label>Reciprocating Engine Supercharger</rdfs:label>
        <rdfs:subClassOf rdf:resource="&m;Reciprocating_engine_part"/>
        <m:generated_time rdf:datatype="&xsd;dateTime">2015-04-09T18:56:27.771+02:00</m:generated_time>
        <rdfs:comment xml:lang="en">(ATA Code:8560) The components and parts of the Supercharger system. Typical parts are case, impeller, rotors, bearings, seals, belts, pulleys or sprockets. Does not include gears in engine rear section.Reciprocating engine supercharger - a blower or compressor driven by the engine, for supplying air under high pressure to the cylinders of an internal combustion engine</rdfs:comment>
        <m:has_related_eccairs_term rdf:resource="http://onto.fel.cvut.cz/ontologies/2014/ECCAIRS_Aviation_1.3.0.12/eccairs-descriptive-factors#category_11856000"/>
    </owl:Class>
    


    <!-- http://onto.fel.cvut.cz/ontologies/aviation-safety/Reciprocating_Engine_System_Wiring -->

    <owl:Class rdf:about="&m;Reciprocating_Engine_System_Wiring">
        <rdfs:subClassOf rdf:resource="&m;Reciprocating_engine_part"/>
    </owl:Class>
    


    <!-- http://onto.fel.cvut.cz/ontologies/aviation-safety/Reciprocating_engine -->

    <owl:Class rdf:about="&m;Reciprocating_engine">
        <rdfs:subClassOf rdf:resource="&m;Aircraft_part"/>
    </owl:Class>
    


    <!-- http://onto.fel.cvut.cz/ontologies/aviation-safety/Reciprocating_engine_cylinder_section -->

    <owl:Class rdf:about="&m;Reciprocating_engine_cylinder_section">
        <rdfs:label>Reciprocating engine cylinder section</rdfs:label>
        <rdfs:subClassOf rdf:resource="&m;Reciprocating_engine_part"/>
        <m:generated_time rdf:datatype="&xsd;dateTime">2015-04-09T18:56:27.771+02:00</m:generated_time>
        <rdfs:comment xml:lang="en">(ATA Code:8530) Reciprocating engine cylinder section: The section of the engine which contains the cylinders and associated parts including the intake pipes and valve push rods/housing. Also includes the cylinder baffles furnished by the engine manufacturer for engine cooling. Does not include the connecting rods or cylinder flange hold down bolts/studs [Code 11852000]. Typical parts are piston, piston pin, exhaust valve, intake valve, valve guide, rocker arm, valve cover, cylinder, pushrod housing, intake pipe, piston pin plug, valve spring, rocker shaft, piston ring, oil drain lines, clamp and baffles.</rdfs:comment>
        <m:has_related_eccairs_term rdf:resource="http://onto.fel.cvut.cz/ontologies/2014/ECCAIRS_Aviation_1.3.0.12/eccairs-descriptive-factors#category_11853000"/>
    </owl:Class>
    


    <!-- http://onto.fel.cvut.cz/ontologies/aviation-safety/Reciprocating_engine_front_section -->

    <owl:Class rdf:about="&m;Reciprocating_engine_front_section">
        <rdfs:label>Reciprocating engine front section</rdfs:label>
        <rdfs:subClassOf rdf:resource="&m;Reciprocating_engine_part"/>
        <m:generated_time rdf:datatype="&xsd;dateTime">2015-04-09T18:56:27.771+02:00</m:generated_time>
        <rdfs:comment xml:lang="en">(ATA Code:8510) Reciprocating engine front section: The piston engine front cases which contain the propeller shaft, reduction gears, and accessory drive. Typical parts are propeller shaft, gear, bearing, bushing, case, seal and pinion gear.</rdfs:comment>
        <m:has_related_eccairs_term rdf:resource="http://onto.fel.cvut.cz/ontologies/2014/ECCAIRS_Aviation_1.3.0.12/eccairs-descriptive-factors#category_11851000"/>
    </owl:Class>
    


    <!-- http://onto.fel.cvut.cz/ontologies/aviation-safety/Reciprocating_engine_oil_system -->

    <owl:Class rdf:about="&m;Reciprocating_engine_oil_system">
        <rdfs:label>Reciprocating engine oil system</rdfs:label>
        <rdfs:subClassOf rdf:resource="&m;Reciprocating_engine_part"/>
        <m:generated_time rdf:datatype="&xsd;dateTime">2015-04-09T18:56:27.771+02:00</m:generated_time>
        <rdfs:comment xml:lang="en">(ATA Code:8550) Reciprocating engine oil system: The reciprocating engine components and parts that provide oil pressure and distribute lubricating oil within the engine. Includes the plumbing leading to and from the using external systems and components which utilize engine system oil for operation. Does not include the externally mounted oil system storage tanks and connecting lines [Code 11791000], or the oil cooler lines, hoses and drain valves [Code 11792000]. Typical parts are pressure and scavenge pump, impeller, housing, filter, air-oil separator, crankcase breather, screen, element, relief valve, drive gear, adapter, pan, dipstick, cap and propeller governor oil lines.</rdfs:comment>
        <m:has_related_eccairs_term rdf:resource="http://onto.fel.cvut.cz/ontologies/2014/ECCAIRS_Aviation_1.3.0.12/eccairs-descriptive-factors#category_11855000"/>
    </owl:Class>
    


    <!-- http://onto.fel.cvut.cz/ontologies/aviation-safety/Reciprocating_engine_part -->

    <owl:Class rdf:about="&m;Reciprocating_engine_part">
        <rdfs:label>Reciprocating engine part</rdfs:label>
        <rdfs:subClassOf rdf:resource="&m;Aircraft_part"/>
        <rdfs:subClassOf>
            <owl:Restriction>
                <owl:onProperty rdf:resource="http://onto.fel.cvut.cz/ontologies/ufo/is_part_of"/>
                <owl:someValuesFrom rdf:resource="&m;Reciprocating_engine"/>
            </owl:Restriction>
        </rdfs:subClassOf>
        <m:generated_time rdf:datatype="&xsd;dateTime">2015-04-12T02:45:54.351+02:00</m:generated_time>
        <m:has_related_eccairs_term rdf:resource="http://onto.fel.cvut.cz/ontologies/2014/ECCAIRS_Aviation_1.3.0.12/eccairs-descriptive-factors#category_11850000"/>
    </owl:Class>
    


    <!-- http://onto.fel.cvut.cz/ontologies/aviation-safety/Reciprocating_engine_power_section -->

    <owl:Class rdf:about="&m;Reciprocating_engine_power_section">
        <rdfs:label>Reciprocating engine power section</rdfs:label>
        <rdfs:subClassOf rdf:resource="&m;Reciprocating_engine_part"/>
        <m:generated_time rdf:datatype="&xsd;dateTime">2015-04-09T18:56:27.771+02:00</m:generated_time>
        <rdfs:comment xml:lang="en">(ATA Code:8520) Reciprocating engine power section: The section of the reciprocating engine which contains the crankshaft, cam shaft, tappet guides, valve lifters, connecting rods and drive gears. Does not include the push rods which are in the cylinder section [Code 11853000] or rear case accessory drives. Typical parts are crankcase, crankshaft, cam ring, lifter, camshaft, cylinder stud, connecting rod, bolt, through bolt, cap, rod bolt, main bearing and rod bearing.</rdfs:comment>
        <m:has_related_eccairs_term rdf:resource="http://onto.fel.cvut.cz/ontologies/2014/ECCAIRS_Aviation_1.3.0.12/eccairs-descriptive-factors#category_11852000"/>
    </owl:Class>
    


    <!-- http://onto.fel.cvut.cz/ontologies/aviation-safety/Reciprocating_engine_rear_section -->

    <owl:Class rdf:about="&m;Reciprocating_engine_rear_section">
        <rdfs:label>Reciprocating engine rear section</rdfs:label>
        <rdfs:subClassOf rdf:resource="&m;Reciprocating_engine_part"/>
        <m:generated_time rdf:datatype="&xsd;dateTime">2015-04-09T18:56:27.771+02:00</m:generated_time>
        <rdfs:comment xml:lang="en">(ATA Code:8540) Reciprocating engine rear section: The reciprocating engine case or section where accessories and associated engine drives are located. Includes the power recovery turbine (PRT) drive shaft, coupling and gears, the accessory pads, drives and drive seals but not the accessories. Does not include oil pump, filter or internal lubricating system [Code 11855000]. Typical parts are seal, gear, drive shaft, case, bearing and spacer.</rdfs:comment>
        <m:has_related_eccairs_term rdf:resource="http://onto.fel.cvut.cz/ontologies/2014/ECCAIRS_Aviation_1.3.0.12/eccairs-descriptive-factors#category_11854000"/>
    </owl:Class>
    


    <!-- http://onto.fel.cvut.cz/ontologies/aviation-safety/Rotor_blades_folding -->

    <owl:Class rdf:about="&m;Rotor_blades_folding">
        <rdfs:label>Rotor blades folding</rdfs:label>
        <rdfs:subClassOf rdf:resource="&m;Folding_blades-pylon_part"/>
        <m:generated_time rdf:datatype="&xsd;dateTime">2015-04-09T18:56:27.771+02:00</m:generated_time>
        <rdfs:comment xml:lang="en">(ATA Code:6610) Part of the system ensuring rotor blade folding and spreading; includes the mechanical, hydraulic and electrical means permanently fitted on the aircraft.</rdfs:comment>
        <m:has_related_eccairs_term rdf:resource="http://onto.fel.cvut.cz/ontologies/2014/ECCAIRS_Aviation_1.3.0.12/eccairs-descriptive-factors#category_11661000"/>
    </owl:Class>
    


    <!-- http://onto.fel.cvut.cz/ontologies/aviation-safety/Rotor_drive_indicating_system -->

    <owl:Class rdf:about="&m;Rotor_drive_indicating_system">
        <rdfs:label>Rotor drive indicating system</rdfs:label>
        <rdfs:subClassOf rdf:resource="&m;Main_rotor_drive_system_part"/>
        <m:generated_time rdf:datatype="&xsd;dateTime">2015-04-09T18:56:27.771+02:00</m:generated_time>
        <rdfs:comment xml:lang="en">(ATA Code:6340) Rotor drive indicating system: The indicators, sensors/transmitters and associated systems which indicate operation or activation of rotor systems. Typical parts are tachometer, transmitter, circuit breaker, wiring harness, light, switch, indicator and needle.</rdfs:comment>
        <m:has_related_eccairs_term rdf:resource="http://onto.fel.cvut.cz/ontologies/2014/ECCAIRS_Aviation_1.3.0.12/eccairs-descriptive-factors#category_11634000"/>
    </owl:Class>
    


    <!-- http://onto.fel.cvut.cz/ontologies/aviation-safety/Rotorcraft_flight_control -->

    <owl:Class rdf:about="&m;Rotorcraft_flight_control">
        <rdfs:label>Rotorcraft flight control</rdfs:label>
        <rdfs:subClassOf rdf:resource="&m;Aircraft_part"/>
        <m:generated_time rdf:datatype="&xsd;dateTime">2015-04-09T18:56:27.771+02:00</m:generated_time>
        <rdfs:comment xml:lang="en">(ATA Code:6700) The rotorcraft control system.</rdfs:comment>
        <m:has_related_eccairs_term rdf:resource="http://onto.fel.cvut.cz/ontologies/2014/ECCAIRS_Aviation_1.3.0.12/eccairs-descriptive-factors#category_11670000"/>
    </owl:Class>
    


    <!-- http://onto.fel.cvut.cz/ontologies/aviation-safety/Rotorcraft_flight_control_part -->

    <owl:Class rdf:about="&m;Rotorcraft_flight_control_part">
        <rdfs:label>Rotorcraft flight control part</rdfs:label>
        <rdfs:subClassOf rdf:resource="&m;Aircraft_part"/>
        <rdfs:subClassOf>
            <owl:Restriction>
                <owl:onProperty rdf:resource="http://onto.fel.cvut.cz/ontologies/ufo/is_part_of"/>
                <owl:someValuesFrom rdf:resource="&m;Rotorcraft_flight_control"/>
            </owl:Restriction>
        </rdfs:subClassOf>
        <m:generated_time rdf:datatype="&xsd;dateTime">2015-04-12T02:45:54.351+02:00</m:generated_time>
        <m:has_related_eccairs_term rdf:resource="http://onto.fel.cvut.cz/ontologies/2014/ECCAIRS_Aviation_1.3.0.12/eccairs-descriptive-factors#category_11670000"/>
    </owl:Class>
    


    <!-- http://onto.fel.cvut.cz/ontologies/aviation-safety/Rotorcraft_main_rotor_system -->

    <owl:Class rdf:about="&m;Rotorcraft_main_rotor_system">
        <rdfs:subClassOf rdf:resource="&m;Aircraft_part"/>
    </owl:Class>
    


    <!-- http://onto.fel.cvut.cz/ontologies/aviation-safety/Rotorcraft_main_rotor_system_part -->

    <owl:Class rdf:about="&m;Rotorcraft_main_rotor_system_part">
        <rdfs:label>Rotorcraft main rotor system part</rdfs:label>
        <rdfs:subClassOf rdf:resource="&m;Aircraft_part"/>
        <rdfs:subClassOf>
            <owl:Restriction>
                <owl:onProperty rdf:resource="http://onto.fel.cvut.cz/ontologies/ufo/is_part_of"/>
                <owl:someValuesFrom rdf:resource="&m;Rotorcraft_main_rotor_system"/>
            </owl:Restriction>
        </rdfs:subClassOf>
        <m:generated_time rdf:datatype="&xsd;dateTime">2015-04-12T02:45:54.351+02:00</m:generated_time>
        <m:has_related_eccairs_term rdf:resource="http://onto.fel.cvut.cz/ontologies/2014/ECCAIRS_Aviation_1.3.0.12/eccairs-descriptive-factors#category_11620000"/>
    </owl:Class>
    


    <!-- http://onto.fel.cvut.cz/ontologies/aviation-safety/Rotorcraft_tail_boom -->

    <owl:Class rdf:about="&m;Rotorcraft_tail_boom">
        <rdfs:label>Rotorcraft tail boom</rdfs:label>
        <rdfs:subClassOf rdf:resource="&m;Fuselage_structure_(general)_part"/>
        <m:generated_time rdf:datatype="&xsd;dateTime">2015-04-09T18:56:27.771+02:00</m:generated_time>
        <rdfs:comment xml:lang="en">(ATA Code:5302) Rotorcraft tail boom: The structure, including exterior skin and truss framework, of tail booms on rotorcraft. Includes attachment fittings for tail boom and stabilizer surfaces. Typical parts are bulkhead, bracket, frame, frame tube and plates.</rdfs:comment>
        <m:has_related_eccairs_term rdf:resource="http://onto.fel.cvut.cz/ontologies/2014/ECCAIRS_Aviation_1.3.0.12/eccairs-descriptive-factors#category_11530200"/>
    </owl:Class>
    


    <!-- http://onto.fel.cvut.cz/ontologies/aviation-safety/Rotors_Flight_Control_System_Wiring -->

    <owl:Class rdf:about="&m;Rotors_Flight_Control_System_Wiring">
        <rdfs:label>Rotors Flight Control System Wiring</rdfs:label>
        <rdfs:subClassOf rdf:resource="&m;Rotorcraft_flight_control_part"/>
        <m:generated_time rdf:datatype="&xsd;dateTime">2015-04-09T18:56:27.771+02:00</m:generated_time>
        <rdfs:comment xml:lang="en">(ATA Code:6797) Wiring specific to the Rotors Flight Control System</rdfs:comment>
        <m:has_related_eccairs_term rdf:resource="http://onto.fel.cvut.cz/ontologies/2014/ECCAIRS_Aviation_1.3.0.12/eccairs-descriptive-factors#category_11679700"/>
    </owl:Class>
    


    <!-- http://onto.fel.cvut.cz/ontologies/aviation-safety/Rudder_&amp;_Tab_control_system -->

    <owl:Class rdf:about="&m;Rudder_&amp;_Tab_control_system">
        <rdfs:label>Rudder &amp; Tab control system</rdfs:label>
        <rdfs:subClassOf rdf:resource="&m;Flight_control_system_part"/>
        <m:generated_time rdf:datatype="&xsd;dateTime">2015-04-09T18:56:27.771+02:00</m:generated_time>
        <rdfs:comment xml:lang="en">(ATA Code:2720) Rudder control system: The system components and parts from the cockpit pedals to the rudder surface which cause movement. Includes manual and power assisted systems other than the actuator and autopilot actuating mechanism. Also includes brackets for the support or attachment of pulleys, pushrods, and bellcranks. Does not include control surface hinges or structure [Code 11554000] or the yaw dampers [Code 11221000]. Typical parts are cable, rod end, turnbuckle, bolt, pedal, spring, torque tube, control valve and stops.</rdfs:comment>
        <m:has_related_eccairs_term rdf:resource="http://onto.fel.cvut.cz/ontologies/2014/ECCAIRS_Aviation_1.3.0.12/eccairs-descriptive-factors#category_11272000"/>
    </owl:Class>
    


    <!-- http://onto.fel.cvut.cz/ontologies/aviation-safety/Rudder_&amp;_Tab_control_system_part -->

    <owl:Class rdf:about="&m;Rudder_&amp;_Tab_control_system_part">
        <rdfs:label>Rudder &amp; Tab control system part</rdfs:label>
        <rdfs:subClassOf rdf:resource="&m;Flight_control_system_part"/>
        <rdfs:subClassOf>
            <owl:Restriction>
                <owl:onProperty rdf:resource="http://onto.fel.cvut.cz/ontologies/ufo/is_part_of"/>
                <owl:someValuesFrom rdf:resource="&m;Rudder_&amp;_Tab_control_system"/>
            </owl:Restriction>
        </rdfs:subClassOf>
        <m:generated_time rdf:datatype="&xsd;dateTime">2015-04-12T02:45:54.351+02:00</m:generated_time>
        <m:has_related_eccairs_term rdf:resource="http://onto.fel.cvut.cz/ontologies/2014/ECCAIRS_Aviation_1.3.0.12/eccairs-descriptive-factors#category_11272000"/>
    </owl:Class>
    


    <!-- http://onto.fel.cvut.cz/ontologies/aviation-safety/Rudder_actuator -->

    <owl:Class rdf:about="&m;Rudder_actuator">
        <rdfs:label>Rudder actuator</rdfs:label>
        <rdfs:subClassOf rdf:resource="&m;Rudder_&amp;_Tab_control_system_part"/>
        <m:generated_time rdf:datatype="&xsd;dateTime">2015-04-09T18:56:27.771+02:00</m:generated_time>
        <rdfs:comment xml:lang="en">(ATA Code:2722) Rudder actuator: The system components and parts which actuate the rudder. Typical parts are motor, actuator, actuator bracket, jackscrew, rod-end and seals.</rdfs:comment>
        <m:has_related_eccairs_term rdf:resource="http://onto.fel.cvut.cz/ontologies/2014/ECCAIRS_Aviation_1.3.0.12/eccairs-descriptive-factors#category_11272200"/>
    </owl:Class>
    


    <!-- http://onto.fel.cvut.cz/ontologies/aviation-safety/Rudder_attachment_fitting -->

    <owl:Class rdf:about="&m;Rudder_attachment_fitting">
        <rdfs:label>Rudder attachment fitting</rdfs:label>
        <rdfs:subClassOf rdf:resource="&m;Attachment_fitting_(empennage_flight_control_surfaces)_part"/>
        <m:generated_time rdf:datatype="&xsd;dateTime">2015-04-09T18:56:27.771+02:00</m:generated_time>
        <rdfs:comment xml:lang="en">(ATA Code:5554) Rudder attachment fitting: The fittings on the rudder which are used to support equipment within the structure.</rdfs:comment>
        <m:has_related_eccairs_term rdf:resource="http://onto.fel.cvut.cz/ontologies/2014/ECCAIRS_Aviation_1.3.0.12/eccairs-descriptive-factors#category_11555400"/>
    </owl:Class>
    


    <!-- http://onto.fel.cvut.cz/ontologies/aviation-safety/Rudder_feel_system -->

    <owl:Class rdf:about="&m;Rudder_feel_system">
        <rdfs:label>Rudder feel system</rdfs:label>
        <rdfs:subClassOf rdf:resource="&m;Rudder_&amp;_Tab_control_system_part"/>
        <m:generated_time rdf:datatype="&xsd;dateTime">2015-04-09T18:56:27.771+02:00</m:generated_time>
        <rdfs:comment xml:lang="en">(ATA Code:2723) Rudder feel system: The system incorporated in the rudder control system which provides artificial resistance to the pilot&apos;s input to the rudder pedals.</rdfs:comment>
        <m:has_related_eccairs_term rdf:resource="http://onto.fel.cvut.cz/ontologies/2014/ECCAIRS_Aviation_1.3.0.12/eccairs-descriptive-factors#category_11272300"/>
    </owl:Class>
    


    <!-- http://onto.fel.cvut.cz/ontologies/aviation-safety/Rudder_structure -->

    <owl:Class rdf:about="&m;Rudder_structure">
        <rdfs:label>Rudder structure</rdfs:label>
        <rdfs:subClassOf rdf:resource="&m;Empennage_structure_part"/>
        <m:generated_time rdf:datatype="&xsd;dateTime">2015-04-09T18:56:27.771+02:00</m:generated_time>
        <rdfs:comment xml:lang="en">(ATA Code:5540) Rudder structure: The vertical aerofoil hinged to the vertical stabilizer. Does not include the actuators, actuator mechanism or mounting [Code 11272000]. Typical parts are hinge, hinge fittings, bearing and bolts.</rdfs:comment>
        <m:has_related_eccairs_term rdf:resource="http://onto.fel.cvut.cz/ontologies/2014/ECCAIRS_Aviation_1.3.0.12/eccairs-descriptive-factors#category_11554000"/>
    </owl:Class>
    


    <!-- http://onto.fel.cvut.cz/ontologies/aviation-safety/Rudder_structure_part -->

    <owl:Class rdf:about="&m;Rudder_structure_part">
        <rdfs:label>Rudder structure part</rdfs:label>
        <rdfs:subClassOf rdf:resource="&m;Empennage_structure_part"/>
        <rdfs:subClassOf>
            <owl:Restriction>
                <owl:onProperty rdf:resource="http://onto.fel.cvut.cz/ontologies/ufo/is_part_of"/>
                <owl:someValuesFrom rdf:resource="&m;Rudder_structure"/>
            </owl:Restriction>
        </rdfs:subClassOf>
        <m:generated_time rdf:datatype="&xsd;dateTime">2015-04-12T02:45:54.351+02:00</m:generated_time>
        <m:has_related_eccairs_term rdf:resource="http://onto.fel.cvut.cz/ontologies/2014/ECCAIRS_Aviation_1.3.0.12/eccairs-descriptive-factors#category_11554000"/>
    </owl:Class>
    


    <!-- http://onto.fel.cvut.cz/ontologies/aviation-safety/Rudder_tab_control_system -->

    <owl:Class rdf:about="&m;Rudder_tab_control_system">
        <rdfs:label>Rudder tab control system</rdfs:label>
        <rdfs:subClassOf rdf:resource="&m;Rudder_&amp;_Tab_control_system_part"/>
        <m:generated_time rdf:datatype="&xsd;dateTime">2015-04-09T18:56:27.771+02:00</m:generated_time>
        <rdfs:comment xml:lang="en">(ATA Code:2721) Rudder tab control system: The system components and parts of the rudder trim control system, from the cockpit control to the rudder tab that causes an aerodynamic bias to the direct input from the pilot or autopilot. Does not include hinges or structure [Code 11554300] nor the yaw dampers [Code 1122100]. Typical parts are actuator, actuator bracket, cable, pulley, chain, rod end and bellcrank.</rdfs:comment>
        <m:has_related_eccairs_term rdf:resource="http://onto.fel.cvut.cz/ontologies/2014/ECCAIRS_Aviation_1.3.0.12/eccairs-descriptive-factors#category_11272100"/>
    </owl:Class>
    


    <!-- http://onto.fel.cvut.cz/ontologies/aviation-safety/Rudder_tab_structure -->

    <owl:Class rdf:about="&m;Rudder_tab_structure">
        <rdfs:label>Rudder tab structure</rdfs:label>
        <rdfs:subClassOf rdf:resource="&m;Rudder_structure_part"/>
        <m:generated_time rdf:datatype="&xsd;dateTime">2015-04-09T18:56:27.771+02:00</m:generated_time>
        <rdfs:comment xml:lang="en">(ATA Code:5543) Rudder tab structure: The structure of the movable surface hinged to the rudder surface for directional trim. Typical parts are skin, hinge fitting, spars and ribs.</rdfs:comment>
        <m:has_related_eccairs_term rdf:resource="http://onto.fel.cvut.cz/ontologies/2014/ECCAIRS_Aviation_1.3.0.12/eccairs-descriptive-factors#category_11554300"/>
    </owl:Class>
    


    <!-- http://onto.fel.cvut.cz/ontologies/aviation-safety/STANDARD_PRACTICES_AND_STRUCTURES_-_GENERAL -->

    <owl:Class rdf:about="&m;STANDARD_PRACTICES_AND_STRUCTURES_-_GENERAL">
        <rdfs:label>STANDARD PRACTICES AND STRUCTURES - GENERAL</rdfs:label>
        <rdfs:subClassOf rdf:resource="&m;Aircraft_part"/>
        <m:generated_time rdf:datatype="&xsd;dateTime">2015-04-09T18:56:27.771+02:00</m:generated_time>
        <rdfs:comment xml:lang="en">(ATA Code:5100) Standard Practices, General Procedures and typical repairs applicable to more than one chapter and are not specifically covered under [Chapter (System) 52] thru [Chapter (System) 57] Sub-Sys/Sect breakdown.Repair. The restoration of an aeronautical product to an airworthy condition to ensure that the aircraft continues to comply with the design aspects of the appropriate airworthiness requirements used for the issuance of the Type Certificate for the respective aircraft type, after it has been damaged or subjected to wear. (Annex 8)</rdfs:comment>
        <m:has_related_eccairs_term rdf:resource="http://onto.fel.cvut.cz/ontologies/2014/ECCAIRS_Aviation_1.3.0.12/eccairs-descriptive-factors#category_11510000"/>
    </owl:Class>
    


    <!-- http://onto.fel.cvut.cz/ontologies/aviation-safety/STANDARD_PRACTICES_AND_STRUCTURES_-_GENERAL_part -->

    <owl:Class rdf:about="&m;STANDARD_PRACTICES_AND_STRUCTURES_-_GENERAL_part">
        <rdfs:label>STANDARD PRACTICES AND STRUCTURES - GENERAL part</rdfs:label>
        <rdfs:subClassOf rdf:resource="&m;Aircraft_part"/>
        <rdfs:subClassOf>
            <owl:Restriction>
                <owl:onProperty rdf:resource="http://onto.fel.cvut.cz/ontologies/ufo/is_part_of"/>
                <owl:someValuesFrom rdf:resource="&m;STANDARD_PRACTICES_AND_STRUCTURES_-_GENERAL"/>
            </owl:Restriction>
        </rdfs:subClassOf>
        <m:generated_time rdf:datatype="&xsd;dateTime">2015-04-12T02:45:54.351+02:00</m:generated_time>
        <m:has_related_eccairs_term rdf:resource="http://onto.fel.cvut.cz/ontologies/2014/ECCAIRS_Aviation_1.3.0.12/eccairs-descriptive-factors#category_11510000"/>
    </owl:Class>
    


    <!-- http://onto.fel.cvut.cz/ontologies/aviation-safety/Satcom -->

    <owl:Class rdf:about="&m;Satcom">
        <rdfs:label>Satcom</rdfs:label>
        <rdfs:subClassOf rdf:resource="&m;speech_communication_system"/>
        <m:generated_time rdf:datatype="&xsd;dateTime">2015-04-09T18:56:27.771+02:00</m:generated_time>
        <rdfs:comment xml:lang="en">(ATA Code:2315) Satcom: That portion of the system which utilizes satellite communication systems (Satcom).</rdfs:comment>
        <m:has_related_eccairs_term rdf:resource="http://onto.fel.cvut.cz/ontologies/2014/ECCAIRS_Aviation_1.3.0.12/eccairs-descriptive-factors#category_11231500"/>
    </owl:Class>
    


    <!-- http://onto.fel.cvut.cz/ontologies/aviation-safety/Seat-cargo_attachment_fittings_(on_fuselage) -->

    <owl:Class rdf:about="&m;Seat-cargo_attachment_fittings_(on_fuselage)">
        <rdfs:label>Seat/cargo attachment fittings (on fuselage)</rdfs:label>
        <rdfs:subClassOf rdf:resource="&m;Fuselage_attachment_fittings_part"/>
        <m:generated_time rdf:datatype="&xsd;dateTime">2015-04-09T18:56:27.771+02:00</m:generated_time>
        <rdfs:comment xml:lang="en">(ATA Code:5347) Seat/cargo attachment fittings (on fuselage): The fittings on the fuselage used for the attachment of seats and cargo restraint mechanisms.</rdfs:comment>
        <m:has_related_eccairs_term rdf:resource="http://onto.fel.cvut.cz/ontologies/2014/ECCAIRS_Aviation_1.3.0.12/eccairs-descriptive-factors#category_11534700"/>
    </owl:Class>
    


    <!-- http://onto.fel.cvut.cz/ontologies/aviation-safety/Selcal -->

    <owl:Class rdf:about="&m;Selcal">
        <rdfs:label>Selcal</rdfs:label>
        <rdfs:subClassOf rdf:resource="&m;Data_transmission_automatic_call_part"/>
        <m:generated_time rdf:datatype="&xsd;dateTime">2015-04-09T18:56:27.771+02:00</m:generated_time>
        <rdfs:comment xml:lang="en">(ATA Code:2321) Selcal: That portion of the system which permits the selective calling of individual aircraft over radiotelephone channels linking a ground station with the aircraft. ICAO Annex 10.A system that provides an automatic and selective method of calling any aircraft. Voice calling is replaced by the transmission of code tones to the aircraft over the international radiotelephony channels.</rdfs:comment>
        <m:has_related_eccairs_term rdf:resource="http://onto.fel.cvut.cz/ontologies/2014/ECCAIRS_Aviation_1.3.0.12/eccairs-descriptive-factors#category_11232100"/>
    </owl:Class>
    


    <!-- http://onto.fel.cvut.cz/ontologies/aviation-safety/Service_doors -->

    <owl:Class rdf:about="&m;Service_doors">
        <rdfs:label>Service doors</rdfs:label>
        <rdfs:subClassOf rdf:resource="&m;Fuselage_doors_part"/>
        <m:generated_time rdf:datatype="&xsd;dateTime">2015-04-09T18:56:27.771+02:00</m:generated_time>
        <rdfs:comment xml:lang="en">(ATA Code:5240) Service doors: The exterior doors used to gain access for servicing aircraft systems and equipment.</rdfs:comment>
        <m:has_related_eccairs_term rdf:resource="http://onto.fel.cvut.cz/ontologies/2014/ECCAIRS_Aviation_1.3.0.12/eccairs-descriptive-factors#category_11524000"/>
    </owl:Class>
    


    <!-- http://onto.fel.cvut.cz/ontologies/aviation-safety/Service_doors_part -->

    <owl:Class rdf:about="&m;Service_doors_part">
        <rdfs:label>Service doors part</rdfs:label>
        <rdfs:subClassOf rdf:resource="&m;Fuselage_doors_part"/>
        <rdfs:subClassOf>
            <owl:Restriction>
                <owl:onProperty rdf:resource="http://onto.fel.cvut.cz/ontologies/ufo/is_part_of"/>
                <owl:someValuesFrom rdf:resource="&m;Service_doors"/>
            </owl:Restriction>
        </rdfs:subClassOf>
        <m:generated_time rdf:datatype="&xsd;dateTime">2015-04-12T02:45:54.351+02:00</m:generated_time>
        <m:has_related_eccairs_term rdf:resource="http://onto.fel.cvut.cz/ontologies/2014/ECCAIRS_Aviation_1.3.0.12/eccairs-descriptive-factors#category_11524000"/>
    </owl:Class>
    


    <!-- http://onto.fel.cvut.cz/ontologies/aviation-safety/Servicing_of_the_aircraft_with_liquids -->

    <owl:Class rdf:about="&m;Servicing_of_the_aircraft_with_liquids">
        <rdfs:label>Servicing of the aircraft with liquids</rdfs:label>
        <rdfs:subClassOf rdf:resource="&m;Aircraft_part"/>
        <m:generated_time rdf:datatype="&xsd;dateTime">2015-04-09T18:56:27.771+02:00</m:generated_time>
        <rdfs:comment xml:lang="en">(ATA Code:1200) Servicing of the aircraft with liquids</rdfs:comment>
        <m:has_related_eccairs_term rdf:resource="http://onto.fel.cvut.cz/ontologies/2014/ECCAIRS_Aviation_1.3.0.12/eccairs-descriptive-factors#category_11120000"/>
    </owl:Class>
    


    <!-- http://onto.fel.cvut.cz/ontologies/aviation-safety/Servicing_of_the_aircraft_with_liquids_part -->

    <owl:Class rdf:about="&m;Servicing_of_the_aircraft_with_liquids_part">
        <rdfs:label>Servicing of the aircraft with liquids part</rdfs:label>
        <rdfs:subClassOf rdf:resource="&m;Aircraft_part"/>
        <rdfs:subClassOf>
            <owl:Restriction>
                <owl:onProperty rdf:resource="http://onto.fel.cvut.cz/ontologies/ufo/is_part_of"/>
                <owl:someValuesFrom rdf:resource="&m;Servicing_of_the_aircraft_with_liquids"/>
            </owl:Restriction>
        </rdfs:subClassOf>
        <m:generated_time rdf:datatype="&xsd;dateTime">2015-04-12T02:45:54.351+02:00</m:generated_time>
        <m:has_related_eccairs_term rdf:resource="http://onto.fel.cvut.cz/ontologies/2014/ECCAIRS_Aviation_1.3.0.12/eccairs-descriptive-factors#category_11120000"/>
    </owl:Class>
    


    <!-- http://onto.fel.cvut.cz/ontologies/aviation-safety/Servicing_the_aircraft_with_any_type_of_aviation_fuel -->

    <owl:Class rdf:about="&m;Servicing_the_aircraft_with_any_type_of_aviation_fuel">
        <rdfs:label>Servicing the aircraft with any type of aviation fuel</rdfs:label>
        <rdfs:subClassOf rdf:resource="&m;Servicing_of_the_aircraft_with_liquids_part"/>
        <m:generated_time rdf:datatype="&xsd;dateTime">2015-04-09T18:56:27.771+02:00</m:generated_time>
        <rdfs:comment xml:lang="en">(ATA Code:1210) Servicing the aircraft with any type of aviation fuel</rdfs:comment>
        <m:has_related_eccairs_term rdf:resource="http://onto.fel.cvut.cz/ontologies/2014/ECCAIRS_Aviation_1.3.0.12/eccairs-descriptive-factors#category_11121000"/>
    </owl:Class>
    


    <!-- http://onto.fel.cvut.cz/ontologies/aviation-safety/Servicing_the_aircraft_with_any_type_of_hydraulic_fluid -->

    <owl:Class rdf:about="&m;Servicing_the_aircraft_with_any_type_of_hydraulic_fluid">
        <rdfs:label>Servicing the aircraft with any type of hydraulic fluid</rdfs:label>
        <rdfs:subClassOf rdf:resource="&m;Servicing_of_the_aircraft_with_liquids_part"/>
        <m:generated_time rdf:datatype="&xsd;dateTime">2015-04-09T18:56:27.771+02:00</m:generated_time>
        <rdfs:comment xml:lang="en">(ATA Code:1230) Servicing the aircraft with any type of hydraulic fluid</rdfs:comment>
        <m:has_related_eccairs_term rdf:resource="http://onto.fel.cvut.cz/ontologies/2014/ECCAIRS_Aviation_1.3.0.12/eccairs-descriptive-factors#category_11123000"/>
    </owl:Class>
    


    <!-- http://onto.fel.cvut.cz/ontologies/aviation-safety/Servicing_the_aircraft_with_aviation_lubricating_oil -->

    <owl:Class rdf:about="&m;Servicing_the_aircraft_with_aviation_lubricating_oil">
        <rdfs:label>Servicing the aircraft with aviation lubricating oil</rdfs:label>
        <rdfs:subClassOf rdf:resource="&m;Servicing_of_the_aircraft_with_liquids_part"/>
        <m:generated_time rdf:datatype="&xsd;dateTime">2015-04-09T18:56:27.771+02:00</m:generated_time>
        <rdfs:comment xml:lang="en">(ATA Code:1220) Servicing the aircraft with aviation lubricating oil</rdfs:comment>
        <m:has_related_eccairs_term rdf:resource="http://onto.fel.cvut.cz/ontologies/2014/ECCAIRS_Aviation_1.3.0.12/eccairs-descriptive-factors#category_11122000"/>
    </owl:Class>
    


    <!-- http://onto.fel.cvut.cz/ontologies/aviation-safety/Servo_system -->

    <owl:Class rdf:about="&m;Servo_system">
        <rdfs:label>Servo system</rdfs:label>
        <rdfs:subClassOf rdf:resource="&m;Rotorcraft_flight_control_part"/>
        <m:generated_time rdf:datatype="&xsd;dateTime">2015-04-09T18:56:27.771+02:00</m:generated_time>
        <rdfs:comment xml:lang="en">(ATA Code:6730) Servo system: The system which ensures distribution of mechanical or electrical power to the rotor servo-control system. Includes items used to monitor and indicate operation of the servo control system. Typical parts are pressure relief valves, electro valves, check valves and accumulators.</rdfs:comment>
        <m:has_related_eccairs_term rdf:resource="http://onto.fel.cvut.cz/ontologies/2014/ECCAIRS_Aviation_1.3.0.12/eccairs-descriptive-factors#category_11673000"/>
    </owl:Class>
    


    <!-- http://onto.fel.cvut.cz/ontologies/aviation-safety/Shoring -->

    <owl:Class rdf:about="&m;Shoring">
        <rdfs:label>Shoring</rdfs:label>
        <rdfs:subClassOf rdf:resource="&m;Lifting_and_shoring_part"/>
        <m:generated_time rdf:datatype="&xsd;dateTime">2015-04-09T18:56:27.771+02:00</m:generated_time>
        <rdfs:comment xml:lang="en">(ATA Code:0720) Data necessary to support the aircraft during maintenance and repair.   Includes information on shoring materials and equipment, contour dimensions, shoring locations, etc.</rdfs:comment>
        <m:has_related_eccairs_term rdf:resource="http://onto.fel.cvut.cz/ontologies/2014/ECCAIRS_Aviation_1.3.0.12/eccairs-descriptive-factors#category_11072000"/>
    </owl:Class>
    


    <!-- http://onto.fel.cvut.cz/ontologies/aviation-safety/Smoke_detection_system -->

    <owl:Class rdf:about="&m;Smoke_detection_system">
        <rdfs:label>Smoke detection system</rdfs:label>
        <rdfs:subClassOf rdf:resource="&m;Fire-smoke-overheat_detection_system_part"/>
        <m:generated_time rdf:datatype="&xsd;dateTime">2015-04-09T18:56:27.771+02:00</m:generated_time>
        <rdfs:comment xml:lang="en">(ATA Code:2611) Smoke detection system: The system used to sense and indicate the presence of smoke in any of the protected areas of the aircraft. Typical parts are detector, sensor, wiring, relay, amplifier and test circuit.</rdfs:comment>
        <m:has_related_eccairs_term rdf:resource="http://onto.fel.cvut.cz/ontologies/2014/ECCAIRS_Aviation_1.3.0.12/eccairs-descriptive-factors#category_11261100"/>
    </owl:Class>
    


    <!-- http://onto.fel.cvut.cz/ontologies/aviation-safety/Spark_plug-igniter -->

    <owl:Class rdf:about="&m;Spark_plug-igniter">
        <rdfs:label>Spark plug/igniter</rdfs:label>
        <rdfs:subClassOf rdf:resource="&m;Ignition_harness_part"/>
        <m:generated_time rdf:datatype="&xsd;dateTime">2015-04-09T18:56:27.771+02:00</m:generated_time>
        <rdfs:comment xml:lang="en">(ATA Code:7421) Spark plug/igniter: The part which provides the spark in the reciprocating engine cylinders or combustion chamber of turbine engines.</rdfs:comment>
        <m:has_related_eccairs_term rdf:resource="http://onto.fel.cvut.cz/ontologies/2014/ECCAIRS_Aviation_1.3.0.12/eccairs-descriptive-factors#category_11742100"/>
    </owl:Class>
    


    <!-- http://onto.fel.cvut.cz/ontologies/aviation-safety/Spars-ribs_(horizontal_stabilizer) -->

    <owl:Class rdf:about="&m;Spars-ribs_(horizontal_stabilizer)">
        <rdfs:label>Spars/ribs (horizontal stabilizer)</rdfs:label>
        <rdfs:subClassOf rdf:resource="&m;Horizontal_stabilizer_structure_part"/>
        <m:generated_time rdf:datatype="&xsd;dateTime">2015-04-09T18:56:27.771+02:00</m:generated_time>
        <rdfs:comment xml:lang="en">(ATA Code:5511) The spars/ribs of the horizontal stabilizer.</rdfs:comment>
        <m:has_related_eccairs_term rdf:resource="http://onto.fel.cvut.cz/ontologies/2014/ECCAIRS_Aviation_1.3.0.12/eccairs-descriptive-factors#category_11551100"/>
    </owl:Class>
    


    <!-- http://onto.fel.cvut.cz/ontologies/aviation-safety/Spars-ribs_(rudder) -->

    <owl:Class rdf:about="&m;Spars-ribs_(rudder)">
        <rdfs:label>Spars/ribs (rudder)</rdfs:label>
        <rdfs:subClassOf rdf:resource="&m;Rudder_structure_part"/>
        <m:generated_time rdf:datatype="&xsd;dateTime">2015-04-09T18:56:27.771+02:00</m:generated_time>
        <rdfs:comment xml:lang="en">(ATA Code:5541) The spars or ribs of the rudder structure.</rdfs:comment>
        <m:has_related_eccairs_term rdf:resource="http://onto.fel.cvut.cz/ontologies/2014/ECCAIRS_Aviation_1.3.0.12/eccairs-descriptive-factors#category_11554100"/>
    </owl:Class>
    


    <!-- http://onto.fel.cvut.cz/ontologies/aviation-safety/Speed-attitude_correction_system -->

    <owl:Class rdf:about="&m;Speed-attitude_correction_system">
        <rdfs:label>Speed-attitude correction system</rdfs:label>
        <rdfs:subClassOf rdf:resource="&m;autoflight_system"/>
        <m:generated_time rdf:datatype="&xsd;dateTime">2015-04-09T18:56:27.771+02:00</m:generated_time>
        <all2:has_ATA_code rdf:datatype="&xsd;integer">2220</all2:has_ATA_code>
        <rdfs:comment xml:lang="en">(ATA Code:2220) Speed-attitude correction: The system which automatically maintains safe flight conditions by correcting for effects of speed and out-of-trim conditions using means such as automatic trim, Mach trim, or speed stability and Mach feel. This includes sensing, computing, actuating, indicating, internal monitoring and warning devices.</rdfs:comment>
        <m:has_related_eccairs_term rdf:resource="http://onto.fel.cvut.cz/ontologies/2014/ECCAIRS_Aviation_1.3.0.12/eccairs-descriptive-factors#category_11222000"/>
    </owl:Class>
    


    <!-- http://onto.fel.cvut.cz/ontologies/aviation-safety/Spoiler_structure -->

    <owl:Class rdf:about="&m;Spoiler_structure">
        <rdfs:label>Spoiler structure</rdfs:label>
        <rdfs:subClassOf rdf:resource="&m;Wing_structure_part"/>
        <m:generated_time rdf:datatype="&xsd;dateTime">2015-04-09T18:56:27.771+02:00</m:generated_time>
        <rdfs:comment xml:lang="en">(ATA Code:5770) Spoiler structure: The structural aspects of the movable surface on the upper surface of the wing for increasing drag and lift reducing functions. Does not include operating mechanism such as actuators, hoses and lines.</rdfs:comment>
        <m:has_related_eccairs_term rdf:resource="http://onto.fel.cvut.cz/ontologies/2014/ECCAIRS_Aviation_1.3.0.12/eccairs-descriptive-factors#category_11577000"/>
    </owl:Class>
    


    <!-- http://onto.fel.cvut.cz/ontologies/aviation-safety/Spoiler_system -->

    <owl:Class rdf:about="&m;Spoiler_system">
        <rdfs:label>Spoiler system</rdfs:label>
        <rdfs:subClassOf rdf:resource="&m;Drag_control_system_part"/>
        <m:generated_time rdf:datatype="&xsd;dateTime">2015-04-09T18:56:27.771+02:00</m:generated_time>
        <rdfs:comment xml:lang="en">(ATA Code:2762) Spoiler system: The components that actuate the aerodynamic spoiler surfaces on the wing for lift reducing purposes. Typical parts are seal, rod end bearing and rod end.</rdfs:comment>
        <m:has_related_eccairs_term rdf:resource="http://onto.fel.cvut.cz/ontologies/2014/ECCAIRS_Aviation_1.3.0.12/eccairs-descriptive-factors#category_11276200"/>
    </owl:Class>
    


    <!-- http://onto.fel.cvut.cz/ontologies/aviation-safety/Stabilizer_System_Wiring -->

    <owl:Class rdf:about="&m;Stabilizer_System_Wiring">
        <rdfs:label>Stabilizer System Wiring</rdfs:label>
        <rdfs:subClassOf rdf:resource="&m;Empennage_structure_part"/>
        <m:generated_time rdf:datatype="&xsd;dateTime">2015-04-09T18:56:27.771+02:00</m:generated_time>
        <rdfs:comment xml:lang="en">(ATA Code:5597) Wiring specific to the Stabilizer System</rdfs:comment>
        <m:has_related_eccairs_term rdf:resource="http://onto.fel.cvut.cz/ontologies/2014/ECCAIRS_Aviation_1.3.0.12/eccairs-descriptive-factors#category_11559700"/>
    </owl:Class>
    


    <!-- http://onto.fel.cvut.cz/ontologies/aviation-safety/Stabilizer_attachment_fittings_(on_fuselage) -->

    <owl:Class rdf:about="&m;Stabilizer_attachment_fittings_(on_fuselage)">
        <rdfs:label>Stabilizer attachment fittings (on fuselage)</rdfs:label>
        <rdfs:subClassOf rdf:resource="&m;Fuselage_attachment_fittings_part"/>
        <m:generated_time rdf:datatype="&xsd;dateTime">2015-04-09T18:56:27.771+02:00</m:generated_time>
        <rdfs:comment xml:lang="en">(ATA Code:5342) Stabilizer attachment fittings (on fuselage): The fittings on the fuselage used for the attachment of the stabilizers.</rdfs:comment>
        <m:has_related_eccairs_term rdf:resource="http://onto.fel.cvut.cz/ontologies/2014/ECCAIRS_Aviation_1.3.0.12/eccairs-descriptive-factors#category_11534200"/>
    </owl:Class>
    


    <!-- http://onto.fel.cvut.cz/ontologies/aviation-safety/Stabilizer_fairing -->

    <owl:Class rdf:about="&m;Stabilizer_fairing">
        <rdfs:label>Stabilizer fairing</rdfs:label>
        <rdfs:subClassOf rdf:resource="&m;Empennage_structure_part"/>
        <m:generated_time rdf:datatype="&xsd;dateTime">2015-04-09T18:56:27.771+02:00</m:generated_time>
        <rdfs:comment xml:lang="en">(ATA Code:5560) Stabilizer fairing: The fixed or removable aerodynamic fairings between the fuselage and the stabilizer.</rdfs:comment>
        <m:has_related_eccairs_term rdf:resource="http://onto.fel.cvut.cz/ontologies/2014/ECCAIRS_Aviation_1.3.0.12/eccairs-descriptive-factors#category_11556000"/>
    </owl:Class>
    


    <!-- http://onto.fel.cvut.cz/ontologies/aviation-safety/Stabilizer_position_indicating_system -->

    <owl:Class rdf:about="&m;Stabilizer_position_indicating_system">
        <rdfs:label>Stabilizer position indicating system</rdfs:label>
        <rdfs:subClassOf rdf:resource="&m;Horizontal_stabilizer_control_system_part"/>
        <m:generated_time rdf:datatype="&xsd;dateTime">2015-04-09T18:56:27.771+02:00</m:generated_time>
        <rdfs:comment xml:lang="en">(ATA Code:2741) Stabilizer position indicating system: The system components and parts that sense, transmit and indicate relative position of movable stabilizers for purpose of pitch trim. Typical parts are indicators and transmitters.</rdfs:comment>
        <m:has_related_eccairs_term rdf:resource="http://onto.fel.cvut.cz/ontologies/2014/ECCAIRS_Aviation_1.3.0.12/eccairs-descriptive-factors#category_11274100"/>
    </owl:Class>
    


    <!-- http://onto.fel.cvut.cz/ontologies/aviation-safety/Stall_protection_system -->

    <owl:Class rdf:about="&m;Stall_protection_system">
        <rdfs:label>Stall protection system</rdfs:label>
        <rdfs:subClassOf rdf:resource="&m;Elevator_&amp;_Tab_control_system_part"/>
        <m:generated_time rdf:datatype="&xsd;dateTime">2015-04-09T18:56:27.771+02:00</m:generated_time>
        <rdfs:comment xml:lang="en">(ATA Code:2734) Stall protection system: The system installed to provide an automatic reduction in the angle of attack if the aircraft approaches a stall.</rdfs:comment>
        <m:has_related_eccairs_term rdf:resource="http://onto.fel.cvut.cz/ontologies/2014/ECCAIRS_Aviation_1.3.0.12/eccairs-descriptive-factors#category_11273400"/>
    </owl:Class>
    


    <!-- http://onto.fel.cvut.cz/ontologies/aviation-safety/Stall_warning_system -->

    <owl:Class rdf:about="&m;Stall_warning_system">
        <rdfs:label>Stall warning system</rdfs:label>
        <rdfs:subClassOf rdf:resource="&m;Flight_environment_data_system"/>
        <m:generated_time rdf:datatype="&xsd;dateTime">2015-04-09T18:56:27.771+02:00</m:generated_time>
        <rdfs:comment xml:lang="en">(ATA Code:3418) Stall warning system: The system components and parts, including the computer, which sense, transmit and provide aural, visual and stick shaker warning of an aircraft in an impending flight stall condition. Typical parts are transducer, stall warning detector, switch, vane, horn, lamp, stick shaker, heater element, warning unit computer and module.</rdfs:comment>
        <m:has_related_eccairs_term rdf:resource="http://onto.fel.cvut.cz/ontologies/2014/ECCAIRS_Aviation_1.3.0.12/eccairs-descriptive-factors#category_11341800"/>
    </owl:Class>
    


    <!-- http://onto.fel.cvut.cz/ontologies/aviation-safety/Starter-generator -->

    <owl:Class rdf:about="&m;Starter-generator">
        <rdfs:label>Starter-generator</rdfs:label>
        <rdfs:subClassOf rdf:resource="&m;Direct_current_generating_system_part"/>
        <m:generated_time rdf:datatype="&xsd;dateTime">2015-04-09T18:56:27.771+02:00</m:generated_time>
        <rdfs:comment xml:lang="en">(ATA Code:2435) Starter-generator: The single component used for both engine starting and direct current generation on turbine engines. Typical parts are bearing, shaft, brush, fan, retainer ring, armature, brush, housing, end bell and terminals.</rdfs:comment>
        <m:has_related_eccairs_term rdf:resource="http://onto.fel.cvut.cz/ontologies/2014/ECCAIRS_Aviation_1.3.0.12/eccairs-descriptive-factors#category_11243500"/>
    </owl:Class>
    


    <!-- http://onto.fel.cvut.cz/ontologies/aviation-safety/Static_discharge_system -->

    <owl:Class rdf:about="&m;Static_discharge_system">
        <rdfs:label>Static discharge system</rdfs:label>
        <rdfs:subClassOf rdf:resource="&m;Aircraft_communication_related_system"/>
        <m:generated_time rdf:datatype="&xsd;dateTime">2015-04-09T18:56:27.771+02:00</m:generated_time>
        <rdfs:comment xml:lang="en">(ATA Code:2360) Static discharge system: That portion of the system which dissipates static electricity. Does not include bonding straps on engine or airframe used to assure paths for DC current. Typical parts are wicks and bonding straps.</rdfs:comment>
        <m:has_related_eccairs_term rdf:resource="http://onto.fel.cvut.cz/ontologies/2014/ECCAIRS_Aviation_1.3.0.12/eccairs-descriptive-factors#category_11236000"/>
    </owl:Class>
    


    <!-- http://onto.fel.cvut.cz/ontologies/aviation-safety/Supplementary_Air -->

    <owl:Class rdf:about="&m;Supplementary_Air">
        <rdfs:label>Supplementary Air</rdfs:label>
        <rdfs:subClassOf rdf:resource="&m;Engine_exhaust_system_part"/>
        <m:generated_time rdf:datatype="&xsd;dateTime">2015-04-09T18:56:27.771+02:00</m:generated_time>
        <rdfs:comment xml:lang="en">(ATA Code:7840) That portion of the system which varies and controls supplementary air flow of the exhaust system.  Includes items such as tertiary air doors, actuators, linkages, springs, plumbing, wiring, position indicators, warning systems, etc.</rdfs:comment>
        <m:has_related_eccairs_term rdf:resource="http://onto.fel.cvut.cz/ontologies/2014/ECCAIRS_Aviation_1.3.0.12/eccairs-descriptive-factors#category_11784000"/>
    </owl:Class>
    


    <!-- http://onto.fel.cvut.cz/ontologies/aviation-safety/System_monitor -->

    <owl:Class rdf:about="&m;System_monitor">
        <rdfs:label>System monitor</rdfs:label>
        <rdfs:subClassOf rdf:resource="&m;autoflight_system"/>
        <m:generated_time rdf:datatype="&xsd;dateTime">2015-04-09T18:56:27.771+02:00</m:generated_time>
        <rdfs:comment xml:lang="en">(ATA Code:2240) System monitor: The unit which provides separate or external monitoring/remote readout (for maintenance or other purposes) not directly related to the internal system monitoring (for system integrity flight crew warning). This includes sensing, computing, indicating and warning devices and control panels.</rdfs:comment>
        <m:has_related_eccairs_term rdf:resource="http://onto.fel.cvut.cz/ontologies/2014/ECCAIRS_Aviation_1.3.0.12/eccairs-descriptive-factors#category_11224000"/>
    </owl:Class>
    


    <!-- http://onto.fel.cvut.cz/ontologies/aviation-safety/Tail_Rotor_Drive_System_Wiring -->

    <owl:Class rdf:about="&m;Tail_Rotor_Drive_System_Wiring">
        <rdfs:label>Tail Rotor Drive System Wiring</rdfs:label>
        <rdfs:subClassOf rdf:resource="&m;Tail_rotor_drive_system_part"/>
        <rdfs:subClassOf rdf:resource="&m;Wiring"/>
        <rdfs:subClassOf>
            <owl:Restriction>
                <owl:onProperty rdf:resource="http://onto.fel.cvut.cz/ontologies/ufo/is_part_of"/>
                <owl:someValuesFrom rdf:resource="&m;Tail_rotor_drive_system"/>
            </owl:Restriction>
        </rdfs:subClassOf>
        <m:generated_time rdf:datatype="&xsd;dateTime">2015-04-09T18:56:27.771+02:00</m:generated_time>
        <rdfs:comment xml:lang="en">(ATA Code:6597) Wiring specific to the Tail Rotor Drive System</rdfs:comment>
        <m:has_related_eccairs_term rdf:resource="http://onto.fel.cvut.cz/ontologies/2014/ECCAIRS_Aviation_1.3.0.12/eccairs-descriptive-factors#category_11659700"/>
    </owl:Class>
    


    <!-- http://onto.fel.cvut.cz/ontologies/aviation-safety/Tail_Rotor_System_Wiring -->

    <owl:Class rdf:about="&m;Tail_Rotor_System_Wiring">
        <rdfs:label>Tail Rotor System Wiring</rdfs:label>
        <rdfs:subClassOf rdf:resource="&m;Tail_rotor_system_part"/>
        <rdfs:subClassOf rdf:resource="&m;Wiring"/>
        <rdfs:subClassOf>
            <owl:Restriction>
                <owl:onProperty rdf:resource="http://onto.fel.cvut.cz/ontologies/ufo/is_part_of"/>
                <owl:someValuesFrom rdf:resource="&m;Tail_rotor_system"/>
            </owl:Restriction>
        </rdfs:subClassOf>
        <m:generated_time rdf:datatype="&xsd;dateTime">2015-04-09T18:56:27.771+02:00</m:generated_time>
        <rdfs:comment xml:lang="en">(ATA Code:6497) Wiring specific to the Tail Rotor System</rdfs:comment>
        <m:has_related_eccairs_term rdf:resource="http://onto.fel.cvut.cz/ontologies/2014/ECCAIRS_Aviation_1.3.0.12/eccairs-descriptive-factors#category_11649700"/>
    </owl:Class>
    


    <!-- http://onto.fel.cvut.cz/ontologies/aviation-safety/Tail_cone_door -->

    <owl:Class rdf:about="&m;Tail_cone_door">
        <rdfs:label>Tail cone door</rdfs:label>
        <rdfs:subClassOf rdf:resource="&m;Service_doors_part"/>
        <m:generated_time rdf:datatype="&xsd;dateTime">2015-04-09T18:56:27.771+02:00</m:generated_time>
        <rdfs:comment xml:lang="en">(ATA Code:5248) The tail cone door. Typical parts are hinges, structure and the latch mechanism.</rdfs:comment>
        <m:has_related_eccairs_term rdf:resource="http://onto.fel.cvut.cz/ontologies/2014/ECCAIRS_Aviation_1.3.0.12/eccairs-descriptive-factors#category_11524800"/>
    </owl:Class>
    


    <!-- http://onto.fel.cvut.cz/ontologies/aviation-safety/Tail_pylon_folding -->

    <owl:Class rdf:about="&m;Tail_pylon_folding">
        <rdfs:label>Tail pylon folding</rdfs:label>
        <rdfs:subClassOf rdf:resource="&m;Folding_blades-pylon_part"/>
        <m:generated_time rdf:datatype="&xsd;dateTime">2015-04-09T18:56:27.771+02:00</m:generated_time>
        <rdfs:comment xml:lang="en">(ATA Code:6620) Part of system ensuring tail pylon folding and spreading; includes mechanical, hydraulic and electrical means permanently fitted on the aircraft.</rdfs:comment>
        <m:has_related_eccairs_term rdf:resource="http://onto.fel.cvut.cz/ontologies/2014/ECCAIRS_Aviation_1.3.0.12/eccairs-descriptive-factors#category_11662000"/>
    </owl:Class>
    


    <!-- http://onto.fel.cvut.cz/ontologies/aviation-safety/Tail_rotor_blade -->

    <owl:Class rdf:about="&m;Tail_rotor_blade">
        <rdfs:label>Tail rotor blade</rdfs:label>
        <rdfs:subClassOf rdf:resource="&m;Tail_rotor_system_part"/>
        <m:generated_time rdf:datatype="&xsd;dateTime">2015-04-09T18:56:27.771+02:00</m:generated_time>
        <rdfs:comment xml:lang="en">(ATA Code:6410) The tail rotor blade assemblies, including the heating mats (electrical resistors) for anti-icing but not the anti-icing system [Code 11306000]. Also includes attachment to rotor head. Typical parts are blade and attach bolt.</rdfs:comment>
        <m:has_related_eccairs_term rdf:resource="http://onto.fel.cvut.cz/ontologies/2014/ECCAIRS_Aviation_1.3.0.12/eccairs-descriptive-factors#category_11641000"/>
    </owl:Class>
    


    <!-- http://onto.fel.cvut.cz/ontologies/aviation-safety/Tail_rotor_drive_indicating_system -->

    <owl:Class rdf:about="&m;Tail_rotor_drive_indicating_system">
        <rdfs:label>Tail rotor drive indicating system</rdfs:label>
        <rdfs:subClassOf rdf:resource="&m;Tail_rotor_drive_system_part"/>
        <m:generated_time rdf:datatype="&xsd;dateTime">2015-04-09T18:56:27.771+02:00</m:generated_time>
        <rdfs:comment xml:lang="en">(ATA Code:6540) Tail rotor drive indicating system: The indicators, sensors, transmitters and associated systems which indicate operation or activation of the tail rotor drive system.</rdfs:comment>
        <m:has_related_eccairs_term rdf:resource="http://onto.fel.cvut.cz/ontologies/2014/ECCAIRS_Aviation_1.3.0.12/eccairs-descriptive-factors#category_11654000"/>
    </owl:Class>
    


    <!-- http://onto.fel.cvut.cz/ontologies/aviation-safety/Tail_rotor_drive_shaft -->

    <owl:Class rdf:about="&m;Tail_rotor_drive_shaft">
        <rdfs:label>Tail rotor drive shaft</rdfs:label>
        <rdfs:subClassOf rdf:resource="&m;Tail_rotor_drive_system_part"/>
        <m:generated_time rdf:datatype="&xsd;dateTime">2015-04-09T18:56:27.771+02:00</m:generated_time>
        <rdfs:comment xml:lang="en">(ATA Code:6510) Tail rotor drive shaft: The shafts, flexible couplings and bearings, from the main rotor transmission to the tail rotor assembly. Typical parts shaft, coupling, bearing and hanger.</rdfs:comment>
        <m:has_related_eccairs_term rdf:resource="http://onto.fel.cvut.cz/ontologies/2014/ECCAIRS_Aviation_1.3.0.12/eccairs-descriptive-factors#category_11651000"/>
    </owl:Class>
    


    <!-- http://onto.fel.cvut.cz/ontologies/aviation-safety/Tail_rotor_drive_system -->

    <owl:Class rdf:about="&m;Tail_rotor_drive_system">
        <rdfs:label>Tail rotor drive system</rdfs:label>
        <rdfs:subClassOf rdf:resource="&m;Aircraft_part"/>
        <m:generated_time rdf:datatype="&xsd;dateTime">2015-04-09T18:56:27.771+02:00</m:generated_time>
        <rdfs:comment xml:lang="en">(ATA Code:6500) Tail rotor drive system: The components transmitting power to the tail rotor.</rdfs:comment>
        <m:has_related_eccairs_term rdf:resource="http://onto.fel.cvut.cz/ontologies/2014/ECCAIRS_Aviation_1.3.0.12/eccairs-descriptive-factors#category_11650000"/>
    </owl:Class>
    


    <!-- http://onto.fel.cvut.cz/ontologies/aviation-safety/Tail_rotor_drive_system_part -->

    <owl:Class rdf:about="&m;Tail_rotor_drive_system_part">
        <rdfs:label>Tail rotor drive system part</rdfs:label>
        <rdfs:subClassOf rdf:resource="&m;Aircraft_part"/>
        <rdfs:subClassOf>
            <owl:Restriction>
                <owl:onProperty rdf:resource="http://onto.fel.cvut.cz/ontologies/ufo/is_part_of"/>
                <owl:someValuesFrom rdf:resource="&m;Tail_rotor_drive_system"/>
            </owl:Restriction>
        </rdfs:subClassOf>
        <m:generated_time rdf:datatype="&xsd;dateTime">2015-04-12T02:45:54.351+02:00</m:generated_time>
        <m:has_related_eccairs_term rdf:resource="http://onto.fel.cvut.cz/ontologies/2014/ECCAIRS_Aviation_1.3.0.12/eccairs-descriptive-factors#category_11650000"/>
    </owl:Class>
    


    <!-- http://onto.fel.cvut.cz/ontologies/aviation-safety/Tail_rotor_gearbox -->

    <owl:Class rdf:about="&m;Tail_rotor_gearbox">
        <rdfs:label>Tail rotor gearbox</rdfs:label>
        <rdfs:subClassOf rdf:resource="&m;Tail_rotor_drive_system_part"/>
        <m:generated_time rdf:datatype="&xsd;dateTime">2015-04-09T18:56:27.771+02:00</m:generated_time>
        <rdfs:comment xml:lang="en">(ATA Code:6520) Tail rotor gearbox: The gearboxes which transmit engine power to the tail rotor, including intermediate gearboxes. Typical parts are case, seal, box, gear and spider gear.</rdfs:comment>
        <m:has_related_eccairs_term rdf:resource="http://onto.fel.cvut.cz/ontologies/2014/ECCAIRS_Aviation_1.3.0.12/eccairs-descriptive-factors#category_11652000"/>
    </owl:Class>
    


    <!-- http://onto.fel.cvut.cz/ontologies/aviation-safety/Tail_rotor_head -->

    <owl:Class rdf:about="&m;Tail_rotor_head">
        <rdfs:label>Tail rotor head</rdfs:label>
        <rdfs:subClassOf rdf:resource="&m;Tail_rotor_system_part"/>
        <m:generated_time rdf:datatype="&xsd;dateTime">2015-04-09T18:56:27.771+02:00</m:generated_time>
        <rdfs:comment xml:lang="en">(ATA Code:6420) Tail rotor head: The rotating assembly which supports the tail rotor blades. Does not include the controlling aspects [Code 11672000]. Typical parts are trunnion, fairing, damper plate, shaft and hub.</rdfs:comment>
        <m:has_related_eccairs_term rdf:resource="http://onto.fel.cvut.cz/ontologies/2014/ECCAIRS_Aviation_1.3.0.12/eccairs-descriptive-factors#category_11642000"/>
    </owl:Class>
    


    <!-- http://onto.fel.cvut.cz/ontologies/aviation-safety/Tail_rotor_indicating_system -->

    <owl:Class rdf:about="&m;Tail_rotor_indicating_system">
        <rdfs:label>Tail rotor indicating system</rdfs:label>
        <rdfs:subClassOf rdf:resource="&m;Tail_rotor_system_part"/>
        <m:generated_time rdf:datatype="&xsd;dateTime">2015-04-09T18:56:27.771+02:00</m:generated_time>
        <rdfs:comment xml:lang="en">(ATA Code:6440) Tail rotor indicating system: The indicators, sensors, transmitters and associated systems which indicate operation or activation of the tail rotor system.</rdfs:comment>
        <m:has_related_eccairs_term rdf:resource="http://onto.fel.cvut.cz/ontologies/2014/ECCAIRS_Aviation_1.3.0.12/eccairs-descriptive-factors#category_11644000"/>
    </owl:Class>
    


    <!-- http://onto.fel.cvut.cz/ontologies/aviation-safety/Tail_rotor_system -->

    <owl:Class rdf:about="&m;Tail_rotor_system">
        <rdfs:label>Tail rotor system</rdfs:label>
        <rdfs:subClassOf rdf:resource="&m;Aircraft_part"/>
        <m:generated_time rdf:datatype="&xsd;dateTime">2015-04-09T18:56:27.771+02:00</m:generated_time>
        <rdfs:comment xml:lang="en">(ATA Code:6400) Tail rotor system: The rotorcraft&apos;s anti-torque rotor, rotating at the tail about a more or less horizontal axis.</rdfs:comment>
        <m:has_related_eccairs_term rdf:resource="http://onto.fel.cvut.cz/ontologies/2014/ECCAIRS_Aviation_1.3.0.12/eccairs-descriptive-factors#category_11640000"/>
    </owl:Class>
    


    <!-- http://onto.fel.cvut.cz/ontologies/aviation-safety/Tail_rotor_system_part -->

    <owl:Class rdf:about="&m;Tail_rotor_system_part">
        <rdfs:label>Tail rotor system part</rdfs:label>
        <rdfs:subClassOf rdf:resource="&m;Aircraft_part"/>
        <rdfs:subClassOf>
            <owl:Restriction>
                <owl:onProperty rdf:resource="http://onto.fel.cvut.cz/ontologies/ufo/is_part_of"/>
                <owl:someValuesFrom rdf:resource="&m;Tail_rotor_system"/>
            </owl:Restriction>
        </rdfs:subClassOf>
        <m:generated_time rdf:datatype="&xsd;dateTime">2015-04-12T02:45:54.351+02:00</m:generated_time>
        <m:has_related_eccairs_term rdf:resource="http://onto.fel.cvut.cz/ontologies/2014/ECCAIRS_Aviation_1.3.0.12/eccairs-descriptive-factors#category_11640000"/>
    </owl:Class>
    


    <!-- http://onto.fel.cvut.cz/ontologies/aviation-safety/Taxiing_equipment -->

    <owl:Class rdf:about="&m;Taxiing_equipment">
        <rdfs:label>Taxiing equipment</rdfs:label>
        <rdfs:subClassOf rdf:resource="&m;Towing_and_taxiing_equipment"/>
    </owl:Class>
    


    <!-- http://onto.fel.cvut.cz/ontologies/aviation-safety/Temperature_control_system -->

    <owl:Class rdf:about="&m;Temperature_control_system">
        <rdfs:label>Temperature control system</rdfs:label>
        <rdfs:subClassOf rdf:resource="&m;Air_conditioning_system_part"/>
        <m:generated_time rdf:datatype="&xsd;dateTime">2015-04-09T18:56:27.771+02:00</m:generated_time>
        <rdfs:comment xml:lang="en">(ATA Code:2160) Temperature control system: The units and circuitry other than the control unit which are used for controlling the temperature of the air in the cockpit and cabin. Typical parts are control valves, thermal sensing devices, switches, amplifiers and wiring.</rdfs:comment>
        <m:has_related_eccairs_term rdf:resource="http://onto.fel.cvut.cz/ontologies/2014/ECCAIRS_Aviation_1.3.0.12/eccairs-descriptive-factors#category_11216000"/>
    </owl:Class>
    


    <!-- http://onto.fel.cvut.cz/ontologies/aviation-safety/Temperature_control_system_part -->

    <owl:Class rdf:about="&m;Temperature_control_system_part">
        <rdfs:label>Temperature control system part</rdfs:label>
        <rdfs:subClassOf rdf:resource="&m;Air_conditioning_system_part"/>
        <rdfs:subClassOf>
            <owl:Restriction>
                <owl:onProperty rdf:resource="http://onto.fel.cvut.cz/ontologies/ufo/is_part_of"/>
                <owl:someValuesFrom rdf:resource="&m;Temperature_control_system"/>
            </owl:Restriction>
        </rdfs:subClassOf>
        <m:generated_time rdf:datatype="&xsd;dateTime">2015-04-12T02:45:54.351+02:00</m:generated_time>
        <m:has_related_eccairs_term rdf:resource="http://onto.fel.cvut.cz/ontologies/2014/ECCAIRS_Aviation_1.3.0.12/eccairs-descriptive-factors#category_11216000"/>
    </owl:Class>
    


    <!-- http://onto.fel.cvut.cz/ontologies/aviation-safety/The_wiring_specific_to_the_Autoflight-Auto_Pilot_System -->

    <owl:Class rdf:about="&m;The_wiring_specific_to_the_Autoflight-Auto_Pilot_System">
        <rdfs:label>The wiring specific to the Autoflight/Auto Pilot System</rdfs:label>
        <rdfs:subClassOf rdf:resource="&m;autoflight_system"/>
        <m:generated_time rdf:datatype="&xsd;dateTime">2015-04-09T18:56:27.771+02:00</m:generated_time>
        <rdfs:comment xml:lang="en">(ATA Code:2297) The wiring specific to the Autoflight/Auto Pilot System</rdfs:comment>
        <m:has_related_eccairs_term rdf:resource="http://onto.fel.cvut.cz/ontologies/2014/ECCAIRS_Aviation_1.3.0.12/eccairs-descriptive-factors#category_11221700"/>
    </owl:Class>
    


    <!-- http://onto.fel.cvut.cz/ontologies/aviation-safety/Tilt_rotor_flight_control -->

    <owl:Class rdf:about="&m;Tilt_rotor_flight_control">
        <rdfs:label>Tilt rotor flight control</rdfs:label>
        <rdfs:subClassOf rdf:resource="&m;Rotorcraft_flight_control_part"/>
        <m:generated_time rdf:datatype="&xsd;dateTime">2015-04-09T18:56:27.771+02:00</m:generated_time>
        <rdfs:comment xml:lang="en">(ATA Code:6711) Tilt rotor flight control: The system components and parts of the tilt rotor control system which controls the direction of thrust of the aircraft&apos;s engines by rotating the dual main rotor assembly through up to 90-degrees. The zero or vertical position allows vertical takeoff. Horizontal take-off runs and run-on landings are achieved by selection of an intermediate angle which gives adequate blade tip clearance from the runway surface.</rdfs:comment>
        <m:has_related_eccairs_term rdf:resource="http://onto.fel.cvut.cz/ontologies/2014/ECCAIRS_Aviation_1.3.0.12/eccairs-descriptive-factors#category_11671100"/>
    </owl:Class>
    


    <!-- http://onto.fel.cvut.cz/ontologies/aviation-safety/Towing_and_taxiing_equipment -->

    <owl:Class rdf:about="&m;Towing_and_taxiing_equipment">
        <rdfs:label>Towing and taxiing equipment</rdfs:label>
        <rdfs:subClassOf rdf:resource="&m;Aircraft_part"/>
        <rdfs:subClassOf>
            <owl:Restriction>
                <owl:onProperty rdf:resource="http://onto.fel.cvut.cz/ontologies/ufo/is_part_of"/>
                <owl:someValuesFrom rdf:resource="&m;Towing_and_taxiing_equipment"/>
            </owl:Restriction>
        </rdfs:subClassOf>
        <m:generated_time rdf:datatype="&xsd;dateTime">2015-04-12T02:45:54.351+02:00</m:generated_time>
        <m:has_related_eccairs_term rdf:resource="http://onto.fel.cvut.cz/ontologies/2014/ECCAIRS_Aviation_1.3.0.12/eccairs-descriptive-factors#category_11090000"/>
    </owl:Class>
    


    <!-- http://onto.fel.cvut.cz/ontologies/aviation-safety/Towing_equipment -->

    <owl:Class rdf:about="&m;Towing_equipment">
        <rdfs:label>Towing equipment</rdfs:label>
        <rdfs:subClassOf rdf:resource="&m;Towing_and_taxiing_equipment"/>
    </owl:Class>
    


    <!-- http://onto.fel.cvut.cz/ontologies/aviation-safety/Traffic_alert_and_collision_avoidance_system-Airborne_collision_avoidance_system -->

    <owl:Class rdf:about="&m;Traffic_alert_and_collision_avoidance_system-Airborne_collision_avoidance_system">
        <rdfs:label>Traffic alert and collision avoidance system/Airborne collision avoidance system</rdfs:label>
        <rdfs:subClassOf rdf:resource="&m;Independent_position_determining_system"/>
        <rdfs:subClassOf>
            <owl:Restriction>
                <owl:onProperty rdf:resource="&m;communicates_with"/>
                <owl:someValuesFrom rdf:resource="&m;Traffic_alert_and_collision_avoidance_system-Airborne_collision_avoidance_system"/>
            </owl:Restriction>
        </rdfs:subClassOf>
        <m:generated_time rdf:datatype="&xsd;dateTime">2015-04-09T18:56:27.771+02:00</m:generated_time>
        <rdfs:comment xml:lang="en">(ATA Code:3445) Traffic alert and collision avoidance system/Airborne collision avoidance system: The system which provides information to determine relative aircraft positions and provides guidance to the flight crew on collision avoidance action. The system is independent of ground installations. Typical parts are the collision avoidance monitoring units.Airborne collision avoidance system (ACAS). An aircraft system based on secondary surveillance radar (SSR) transponder signals which operates independently of ground-based equipment to provide advice to the pilot on potential conflicting aircraft that are equipped with SSR transponders. (Annex 10, Vol 4, Chapter 1)ACAS I. An ACAS which provides information as an aid to &quot;see and avoid&quot; action but does not include the capability for generating resolution advisories (RAs). Note. ACAS I is not intended for international implementation and standardization by ICAO. Therefore, only ACAS I characteristics required to ensure compatible operation with other ACAS configurations and interference limiting are defined in 4.2.ACAS II. An ACAS which provides vertical resolution advisories (RAs) in addition to traffic advisories (TAs).ACAS III. An ACAS which provides vertical and horizontal resolution advisories (RAs) in addition to traffic advisories (TAs).</rdfs:comment>
        <m:has_related_eccairs_term rdf:resource="http://onto.fel.cvut.cz/ontologies/2014/ECCAIRS_Aviation_1.3.0.12/eccairs-descriptive-factors#category_11344500"/>
    </owl:Class>
    


    <!-- http://onto.fel.cvut.cz/ontologies/aviation-safety/Trailing_edge_flap_actuator -->

    <owl:Class rdf:about="&m;Trailing_edge_flap_actuator">
        <rdfs:label>Trailing edge flap actuator</rdfs:label>
        <rdfs:subClassOf rdf:resource="&m;Trailing_edge_flap_control_system_part"/>
        <m:generated_time rdf:datatype="&xsd;dateTime">2015-04-09T18:56:27.771+02:00</m:generated_time>
        <rdfs:comment xml:lang="en">(ATA Code:2752) Trailing edge flap actuator: The components which actuate the trailing edge flaps. Typical parts are motor, actuator, seal, jackscrew, rod end, actuator and support fittings.</rdfs:comment>
        <m:has_related_eccairs_term rdf:resource="http://onto.fel.cvut.cz/ontologies/2014/ECCAIRS_Aviation_1.3.0.12/eccairs-descriptive-factors#category_11275200"/>
    </owl:Class>
    


    <!-- http://onto.fel.cvut.cz/ontologies/aviation-safety/Trailing_edge_flap_control_system -->

    <owl:Class rdf:about="&m;Trailing_edge_flap_control_system">
        <rdfs:subClassOf rdf:resource="&m;Flight_control_system_part"/>
        <rdfs:subClassOf>
            <owl:Restriction>
                <owl:onProperty rdf:resource="http://onto.fel.cvut.cz/ontologies/ufo/has_part"/>
                <owl:someValuesFrom rdf:resource="&m;Trailing_edge_flap_control_system_part"/>
            </owl:Restriction>
        </rdfs:subClassOf>
        <rdfs:subClassOf>
            <owl:Restriction>
                <owl:onProperty rdf:resource="http://onto.fel.cvut.cz/ontologies/ufo/has_part"/>
                <owl:allValuesFrom rdf:resource="&m;Trailing_edge_flap_control_system_part"/>
            </owl:Restriction>
        </rdfs:subClassOf>
    </owl:Class>
    


    <!-- http://onto.fel.cvut.cz/ontologies/aviation-safety/Trailing_edge_flap_control_system_part -->

    <owl:Class rdf:about="&m;Trailing_edge_flap_control_system_part">
        <rdfs:label>Trailing edge flap control system part</rdfs:label>
        <rdfs:subClassOf rdf:resource="&m;Flight_control_system_part"/>
        <rdfs:subClassOf>
            <owl:Restriction>
                <owl:onProperty rdf:resource="http://onto.fel.cvut.cz/ontologies/ufo/is_part_of"/>
                <owl:someValuesFrom rdf:resource="&m;Trailing_edge_flap_control_system"/>
            </owl:Restriction>
        </rdfs:subClassOf>
        <m:generated_time rdf:datatype="&xsd;dateTime">2015-04-12T02:45:54.351+02:00</m:generated_time>
        <m:has_related_eccairs_term rdf:resource="http://onto.fel.cvut.cz/ontologies/2014/ECCAIRS_Aviation_1.3.0.12/eccairs-descriptive-factors#category_11275000"/>
    </owl:Class>
    


    <!-- http://onto.fel.cvut.cz/ontologies/aviation-safety/Trailing_edge_flap_position_indicating_system -->

    <owl:Class rdf:about="&m;Trailing_edge_flap_position_indicating_system">
        <rdfs:label>Trailing edge flap position indicating system</rdfs:label>
        <rdfs:subClassOf rdf:resource="&m;Trailing_edge_flap_control_system_part"/>
        <m:generated_time rdf:datatype="&xsd;dateTime">2015-04-09T18:56:27.771+02:00</m:generated_time>
        <rdfs:comment xml:lang="en">(ATA Code:2751) Trailing edge flap position indicating system: The system components and parts that sense, transmit and indicate trailing edge flap position relative to the wing surface. Typical parts are indicator, transmitter, position module, asymmetry switch and comparator.</rdfs:comment>
        <m:has_related_eccairs_term rdf:resource="http://onto.fel.cvut.cz/ontologies/2014/ECCAIRS_Aviation_1.3.0.12/eccairs-descriptive-factors#category_11275100"/>
    </owl:Class>
    


    <!-- http://onto.fel.cvut.cz/ontologies/aviation-safety/Trailing_edge_flap_structure -->

    <owl:Class rdf:about="&m;Trailing_edge_flap_structure">
        <rdfs:label>Trailing edge flap structure</rdfs:label>
        <rdfs:subClassOf rdf:resource="&m;Wing_flight_control_surface_part"/>
        <m:generated_time rdf:datatype="&xsd;dateTime">2015-04-09T18:56:27.771+02:00</m:generated_time>
        <rdfs:comment xml:lang="en">(ATA Code:5753) Trailing edge flap structure: The structural aspects of the fore, mid and aft segments of the flap surface mounted on the trailing edge of the wing. Does not include the operating mechanism such as the actuators, brackets, hydraulic or electric motors. Typical parts are skin, rib, spar, flap track, roller, flap carriage, bearing, bolt and rivet.</rdfs:comment>
        <m:has_related_eccairs_term rdf:resource="http://onto.fel.cvut.cz/ontologies/2014/ECCAIRS_Aviation_1.3.0.12/eccairs-descriptive-factors#category_11575300"/>
    </owl:Class>
    


    <!-- http://onto.fel.cvut.cz/ontologies/aviation-safety/Turbine_Engine_Propulsor_Section_(Rear_Mounted) -->

    <owl:Class rdf:about="&m;Turbine_Engine_Propulsor_Section_(Rear_Mounted)">
        <rdfs:label>Turbine Engine Propulsor Section (Rear Mounted)</rdfs:label>
        <rdfs:subClassOf rdf:resource="&m;ENGINE_TURBINE-TURBO_PROP_DUCTED_FAN-UNDUCTED_FAN_part"/>
        <m:generated_time rdf:datatype="&xsd;dateTime">2015-04-09T18:56:27.771+02:00</m:generated_time>
        <rdfs:comment xml:lang="en">(ATA Code:7280) The section of the engine which contains a propulsor(s) and provides the majority of the energy generated. The propulsor may be turbine-driven or gear-driven. Includes such items as propulsor turbines, propulsor blades, blade actuation, and frames (rotating and/or stationary).</rdfs:comment>
        <m:has_related_eccairs_term rdf:resource="http://onto.fel.cvut.cz/ontologies/2014/ECCAIRS_Aviation_1.3.0.12/eccairs-descriptive-factors#category_11728000"/>
    </owl:Class>
    


    <!-- http://onto.fel.cvut.cz/ontologies/aviation-safety/Turbine_Engine_System_Wiring -->

    <owl:Class rdf:about="&m;Turbine_Engine_System_Wiring">
        <rdfs:subClassOf rdf:resource="&m;ENGINE_TURBINE-TURBO_PROP_DUCTED_FAN-UNDUCTED_FAN_part"/>
    </owl:Class>
    


    <!-- http://onto.fel.cvut.cz/ontologies/aviation-safety/Turbine_assembly -->

    <owl:Class rdf:about="&m;Turbine_assembly">
        <rdfs:label>Turbine assembly</rdfs:label>
        <rdfs:subClassOf rdf:resource="&m;ENGINE_TURBINE-TURBO_PROP_DUCTED_FAN-UNDUCTED_FAN_part"/>
        <m:generated_time rdf:datatype="&xsd;dateTime">2015-04-09T18:56:27.771+02:00</m:generated_time>
        <rdfs:comment xml:lang="en">(ATA Code:7250) Turbine assembly: The turbine engine section which contains the turbine disc and associated nozzles and cases. Typical parts are case, disc, blade, nozzle, bearing, bearing cover, power turbine, shaft, tie bolts and seals.</rdfs:comment>
        <m:has_related_eccairs_term rdf:resource="http://onto.fel.cvut.cz/ontologies/2014/ECCAIRS_Aviation_1.3.0.12/eccairs-descriptive-factors#category_11725000"/>
    </owl:Class>
    


    <!-- http://onto.fel.cvut.cz/ontologies/aviation-safety/Turbine_engine_accessory_drive -->

    <owl:Class rdf:about="&m;Turbine_engine_accessory_drive">
        <rdfs:label>Turbine engine accessory drive</rdfs:label>
        <rdfs:subClassOf rdf:resource="&m;ENGINE_TURBINE-TURBO_PROP_DUCTED_FAN-UNDUCTED_FAN_part"/>
        <m:generated_time rdf:datatype="&xsd;dateTime">2015-04-09T18:56:27.771+02:00</m:generated_time>
        <rdfs:comment xml:lang="en">(ATA Code:7260) Turbine engine accessory drive: The turbine engine mounted gearbox which provides mechanical power take-offs [to drive accessories such as pumps and generators] and chip detectors. Does not include the remote gearboxes. [Code 11830000].JAR:‘Accessory drives’ means any drive shaft or utility mounting pad, furnished as a part of the auxiliary power unit, that is used for the extraction of power to drive accessories, components, or controls essential to the operation of the auxiliary power unit or any of its associated systems.</rdfs:comment>
        <m:has_related_eccairs_term rdf:resource="http://onto.fel.cvut.cz/ontologies/2014/ECCAIRS_Aviation_1.3.0.12/eccairs-descriptive-factors#category_11726000"/>
    </owl:Class>
    


    <!-- http://onto.fel.cvut.cz/ontologies/aviation-safety/Turbine_engine_accessory_drive_part -->

    <owl:Class rdf:about="&m;Turbine_engine_accessory_drive_part">
        <rdfs:label>Turbine engine accessory drive part</rdfs:label>
        <rdfs:subClassOf rdf:resource="&m;ENGINE_TURBINE-TURBO_PROP_DUCTED_FAN-UNDUCTED_FAN_part"/>
        <rdfs:subClassOf>
            <owl:Restriction>
                <owl:onProperty rdf:resource="http://onto.fel.cvut.cz/ontologies/ufo/is_part_of"/>
                <owl:someValuesFrom rdf:resource="&m;Turbine_engine_accessory_drive"/>
            </owl:Restriction>
        </rdfs:subClassOf>
        <m:generated_time rdf:datatype="&xsd;dateTime">2015-04-12T02:45:54.351+02:00</m:generated_time>
        <m:has_related_eccairs_term rdf:resource="http://onto.fel.cvut.cz/ontologies/2014/ECCAIRS_Aviation_1.3.0.12/eccairs-descriptive-factors#category_11726000"/>
    </owl:Class>
    


    <!-- http://onto.fel.cvut.cz/ontologies/aviation-safety/Turbine_engine_air_inlet -->

    <owl:Class rdf:about="&m;Turbine_engine_air_inlet">
        <rdfs:label>Turbine engine air inlet</rdfs:label>
        <rdfs:subClassOf rdf:resource="&m;ENGINE_TURBINE-TURBO_PROP_DUCTED_FAN-UNDUCTED_FAN_part"/>
        <m:generated_time rdf:datatype="&xsd;dateTime">2015-04-09T18:56:27.771+02:00</m:generated_time>
        <rdfs:comment xml:lang="en">(ATA Code:7220) Turbine engine air inlet: The engine section through which air enters the compressor section. Typical parts are inlet case, inlet cone, inlet screen, guide vane and inlet scroll.</rdfs:comment>
        <m:has_related_eccairs_term rdf:resource="http://onto.fel.cvut.cz/ontologies/2014/ECCAIRS_Aviation_1.3.0.12/eccairs-descriptive-factors#category_11722000"/>
    </owl:Class>
    


    <!-- http://onto.fel.cvut.cz/ontologies/aviation-safety/Turbine_engine_by-pass_section -->

    <owl:Class rdf:about="&m;Turbine_engine_by-pass_section">
        <rdfs:label>Turbine engine by-pass section</rdfs:label>
        <rdfs:subClassOf rdf:resource="&m;ENGINE_TURBINE-TURBO_PROP_DUCTED_FAN-UNDUCTED_FAN_part"/>
        <m:generated_time rdf:datatype="&xsd;dateTime">2015-04-09T18:56:27.771+02:00</m:generated_time>
        <rdfs:comment xml:lang="en">(ATA Code:7270) Turbine engine by-pass section: The turbine engine non-rotating portion of engine airflow ducting for the prime purpose of adding to the thrust of turbo-jet engines. Does not include the rotating components such as blades. Typical parts are duct, skin and duct segment.</rdfs:comment>
        <m:has_related_eccairs_term rdf:resource="http://onto.fel.cvut.cz/ontologies/2014/ECCAIRS_Aviation_1.3.0.12/eccairs-descriptive-factors#category_11727000"/>
    </owl:Class>
    


    <!-- http://onto.fel.cvut.cz/ontologies/aviation-safety/Turbine_engine_by-pass_section_part -->

    <owl:Class rdf:about="&m;Turbine_engine_by-pass_section_part">
        <rdfs:label>Turbine engine by-pass section part</rdfs:label>
        <rdfs:subClassOf rdf:resource="&m;ENGINE_TURBINE-TURBO_PROP_DUCTED_FAN-UNDUCTED_FAN_part"/>
        <rdfs:subClassOf>
            <owl:Restriction>
                <owl:onProperty rdf:resource="http://onto.fel.cvut.cz/ontologies/ufo/is_part_of"/>
                <owl:someValuesFrom rdf:resource="&m;Turbine_engine_by-pass_section"/>
            </owl:Restriction>
        </rdfs:subClassOf>
        <m:generated_time rdf:datatype="&xsd;dateTime">2015-04-12T02:45:54.351+02:00</m:generated_time>
        <m:has_related_eccairs_term rdf:resource="http://onto.fel.cvut.cz/ontologies/2014/ECCAIRS_Aviation_1.3.0.12/eccairs-descriptive-factors#category_11727000"/>
    </owl:Class>
    


    <!-- http://onto.fel.cvut.cz/ontologies/aviation-safety/Turbine_engine_combustion_section -->

    <owl:Class rdf:about="&m;Turbine_engine_combustion_section">
        <rdfs:label>Turbine engine combustion section</rdfs:label>
        <rdfs:subClassOf rdf:resource="&m;ENGINE_TURBINE-TURBO_PROP_DUCTED_FAN-UNDUCTED_FAN_part"/>
        <m:generated_time rdf:datatype="&xsd;dateTime">2015-04-09T18:56:27.771+02:00</m:generated_time>
        <rdfs:comment xml:lang="en">(ATA Code:7240) Turbine engine combustion section: The engine section in which fuel and air are mixed and burned. Typical parts are case, burner can, liner and vane ring.</rdfs:comment>
        <m:has_related_eccairs_term rdf:resource="http://onto.fel.cvut.cz/ontologies/2014/ECCAIRS_Aviation_1.3.0.12/eccairs-descriptive-factors#category_11724000"/>
    </owl:Class>
    


    <!-- http://onto.fel.cvut.cz/ontologies/aviation-safety/Turbine_engine_compressor -->

    <owl:Class rdf:about="&m;Turbine_engine_compressor">
        <rdfs:label>Turbine engine compressor</rdfs:label>
        <rdfs:subClassOf rdf:resource="&m;ENGINE_TURBINE-TURBO_PROP_DUCTED_FAN-UNDUCTED_FAN_part"/>
        <m:generated_time rdf:datatype="&xsd;dateTime">2015-04-09T18:56:27.771+02:00</m:generated_time>
        <rdfs:comment xml:lang="en">(ATA Code:7230) Turbine engine compressor: The section of the engine in which the incoming air is compressed. Does not include the operation of variable stator blades or linkage to the various valves and sense lines. [Code 11753000] Includes items such as case, the rotating portion of the compressor, lines, fan blades, disc, bearings, seals, mounts, carbon seals, disc tie bolts and shaft.</rdfs:comment>
        <m:has_related_eccairs_term rdf:resource="http://onto.fel.cvut.cz/ontologies/2014/ECCAIRS_Aviation_1.3.0.12/eccairs-descriptive-factors#category_11723000"/>
    </owl:Class>
    


    <!-- http://onto.fel.cvut.cz/ontologies/aviation-safety/Turbine_engine_oil_system -->

    <owl:Class rdf:about="&m;Turbine_engine_oil_system">
        <rdfs:label>Turbine engine oil system</rdfs:label>
        <rdfs:subClassOf rdf:resource="&m;Turbine_engine_accessory_drive_part"/>
        <m:generated_time rdf:datatype="&xsd;dateTime">2015-04-09T18:56:27.771+02:00</m:generated_time>
        <rdfs:comment xml:lang="en">(ATA Code:7261) Turbine engine oil system: The turbine engine system components and parts which provide lubricating oil pressure, circulation and scavenging throughout the engine. Does not include externally mounted storage tanks [Code 11791000], connecting lines [Code 11792000] or coolers [Code 11792100]. Typical parts are relief valve, fitting, seal, pump, screen, filter, seal, check valve and elements.</rdfs:comment>
        <m:has_related_eccairs_term rdf:resource="http://onto.fel.cvut.cz/ontologies/2014/ECCAIRS_Aviation_1.3.0.12/eccairs-descriptive-factors#category_11726100"/>
    </owl:Class>
    


    <!-- http://onto.fel.cvut.cz/ontologies/aviation-safety/Turbine_engine_reduction_gear,_shaft_Section_Section_(TurboProp_and-or_Front_Mounted_Gear_Driven_Propulsor) -->

    <owl:Class rdf:about="&m;Turbine_engine_reduction_gear,_shaft_Section_Section_(TurboProp_and-or_Front_Mounted_Gear_Driven_Propulsor)">
        <rdfs:label>Turbine engine reduction gear, shaft Section Section (TurboProp and/or Front Mounted Gear Driven Propulsor)</rdfs:label>
        <rdfs:subClassOf rdf:resource="&m;ENGINE_TURBINE-TURBO_PROP_DUCTED_FAN-UNDUCTED_FAN_part"/>
        <m:generated_time rdf:datatype="&xsd;dateTime">2015-04-09T18:56:27.771+02:00</m:generated_time>
        <rdfs:comment xml:lang="en">(ATA Code:7210) The section of the engine which contains the propeller shafts and reduction gears. Includes items such as drives for hose mounted accessories, etc. If applicable, the section of the engine which uses mechanical force, through a gear-driven system, to drive front mounted propulsors which provide the majority of the energy generated. Includes items such as Propulsor Blades, Actuation Systems, Reduction Gears, Drive-Shafts, etc.</rdfs:comment>
        <m:has_related_eccairs_term rdf:resource="http://onto.fel.cvut.cz/ontologies/2014/ECCAIRS_Aviation_1.3.0.12/eccairs-descriptive-factors#category_11721000"/>
    </owl:Class>
    


    <!-- http://onto.fel.cvut.cz/ontologies/aviation-safety/Turbine_governor -->

    <owl:Class rdf:about="&m;Turbine_governor">
        <rdfs:label>Turbine governor</rdfs:label>
        <rdfs:subClassOf rdf:resource="&m;Fuel_control_system_part"/>
        <m:generated_time rdf:datatype="&xsd;dateTime">2015-04-09T18:56:27.771+02:00</m:generated_time>
        <rdfs:comment xml:lang="en">(ATA Code:7323) Turbine governor: The component which controls the rpm of turbine engines. Typical parts are governor, shaft, overspeed limiter and topping governor.</rdfs:comment>
        <m:has_related_eccairs_term rdf:resource="http://onto.fel.cvut.cz/ontologies/2014/ECCAIRS_Aviation_1.3.0.12/eccairs-descriptive-factors#category_11732300"/>
    </owl:Class>
    


    <!-- http://onto.fel.cvut.cz/ontologies/aviation-safety/Turbocharger_System_Wiring -->

    <owl:Class rdf:about="&m;Turbocharger_System_Wiring">
        <rdfs:subClassOf rdf:resource="&m;Exhaust_turbine_system_(reciprocating)_part"/>
    </owl:Class>
    


    <!-- http://onto.fel.cvut.cz/ontologies/aviation-safety/Turn_and_bank-rate_of_turn_indicator -->

    <owl:Class rdf:about="&m;Turn_and_bank-rate_of_turn_indicator">
        <rdfs:label>Turn and bank/rate of turn indicator</rdfs:label>
        <rdfs:subClassOf rdf:resource="&m;Attitude_and_direction_data_system_part"/>
        <m:generated_time rdf:datatype="&xsd;dateTime">2015-04-09T18:56:27.771+02:00</m:generated_time>
        <rdfs:comment xml:lang="en">(ATA Code:3424) Turn and bank/rate of turn indicator: The instrument actuated by gyroscopic forces and driven by air flow or electric motor to indicate both rate of turn and angle of bank.</rdfs:comment>
        <m:has_related_eccairs_term rdf:resource="http://onto.fel.cvut.cz/ontologies/2014/ECCAIRS_Aviation_1.3.0.12/eccairs-descriptive-factors#category_11342400"/>
    </owl:Class>
    


    <!-- http://onto.fel.cvut.cz/ontologies/aviation-safety/UHF_radio_telephony -->

    <owl:Class rdf:about="&m;UHF_radio_telephony">
        <rdfs:label xml:lang="en">Ultra high frequency radio telephony</rdfs:label>
        <rdfs:subClassOf>
            <owl:Class>
                <owl:intersectionOf rdf:parseType="Collection">
                    <rdf:Description rdf:about="&m;Radio_communication_equipment"/>
                    <owl:Restriction>
                        <owl:onProperty rdf:resource="&m;relates_to"/>
                        <owl:someValuesFrom rdf:resource="&m;Ultra_high_frequency_communication_system"/>
                    </owl:Restriction>
                </owl:intersectionOf>
            </owl:Class>
        </rdfs:subClassOf>
        <m:generated_time rdf:datatype="&xsd;dateTime">2015-04-17T16:49:10.062+02:00</m:generated_time>
        <m:has_abbreviation xml:lang="en">UHF</m:has_abbreviation>
        <m:has_related_eccairs_term rdf:resource="http://onto.fel.cvut.cz/ontologies/2014/ECCAIRS_Aviation_1.3.0.12/eccairs-descriptive-factors#category_21010200"/>
    </owl:Class>
    


    <!-- http://onto.fel.cvut.cz/ontologies/aviation-safety/Ultra_high_frequency_communication_system -->

    <owl:Class rdf:about="&m;Ultra_high_frequency_communication_system">
        <rdfs:label>Ultra high frequency communication system</rdfs:label>
        <rdfs:subClassOf rdf:resource="&m;speech_communication_system"/>
        <m:generated_time rdf:datatype="&xsd;dateTime">2015-04-09T18:56:27.771+02:00</m:generated_time>
        <rdfs:comment xml:lang="en">(ATA Code:2311) UHF communication system: The system parts and circuitry including the receiver, transmitter and antenna used exclusively for ultra high frequency communications.</rdfs:comment>
        <m:has_related_eccairs_term rdf:resource="http://onto.fel.cvut.cz/ontologies/2014/ECCAIRS_Aviation_1.3.0.12/eccairs-descriptive-factors#category_11231100"/>
    </owl:Class>
    


    <!-- http://onto.fel.cvut.cz/ontologies/aviation-safety/VHF_radio_telephony -->

    <owl:Class rdf:about="&m;VHF_radio_telephony">
        <rdfs:label xml:lang="en">Very high frequency radio telephony</rdfs:label>
        <rdfs:subClassOf>
            <owl:Class>
                <owl:intersectionOf rdf:parseType="Collection">
                    <rdf:Description rdf:about="&m;Radio_communication_equipment"/>
                    <owl:Restriction>
                        <owl:onProperty rdf:resource="&m;relates_to"/>
                        <owl:someValuesFrom rdf:resource="&m;Very_high_frequency_communication_system"/>
                    </owl:Restriction>
                </owl:intersectionOf>
            </owl:Class>
        </rdfs:subClassOf>
        <m:generated_time rdf:datatype="&xsd;dateTime">2015-04-17T16:49:10.062+02:00</m:generated_time>
        <m:has_abbreviation xml:lang="en">VHF</m:has_abbreviation>
        <m:has_related_eccairs_term rdf:resource="http://onto.fel.cvut.cz/ontologies/2014/ECCAIRS_Aviation_1.3.0.12/eccairs-descriptive-factors#category_21010100"/>
    </owl:Class>
    


    <!-- http://onto.fel.cvut.cz/ontologies/aviation-safety/VOR_signal -->

    <owl:Class rdf:about="&m;VOR_signal">
        <rdfs:subClassOf>
            <owl:Class>
                <owl:intersectionOf rdf:parseType="Collection">
                    <owl:Restriction>
                        <owl:onProperty rdf:resource="&m;is_produced_by"/>
                        <owl:someValuesFrom rdf:resource="&m;very_high_frequency_omni-directional_radio_range_ground_system"/>
                    </owl:Restriction>
                    <owl:Restriction>
                        <owl:onProperty rdf:resource="&m;is_received_by"/>
                        <owl:someValuesFrom rdf:resource="&m;Very_high_frequency_omni-directional_radio_range_aircraft_system"/>
                    </owl:Restriction>
                </owl:intersectionOf>
            </owl:Class>
        </rdfs:subClassOf>
    </owl:Class>
    


    <!-- http://onto.fel.cvut.cz/ontologies/aviation-safety/Vacuum_System_Wiring -->

    <owl:Class rdf:about="&m;Vacuum_System_Wiring">
        <rdfs:label>Vacuum System Wiring</rdfs:label>
        <rdfs:subClassOf rdf:resource="&m;Vacuum_system_part"/>
        <rdfs:subClassOf rdf:resource="&m;Wiring"/>
        <rdfs:subClassOf>
            <owl:Restriction>
                <owl:onProperty rdf:resource="http://onto.fel.cvut.cz/ontologies/ufo/is_part_of"/>
                <owl:someValuesFrom rdf:resource="&m;Vacuum_system"/>
            </owl:Restriction>
        </rdfs:subClassOf>
        <m:generated_time rdf:datatype="&xsd;dateTime">2015-04-09T18:56:27.771+02:00</m:generated_time>
        <rdfs:comment xml:lang="en">(ATA Code:3797) Wiring specific to the Vacuum System.</rdfs:comment>
        <m:has_related_eccairs_term rdf:resource="http://onto.fel.cvut.cz/ontologies/2014/ECCAIRS_Aviation_1.3.0.12/eccairs-descriptive-factors#category_11379700"/>
    </owl:Class>
    


    <!-- http://onto.fel.cvut.cz/ontologies/aviation-safety/Vacuum_distribution_system -->

    <owl:Class rdf:about="&m;Vacuum_distribution_system">
        <rdfs:label>Vacuum distribution system</rdfs:label>
        <rdfs:subClassOf rdf:resource="&m;Vacuum_system_part"/>
        <m:generated_time rdf:datatype="&xsd;dateTime">2015-04-09T18:56:27.771+02:00</m:generated_time>
        <rdfs:comment xml:lang="en">(ATA Code:3710) Vacuum distribution system: The system components and parts, other than the pump, regulator, oil separator or indication system, which are used to distribute low volume, negative pressure air (suction) to systems such as gyroscopic flight instruments and cabin rate controller and to distribute low volume, positive pressure air to systems such as air foil de-icer boots. Does not include the using systems. Typical parts are pump, filter, regulator, lines, manifold, check valves and element.</rdfs:comment>
        <m:has_related_eccairs_term rdf:resource="http://onto.fel.cvut.cz/ontologies/2014/ECCAIRS_Aviation_1.3.0.12/eccairs-descriptive-factors#category_11371000"/>
    </owl:Class>
    


    <!-- http://onto.fel.cvut.cz/ontologies/aviation-safety/Vacuum_indicating_system -->

    <owl:Class rdf:about="&m;Vacuum_indicating_system">
        <rdfs:label>Vacuum indicating system</rdfs:label>
        <rdfs:subClassOf rdf:resource="&m;Vacuum_system_part"/>
        <m:generated_time rdf:datatype="&xsd;dateTime">2015-04-09T18:56:27.771+02:00</m:generated_time>
        <rdfs:comment xml:lang="en">(ATA Code:3720) Vacuum indicating system: The system components and parts including those which indicate negative air pressure in the vacuum lines. Includes the indicator and warning systems. Typical parts are the vacuum indicator and associated lines.</rdfs:comment>
        <m:has_related_eccairs_term rdf:resource="http://onto.fel.cvut.cz/ontologies/2014/ECCAIRS_Aviation_1.3.0.12/eccairs-descriptive-factors#category_11372000"/>
    </owl:Class>
    


    <!-- http://onto.fel.cvut.cz/ontologies/aviation-safety/Vacuum_system -->

    <owl:Class rdf:about="&m;Vacuum_system">
        <rdfs:label>Vacuum system</rdfs:label>
        <rdfs:subClassOf rdf:resource="&m;Aircraft_part"/>
        <m:generated_time rdf:datatype="&xsd;dateTime">2015-04-09T18:56:27.771+02:00</m:generated_time>
        <rdfs:comment xml:lang="en">(ATA Code:3700) Vacuum system: The units and components used to generate, deliver and regulate negative air pressure.</rdfs:comment>
        <m:has_related_eccairs_term rdf:resource="http://onto.fel.cvut.cz/ontologies/2014/ECCAIRS_Aviation_1.3.0.12/eccairs-descriptive-factors#category_11370000"/>
    </owl:Class>
    


    <!-- http://onto.fel.cvut.cz/ontologies/aviation-safety/Vacuum_system_part -->

    <owl:Class rdf:about="&m;Vacuum_system_part">
        <rdfs:label>Vacuum system part</rdfs:label>
        <rdfs:subClassOf rdf:resource="&m;Aircraft_part"/>
        <rdfs:subClassOf>
            <owl:Restriction>
                <owl:onProperty rdf:resource="http://onto.fel.cvut.cz/ontologies/ufo/is_part_of"/>
                <owl:someValuesFrom rdf:resource="&m;Vacuum_system"/>
            </owl:Restriction>
        </rdfs:subClassOf>
        <m:generated_time rdf:datatype="&xsd;dateTime">2015-04-12T02:45:54.351+02:00</m:generated_time>
        <m:has_related_eccairs_term rdf:resource="http://onto.fel.cvut.cz/ontologies/2014/ECCAIRS_Aviation_1.3.0.12/eccairs-descriptive-factors#category_11370000"/>
    </owl:Class>
    


    <!-- http://onto.fel.cvut.cz/ontologies/aviation-safety/Ventral_structure -->

    <owl:Class rdf:about="&m;Ventral_structure">
        <rdfs:label>Ventral structure</rdfs:label>
        <rdfs:subClassOf rdf:resource="&m;Vertical_stabilizer_part"/>
        <m:generated_time rdf:datatype="&xsd;dateTime">2015-04-09T18:56:27.771+02:00</m:generated_time>
        <rdfs:comment xml:lang="en">(ATA Code:5533) The ventral structure and skin of the ventral fin mounted on the lower, aft fuselage for added directional stability. Typical parts are skin, rib and rivets.</rdfs:comment>
        <m:has_related_eccairs_term rdf:resource="http://onto.fel.cvut.cz/ontologies/2014/ECCAIRS_Aviation_1.3.0.12/eccairs-descriptive-factors#category_11553300"/>
    </owl:Class>
    


    <!-- http://onto.fel.cvut.cz/ontologies/aviation-safety/Vertical_stabilizer -->

    <owl:Class rdf:about="&m;Vertical_stabilizer">
        <rdfs:label>Vertical stabilizer</rdfs:label>
        <rdfs:subClassOf rdf:resource="&m;Empennage_structure_part"/>
        <m:generated_time rdf:datatype="&xsd;dateTime">2015-04-09T18:56:27.771+02:00</m:generated_time>
        <rdfs:comment xml:lang="en">(ATA Code:5530) Vertical stabilizer: The structural aspects of the fixed vertical surface attached to the fuselage including the dorsal fin.</rdfs:comment>
        <m:has_related_eccairs_term rdf:resource="http://onto.fel.cvut.cz/ontologies/2014/ECCAIRS_Aviation_1.3.0.12/eccairs-descriptive-factors#category_11553000"/>
    </owl:Class>
    


    <!-- http://onto.fel.cvut.cz/ontologies/aviation-safety/Vertical_stabilizer_attachment_fitting -->

    <owl:Class rdf:about="&m;Vertical_stabilizer_attachment_fitting">
        <rdfs:label>Vertical stabilizer attachment fitting</rdfs:label>
        <rdfs:subClassOf rdf:resource="&m;Attachment_fitting_(empennage_flight_control_surfaces)_part"/>
        <m:generated_time rdf:datatype="&xsd;dateTime">2015-04-09T18:56:27.771+02:00</m:generated_time>
        <rdfs:comment xml:lang="en">(ATA Code:5553) Vertical stabilizer attachment fitting: The fittings on the vertical stabilizer which are used to support equipment within the structure.</rdfs:comment>
        <m:has_related_eccairs_term rdf:resource="http://onto.fel.cvut.cz/ontologies/2014/ECCAIRS_Aviation_1.3.0.12/eccairs-descriptive-factors#category_11555300"/>
    </owl:Class>
    


    <!-- http://onto.fel.cvut.cz/ontologies/aviation-safety/Vertical_stabilizer_part -->

    <owl:Class rdf:about="&m;Vertical_stabilizer_part">
        <rdfs:label>Vertical stabilizer part</rdfs:label>
        <rdfs:subClassOf rdf:resource="&m;Empennage_structure_part"/>
        <rdfs:subClassOf>
            <owl:Restriction>
                <owl:onProperty rdf:resource="http://onto.fel.cvut.cz/ontologies/ufo/is_part_of"/>
                <owl:someValuesFrom rdf:resource="&m;Vertical_stabilizer"/>
            </owl:Restriction>
        </rdfs:subClassOf>
        <m:generated_time rdf:datatype="&xsd;dateTime">2015-04-12T02:45:54.351+02:00</m:generated_time>
        <m:has_related_eccairs_term rdf:resource="http://onto.fel.cvut.cz/ontologies/2014/ECCAIRS_Aviation_1.3.0.12/eccairs-descriptive-factors#category_11553000"/>
    </owl:Class>
    


    <!-- http://onto.fel.cvut.cz/ontologies/aviation-safety/Very_high_frequency_communication_system -->

    <owl:Class rdf:about="&m;Very_high_frequency_communication_system">
        <rdfs:label>Very high frequency communication system</rdfs:label>
        <rdfs:subClassOf rdf:resource="&m;speech_communication_system"/>
        <m:generated_time rdf:datatype="&xsd;dateTime">2015-04-09T18:56:27.771+02:00</m:generated_time>
        <rdfs:comment xml:lang="en">(ATA Code:2312) VHF communication system: The system parts and circuitry including the receiver, transmitter and antenna used exclusively for very high frequency communications.</rdfs:comment>
        <m:has_related_eccairs_term rdf:resource="http://onto.fel.cvut.cz/ontologies/2014/ECCAIRS_Aviation_1.3.0.12/eccairs-descriptive-factors#category_11231200"/>
    </owl:Class>
    


    <!-- http://onto.fel.cvut.cz/ontologies/aviation-safety/Very_high_frequency_omni-directional_radio_range_aircraft_system -->

    <owl:Class rdf:about="&m;Very_high_frequency_omni-directional_radio_range_aircraft_system">
        <rdfs:label>Very high frequency omni-directional radio range aircraft system</rdfs:label>
        <rdfs:subClassOf rdf:resource="&m;Dependent_position_determining_system"/>
        <m:generated_time rdf:datatype="&xsd;dateTime">2015-04-09T18:56:27.771+02:00</m:generated_time>
        <rdfs:comment xml:lang="en">(ATA Code:3454) Very high frequency omni-directional radio range system: The radio navigation system in the very high frequency band used for determining a bearing relative to a ground transmitter and permits selection of one of 360 magnetic courses for navigation to a transmitter. Typical parts are receiver, antenna and control panel.</rdfs:comment>
        <m:has_abbreviation>VOR aircraft system</m:has_abbreviation>
        <m:has_related_eccairs_term rdf:resource="http://onto.fel.cvut.cz/ontologies/2014/ECCAIRS_Aviation_1.3.0.12/eccairs-descriptive-factors#category_11345400"/>
    </owl:Class>
    


    <!-- http://onto.fel.cvut.cz/ontologies/aviation-safety/Wash_water_system -->

    <owl:Class rdf:about="&m;Wash_water_system">
        <rdfs:label>Wash water system</rdfs:label>
        <rdfs:subClassOf rdf:resource="&m;Water_and_waste_system_part"/>
        <m:generated_time rdf:datatype="&xsd;dateTime">2015-04-09T18:56:27.771+02:00</m:generated_time>
        <rdfs:comment xml:lang="en">(ATA Code:3820) Wash water system: The system which is used to store and deliver wash water.</rdfs:comment>
        <m:has_related_eccairs_term rdf:resource="http://onto.fel.cvut.cz/ontologies/2014/ECCAIRS_Aviation_1.3.0.12/eccairs-descriptive-factors#category_11382000"/>
    </owl:Class>
    


    <!-- http://onto.fel.cvut.cz/ontologies/aviation-safety/Waste_disposal_system -->

    <owl:Class rdf:about="&m;Waste_disposal_system">
        <rdfs:label>Waste disposal system</rdfs:label>
        <rdfs:subClassOf rdf:resource="&m;Water_and_waste_system_part"/>
        <m:generated_time rdf:datatype="&xsd;dateTime">2015-04-09T18:56:27.771+02:00</m:generated_time>
        <rdfs:comment xml:lang="en">(ATA Code:3830) Waste disposal system: The system and components used for the disposal of water and waste. Includes wash basins, water closets, flush systems and collection tanks. Typical parts are valve, flush motor, lines and timer.</rdfs:comment>
        <m:has_related_eccairs_term rdf:resource="http://onto.fel.cvut.cz/ontologies/2014/ECCAIRS_Aviation_1.3.0.12/eccairs-descriptive-factors#category_11383000"/>
    </owl:Class>
    


    <!-- http://onto.fel.cvut.cz/ontologies/aviation-safety/Water-Waste_System_Wiring -->

    <owl:Class rdf:about="&m;Water-Waste_System_Wiring">
        <rdfs:label>Water/Waste System Wiring</rdfs:label>
        <rdfs:subClassOf rdf:resource="&m;Water_and_waste_system_part"/>
        <m:generated_time rdf:datatype="&xsd;dateTime">2015-04-09T18:56:27.771+02:00</m:generated_time>
        <rdfs:comment xml:lang="en">(ATA Code:3897) Wiring specific to the Water/Waste System.</rdfs:comment>
        <m:has_related_eccairs_term rdf:resource="http://onto.fel.cvut.cz/ontologies/2014/ECCAIRS_Aviation_1.3.0.12/eccairs-descriptive-factors#category_11389700"/>
    </owl:Class>
    


    <!-- http://onto.fel.cvut.cz/ontologies/aviation-safety/Water_Injection_-_Distribution -->

    <owl:Class rdf:about="&m;Water_Injection_-_Distribution">
        <rdfs:label>Water Injection - Distribution</rdfs:label>
        <rdfs:subClassOf rdf:resource="&m;Water_injection_system_part"/>
        <m:generated_time rdf:datatype="&xsd;dateTime">2015-04-09T18:56:27.771+02:00</m:generated_time>
        <rdfs:comment xml:lang="en">(ATA Code:8220) That portion of the system which is used to conduct water or water mixtures from the tanks or cells to the engine.  Includes items such as plumbing, crossfeed system, pumps, valves, controls, etc.</rdfs:comment>
        <m:has_related_eccairs_term rdf:resource="http://onto.fel.cvut.cz/ontologies/2014/ECCAIRS_Aviation_1.3.0.12/eccairs-descriptive-factors#category_11822000"/>
    </owl:Class>
    


    <!-- http://onto.fel.cvut.cz/ontologies/aviation-safety/Water_Injection_-_Dumping_and_Purging -->

    <owl:Class rdf:about="&m;Water_Injection_-_Dumping_and_Purging">
        <rdfs:label>Water Injection - Dumping and Purging</rdfs:label>
        <rdfs:subClassOf rdf:resource="&m;Water_injection_system_part"/>
        <m:generated_time rdf:datatype="&xsd;dateTime">2015-04-09T18:56:27.771+02:00</m:generated_time>
        <rdfs:comment xml:lang="en">(ATA Code:8230) That portion of the system which is used to dump injection water and to purge the system.  Includes items such as plumbing, valves, controls, etc.</rdfs:comment>
        <m:has_related_eccairs_term rdf:resource="http://onto.fel.cvut.cz/ontologies/2014/ECCAIRS_Aviation_1.3.0.12/eccairs-descriptive-factors#category_11823000"/>
    </owl:Class>
    


    <!-- http://onto.fel.cvut.cz/ontologies/aviation-safety/Water_Injection_-_Indicating -->

    <owl:Class rdf:about="&m;Water_Injection_-_Indicating">
        <rdfs:label>Water Injection - Indicating</rdfs:label>
        <rdfs:subClassOf rdf:resource="&m;Water_injection_system_part"/>
        <m:generated_time rdf:datatype="&xsd;dateTime">2015-04-09T18:56:27.771+02:00</m:generated_time>
        <rdfs:comment xml:lang="en">(ATA Code:8240) That portion of the system which is used to indicate the quantity, temperature and pressure of the water mixtures.  Includes items such as transmitters, indicators, wiring, etc.</rdfs:comment>
        <m:has_related_eccairs_term rdf:resource="http://onto.fel.cvut.cz/ontologies/2014/ECCAIRS_Aviation_1.3.0.12/eccairs-descriptive-factors#category_11824000"/>
    </owl:Class>
    


    <!-- http://onto.fel.cvut.cz/ontologies/aviation-safety/Water_Injection_System_Wiring -->

    <owl:Class rdf:about="&m;Water_Injection_System_Wiring">
        <rdfs:label>Water Injection System Wiring</rdfs:label>
        <rdfs:subClassOf rdf:resource="&m;Water_injection_system_part"/>
        <m:generated_time rdf:datatype="&xsd;dateTime">2015-04-09T18:56:27.771+02:00</m:generated_time>
        <rdfs:comment xml:lang="en">(ATA Code:8297) Wiring specific to the Water Injection System</rdfs:comment>
        <m:has_related_eccairs_term rdf:resource="http://onto.fel.cvut.cz/ontologies/2014/ECCAIRS_Aviation_1.3.0.12/eccairs-descriptive-factors#category_11829700"/>
    </owl:Class>
    


    <!-- http://onto.fel.cvut.cz/ontologies/aviation-safety/Water_and_waste_system -->

    <owl:Class rdf:about="&m;Water_and_waste_system">
        <rdfs:label>Water and waste system</rdfs:label>
        <rdfs:subClassOf rdf:resource="&m;Aircraft_part"/>
        <m:generated_time rdf:datatype="&xsd;dateTime">2015-04-09T18:56:27.771+02:00</m:generated_time>
        <rdfs:comment xml:lang="en">(ATA Code:3800) Water and waste system: The fixed units and components which store and deliver for use, fresh water and those fixed components which store and deliver waste water.</rdfs:comment>
        <m:has_related_eccairs_term rdf:resource="http://onto.fel.cvut.cz/ontologies/2014/ECCAIRS_Aviation_1.3.0.12/eccairs-descriptive-factors#category_11380000"/>
    </owl:Class>
    


    <!-- http://onto.fel.cvut.cz/ontologies/aviation-safety/Water_and_waste_system_part -->

    <owl:Class rdf:about="&m;Water_and_waste_system_part">
        <rdfs:label>Water and waste system part</rdfs:label>
        <rdfs:subClassOf rdf:resource="&m;Aircraft_part"/>
        <rdfs:subClassOf>
            <owl:Restriction>
                <owl:onProperty rdf:resource="http://onto.fel.cvut.cz/ontologies/ufo/is_part_of"/>
                <owl:someValuesFrom rdf:resource="&m;Water_and_waste_system"/>
            </owl:Restriction>
        </rdfs:subClassOf>
        <m:generated_time rdf:datatype="&xsd;dateTime">2015-04-12T02:45:54.351+02:00</m:generated_time>
        <m:has_related_eccairs_term rdf:resource="http://onto.fel.cvut.cz/ontologies/2014/ECCAIRS_Aviation_1.3.0.12/eccairs-descriptive-factors#category_11380000"/>
    </owl:Class>
    


    <!-- http://onto.fel.cvut.cz/ontologies/aviation-safety/Water_ballast -->

    <owl:Class rdf:about="&m;Water_ballast">
        <rdfs:label>Water ballast</rdfs:label>
        <rdfs:subClassOf rdf:resource="&m;Aircraft_part"/>
        <m:generated_time rdf:datatype="&xsd;dateTime">2015-04-09T18:56:27.771+02:00</m:generated_time>
        <rdfs:comment xml:lang="en">(ATA Code:4100) Water ballast: The units and components provided for the storage, balancing, control, filling, discharge and dumping of water ballast.</rdfs:comment>
        <m:has_related_eccairs_term rdf:resource="http://onto.fel.cvut.cz/ontologies/2014/ECCAIRS_Aviation_1.3.0.12/eccairs-descriptive-factors#category_11410000"/>
    </owl:Class>
    


    <!-- http://onto.fel.cvut.cz/ontologies/aviation-safety/Water_ballast_dump_system -->

    <owl:Class rdf:about="&m;Water_ballast_dump_system">
        <rdfs:label>Water ballast dump system</rdfs:label>
        <rdfs:subClassOf rdf:resource="&m;Water_ballast_part"/>
        <m:generated_time rdf:datatype="&xsd;dateTime">2015-04-09T18:56:27.771+02:00</m:generated_time>
        <rdfs:comment xml:lang="en">(ATA Code:4120) That portion of the system used to dump water ballast during flight.   Includes valves, remote/direct, manual/automatic controls, etc.</rdfs:comment>
        <m:has_related_eccairs_term rdf:resource="http://onto.fel.cvut.cz/ontologies/2014/ECCAIRS_Aviation_1.3.0.12/eccairs-descriptive-factors#category_11412000"/>
    </owl:Class>
    


    <!-- http://onto.fel.cvut.cz/ontologies/aviation-safety/Water_ballast_indicating_system -->

    <owl:Class rdf:about="&m;Water_ballast_indicating_system">
        <rdfs:label>Water ballast indicating system</rdfs:label>
        <rdfs:subClassOf rdf:resource="&m;Water_ballast_part"/>
        <m:generated_time rdf:datatype="&xsd;dateTime">2015-04-09T18:56:27.771+02:00</m:generated_time>
        <rdfs:comment xml:lang="en">(ATA Code:4130) That portion of the system used to indicate quantity, condition and relative distribution of the water ballast.</rdfs:comment>
        <m:has_related_eccairs_term rdf:resource="http://onto.fel.cvut.cz/ontologies/2014/ECCAIRS_Aviation_1.3.0.12/eccairs-descriptive-factors#category_11413000"/>
    </owl:Class>
    


    <!-- http://onto.fel.cvut.cz/ontologies/aviation-safety/Water_ballast_part -->

    <owl:Class rdf:about="&m;Water_ballast_part">
        <rdfs:label>Water ballast part</rdfs:label>
        <rdfs:subClassOf rdf:resource="&m;Water_injection_system_part"/>
        <rdfs:subClassOf>
            <owl:Restriction>
                <owl:onProperty rdf:resource="http://onto.fel.cvut.cz/ontologies/ufo/is_part_of"/>
                <owl:someValuesFrom rdf:resource="&m;Water_ballast"/>
            </owl:Restriction>
        </rdfs:subClassOf>
        <m:generated_time rdf:datatype="&xsd;dateTime">2015-04-12T02:45:54.351+02:00</m:generated_time>
        <m:has_related_eccairs_term rdf:resource="http://onto.fel.cvut.cz/ontologies/2014/ECCAIRS_Aviation_1.3.0.12/eccairs-descriptive-factors#category_11410000"/>
    </owl:Class>
    


    <!-- http://onto.fel.cvut.cz/ontologies/aviation-safety/Water_ballast_storage -->

    <owl:Class rdf:about="&m;Water_ballast_storage">
        <rdfs:label>Water ballast storage</rdfs:label>
        <rdfs:subClassOf rdf:resource="&m;Water_ballast_part"/>
        <m:generated_time rdf:datatype="&xsd;dateTime">2015-04-09T18:56:27.771+02:00</m:generated_time>
        <rdfs:comment xml:lang="en">(ATA Code:4110) That portion of the system which stores water solely for the purpose of providing airship ballast.   Includes removable tanks (bladder cells), interconnecting balance pipes, filler valves, etc.</rdfs:comment>
        <m:has_related_eccairs_term rdf:resource="http://onto.fel.cvut.cz/ontologies/2014/ECCAIRS_Aviation_1.3.0.12/eccairs-descriptive-factors#category_11411000"/>
    </owl:Class>
    


    <!-- http://onto.fel.cvut.cz/ontologies/aviation-safety/Water_ballast_wiring -->

    <owl:Class rdf:about="&m;Water_ballast_wiring">
        <rdfs:label>Water ballast wiring</rdfs:label>
        <rdfs:subClassOf rdf:resource="&m;Water_ballast_part"/>
        <m:generated_time rdf:datatype="&xsd;dateTime">2015-04-09T18:56:27.771+02:00</m:generated_time>
        <rdfs:comment xml:lang="en">(ATA Code:4197) Wiring of the water ballast system.</rdfs:comment>
        <m:has_related_eccairs_term rdf:resource="http://onto.fel.cvut.cz/ontologies/2014/ECCAIRS_Aviation_1.3.0.12/eccairs-descriptive-factors#category_11419700"/>
    </owl:Class>
    


    <!-- http://onto.fel.cvut.cz/ontologies/aviation-safety/Water_injection_-_Storage -->

    <owl:Class rdf:about="&m;Water_injection_-_Storage">
        <rdfs:label>Water injection - Storage</rdfs:label>
        <rdfs:subClassOf rdf:resource="&m;Water_injection_system_part"/>
        <m:generated_time rdf:datatype="&xsd;dateTime">2015-04-09T18:56:27.771+02:00</m:generated_time>
        <rdfs:comment xml:lang="en">(ATA Code:8210) That portion of the system which is used for the storage of water or water mixtures.  Includes tank sealing, attachment of bladder type cells, ventilating system, cell and tank interconnectors, filling systems, etc.</rdfs:comment>
        <m:has_related_eccairs_term rdf:resource="http://onto.fel.cvut.cz/ontologies/2014/ECCAIRS_Aviation_1.3.0.12/eccairs-descriptive-factors#category_11821000"/>
    </owl:Class>
    


    <!-- http://onto.fel.cvut.cz/ontologies/aviation-safety/Water_injection_-_Storage_part -->

    <owl:Class rdf:about="&m;Water_injection_-_Storage_part">
        <rdfs:label>Water injection - Storage part</rdfs:label>
        <rdfs:subClassOf rdf:resource="&m;Aircraft_part"/>
        <rdfs:subClassOf>
            <owl:Restriction>
                <owl:onProperty rdf:resource="http://onto.fel.cvut.cz/ontologies/ufo/is_part_of"/>
                <owl:someValuesFrom rdf:resource="&m;Water_injection_-_Storage"/>
            </owl:Restriction>
        </rdfs:subClassOf>
        <m:generated_time rdf:datatype="&xsd;dateTime">2015-04-12T02:45:54.351+02:00</m:generated_time>
        <m:has_related_eccairs_term rdf:resource="http://onto.fel.cvut.cz/ontologies/2014/ECCAIRS_Aviation_1.3.0.12/eccairs-descriptive-factors#category_11821000"/>
    </owl:Class>
    


    <!-- http://onto.fel.cvut.cz/ontologies/aviation-safety/Water_injection_system -->

    <owl:Class rdf:about="&m;Water_injection_system">
        <rdfs:label>Water injection system</rdfs:label>
        <rdfs:subClassOf rdf:resource="&m;Aircraft_part"/>
        <m:generated_time rdf:datatype="&xsd;dateTime">2015-04-09T18:56:27.771+02:00</m:generated_time>
        <rdfs:comment xml:lang="en">(ATA Code:8200) Water injection system: The system components and parts which inject a water mixture into induction system of turbine and reciprocating engines. Typical parts are pump, switch, tank and valve.</rdfs:comment>
        <m:has_related_eccairs_term rdf:resource="http://onto.fel.cvut.cz/ontologies/2014/ECCAIRS_Aviation_1.3.0.12/eccairs-descriptive-factors#category_11820000"/>
    </owl:Class>
    


    <!-- http://onto.fel.cvut.cz/ontologies/aviation-safety/Water_injection_system_part -->

    <owl:Class rdf:about="&m;Water_injection_system_part">
        <rdfs:label>Water injection system part</rdfs:label>
        <rdfs:subClassOf rdf:resource="&m;Aircraft_part"/>
        <rdfs:subClassOf>
            <owl:Restriction>
                <owl:onProperty rdf:resource="http://onto.fel.cvut.cz/ontologies/ufo/is_part_of"/>
                <owl:someValuesFrom rdf:resource="&m;Water_injection_system"/>
            </owl:Restriction>
        </rdfs:subClassOf>
        <m:generated_time rdf:datatype="&xsd;dateTime">2015-04-12T02:45:54.351+02:00</m:generated_time>
        <m:has_related_eccairs_term rdf:resource="http://onto.fel.cvut.cz/ontologies/2014/ECCAIRS_Aviation_1.3.0.12/eccairs-descriptive-factors#category_11820000"/>
    </owl:Class>
    


    <!-- http://onto.fel.cvut.cz/ontologies/aviation-safety/Water_line_anti-ice_system -->

    <owl:Class rdf:about="&m;Water_line_anti-ice_system">
        <rdfs:subClassOf rdf:resource="&m;Ice-rain_protection_systems"/>
    </owl:Class>
    


    <!-- http://onto.fel.cvut.cz/ontologies/aviation-safety/Weather_radar_system -->

    <owl:Class rdf:about="&m;Weather_radar_system">
        <rdfs:label>Weather radar system</rdfs:label>
        <rdfs:subClassOf rdf:resource="&m;Independent_position_determining_system"/>
        <m:generated_time rdf:datatype="&xsd;dateTime">2015-04-09T18:56:27.771+02:00</m:generated_time>
        <rdfs:comment xml:lang="en">(ATA Code:3442) Weather radar system: The system components and parts which transmit and receive signals independent of ground facilities to determine the relative position of adverse weather cells. Typical parts are transceiver, antenna, the control panel for the weather avoidance radar system, accessory synchronizers, servo amplifier and scope.</rdfs:comment>
        <m:has_related_eccairs_term rdf:resource="http://onto.fel.cvut.cz/ontologies/2014/ECCAIRS_Aviation_1.3.0.12/eccairs-descriptive-factors#category_11344200"/>
    </owl:Class>
    


    <!-- http://onto.fel.cvut.cz/ontologies/aviation-safety/Weighing_and_Balancing -->

    <owl:Class rdf:about="&m;Weighing_and_Balancing">
        <rdfs:label>Weighing and Balancing</rdfs:label>
        <rdfs:subClassOf rdf:resource="&m;Leveling_and_weighting_part"/>
        <m:generated_time rdf:datatype="&xsd;dateTime">2015-04-09T18:56:27.771+02:00</m:generated_time>
        <rdfs:comment xml:lang="en">(ATA Code:0810) Those units or components dedicated to the specific function of recording, storing or computing weight and balance data.</rdfs:comment>
        <m:has_related_eccairs_term rdf:resource="http://onto.fel.cvut.cz/ontologies/2014/ECCAIRS_Aviation_1.3.0.12/eccairs-descriptive-factors#category_11081000"/>
    </owl:Class>
    


    <!-- http://onto.fel.cvut.cz/ontologies/aviation-safety/Wind_shear_detection_system -->

    <owl:Class rdf:about="&m;Wind_shear_detection_system">
        <rdfs:label>Wind shear detection system</rdfs:label>
        <rdfs:subClassOf rdf:resource="&m;Landing_and_taxi_aid"/>
        <rdfs:subClassOf>
            <owl:Restriction>
                <owl:onProperty rdf:resource="&m;is_used_for"/>
                <owl:someValuesFrom>
                    <owl:Class>
                        <owl:intersectionOf rdf:parseType="Collection">
                            <rdf:Description rdf:about="&m;Danger_detection"/>
                            <owl:Restriction>
                                <owl:onProperty rdf:resource="&m;is_detection_of"/>
                                <owl:someValuesFrom rdf:resource="&m;Wind_shear"/>
                            </owl:Restriction>
                        </owl:intersectionOf>
                    </owl:Class>
                </owl:someValuesFrom>
            </owl:Restriction>
        </rdfs:subClassOf>
        <m:generated_time rdf:datatype="&xsd;dateTime">2015-04-09T18:56:27.771+02:00</m:generated_time>
        <rdfs:comment xml:lang="en">(ATA Code:3436) Wind shear detection system: The flight instrument system that allows the pilot to detect a change in wind speed and/or direction in space, including updrafts and downdrafts. Includes the outboard sensors, indicators and the warning system which notifies the pilot of the appropriate corrective action manoeuvre to take.</rdfs:comment>
        <m:has_related_eccairs_term rdf:resource="http://onto.fel.cvut.cz/ontologies/2014/ECCAIRS_Aviation_1.3.0.12/eccairs-descriptive-factors#category_11343600"/>
    </owl:Class>
    


    <!-- http://onto.fel.cvut.cz/ontologies/aviation-safety/Window-windshield_system -->

    <owl:Class rdf:about="&m;Window-windshield_system">
        <rdfs:label>Window/windshield system</rdfs:label>
        <rdfs:subClassOf rdf:resource="&m;Aircraft_part"/>
        <m:generated_time rdf:datatype="&xsd;dateTime">2015-04-09T18:56:27.771+02:00</m:generated_time>
        <rdfs:comment xml:lang="en">(ATA Code:5600) Window/windshield system: The fuselage and crew compartment windows inclusive of windshield and those windows installed in doors.</rdfs:comment>
        <m:has_related_eccairs_term rdf:resource="http://onto.fel.cvut.cz/ontologies/2014/ECCAIRS_Aviation_1.3.0.12/eccairs-descriptive-factors#category_11560000"/>
    </owl:Class>
    


    <!-- http://onto.fel.cvut.cz/ontologies/aviation-safety/Window-windshield_system_part -->

    <owl:Class rdf:about="&m;Window-windshield_system_part">
        <rdfs:label>Window/windshield system part</rdfs:label>
        <rdfs:subClassOf rdf:resource="&m;Aircraft_part"/>
        <rdfs:subClassOf>
            <owl:Restriction>
                <owl:onProperty rdf:resource="http://onto.fel.cvut.cz/ontologies/ufo/is_part_of"/>
                <owl:someValuesFrom rdf:resource="&m;Window-windshield_system"/>
            </owl:Restriction>
        </rdfs:subClassOf>
        <m:generated_time rdf:datatype="&xsd;dateTime">2015-04-12T02:45:54.351+02:00</m:generated_time>
        <m:has_related_eccairs_term rdf:resource="http://onto.fel.cvut.cz/ontologies/2014/ECCAIRS_Aviation_1.3.0.12/eccairs-descriptive-factors#category_11560000"/>
    </owl:Class>
    


    <!-- http://onto.fel.cvut.cz/ontologies/aviation-safety/Window_System_Wiring -->

    <owl:Class rdf:about="&m;Window_System_Wiring">
        <rdfs:label>Window System Wiring</rdfs:label>
        <rdfs:subClassOf rdf:resource="&m;Window-windshield_system_part"/>
        <m:generated_time rdf:datatype="&xsd;dateTime">2015-04-09T18:56:27.771+02:00</m:generated_time>
        <rdfs:comment xml:lang="en">(ATA Code:5697) Wiring specific to the Window System</rdfs:comment>
        <m:has_related_eccairs_term rdf:resource="http://onto.fel.cvut.cz/ontologies/2014/ECCAIRS_Aviation_1.3.0.12/eccairs-descriptive-factors#category_11569700"/>
    </owl:Class>
    


    <!-- http://onto.fel.cvut.cz/ontologies/aviation-safety/Windshield-door_rain-ice_removal -->

    <owl:Class rdf:about="&m;Windshield-door_rain-ice_removal">
        <rdfs:label>Windshield/door rain/ice removal</rdfs:label>
        <rdfs:subClassOf rdf:resource="&m;Ice-rain_protection_systems"/>
        <m:generated_time rdf:datatype="&xsd;dateTime">2015-04-09T18:56:27.771+02:00</m:generated_time>
        <rdfs:comment xml:lang="en">(ATA Code:3040) Windshield/door rain/ice removal: The system and components which is used to clear, eliminate or prevent the formation of rain, ice or frost on the windshield or windows. Excludes reports of glass panel cracking [Code 11561000]. Typical parts are motor, actuator, wiper blade, hydraulic converter, shaft, line, switch, the electrical heating portion of heated glass panels, control units, alcohol de-ice system lines, tanks, pumps and valves.</rdfs:comment>
        <m:has_related_eccairs_term rdf:resource="http://onto.fel.cvut.cz/ontologies/2014/ECCAIRS_Aviation_1.3.0.12/eccairs-descriptive-factors#category_11304000"/>
    </owl:Class>
    


    <!-- http://onto.fel.cvut.cz/ontologies/aviation-safety/Windshield-door_rain-ice_removal_part -->

    <owl:Class rdf:about="&m;Windshield-door_rain-ice_removal_part">
        <rdfs:label>Windshield/door rain/ice removal part</rdfs:label>
        <rdfs:subClassOf rdf:resource="&m;Ice-rain_protection_systems"/>
        <rdfs:subClassOf>
            <owl:Restriction>
                <owl:onProperty rdf:resource="http://onto.fel.cvut.cz/ontologies/ufo/is_part_of"/>
                <owl:someValuesFrom rdf:resource="&m;Windshield-door_rain-ice_removal"/>
            </owl:Restriction>
        </rdfs:subClassOf>
        <m:generated_time rdf:datatype="&xsd;dateTime">2015-04-12T02:45:54.351+02:00</m:generated_time>
        <m:has_related_eccairs_term rdf:resource="http://onto.fel.cvut.cz/ontologies/2014/ECCAIRS_Aviation_1.3.0.12/eccairs-descriptive-factors#category_11304000"/>
    </owl:Class>
    


    <!-- http://onto.fel.cvut.cz/ontologies/aviation-safety/Windshield_washer_system -->

    <owl:Class rdf:about="&m;Windshield_washer_system">
        <rdfs:label>Windshield washer system</rdfs:label>
        <rdfs:subClassOf rdf:resource="&m;Windshield-door_rain-ice_removal_part"/>
        <m:generated_time rdf:datatype="&xsd;dateTime">2015-04-09T18:56:27.771+02:00</m:generated_time>
        <rdfs:comment xml:lang="en">(ATA Code:3042) Windshield washer system: The system and components used to remove any build up of rain and contaminants on the aircraft windshield. Typical parts are motor, actuator and storage tank.</rdfs:comment>
        <m:has_related_eccairs_term rdf:resource="http://onto.fel.cvut.cz/ontologies/2014/ECCAIRS_Aviation_1.3.0.12/eccairs-descriptive-factors#category_11304200"/>
    </owl:Class>
    


    <!-- http://onto.fel.cvut.cz/ontologies/aviation-safety/Windshield_wiper_system -->

    <owl:Class rdf:about="&m;Windshield_wiper_system">
        <rdfs:label>Windshield wiper system</rdfs:label>
        <rdfs:subClassOf rdf:resource="&m;Windshield-door_rain-ice_removal_part"/>
        <m:generated_time rdf:datatype="&xsd;dateTime">2015-04-09T18:56:27.771+02:00</m:generated_time>
        <rdfs:comment xml:lang="en">(ATA Code:3043) Windshield wiper system: The system and components used to remove any build up of rain and contaminants on the aircraft windshield. Typical parts are motor, actuator and wipers.</rdfs:comment>
        <m:has_related_eccairs_term rdf:resource="http://onto.fel.cvut.cz/ontologies/2014/ECCAIRS_Aviation_1.3.0.12/eccairs-descriptive-factors#category_11304300"/>
    </owl:Class>
    


    <!-- http://onto.fel.cvut.cz/ontologies/aviation-safety/Wing_attachment_fitting -->

    <owl:Class rdf:about="&m;Wing_attachment_fitting">
        <rdfs:label>Wing attachment fitting</rdfs:label>
        <rdfs:subClassOf rdf:resource="&m;Wing_structure_part"/>
        <m:generated_time rdf:datatype="&xsd;dateTime">2015-04-09T18:56:27.771+02:00</m:generated_time>
        <rdfs:comment xml:lang="en">(ATA Code:5740) Wing attachment fitting: The structure on the wing used for the attachment of fuselage, nacelle or pylon and landing gear to the wing and for the support of equipment within the wing.</rdfs:comment>
        <m:has_related_eccairs_term rdf:resource="http://onto.fel.cvut.cz/ontologies/2014/ECCAIRS_Aviation_1.3.0.12/eccairs-descriptive-factors#category_11574000"/>
    </owl:Class>
    


    <!-- http://onto.fel.cvut.cz/ontologies/aviation-safety/Wing_attachment_fitting_part -->

    <owl:Class rdf:about="&m;Wing_attachment_fitting_part">
        <rdfs:label>Wing attachment fitting part</rdfs:label>
        <rdfs:subClassOf rdf:resource="&m;Wing_structure_part"/>
        <rdfs:subClassOf>
            <owl:Restriction>
                <owl:onProperty rdf:resource="http://onto.fel.cvut.cz/ontologies/ufo/is_part_of"/>
                <owl:someValuesFrom rdf:resource="&m;Wing_attachment_fitting"/>
            </owl:Restriction>
        </rdfs:subClassOf>
        <m:generated_time rdf:datatype="&xsd;dateTime">2015-04-12T02:45:54.351+02:00</m:generated_time>
        <m:has_related_eccairs_term rdf:resource="http://onto.fel.cvut.cz/ontologies/2014/ECCAIRS_Aviation_1.3.0.12/eccairs-descriptive-factors#category_11574000"/>
    </owl:Class>
    


    <!-- http://onto.fel.cvut.cz/ontologies/aviation-safety/Wing_attachment_fittings_(on_fuselage) -->

    <owl:Class rdf:about="&m;Wing_attachment_fittings_(on_fuselage)">
        <rdfs:label>Wing attachment fittings (on fuselage)</rdfs:label>
        <rdfs:subClassOf rdf:resource="&m;Fuselage_attachment_fittings_part"/>
        <m:generated_time rdf:datatype="&xsd;dateTime">2015-04-09T18:56:27.771+02:00</m:generated_time>
        <rdfs:comment xml:lang="en">(ATA Code:5341) Wing attachment fittings (on fuselage): The fittings on the fuselage used for the attachment of the wings.</rdfs:comment>
        <m:has_related_eccairs_term rdf:resource="http://onto.fel.cvut.cz/ontologies/2014/ECCAIRS_Aviation_1.3.0.12/eccairs-descriptive-factors#category_11534100"/>
    </owl:Class>
    


    <!-- http://onto.fel.cvut.cz/ontologies/aviation-safety/Wing_centre_box -->

    <owl:Class rdf:about="&m;Wing_centre_box">
        <rdfs:label>Wing centre box</rdfs:label>
        <rdfs:subClassOf rdf:resource="&m;Wing_main_frame_structure_part"/>
        <m:generated_time rdf:datatype="&xsd;dateTime">2015-04-09T18:56:27.771+02:00</m:generated_time>
        <rdfs:comment xml:lang="en">(ATA Code:5714) The centre wing box structure.</rdfs:comment>
        <m:has_related_eccairs_term rdf:resource="http://onto.fel.cvut.cz/ontologies/2014/ECCAIRS_Aviation_1.3.0.12/eccairs-descriptive-factors#category_11571400"/>
    </owl:Class>
    


    <!-- http://onto.fel.cvut.cz/ontologies/aviation-safety/Wing_control_surface_attachment_fittings -->

    <owl:Class rdf:about="&m;Wing_control_surface_attachment_fittings">
        <rdfs:label>Wing control surface attachment fittings</rdfs:label>
        <rdfs:subClassOf rdf:resource="&m;Wing_attachment_fitting_part"/>
        <m:generated_time rdf:datatype="&xsd;dateTime">2015-04-09T18:56:27.771+02:00</m:generated_time>
        <rdfs:comment xml:lang="en">(ATA Code:5744) The fittings on the wing used for attachment of the control surface. Includes flap attachment fittings.</rdfs:comment>
        <m:has_related_eccairs_term rdf:resource="http://onto.fel.cvut.cz/ontologies/2014/ECCAIRS_Aviation_1.3.0.12/eccairs-descriptive-factors#category_11574400"/>
    </owl:Class>
    


    <!-- http://onto.fel.cvut.cz/ontologies/aviation-safety/Wing_flight_control_surface -->

    <owl:Class rdf:about="&m;Wing_flight_control_surface">
        <rdfs:label>Wing flight control surface</rdfs:label>
        <rdfs:subClassOf rdf:resource="&m;Wing_structure_part"/>
        <m:generated_time rdf:datatype="&xsd;dateTime">2015-04-09T18:56:27.771+02:00</m:generated_time>
        <rdfs:comment xml:lang="en">(ATA Code:5750) Wing flight control surface</rdfs:comment>
        <m:has_related_eccairs_term rdf:resource="http://onto.fel.cvut.cz/ontologies/2014/ECCAIRS_Aviation_1.3.0.12/eccairs-descriptive-factors#category_11575000"/>
    </owl:Class>
    


    <!-- http://onto.fel.cvut.cz/ontologies/aviation-safety/Wing_flight_control_surface_part -->

    <owl:Class rdf:about="&m;Wing_flight_control_surface_part">
        <rdfs:label>Wing flight control surface part</rdfs:label>
        <rdfs:subClassOf rdf:resource="&m;Wing_structure_part"/>
        <rdfs:subClassOf>
            <owl:Restriction>
                <owl:onProperty rdf:resource="http://onto.fel.cvut.cz/ontologies/ufo/is_part_of"/>
                <owl:someValuesFrom rdf:resource="&m;Wing_flight_control_surface"/>
            </owl:Restriction>
        </rdfs:subClassOf>
        <m:generated_time rdf:datatype="&xsd;dateTime">2015-04-12T02:45:54.351+02:00</m:generated_time>
        <m:has_related_eccairs_term rdf:resource="http://onto.fel.cvut.cz/ontologies/2014/ECCAIRS_Aviation_1.3.0.12/eccairs-descriptive-factors#category_11575000"/>
    </owl:Class>
    


    <!-- http://onto.fel.cvut.cz/ontologies/aviation-safety/Wing_folding_system -->

    <owl:Class rdf:about="&m;Wing_folding_system">
        <rdfs:label>Wing folding system</rdfs:label>
        <rdfs:subClassOf rdf:resource="&m;Wing_structure_part"/>
        <m:generated_time rdf:datatype="&xsd;dateTime">2015-04-09T18:56:27.771+02:00</m:generated_time>
        <rdfs:comment xml:lang="en">(ATA Code:5790) System that controls the on-ground movement of any portion of the main wing structure.   Includes mechanisms, linkages, actuators, locks, indicating/warning systems, etc.</rdfs:comment>
        <m:has_related_eccairs_term rdf:resource="http://onto.fel.cvut.cz/ontologies/2014/ECCAIRS_Aviation_1.3.0.12/eccairs-descriptive-factors#category_11579000"/>
    </owl:Class>
    


    <!-- http://onto.fel.cvut.cz/ontologies/aviation-safety/Wing_folding_system_part -->

    <owl:Class rdf:about="&m;Wing_folding_system_part">
        <rdfs:label>Wing folding system part</rdfs:label>
        <rdfs:subClassOf rdf:resource="&m;Wing_structure_part"/>
        <rdfs:subClassOf>
            <owl:Restriction>
                <owl:onProperty rdf:resource="http://onto.fel.cvut.cz/ontologies/ufo/is_part_of"/>
                <owl:someValuesFrom rdf:resource="&m;Wing_folding_system"/>
            </owl:Restriction>
        </rdfs:subClassOf>
        <m:generated_time rdf:datatype="&xsd;dateTime">2015-04-12T02:45:54.351+02:00</m:generated_time>
        <m:has_related_eccairs_term rdf:resource="http://onto.fel.cvut.cz/ontologies/2014/ECCAIRS_Aviation_1.3.0.12/eccairs-descriptive-factors#category_11579000"/>
    </owl:Class>
    


    <!-- http://onto.fel.cvut.cz/ontologies/aviation-safety/Wing_fuselage_attachment_fitting -->

    <owl:Class rdf:about="&m;Wing_fuselage_attachment_fitting">
        <rdfs:label>Wing fuselage attachment fitting</rdfs:label>
        <rdfs:subClassOf rdf:resource="&m;Wing_attachment_fitting_part"/>
        <m:generated_time rdf:datatype="&xsd;dateTime">2015-04-09T18:56:27.771+02:00</m:generated_time>
        <rdfs:comment xml:lang="en">(ATA Code:5741) The fittings on the wing used for attachment to the fuselage structure.</rdfs:comment>
        <m:has_related_eccairs_term rdf:resource="http://onto.fel.cvut.cz/ontologies/2014/ECCAIRS_Aviation_1.3.0.12/eccairs-descriptive-factors#category_11574100"/>
    </owl:Class>
    


    <!-- http://onto.fel.cvut.cz/ontologies/aviation-safety/Wing_landing_gear_attachment_fitting -->

    <owl:Class rdf:about="&m;Wing_landing_gear_attachment_fitting">
        <rdfs:label>Wing landing gear attachment fitting</rdfs:label>
        <rdfs:subClassOf rdf:resource="&m;Wing_attachment_fitting_part"/>
        <m:generated_time rdf:datatype="&xsd;dateTime">2015-04-09T18:56:27.771+02:00</m:generated_time>
        <rdfs:comment xml:lang="en">(ATA Code:5743) The fittings on the wing used for attachment of the landing gear.</rdfs:comment>
        <m:has_related_eccairs_term rdf:resource="http://onto.fel.cvut.cz/ontologies/2014/ECCAIRS_Aviation_1.3.0.12/eccairs-descriptive-factors#category_11574300"/>
    </owl:Class>
    


    <!-- http://onto.fel.cvut.cz/ontologies/aviation-safety/Wing_longeron-stringer -->

    <owl:Class rdf:about="&m;Wing_longeron-stringer">
        <rdfs:label>Wing longeron/stringer</rdfs:label>
        <rdfs:subClassOf rdf:resource="&m;Wing_main_frame_structure_part"/>
        <m:generated_time rdf:datatype="&xsd;dateTime">2015-04-09T18:56:27.771+02:00</m:generated_time>
        <rdfs:comment xml:lang="en">(ATA Code:5713) The longerons or stringers in the wing structure.</rdfs:comment>
        <m:has_related_eccairs_term rdf:resource="http://onto.fel.cvut.cz/ontologies/2014/ECCAIRS_Aviation_1.3.0.12/eccairs-descriptive-factors#category_11571300"/>
    </owl:Class>
    


    <!-- http://onto.fel.cvut.cz/ontologies/aviation-safety/Wing_main_frame_structure -->

    <owl:Class rdf:about="&m;Wing_main_frame_structure">
        <rdfs:label>Wing main frame structure</rdfs:label>
        <rdfs:subClassOf rdf:resource="&m;Wing_structure_part"/>
        <m:generated_time rdf:datatype="&xsd;dateTime">2015-04-09T18:56:27.771+02:00</m:generated_time>
        <rdfs:comment xml:lang="en">(ATA Code:5710) Wing main frame structure: The main frame structure of the wing.</rdfs:comment>
        <m:has_related_eccairs_term rdf:resource="http://onto.fel.cvut.cz/ontologies/2014/ECCAIRS_Aviation_1.3.0.12/eccairs-descriptive-factors#category_11571000"/>
    </owl:Class>
    


    <!-- http://onto.fel.cvut.cz/ontologies/aviation-safety/Wing_main_frame_structure_part -->

    <owl:Class rdf:about="&m;Wing_main_frame_structure_part">
        <rdfs:label>Wing main frame structure part</rdfs:label>
        <rdfs:subClassOf rdf:resource="&m;Wing_structure_part"/>
        <rdfs:subClassOf>
            <owl:Restriction>
                <owl:onProperty rdf:resource="http://onto.fel.cvut.cz/ontologies/ufo/is_part_of"/>
                <owl:someValuesFrom rdf:resource="&m;Wing_main_frame_structure"/>
            </owl:Restriction>
        </rdfs:subClassOf>
        <m:generated_time rdf:datatype="&xsd;dateTime">2015-04-12T02:45:54.351+02:00</m:generated_time>
        <m:has_related_eccairs_term rdf:resource="http://onto.fel.cvut.cz/ontologies/2014/ECCAIRS_Aviation_1.3.0.12/eccairs-descriptive-factors#category_11571000"/>
    </owl:Class>
    


    <!-- http://onto.fel.cvut.cz/ontologies/aviation-safety/Wing_miscellaneous_structure -->

    <owl:Class rdf:about="&m;Wing_miscellaneous_structure">
        <rdfs:label>Wing miscellaneous structure</rdfs:label>
        <rdfs:subClassOf rdf:resource="&m;Wing_structure_part"/>
        <m:generated_time rdf:datatype="&xsd;dateTime">2015-04-09T18:56:27.771+02:00</m:generated_time>
        <rdfs:comment xml:lang="en">(ATA Code:5720) Wing miscellaneous structure: The auxiliary or miscellaneous wing structure which includes the secondary items used for attachment. Does not include plates or skins. Typical parts are wing tip, clips, brackets, channels, angles and stiffeners.</rdfs:comment>
        <m:has_related_eccairs_term rdf:resource="http://onto.fel.cvut.cz/ontologies/2014/ECCAIRS_Aviation_1.3.0.12/eccairs-descriptive-factors#category_11572000"/>
    </owl:Class>
    


    <!-- http://onto.fel.cvut.cz/ontologies/aviation-safety/Wing_plates-skins -->

    <owl:Class rdf:about="&m;Wing_plates-skins">
        <rdfs:label>Wing plates/skins</rdfs:label>
        <rdfs:subClassOf rdf:resource="&m;Wing_structure_part"/>
        <m:generated_time rdf:datatype="&xsd;dateTime">2015-04-09T18:56:27.771+02:00</m:generated_time>
        <rdfs:comment xml:lang="en">(ATA Code:5730) Wing plates/skins: The exterior covering of the wing including the access covers, tip tank fillets or fairings. Includes the leading edge and trailing edge skin and wing mounted fuel compartment panels.</rdfs:comment>
        <m:has_related_eccairs_term rdf:resource="http://onto.fel.cvut.cz/ontologies/2014/ECCAIRS_Aviation_1.3.0.12/eccairs-descriptive-factors#category_11573000"/>
    </owl:Class>
    


    <!-- http://onto.fel.cvut.cz/ontologies/aviation-safety/Wing_ribs-bulkheads -->

    <owl:Class rdf:about="&m;Wing_ribs-bulkheads">
        <rdfs:label>Wing ribs/bulkheads</rdfs:label>
        <rdfs:subClassOf rdf:resource="&m;Wing_main_frame_structure_part"/>
        <m:generated_time rdf:datatype="&xsd;dateTime">2015-04-09T18:56:27.771+02:00</m:generated_time>
        <rdfs:comment xml:lang="en">(ATA Code:5712) The ribs/bulkhead in the wing structure.</rdfs:comment>
        <m:has_related_eccairs_term rdf:resource="http://onto.fel.cvut.cz/ontologies/2014/ECCAIRS_Aviation_1.3.0.12/eccairs-descriptive-factors#category_11571200"/>
    </owl:Class>
    


    <!-- http://onto.fel.cvut.cz/ontologies/aviation-safety/Wing_spar -->

    <owl:Class rdf:about="&m;Wing_spar">
        <rdfs:label>Wing spar</rdfs:label>
        <rdfs:subClassOf rdf:resource="&m;Wing_main_frame_structure_part"/>
        <m:generated_time rdf:datatype="&xsd;dateTime">2015-04-09T18:56:27.771+02:00</m:generated_time>
        <rdfs:comment xml:lang="en">(ATA Code:5711) A spar in the wing structure.</rdfs:comment>
        <m:has_related_eccairs_term rdf:resource="http://onto.fel.cvut.cz/ontologies/2014/ECCAIRS_Aviation_1.3.0.12/eccairs-descriptive-factors#category_11571100"/>
    </owl:Class>
    


    <!-- http://onto.fel.cvut.cz/ontologies/aviation-safety/Wing_structure -->

    <owl:Class rdf:about="&m;Wing_structure">
        <rdfs:label>Wing structure</rdfs:label>
        <rdfs:subClassOf rdf:resource="&m;Aircraft_part"/>
        <m:generated_time rdf:datatype="&xsd;dateTime">2015-04-09T18:56:27.771+02:00</m:generated_time>
        <rdfs:comment xml:lang="en">(ATA Code:5700) Wing structure: The centre wing and outer wing structural units and associated components and members which support the aircraft in flight.</rdfs:comment>
        <m:has_related_eccairs_term rdf:resource="http://onto.fel.cvut.cz/ontologies/2014/ECCAIRS_Aviation_1.3.0.12/eccairs-descriptive-factors#category_11570000"/>
    </owl:Class>
    


    <!-- http://onto.fel.cvut.cz/ontologies/aviation-safety/Wing_structure_part -->

    <owl:Class rdf:about="&m;Wing_structure_part">
        <rdfs:label>Wing structure part</rdfs:label>
        <rdfs:subClassOf rdf:resource="&m;Aircraft_part"/>
        <rdfs:subClassOf>
            <owl:Restriction>
                <owl:onProperty rdf:resource="http://onto.fel.cvut.cz/ontologies/ufo/is_part_of"/>
                <owl:someValuesFrom rdf:resource="&m;Wing_structure"/>
            </owl:Restriction>
        </rdfs:subClassOf>
        <m:generated_time rdf:datatype="&xsd;dateTime">2015-04-12T02:45:54.351+02:00</m:generated_time>
        <m:has_related_eccairs_term rdf:resource="http://onto.fel.cvut.cz/ontologies/2014/ECCAIRS_Aviation_1.3.0.12/eccairs-descriptive-factors#category_11570000"/>
    </owl:Class>
    


    <!-- http://onto.fel.cvut.cz/ontologies/aviation-safety/Wing_systems_wiring -->

    <owl:Class rdf:about="&m;Wing_systems_wiring">
        <rdfs:label>Wing systems wiring</rdfs:label>
        <rdfs:subClassOf rdf:resource="&m;Wing_folding_system_part"/>
        <m:generated_time rdf:datatype="&xsd;dateTime">2015-04-09T18:56:27.771+02:00</m:generated_time>
        <rdfs:comment xml:lang="en">(ATA Code:5797) Wiring specific to the wing systems.</rdfs:comment>
        <m:has_related_eccairs_term rdf:resource="http://onto.fel.cvut.cz/ontologies/2014/ECCAIRS_Aviation_1.3.0.12/eccairs-descriptive-factors#category_11579700"/>
    </owl:Class>
    


    <!-- http://onto.fel.cvut.cz/ontologies/aviation-safety/Wiring -->

    <owl:Class rdf:about="&m;Wiring"/>
    


    <!-- http://onto.fel.cvut.cz/ontologies/aviation-safety/Wiring_specific_to_the_Ignition_System -->

    <owl:Class rdf:about="&m;Wiring_specific_to_the_Ignition_System">
        <rdfs:label>Wiring specific to the Ignition System</rdfs:label>
        <rdfs:subClassOf rdf:resource="&m;Ignition_system_part"/>
        <rdfs:subClassOf rdf:resource="&m;Wiring"/>
        <rdfs:subClassOf>
            <owl:Restriction>
                <owl:onProperty rdf:resource="http://onto.fel.cvut.cz/ontologies/ufo/is_part_of"/>
                <owl:someValuesFrom rdf:resource="&m;Ignition_system"/>
            </owl:Restriction>
        </rdfs:subClassOf>
        <m:generated_time rdf:datatype="&xsd;dateTime">2015-04-09T18:56:27.771+02:00</m:generated_time>
        <rdfs:comment xml:lang="en">(ATA Code:7497) Wiring specific to the Ignition System</rdfs:comment>
        <m:has_related_eccairs_term rdf:resource="http://onto.fel.cvut.cz/ontologies/2014/ECCAIRS_Aviation_1.3.0.12/eccairs-descriptive-factors#category_11749700"/>
    </owl:Class>
    


    <!-- http://onto.fel.cvut.cz/ontologies/aviation-safety/Wiring_specific_to_the_electrical_power_system_not_part_of_the_power_distribution_systems -->

    <owl:Class rdf:about="&m;Wiring_specific_to_the_electrical_power_system_not_part_of_the_power_distribution_systems">
        <rdfs:subClassOf rdf:resource="&m;Electrical_power_system_part"/>
    </owl:Class>
    


    <!-- http://onto.fel.cvut.cz/ontologies/aviation-safety/Yaw_damper_system -->

    <owl:Class rdf:about="&m;Yaw_damper_system">
        <rdfs:label>Yaw damper system</rdfs:label>
        <rdfs:subClassOf rdf:resource="&m;Rudder_&amp;_Tab_control_system_part"/>
        <m:generated_time rdf:datatype="&xsd;dateTime">2015-04-09T18:56:27.771+02:00</m:generated_time>
        <rdfs:comment xml:lang="en">(ATA Code:2724) The yaw damper system associated with the autopilot system used for controlling direction.</rdfs:comment>
        <m:has_related_eccairs_term rdf:resource="http://onto.fel.cvut.cz/ontologies/2014/ECCAIRS_Aviation_1.3.0.12/eccairs-descriptive-factors#category_11272400"/>
    </owl:Class>
    


    <!-- http://onto.fel.cvut.cz/ontologies/aviation-safety/aerotow -->

    <owl:Class rdf:about="&m;aerotow">
        <rdfs:label xml:lang="en">Aerotow</rdfs:label>
        <rdfs:subClassOf rdf:resource="&m;Aircraft_operation"/>
        <rdfs:subClassOf>
            <owl:Restriction>
                <owl:onProperty rdf:resource="http://onto.fel.cvut.cz/ontologies/ufo/has_participant"/>
                <owl:onClass rdf:resource="&m;Aircraft"/>
                <owl:minQualifiedCardinality rdf:datatype="&xsd;nonNegativeInteger">2</owl:minQualifiedCardinality>
            </owl:Restriction>
        </rdfs:subClassOf>
    </owl:Class>
    


    <!-- http://onto.fel.cvut.cz/ontologies/aviation-safety/air_traffic_control_transponder_system -->

    <owl:Class rdf:about="&m;air_traffic_control_transponder_system">
        <rdfs:label>Air traffic control transponder system</rdfs:label>
        <rdfs:subClassOf rdf:resource="&m;Dependent_position_determining_system"/>
        <m:generated_time rdf:datatype="&xsd;dateTime">2015-04-09T18:56:27.771+02:00</m:generated_time>
        <m:generated_time rdf:datatype="&xsd;dateTime">2015-04-17T16:49:10.062+02:00</m:generated_time>
        <rdfs:comment xml:lang="en">(ATA Code:3452) Air traffic control transponder system: The air traffic control system which receives coded signals from a ground station and transmits a coded reply for altitude reporting and identification purposes. Typical parts are transponder, antenna, control unit, transceiver and coaxial connecting cable.</rdfs:comment>
        <m:has_related_eccairs_term rdf:resource="http://onto.fel.cvut.cz/ontologies/2014/ECCAIRS_Aviation_1.3.0.12/eccairs-descriptive-factors#category_11345200"/>
        <m:has_related_eccairs_term rdf:resource="http://onto.fel.cvut.cz/ontologies/2014/ECCAIRS_Aviation_1.3.0.12/eccairs-descriptive-factors#category_21030201"/>
    </owl:Class>
    


    <!-- http://onto.fel.cvut.cz/ontologies/aviation-safety/airborne_collision_avoidance_system -->

    <owl:Class rdf:about="&m;airborne_collision_avoidance_system">
        <rdfs:label xml:lang="en">Airborne collision avoidance system</rdfs:label>
        <rdfs:subClassOf rdf:resource="&m;Traffic_alert_and_collision_avoidance_system-Airborne_collision_avoidance_system"/>
        <rdfs:subClassOf>
            <owl:Restriction>
                <owl:onProperty rdf:resource="&m;communicates_with"/>
                <owl:someValuesFrom rdf:resource="&m;airborne_collision_avoidance_system"/>
            </owl:Restriction>
        </rdfs:subClassOf>
        <m:has_abbreviation xml:lang="en">ACAS</m:has_abbreviation>
    </owl:Class>
    


    <!-- http://onto.fel.cvut.cz/ontologies/aviation-safety/autoflight_system -->

    <owl:Class rdf:about="&m;autoflight_system">
        <rdfs:label xml:lang="en">Autoflight system</rdfs:label>
        <rdfs:subClassOf rdf:resource="&m;Aircraft_part"/>
        <rdfs:subClassOf>
            <owl:Restriction>
                <owl:onProperty rdf:resource="http://onto.fel.cvut.cz/ontologies/ufo/is_part_of"/>
                <owl:someValuesFrom rdf:resource="&m;autoflight_system"/>
            </owl:Restriction>
        </rdfs:subClassOf>
        <m:generated_time rdf:datatype="&xsd;dateTime">2015-04-12T02:45:54.351+02:00</m:generated_time>
        <m:has_related_eccairs_term rdf:resource="http://onto.fel.cvut.cz/ontologies/2014/ECCAIRS_Aviation_1.3.0.12/eccairs-descriptive-factors#category_11220000"/>
    </owl:Class>
    


    <!-- http://onto.fel.cvut.cz/ontologies/aviation-safety/cabin_system -->

    <owl:Class rdf:about="&m;cabin_system">
        <rdfs:label xml:lang="en">Cabin system</rdfs:label>
        <rdfs:subClassOf rdf:resource="&m;Aircraft_part"/>
        <rdfs:subClassOf>
            <owl:Restriction>
                <owl:onProperty rdf:resource="http://onto.fel.cvut.cz/ontologies/ufo/is_part_of"/>
                <owl:someValuesFrom rdf:resource="&m;cabin_system"/>
            </owl:Restriction>
        </rdfs:subClassOf>
        <m:generated_time rdf:datatype="&xsd;dateTime">2015-04-12T02:45:54.351+02:00</m:generated_time>
        <m:has_related_eccairs_term rdf:resource="http://onto.fel.cvut.cz/ontologies/2014/ECCAIRS_Aviation_1.3.0.12/eccairs-descriptive-factors#category_11440000"/>
    </owl:Class>
    


    <!-- http://onto.fel.cvut.cz/ontologies/aviation-safety/distance_measuring_equipment_ground_system -->

    <owl:Class rdf:about="&m;distance_measuring_equipment_ground_system"/>
    


    <!-- http://onto.fel.cvut.cz/ontologies/aviation-safety/distance_measuring_equipment_signal -->

    <owl:Class rdf:about="&m;distance_measuring_equipment_signal">
        <rdfs:subClassOf>
            <owl:Class>
                <owl:intersectionOf rdf:parseType="Collection">
                    <owl:Restriction>
                        <owl:onProperty rdf:resource="&m;is_produced_by"/>
                        <owl:someValuesFrom rdf:resource="&m;distance_measuring_equipment_ground_system"/>
                    </owl:Restriction>
                    <owl:Restriction>
                        <owl:onProperty rdf:resource="&m;is_received_by"/>
                        <owl:someValuesFrom rdf:resource="&m;Distance_measuring_equipment-ultra_high_frequency_tactical_air_navigation_aid"/>
                    </owl:Restriction>
                </owl:intersectionOf>
            </owl:Class>
        </rdfs:subClassOf>
    </owl:Class>
    


    <!-- http://onto.fel.cvut.cz/ontologies/aviation-safety/instrument_landing_system_ground_system -->

    <owl:Class rdf:about="&m;instrument_landing_system_ground_system"/>
    


    <!-- http://onto.fel.cvut.cz/ontologies/aviation-safety/lavatory -->

    <owl:Class rdf:about="&m;lavatory">
        <rdfs:label xml:lang="en">Lavatory</rdfs:label>
        <rdfs:subClassOf rdf:resource="&m;Cabin_equipment-furnishings"/>
        <m:generated_time rdf:datatype="&xsd;dateTime">2015-04-09T18:56:27.771+02:00</m:generated_time>
        <rdfs:comment xml:lang="en">(ATA Code:2540) Lavatories: The units and associated systems and parts located in lavatories. Does not include wash basins and other waste disposal items [Code 11383000]. Typical parts are trash containers and dispensers.</rdfs:comment>
        <m:has_related_eccairs_term rdf:resource="http://onto.fel.cvut.cz/ontologies/2014/ECCAIRS_Aviation_1.3.0.12/eccairs-descriptive-factors#category_11254000"/>
    </owl:Class>
    


    <!-- http://onto.fel.cvut.cz/ontologies/aviation-safety/microwave_landing_system_ground_system -->

    <owl:Class rdf:about="&m;microwave_landing_system_ground_system"/>
    


    <!-- http://onto.fel.cvut.cz/ontologies/aviation-safety/mooring_instructions -->

    <owl:Class rdf:about="&m;mooring_instructions">
        <rdfs:label xml:lang="en">Mooring instructions</rdfs:label>
        <rdfs:subClassOf rdf:resource="&m;Parking_mooring_storage_and_return_to_service"/>
        <rdfs:subClassOf>
            <owl:Class>
                <owl:intersectionOf rdf:parseType="Collection">
                    <rdf:Description rdf:about="&m;regulation"/>
                    <owl:Restriction>
                        <owl:onProperty rdf:resource="&m;prescribes"/>
                        <owl:someValuesFrom>
                            <owl:Class>
                                <owl:intersectionOf rdf:parseType="Collection">
                                    <rdf:Description rdf:about="&m;Mooring"/>
                                    <owl:Restriction>
                                        <owl:onProperty rdf:resource="http://onto.fel.cvut.cz/ontologies/ufo/is_performed_by"/>
                                        <owl:someValuesFrom rdf:resource="&m;Aircraft"/>
                                    </owl:Restriction>
                                </owl:intersectionOf>
                            </owl:Class>
                        </owl:someValuesFrom>
                    </owl:Restriction>
                </owl:intersectionOf>
            </owl:Class>
        </rdfs:subClassOf>
    </owl:Class>
    


    <!-- http://onto.fel.cvut.cz/ontologies/aviation-safety/parking-storage_instructions -->

    <owl:Class rdf:about="&m;parking-storage_instructions">
        <rdfs:label xml:lang="en">Parking-storage instructions</rdfs:label>
        <rdfs:subClassOf rdf:resource="&m;Parking_mooring_storage_and_return_to_service"/>
        <m:generated_time rdf:datatype="&xsd;dateTime">2015-04-09T18:56:27.771+02:00</m:generated_time>
        <rdfs:comment xml:lang="en">(ATA Code:1010) Those instructions necessary to park, store, moor and prepare the aircraft for service in any of the conditions to which it may be subjected. Charts showing location of landing gear and control surface locks, blanking plugs and covers, mooring points, etc., shall be included. Includes those maintenance practices necessary to prepare the aircraft for parking, mooring, or storage.</rdfs:comment>
        <m:has_related_eccairs_term rdf:resource="http://onto.fel.cvut.cz/ontologies/2014/ECCAIRS_Aviation_1.3.0.12/eccairs-descriptive-factors#category_11101000"/>
    </owl:Class>
    


    <!-- http://onto.fel.cvut.cz/ontologies/aviation-safety/plates-skins_(elevator) -->

    <owl:Class rdf:about="&m;plates-skins_(elevator)">
        <rdfs:label>plates/skins (elevator)</rdfs:label>
        <rdfs:subClassOf rdf:resource="&m;Elevator_structure_part"/>
        <m:generated_time rdf:datatype="&xsd;dateTime">2015-04-09T18:56:27.771+02:00</m:generated_time>
        <rdfs:comment xml:lang="en">(ATA Code:5522) plates/skins (elevator)</rdfs:comment>
        <m:has_related_eccairs_term rdf:resource="http://onto.fel.cvut.cz/ontologies/2014/ECCAIRS_Aviation_1.3.0.12/eccairs-descriptive-factors#category_11552200"/>
    </owl:Class>
    


    <!-- http://onto.fel.cvut.cz/ontologies/aviation-safety/plates-skins_(vertical_stabilizer) -->

    <owl:Class rdf:about="&m;plates-skins_(vertical_stabilizer)">
        <rdfs:label>plates/skins (vertical stabilizer)</rdfs:label>
        <rdfs:subClassOf rdf:resource="&m;Vertical_stabilizer_part"/>
        <m:generated_time rdf:datatype="&xsd;dateTime">2015-04-09T18:56:27.771+02:00</m:generated_time>
        <rdfs:comment xml:lang="en">(ATA Code:5532) plates/skins (vertical stabilizer)</rdfs:comment>
        <m:has_related_eccairs_term rdf:resource="http://onto.fel.cvut.cz/ontologies/2014/ECCAIRS_Aviation_1.3.0.12/eccairs-descriptive-factors#category_11553200"/>
    </owl:Class>
    


    <!-- http://onto.fel.cvut.cz/ontologies/aviation-safety/return_to_service_instructions -->

    <owl:Class rdf:about="&m;return_to_service_instructions">
        <rdfs:label xml:lang="en">Return to service instructions</rdfs:label>
        <rdfs:subClassOf rdf:resource="&m;Parking_mooring_storage_and_return_to_service"/>
        <m:generated_time rdf:datatype="&xsd;dateTime">2015-04-09T18:56:27.771+02:00</m:generated_time>
        <rdfs:comment xml:lang="en">(ATA Code:1030) Those instructions necessary to prepare the aircraft for operation following mooring, parking, or a period of storage.</rdfs:comment>
        <m:has_related_eccairs_term rdf:resource="http://onto.fel.cvut.cz/ontologies/2014/ECCAIRS_Aviation_1.3.0.12/eccairs-descriptive-factors#category_11103000"/>
    </owl:Class>
    


    <!-- http://onto.fel.cvut.cz/ontologies/aviation-safety/spars-ribs_(elevator) -->

    <owl:Class rdf:about="&m;spars-ribs_(elevator)">
        <rdfs:label>spars/ribs (elevator)</rdfs:label>
        <rdfs:subClassOf rdf:resource="&m;Elevator_structure_part"/>
        <m:generated_time rdf:datatype="&xsd;dateTime">2015-04-09T18:56:27.771+02:00</m:generated_time>
        <rdfs:comment xml:lang="en">(ATA Code:5521) spars/ribs (elevator)</rdfs:comment>
        <m:has_related_eccairs_term rdf:resource="http://onto.fel.cvut.cz/ontologies/2014/ECCAIRS_Aviation_1.3.0.12/eccairs-descriptive-factors#category_11552100"/>
    </owl:Class>
    


    <!-- http://onto.fel.cvut.cz/ontologies/aviation-safety/spars-ribs_(vertical_stabilizer) -->

    <owl:Class rdf:about="&m;spars-ribs_(vertical_stabilizer)">
        <rdfs:label>spars/ribs (vertical stabilizer)</rdfs:label>
        <rdfs:subClassOf rdf:resource="&m;Vertical_stabilizer_part"/>
        <m:generated_time rdf:datatype="&xsd;dateTime">2015-04-09T18:56:27.771+02:00</m:generated_time>
        <rdfs:comment xml:lang="en">(ATA Code:5531) spars/ribs (vertical stabilizer)</rdfs:comment>
        <m:has_related_eccairs_term rdf:resource="http://onto.fel.cvut.cz/ontologies/2014/ECCAIRS_Aviation_1.3.0.12/eccairs-descriptive-factors#category_11553100"/>
    </owl:Class>
    


    <!-- http://onto.fel.cvut.cz/ontologies/aviation-safety/speech_communication_system -->

    <owl:Class rdf:about="&m;speech_communication_system">
        <rdfs:label xml:lang="en">Speech Communication system</rdfs:label>
        <rdfs:subClassOf rdf:resource="&m;Aircraft_communication_related_system"/>
        <m:generated_time rdf:datatype="&xsd;dateTime">2015-04-09T18:56:27.771+02:00</m:generated_time>
        <m:generated_time rdf:datatype="&xsd;dateTime">2015-04-12T02:45:54.351+02:00</m:generated_time>
        <rdfs:comment xml:lang="en">(ATA Code:2310) Speech communications: That portion of the system which utilizes voice modulated electromagnetic waves to transmit and/or receive messages from air to air, or between air and ground installations. Includes HF, VHF and UHF in-flight radio telephone, communication transmitting and receiving equipment.</rdfs:comment>
        <rdfs:comment xml:lang="en">(ATA Code:2310) That portion of the system which utilizes voice modulated electromagnetic waves to transmit and/or receive messages from air to air, or air to ground installations.  Includes H.F., VHF., UHF., etc., inflight telephone, communication transmitting &amp; receiving equipment.</rdfs:comment>
        <m:has_related_eccairs_term rdf:resource="http://onto.fel.cvut.cz/ontologies/2014/ECCAIRS_Aviation_1.3.0.12/eccairs-descriptive-factors#category_100000054"/>
        <m:has_related_eccairs_term rdf:resource="http://onto.fel.cvut.cz/ontologies/2014/ECCAIRS_Aviation_1.3.0.12/eccairs-descriptive-factors#category_11231000"/>
    </owl:Class>
    


    <!-- http://onto.fel.cvut.cz/ontologies/aviation-safety/traffic_alert_and_collision_avoidance_system -->

    <owl:Class rdf:about="&m;traffic_alert_and_collision_avoidance_system">
        <rdfs:label xml:lang="en">Traffic alert and collision avoidance system</rdfs:label>
        <rdfs:subClassOf rdf:resource="&m;Traffic_alert_and_collision_avoidance_system-Airborne_collision_avoidance_system"/>
        <rdfs:subClassOf>
            <owl:Restriction>
                <owl:onProperty rdf:resource="&m;communicates_with"/>
                <owl:someValuesFrom rdf:resource="&m;traffic_alert_and_collision_avoidance_system"/>
            </owl:Restriction>
        </rdfs:subClassOf>
        <m:has_abbreviation xml:lang="en">TCAS</m:has_abbreviation>
    </owl:Class>
    


    <!-- http://onto.fel.cvut.cz/ontologies/aviation-safety/very_high_frequency_omni-directional_radio_range_ground_system -->

    <owl:Class rdf:about="&m;very_high_frequency_omni-directional_radio_range_ground_system"/>
</rdf:RDF>



<!-- Generated by the OWL API (version 3.4.2) http://owlapi.sourceforge.net -->

